<?xml version='1.0' encoding='UTF-8'?>
<rdf:RDF xmlns:cim="http://iec.ch/TC57/2013/CIM-schema-cim16#" xmlns:rdf="http://www.w3.org/1999/02/22-rdf-syntax-ns#" xmlns:rdfs="http://www.w3.org/2000/01/rdf-schema#" xmlns:dcat="http://www.w3.org/ns/dcat#" xmlns:dc="http://purl.org/dc/elements/1.1/" xmlns:dcterms="http://purl.org/dc/terms/" xmlns:skos="http://www.w3.org/2004/02/skos/core#" xmlns:ecl="urn:entsoe.eu:wgedi:codelists" xmlns:xs="http://www.w3.org/2001/XMLSchema">
  <skos:ConceptScheme rdf:about="http://energy.referencedata.eu/StandardAssetTypeList">
    <rdf:type rdf:resource="http://www.w3.org/ns/dcat#Dataset"/>
    <dcterms:modified>2023-12-14</dcterms:modified>
    <dcat:version>91</dcat:version>
    <skos:prefLabel>StandardAssetTypeList</skos:prefLabel>
    <dcterms:identifier>ET0031</dcterms:identifier>
    <skos:definition xml:lang="en">The identification of the type of asset.</skos:definition>
  </skos:ConceptScheme>
  <skos:Concept rdf:about="http://energy.referencedata.eu/StandardAssetTypeList/A01">
    <skos:inScheme rdf:resource="http://energy.referencedata.eu/StandardAssetTypeList"/>
    <skos:topConceptOf rdf:resource="http://energy.referencedata.eu/StandardAssetTypeList"/>
    <dcterms:identifier>A01</dcterms:identifier>
    <skos:prefLabel>Tie line</skos:prefLabel>
    <skos:definition xml:lang="en">A high voltage line used for cross border energy interconnections.</skos:definition>
  </skos:Concept>
  <skos:Concept rdf:about="http://energy.referencedata.eu/StandardAssetTypeList/A02">
    <skos:inScheme rdf:resource="http://energy.referencedata.eu/StandardAssetTypeList"/>
    <skos:topConceptOf rdf:resource="http://energy.referencedata.eu/StandardAssetTypeList"/>
    <dcterms:identifier>A02</dcterms:identifier>
    <skos:prefLabel>Line</skos:prefLabel>
    <skos:definition xml:lang="en">A specific electric line within a country.</skos:definition>
  </skos:Concept>
  <skos:Concept rdf:about="http://energy.referencedata.eu/StandardAssetTypeList/A03">
    <skos:inScheme rdf:resource="http://energy.referencedata.eu/StandardAssetTypeList"/>
    <skos:topConceptOf rdf:resource="http://energy.referencedata.eu/StandardAssetTypeList"/>
    <dcterms:identifier>A03</dcterms:identifier>
    <skos:prefLabel>Resource Object</skos:prefLabel>
    <skos:definition xml:lang="en">A resource that can either produce or consume energy.</skos:definition>
  </skos:Concept>
  <skos:Concept rdf:about="http://energy.referencedata.eu/StandardAssetTypeList/A04">
    <skos:inScheme rdf:resource="http://energy.referencedata.eu/StandardAssetTypeList"/>
    <skos:topConceptOf rdf:resource="http://energy.referencedata.eu/StandardAssetTypeList"/>
    <dcterms:identifier>A04</dcterms:identifier>
    <skos:prefLabel>Generation</skos:prefLabel>
    <skos:definition xml:lang="en">A resource that can produce energy.</skos:definition>
  </skos:Concept>
  <skos:Concept rdf:about="http://energy.referencedata.eu/StandardAssetTypeList/A05">
    <skos:inScheme rdf:resource="http://energy.referencedata.eu/StandardAssetTypeList"/>
    <skos:topConceptOf rdf:resource="http://energy.referencedata.eu/StandardAssetTypeList"/>
    <dcterms:identifier>A05</dcterms:identifier>
    <skos:prefLabel>Load</skos:prefLabel>
    <skos:definition xml:lang="en">A resource that can consume energy.</skos:definition>
  </skos:Concept>
  <skos:Concept rdf:about="http://energy.referencedata.eu/StandardAssetTypeList/A06">
    <skos:inScheme rdf:resource="http://energy.referencedata.eu/StandardAssetTypeList"/>
    <skos:topConceptOf rdf:resource="http://energy.referencedata.eu/StandardAssetTypeList"/>
    <dcterms:identifier>A06</dcterms:identifier>
    <skos:prefLabel>Phase Shift Transformer</skos:prefLabel>
    <skos:definition xml:lang="en">An electrical device for controlling the power flow through specific lines in a power transmission network.</skos:definition>
  </skos:Concept>
  <skos:Concept rdf:about="http://energy.referencedata.eu/StandardAssetTypeList/A07">
    <skos:inScheme rdf:resource="http://energy.referencedata.eu/StandardAssetTypeList"/>
    <skos:topConceptOf rdf:resource="http://energy.referencedata.eu/StandardAssetTypeList"/>
    <dcterms:identifier>A07</dcterms:identifier>
    <skos:prefLabel>Circuit Breaker</skos:prefLabel>
    <skos:definition xml:lang="en">An electrical switch designed to protect an electrical circuit from damage caused by overcurrent/overload or short circuit.</skos:definition>
  </skos:Concept>
  <skos:Concept rdf:about="http://energy.referencedata.eu/StandardAssetTypeList/A08">
    <skos:inScheme rdf:resource="http://energy.referencedata.eu/StandardAssetTypeList"/>
    <skos:topConceptOf rdf:resource="http://energy.referencedata.eu/StandardAssetTypeList"/>
    <dcterms:identifier>A08</dcterms:identifier>
    <skos:prefLabel>Busbar</skos:prefLabel>
    <skos:definition xml:lang="en">A specific element within a substation to connect grid elements for energy distribution purposes.</skos:definition>
  </skos:Concept>
  <skos:Concept rdf:about="http://energy.referencedata.eu/StandardAssetTypeList/A09">
    <skos:inScheme rdf:resource="http://energy.referencedata.eu/StandardAssetTypeList"/>
    <skos:topConceptOf rdf:resource="http://energy.referencedata.eu/StandardAssetTypeList"/>
    <dcterms:identifier>A09</dcterms:identifier>
    <skos:prefLabel>Capacitor</skos:prefLabel>
    <skos:definition xml:lang="en">A transmission element designed to inject reactive power into the transmission network. </skos:definition>
  </skos:Concept>
  <skos:Concept rdf:about="http://energy.referencedata.eu/StandardAssetTypeList/A10">
    <skos:inScheme rdf:resource="http://energy.referencedata.eu/StandardAssetTypeList"/>
    <skos:topConceptOf rdf:resource="http://energy.referencedata.eu/StandardAssetTypeList"/>
    <dcterms:identifier>A10</dcterms:identifier>
    <skos:prefLabel>Inductor</skos:prefLabel>
    <skos:definition xml:lang="en">A transmission element designed to compensate reactive power in the transmission network.</skos:definition>
  </skos:Concept>
  <skos:Concept rdf:about="http://energy.referencedata.eu/StandardAssetTypeList/A11">
    <skos:inScheme rdf:resource="http://energy.referencedata.eu/StandardAssetTypeList"/>
    <skos:topConceptOf rdf:resource="http://energy.referencedata.eu/StandardAssetTypeList"/>
    <dcterms:identifier>A11</dcterms:identifier>
    <skos:prefLabel>Power plant connection</skos:prefLabel>
    <skos:definition xml:lang="en">All the network equipment that link the generating unit to the grid.</skos:definition>
  </skos:Concept>
  <skos:Concept rdf:about="http://energy.referencedata.eu/StandardAssetTypeList/A12">
    <skos:inScheme rdf:resource="http://energy.referencedata.eu/StandardAssetTypeList"/>
    <skos:topConceptOf rdf:resource="http://energy.referencedata.eu/StandardAssetTypeList"/>
    <dcterms:identifier>A12</dcterms:identifier>
    <skos:prefLabel>FACTS</skos:prefLabel>
    <skos:definition xml:lang="en">Flexible Alternating Current Transmission System</skos:definition>
  </skos:Concept>
  <skos:Concept rdf:about="http://energy.referencedata.eu/StandardAssetTypeList/A13">
    <skos:inScheme rdf:resource="http://energy.referencedata.eu/StandardAssetTypeList"/>
    <skos:topConceptOf rdf:resource="http://energy.referencedata.eu/StandardAssetTypeList"/>
    <dcterms:identifier>A13</dcterms:identifier>
    <skos:prefLabel>Production unit</skos:prefLabel>
    <skos:definition xml:lang="en">A production unit is a composition of one or several generation units.</skos:definition>
  </skos:Concept>
  <skos:Concept rdf:about="http://energy.referencedata.eu/StandardAssetTypeList/A14">
    <skos:inScheme rdf:resource="http://energy.referencedata.eu/StandardAssetTypeList"/>
    <skos:topConceptOf rdf:resource="http://energy.referencedata.eu/StandardAssetTypeList"/>
    <dcterms:identifier>A14</dcterms:identifier>
    <skos:prefLabel>Internal tie line</skos:prefLabel>
    <skos:definition xml:lang="en">An internal tie line is a line between two scheduling areas within the same bidding zone.</skos:definition>
  </skos:Concept>
  <skos:Concept rdf:about="http://energy.referencedata.eu/StandardAssetTypeList/B01">
    <skos:inScheme rdf:resource="http://energy.referencedata.eu/StandardAssetTypeList"/>
    <skos:topConceptOf rdf:resource="http://energy.referencedata.eu/StandardAssetTypeList"/>
    <dcterms:identifier>B01</dcterms:identifier>
    <skos:prefLabel>Biomass</skos:prefLabel>
    <skos:definition xml:lang="en">A resource using biomass for energy.</skos:definition>
  </skos:Concept>
  <skos:Concept rdf:about="http://energy.referencedata.eu/StandardAssetTypeList/B02">
    <skos:inScheme rdf:resource="http://energy.referencedata.eu/StandardAssetTypeList"/>
    <skos:topConceptOf rdf:resource="http://energy.referencedata.eu/StandardAssetTypeList"/>
    <dcterms:identifier>B02</dcterms:identifier>
    <skos:prefLabel>Fossil Brown coal/Lignite</skos:prefLabel>
    <skos:definition xml:lang="en">A resource using Fossil Brown coal/Lignite for energy.</skos:definition>
  </skos:Concept>
  <skos:Concept rdf:about="http://energy.referencedata.eu/StandardAssetTypeList/B03">
    <skos:inScheme rdf:resource="http://energy.referencedata.eu/StandardAssetTypeList"/>
    <skos:topConceptOf rdf:resource="http://energy.referencedata.eu/StandardAssetTypeList"/>
    <dcterms:identifier>B03</dcterms:identifier>
    <skos:prefLabel>Fossil Coal-derived gas</skos:prefLabel>
    <skos:definition xml:lang="en">A resource using Fossil Coal-derived gas for energy.</skos:definition>
  </skos:Concept>
  <skos:Concept rdf:about="http://energy.referencedata.eu/StandardAssetTypeList/B04">
    <skos:inScheme rdf:resource="http://energy.referencedata.eu/StandardAssetTypeList"/>
    <skos:topConceptOf rdf:resource="http://energy.referencedata.eu/StandardAssetTypeList"/>
    <dcterms:identifier>B04</dcterms:identifier>
    <skos:prefLabel>Fossil Gas</skos:prefLabel>
    <skos:definition xml:lang="en">A resource using Fossil Gas for energy.</skos:definition>
  </skos:Concept>
  <skos:Concept rdf:about="http://energy.referencedata.eu/StandardAssetTypeList/B05">
    <skos:inScheme rdf:resource="http://energy.referencedata.eu/StandardAssetTypeList"/>
    <skos:topConceptOf rdf:resource="http://energy.referencedata.eu/StandardAssetTypeList"/>
    <dcterms:identifier>B05</dcterms:identifier>
    <skos:prefLabel>Fossil Hard coal</skos:prefLabel>
    <skos:definition xml:lang="en">A resource using Fossil Hard coal for energy.</skos:definition>
  </skos:Concept>
  <skos:Concept rdf:about="http://energy.referencedata.eu/StandardAssetTypeList/B06">
    <skos:inScheme rdf:resource="http://energy.referencedata.eu/StandardAssetTypeList"/>
    <skos:topConceptOf rdf:resource="http://energy.referencedata.eu/StandardAssetTypeList"/>
    <dcterms:identifier>B06</dcterms:identifier>
    <skos:prefLabel>Fossil Oil</skos:prefLabel>
    <skos:definition xml:lang="en">A resource using Fossil Oil for energy.</skos:definition>
  </skos:Concept>
  <skos:Concept rdf:about="http://energy.referencedata.eu/StandardAssetTypeList/B07">
    <skos:inScheme rdf:resource="http://energy.referencedata.eu/StandardAssetTypeList"/>
    <skos:topConceptOf rdf:resource="http://energy.referencedata.eu/StandardAssetTypeList"/>
    <dcterms:identifier>B07</dcterms:identifier>
    <skos:prefLabel>Fossil Oil shale</skos:prefLabel>
    <skos:definition xml:lang="en">A resource using Fossil Oil shale for energy.</skos:definition>
  </skos:Concept>
  <skos:Concept rdf:about="http://energy.referencedata.eu/StandardAssetTypeList/B08">
    <skos:inScheme rdf:resource="http://energy.referencedata.eu/StandardAssetTypeList"/>
    <skos:topConceptOf rdf:resource="http://energy.referencedata.eu/StandardAssetTypeList"/>
    <dcterms:identifier>B08</dcterms:identifier>
    <skos:prefLabel>Fossil Peat</skos:prefLabel>
    <skos:definition xml:lang="en">A resource using Fossil Peat for energy.</skos:definition>
  </skos:Concept>
  <skos:Concept rdf:about="http://energy.referencedata.eu/StandardAssetTypeList/B09">
    <skos:inScheme rdf:resource="http://energy.referencedata.eu/StandardAssetTypeList"/>
    <skos:topConceptOf rdf:resource="http://energy.referencedata.eu/StandardAssetTypeList"/>
    <dcterms:identifier>B09</dcterms:identifier>
    <skos:prefLabel>Geothermal</skos:prefLabel>
    <skos:definition xml:lang="en">A resource using Geothermal for energy.</skos:definition>
  </skos:Concept>
  <skos:Concept rdf:about="http://energy.referencedata.eu/StandardAssetTypeList/B10">
    <skos:inScheme rdf:resource="http://energy.referencedata.eu/StandardAssetTypeList"/>
    <skos:topConceptOf rdf:resource="http://energy.referencedata.eu/StandardAssetTypeList"/>
    <dcterms:identifier>B10</dcterms:identifier>
    <skos:prefLabel>Hydro-electric pure pumped storage head installation</skos:prefLabel>
    <skos:definition xml:lang="en">Unit in which moving water energy is converted to electricity using flowing water to generate electricity with a large dam and reservoirs. Pure pumped storage plants store water in an upper reservoir with no natural inflows.</skos:definition>
  </skos:Concept>
  <skos:Concept rdf:about="http://energy.referencedata.eu/StandardAssetTypeList/B11">
    <skos:inScheme rdf:resource="http://energy.referencedata.eu/StandardAssetTypeList"/>
    <skos:topConceptOf rdf:resource="http://energy.referencedata.eu/StandardAssetTypeList"/>
    <dcterms:identifier>B11</dcterms:identifier>
    <skos:prefLabel>Hydro Run-of-river head installation</skos:prefLabel>
    <skos:definition xml:lang="en">Unit in which moving water energy is converted to electricity using flowing water to generate electricity in the absence of a large dam and reservoirs.</skos:definition>
  </skos:Concept>
  <skos:Concept rdf:about="http://energy.referencedata.eu/StandardAssetTypeList/B12">
    <skos:inScheme rdf:resource="http://energy.referencedata.eu/StandardAssetTypeList"/>
    <skos:topConceptOf rdf:resource="http://energy.referencedata.eu/StandardAssetTypeList"/>
    <dcterms:identifier>B12</dcterms:identifier>
    <skos:prefLabel>Hydro-electric storage head installation</skos:prefLabel>
    <skos:definition xml:lang="en">Unit in which moving water energy is converted to electricity using flowing water to generate electricity with a large dam and reservoirs.</skos:definition>
  </skos:Concept>
  <skos:Concept rdf:about="http://energy.referencedata.eu/StandardAssetTypeList/B13">
    <skos:inScheme rdf:resource="http://energy.referencedata.eu/StandardAssetTypeList"/>
    <skos:topConceptOf rdf:resource="http://energy.referencedata.eu/StandardAssetTypeList"/>
    <dcterms:identifier>B13</dcterms:identifier>
    <skos:prefLabel>Marine unspecified</skos:prefLabel>
    <skos:definition xml:lang="en">Unit in which marine energy is converted to electricity with equipment/devices not specified.</skos:definition>
  </skos:Concept>
  <skos:Concept rdf:about="http://energy.referencedata.eu/StandardAssetTypeList/B14">
    <skos:inScheme rdf:resource="http://energy.referencedata.eu/StandardAssetTypeList"/>
    <skos:topConceptOf rdf:resource="http://energy.referencedata.eu/StandardAssetTypeList"/>
    <dcterms:identifier>B14</dcterms:identifier>
    <skos:prefLabel>Nuclear unspecified</skos:prefLabel>
    <skos:definition xml:lang="en">A unit in which the heat source is a nuclear reactor of type that is not specified in other nuclear types. </skos:definition>
  </skos:Concept>
  <skos:Concept rdf:about="http://energy.referencedata.eu/StandardAssetTypeList/B15">
    <skos:inScheme rdf:resource="http://energy.referencedata.eu/StandardAssetTypeList"/>
    <skos:topConceptOf rdf:resource="http://energy.referencedata.eu/StandardAssetTypeList"/>
    <dcterms:identifier>B15</dcterms:identifier>
    <skos:prefLabel>Other renewable</skos:prefLabel>
    <skos:definition xml:lang="en">A resource using Other renewable for energy.</skos:definition>
  </skos:Concept>
  <skos:Concept rdf:about="http://energy.referencedata.eu/StandardAssetTypeList/B16">
    <skos:inScheme rdf:resource="http://energy.referencedata.eu/StandardAssetTypeList"/>
    <skos:topConceptOf rdf:resource="http://energy.referencedata.eu/StandardAssetTypeList"/>
    <dcterms:identifier>B16</dcterms:identifier>
    <skos:prefLabel>Solar unspecified</skos:prefLabel>
    <skos:definition xml:lang="en">Unit in which solar energy is converted to electricity with equipment/devices not specified.</skos:definition>
  </skos:Concept>
  <skos:Concept rdf:about="http://energy.referencedata.eu/StandardAssetTypeList/B17">
    <skos:inScheme rdf:resource="http://energy.referencedata.eu/StandardAssetTypeList"/>
    <skos:topConceptOf rdf:resource="http://energy.referencedata.eu/StandardAssetTypeList"/>
    <dcterms:identifier>B17</dcterms:identifier>
    <skos:prefLabel>Waste</skos:prefLabel>
    <skos:definition xml:lang="en">A resource using Waste for energy.</skos:definition>
  </skos:Concept>
  <skos:Concept rdf:about="http://energy.referencedata.eu/StandardAssetTypeList/B18">
    <skos:inScheme rdf:resource="http://energy.referencedata.eu/StandardAssetTypeList"/>
    <skos:topConceptOf rdf:resource="http://energy.referencedata.eu/StandardAssetTypeList"/>
    <dcterms:identifier>B18</dcterms:identifier>
    <skos:prefLabel>Wind Offshore</skos:prefLabel>
    <skos:definition xml:lang="en">Unit in which wind energy is converted to electricity using wind farms constructed in bodies of water, usually in the ocean.</skos:definition>
  </skos:Concept>
  <skos:Concept rdf:about="http://energy.referencedata.eu/StandardAssetTypeList/B19">
    <skos:inScheme rdf:resource="http://energy.referencedata.eu/StandardAssetTypeList"/>
    <skos:topConceptOf rdf:resource="http://energy.referencedata.eu/StandardAssetTypeList"/>
    <dcterms:identifier>B19</dcterms:identifier>
    <skos:prefLabel>Wind Onshore</skos:prefLabel>
    <skos:definition xml:lang="en">Unit in which wind energy is converted to electricity using wind farms constructed on land.</skos:definition>
  </skos:Concept>
  <skos:Concept rdf:about="http://energy.referencedata.eu/StandardAssetTypeList/B20">
    <skos:inScheme rdf:resource="http://energy.referencedata.eu/StandardAssetTypeList"/>
    <skos:topConceptOf rdf:resource="http://energy.referencedata.eu/StandardAssetTypeList"/>
    <dcterms:identifier>B20</dcterms:identifier>
    <skos:prefLabel>Other unspecified</skos:prefLabel>
    <skos:definition xml:lang="en">Other unspecified technology.</skos:definition>
  </skos:Concept>
  <skos:Concept rdf:about="http://energy.referencedata.eu/StandardAssetTypeList/B21">
    <skos:inScheme rdf:resource="http://energy.referencedata.eu/StandardAssetTypeList"/>
    <skos:topConceptOf rdf:resource="http://energy.referencedata.eu/StandardAssetTypeList"/>
    <dcterms:identifier>B21</dcterms:identifier>
    <skos:prefLabel>AC Link</skos:prefLabel>
    <skos:definition xml:lang="en">Overhead line or cable which is used to transmit electrical power via Alternative Current.</skos:definition>
  </skos:Concept>
  <skos:Concept rdf:about="http://energy.referencedata.eu/StandardAssetTypeList/B22">
    <skos:inScheme rdf:resource="http://energy.referencedata.eu/StandardAssetTypeList"/>
    <skos:topConceptOf rdf:resource="http://energy.referencedata.eu/StandardAssetTypeList"/>
    <dcterms:identifier>B22</dcterms:identifier>
    <skos:prefLabel>DC Link</skos:prefLabel>
    <skos:definition xml:lang="en">Overhead line or cable which is used to transmit electrical power via Direct Current.</skos:definition>
  </skos:Concept>
  <skos:Concept rdf:about="http://energy.referencedata.eu/StandardAssetTypeList/B23">
    <skos:inScheme rdf:resource="http://energy.referencedata.eu/StandardAssetTypeList"/>
    <skos:topConceptOf rdf:resource="http://energy.referencedata.eu/StandardAssetTypeList"/>
    <dcterms:identifier>B23</dcterms:identifier>
    <skos:prefLabel>Substation</skos:prefLabel>
    <skos:definition xml:lang="en">An assembly of equipment in an electric power system through which electric energy is passed for transmission, transformation, distribution or switching.</skos:definition>
  </skos:Concept>
  <skos:Concept rdf:about="http://energy.referencedata.eu/StandardAssetTypeList/B24">
    <skos:inScheme rdf:resource="http://energy.referencedata.eu/StandardAssetTypeList"/>
    <skos:topConceptOf rdf:resource="http://energy.referencedata.eu/StandardAssetTypeList"/>
    <dcterms:identifier>B24</dcterms:identifier>
    <skos:prefLabel>Transformer</skos:prefLabel>
    <skos:definition xml:lang="en">Electrical device that transfers energy from one voltage level to another voltage level.</skos:definition>
  </skos:Concept>
  <skos:Concept rdf:about="http://energy.referencedata.eu/StandardAssetTypeList/B25">
    <skos:inScheme rdf:resource="http://energy.referencedata.eu/StandardAssetTypeList"/>
    <skos:topConceptOf rdf:resource="http://energy.referencedata.eu/StandardAssetTypeList"/>
    <dcterms:identifier>B25</dcterms:identifier>
    <skos:prefLabel>Energy storage</skos:prefLabel>
    <skos:definition xml:lang="en">A resource that stores energy. It could be gas, electricity, etc.</skos:definition>
  </skos:Concept>
  <skos:Concept rdf:about="http://energy.referencedata.eu/StandardAssetTypeList/B26">
    <skos:inScheme rdf:resource="http://energy.referencedata.eu/StandardAssetTypeList"/>
    <skos:topConceptOf rdf:resource="http://energy.referencedata.eu/StandardAssetTypeList"/>
    <dcterms:identifier>B26</dcterms:identifier>
    <skos:prefLabel>Demand Side Response</skos:prefLabel>
    <skos:definition xml:lang="en">A resource that change its electricity consumption patterns in response to a signal or incentive.</skos:definition>
  </skos:Concept>
  <skos:Concept rdf:about="http://energy.referencedata.eu/StandardAssetTypeList/B27">
    <skos:inScheme rdf:resource="http://energy.referencedata.eu/StandardAssetTypeList"/>
    <skos:topConceptOf rdf:resource="http://energy.referencedata.eu/StandardAssetTypeList"/>
    <dcterms:identifier>B27</dcterms:identifier>
    <skos:prefLabel>Dispatchable hydro resource</skos:prefLabel>
    <skos:definition xml:lang="en">A resource referring to dispatchable hydro generation.</skos:definition>
  </skos:Concept>
  <skos:Concept rdf:about="http://energy.referencedata.eu/StandardAssetTypeList/B28">
    <skos:inScheme rdf:resource="http://energy.referencedata.eu/StandardAssetTypeList"/>
    <skos:topConceptOf rdf:resource="http://energy.referencedata.eu/StandardAssetTypeList"/>
    <dcterms:identifier>B28</dcterms:identifier>
    <skos:prefLabel>Solar photovoltaic</skos:prefLabel>
    <skos:definition xml:lang="en">Unit in which solar energy is converted to electricity using a technology based on the photoelectric effect.</skos:definition>
  </skos:Concept>
  <skos:Concept rdf:about="http://energy.referencedata.eu/StandardAssetTypeList/B29">
    <skos:inScheme rdf:resource="http://energy.referencedata.eu/StandardAssetTypeList"/>
    <skos:topConceptOf rdf:resource="http://energy.referencedata.eu/StandardAssetTypeList"/>
    <dcterms:identifier>B29</dcterms:identifier>
    <skos:prefLabel>Solar concentration</skos:prefLabel>
    <skos:definition xml:lang="en">Unit in which solar energy is converted to electricity using mirrors to concentrate the sun's energy to drive traditional steam turbines or engines.</skos:definition>
  </skos:Concept>
  <skos:Concept rdf:about="http://energy.referencedata.eu/StandardAssetTypeList/B30">
    <skos:inScheme rdf:resource="http://energy.referencedata.eu/StandardAssetTypeList"/>
    <skos:topConceptOf rdf:resource="http://energy.referencedata.eu/StandardAssetTypeList"/>
    <dcterms:identifier>B30</dcterms:identifier>
    <skos:prefLabel>Wind unspecified</skos:prefLabel>
    <skos:definition xml:lang="en">Unit in which wind energy is converted to electricity with equipment/devices not specified.</skos:definition>
  </skos:Concept>
  <skos:Concept rdf:about="http://energy.referencedata.eu/StandardAssetTypeList/B31">
    <skos:inScheme rdf:resource="http://energy.referencedata.eu/StandardAssetTypeList"/>
    <skos:topConceptOf rdf:resource="http://energy.referencedata.eu/StandardAssetTypeList"/>
    <dcterms:identifier>B31</dcterms:identifier>
    <skos:prefLabel>Hydro-electric unspecified</skos:prefLabel>
    <skos:definition xml:lang="en">Unit in which moving water energy is converted to electricity with equipment/devices not specified. </skos:definition>
  </skos:Concept>
  <skos:Concept rdf:about="http://energy.referencedata.eu/StandardAssetTypeList/B32">
    <skos:inScheme rdf:resource="http://energy.referencedata.eu/StandardAssetTypeList"/>
    <skos:topConceptOf rdf:resource="http://energy.referencedata.eu/StandardAssetTypeList"/>
    <dcterms:identifier>B32</dcterms:identifier>
    <skos:prefLabel>Hydro-electric mixed pumped storage head installation</skos:prefLabel>
    <skos:definition xml:lang="en">Unit in which moving water energy is converted to electricity using flowing water to generate electricity with a large dam and reservoirs. Mixed pumped storage plants use a combination of pumped storage and conventional hydroelectric plants with an upper reservoir that is replenished in part by natural inflows from a stream or river.</skos:definition>
  </skos:Concept>
  <skos:Concept rdf:about="http://energy.referencedata.eu/StandardAssetTypeList/B33">
    <skos:inScheme rdf:resource="http://energy.referencedata.eu/StandardAssetTypeList"/>
    <skos:topConceptOf rdf:resource="http://energy.referencedata.eu/StandardAssetTypeList"/>
    <dcterms:identifier>B33</dcterms:identifier>
    <skos:prefLabel>Marine tidal</skos:prefLabel>
    <skos:definition xml:lang="en">Unit in which marine energy from tides is converted to electricity.</skos:definition>
  </skos:Concept>
  <skos:Concept rdf:about="http://energy.referencedata.eu/StandardAssetTypeList/B34">
    <skos:inScheme rdf:resource="http://energy.referencedata.eu/StandardAssetTypeList"/>
    <skos:topConceptOf rdf:resource="http://energy.referencedata.eu/StandardAssetTypeList"/>
    <dcterms:identifier>B34</dcterms:identifier>
    <skos:prefLabel>Marine wave</skos:prefLabel>
    <skos:definition xml:lang="en">Unit in which marine energy from waves is converted to electricity.</skos:definition>
  </skos:Concept>
  <skos:Concept rdf:about="http://energy.referencedata.eu/StandardAssetTypeList/B35">
    <skos:inScheme rdf:resource="http://energy.referencedata.eu/StandardAssetTypeList"/>
    <skos:topConceptOf rdf:resource="http://energy.referencedata.eu/StandardAssetTypeList"/>
    <dcterms:identifier>B35</dcterms:identifier>
    <skos:prefLabel>Marine currents</skos:prefLabel>
    <skos:definition xml:lang="en">Unit in which marine energy from currents is converted to electricity.</skos:definition>
  </skos:Concept>
  <skos:Concept rdf:about="http://energy.referencedata.eu/StandardAssetTypeList/B36">
    <skos:inScheme rdf:resource="http://energy.referencedata.eu/StandardAssetTypeList"/>
    <skos:topConceptOf rdf:resource="http://energy.referencedata.eu/StandardAssetTypeList"/>
    <dcterms:identifier>B36</dcterms:identifier>
    <skos:prefLabel>Marine pressure</skos:prefLabel>
    <skos:definition xml:lang="en">Unit in which marine energy from pressure is converted to electricity.</skos:definition>
  </skos:Concept>
  <skos:Concept rdf:about="http://energy.referencedata.eu/StandardAssetTypeList/B37">
    <skos:inScheme rdf:resource="http://energy.referencedata.eu/StandardAssetTypeList"/>
    <skos:topConceptOf rdf:resource="http://energy.referencedata.eu/StandardAssetTypeList"/>
    <dcterms:identifier>B37</dcterms:identifier>
    <skos:prefLabel>Thermal unspecified</skos:prefLabel>
    <skos:definition xml:lang="en">Unit in which heat energy is converted to electricity with equipment/devices not specified in other thermal types.</skos:definition>
  </skos:Concept>
  <skos:Concept rdf:about="http://energy.referencedata.eu/StandardAssetTypeList/B38">
    <skos:inScheme rdf:resource="http://energy.referencedata.eu/StandardAssetTypeList"/>
    <skos:topConceptOf rdf:resource="http://energy.referencedata.eu/StandardAssetTypeList"/>
    <dcterms:identifier>B38</dcterms:identifier>
    <skos:prefLabel>Thermal combined cycle gas turbine with heat recovery</skos:prefLabel>
    <skos:definition xml:lang="en">Unit in which heat energy is converted to electricity called Combined Cycle Gas Turbine. The power is generated by the single or multiple gas turbine(s) in combination with the steam turbine(s). The unit might be equipped with waste heat recovery (e.g. to district heating network).</skos:definition>
  </skos:Concept>
  <skos:Concept rdf:about="http://energy.referencedata.eu/StandardAssetTypeList/B39">
    <skos:inScheme rdf:resource="http://energy.referencedata.eu/StandardAssetTypeList"/>
    <skos:topConceptOf rdf:resource="http://energy.referencedata.eu/StandardAssetTypeList"/>
    <dcterms:identifier>B39</dcterms:identifier>
    <skos:prefLabel>Thermal steam turbine with back-pressure turbine (open cycle)</skos:prefLabel>
    <skos:definition xml:lang="en">Unit in which heat energy is converted to electricity. The power is generated with the steam that is expanded in the back-pressure steam turbine with or without heat output (e.g. to district heating network).</skos:definition>
  </skos:Concept>
  <skos:Concept rdf:about="http://energy.referencedata.eu/StandardAssetTypeList/B40">
    <skos:inScheme rdf:resource="http://energy.referencedata.eu/StandardAssetTypeList"/>
    <skos:topConceptOf rdf:resource="http://energy.referencedata.eu/StandardAssetTypeList"/>
    <dcterms:identifier>B40</dcterms:identifier>
    <skos:prefLabel>Thermal steam turbine with condensation turbine (closed cycle)</skos:prefLabel>
    <skos:definition xml:lang="en">Unit in which heat energy is converted to electricity. The power is generated with the steam that is expanded in the condensation steam turbine with or without heat output (e.g. to district heating network).</skos:definition>
  </skos:Concept>
  <skos:Concept rdf:about="http://energy.referencedata.eu/StandardAssetTypeList/B41">
    <skos:inScheme rdf:resource="http://energy.referencedata.eu/StandardAssetTypeList"/>
    <skos:topConceptOf rdf:resource="http://energy.referencedata.eu/StandardAssetTypeList"/>
    <dcterms:identifier>B41</dcterms:identifier>
    <skos:prefLabel>Thermal gas turbine with heat recovery</skos:prefLabel>
    <skos:definition xml:lang="en">Unit in which heat energy is converted to electricity called Simple Cycle Gas Turbine. The power is generated by the gas turbine and the flue gas waste heat is recovered (e.g. to district heating network).</skos:definition>
  </skos:Concept>
  <skos:Concept rdf:about="http://energy.referencedata.eu/StandardAssetTypeList/B42">
    <skos:inScheme rdf:resource="http://energy.referencedata.eu/StandardAssetTypeList"/>
    <skos:topConceptOf rdf:resource="http://energy.referencedata.eu/StandardAssetTypeList"/>
    <dcterms:identifier>B42</dcterms:identifier>
    <skos:prefLabel>Thermal internal combustion engine</skos:prefLabel>
    <skos:definition xml:lang="en">An internal combustion engine is a heat engine in which the combustion of a fuel occurs with an oxidizer (usually air) in a combustion chamber that is an integral part of the working fluid flow circuit (e.g. reciprocating engine). The unit might be equipped with waste heat recovery (e.g. to district heating network).</skos:definition>
  </skos:Concept>
  <skos:Concept rdf:about="http://energy.referencedata.eu/StandardAssetTypeList/B43">
    <skos:inScheme rdf:resource="http://energy.referencedata.eu/StandardAssetTypeList"/>
    <skos:topConceptOf rdf:resource="http://energy.referencedata.eu/StandardAssetTypeList"/>
    <dcterms:identifier>B43</dcterms:identifier>
    <skos:prefLabel>Thermal micro-turbine</skos:prefLabel>
    <skos:definition xml:lang="en">Unit in which heat energy is converted to electricity called Simple Cycle Gas Turbine. The power is generated by the gas turbine (capacity less than 500kWe). The unit might be equipped with waste heat recovery (e.g. to district heating network).</skos:definition>
  </skos:Concept>
  <skos:Concept rdf:about="http://energy.referencedata.eu/StandardAssetTypeList/B44">
    <skos:inScheme rdf:resource="http://energy.referencedata.eu/StandardAssetTypeList"/>
    <skos:topConceptOf rdf:resource="http://energy.referencedata.eu/StandardAssetTypeList"/>
    <dcterms:identifier>B44</dcterms:identifier>
    <skos:prefLabel>Thermal Stirling engine</skos:prefLabel>
    <skos:definition xml:lang="en">A Stirling engine is a heat engine that is operated by the cyclic compression and expansion of air or other gas (the working fluid) at different temperatures, resulting in a net conversion of heat energy to mechanical work.</skos:definition>
  </skos:Concept>
  <skos:Concept rdf:about="http://energy.referencedata.eu/StandardAssetTypeList/B45">
    <skos:inScheme rdf:resource="http://energy.referencedata.eu/StandardAssetTypeList"/>
    <skos:topConceptOf rdf:resource="http://energy.referencedata.eu/StandardAssetTypeList"/>
    <dcterms:identifier>B45</dcterms:identifier>
    <skos:prefLabel>Thermal fuel cell</skos:prefLabel>
    <skos:definition xml:lang="en">A fuel cell is an electrochemical cell that converts the chemical energy of a fuel (e.g. hydrogen) and an oxidizing agent (e.g. oxygen) into electricity through a pair of redox reactions.</skos:definition>
  </skos:Concept>
  <skos:Concept rdf:about="http://energy.referencedata.eu/StandardAssetTypeList/B46">
    <skos:inScheme rdf:resource="http://energy.referencedata.eu/StandardAssetTypeList"/>
    <skos:topConceptOf rdf:resource="http://energy.referencedata.eu/StandardAssetTypeList"/>
    <dcterms:identifier>B46</dcterms:identifier>
    <skos:prefLabel>Thermal steam engine</skos:prefLabel>
    <skos:definition xml:lang="en">A steam engine is a heat engine that performs mechanical work using steam as its working fluid. The steam engine uses the force produced by steam pressure to push a piston back and forth inside a cylinder.</skos:definition>
  </skos:Concept>
  <skos:Concept rdf:about="http://energy.referencedata.eu/StandardAssetTypeList/B47">
    <skos:inScheme rdf:resource="http://energy.referencedata.eu/StandardAssetTypeList"/>
    <skos:topConceptOf rdf:resource="http://energy.referencedata.eu/StandardAssetTypeList"/>
    <dcterms:identifier>B47</dcterms:identifier>
    <skos:prefLabel>Thermal organic Rankine cycle</skos:prefLabel>
    <skos:definition xml:lang="en">The Organic Rankine Cycle (ORC) is named for its use of an organic, high molecular mass fluid with a liquid-vapor phase change, or boiling point, occurring at a lower temperature than the water-steam phase change. The fluid allows Rankine cycle heat recovery from lower temperature sources such as biomass combustion, industrial waste heat, geothermal heat, solar ponds etc. The low-temperature heat is converted into useful work, that can itself be converted into electricity.</skos:definition>
  </skos:Concept>
  <skos:Concept rdf:about="http://energy.referencedata.eu/StandardAssetTypeList/B48">
    <skos:inScheme rdf:resource="http://energy.referencedata.eu/StandardAssetTypeList"/>
    <skos:topConceptOf rdf:resource="http://energy.referencedata.eu/StandardAssetTypeList"/>
    <dcterms:identifier>B48</dcterms:identifier>
    <skos:prefLabel>Thermal gas turbine without heat recovery</skos:prefLabel>
    <skos:definition xml:lang="en">Unit in which heat energy is converted to electricity called Simple Cycle Gas Turbine. The power is generated by the gas turbine and there is no flue gas waste heat recovery.</skos:definition>
  </skos:Concept>
  <skos:Concept rdf:about="http://energy.referencedata.eu/StandardAssetTypeList/B49">
    <skos:inScheme rdf:resource="http://energy.referencedata.eu/StandardAssetTypeList"/>
    <skos:topConceptOf rdf:resource="http://energy.referencedata.eu/StandardAssetTypeList"/>
    <dcterms:identifier>B49</dcterms:identifier>
    <skos:prefLabel>Nuclear heavy water reactor</skos:prefLabel>
    <skos:definition xml:lang="en">A unit in which the heat source is a pressurized heavy-water reactor (PHWR) that is a nuclear reactor that uses heavy water (deuterium oxide D2O) as its coolant and neutron moderator.</skos:definition>
  </skos:Concept>
  <skos:Concept rdf:about="http://energy.referencedata.eu/StandardAssetTypeList/B50">
    <skos:inScheme rdf:resource="http://energy.referencedata.eu/StandardAssetTypeList"/>
    <skos:topConceptOf rdf:resource="http://energy.referencedata.eu/StandardAssetTypeList"/>
    <dcterms:identifier>B50</dcterms:identifier>
    <skos:prefLabel>Nuclear light water reactor</skos:prefLabel>
    <skos:definition xml:lang="en">A unit in which the heat source is a light-water reactor (LWR) that is a type of thermal-neutron reactor that uses normal water, as both its coolant and neutron moderator â€“ furthermore a solid form of fissile elements is used as fuel. </skos:definition>
  </skos:Concept>
  <skos:Concept rdf:about="http://energy.referencedata.eu/StandardAssetTypeList/B51">
    <skos:inScheme rdf:resource="http://energy.referencedata.eu/StandardAssetTypeList"/>
    <skos:topConceptOf rdf:resource="http://energy.referencedata.eu/StandardAssetTypeList"/>
    <dcterms:identifier>B51</dcterms:identifier>
    <skos:prefLabel>Nuclear breeder</skos:prefLabel>
    <skos:definition xml:lang="en">A unit in which the heat source is a nuclear reactor that generates more fissile material than it consumes.</skos:definition>
  </skos:Concept>
  <skos:Concept rdf:about="http://energy.referencedata.eu/StandardAssetTypeList/B52">
    <skos:inScheme rdf:resource="http://energy.referencedata.eu/StandardAssetTypeList"/>
    <skos:topConceptOf rdf:resource="http://energy.referencedata.eu/StandardAssetTypeList"/>
    <dcterms:identifier>B52</dcterms:identifier>
    <skos:prefLabel>Nuclear graphite reactor</skos:prefLabel>
    <skos:definition xml:lang="en">A unit in which the heat source is a graphite-moderated reactor that is a nuclear reactor that uses carbon as a neutron moderator, which allows natural uranium to be used as nuclear fuel.</skos:definition>
  </skos:Concept>
  <skos:Concept rdf:about="http://energy.referencedata.eu/StandardAssetTypeList/B53">
    <skos:inScheme rdf:resource="http://energy.referencedata.eu/StandardAssetTypeList"/>
    <skos:topConceptOf rdf:resource="http://energy.referencedata.eu/StandardAssetTypeList"/>
    <dcterms:identifier>B53</dcterms:identifier>
    <skos:prefLabel>Temporary energy storage</skos:prefLabel>
    <skos:definition xml:lang="en">A resource that is temporarily connected to the grid and that may store energy when connected, such as an electric vehicle.</skos:definition>
  </skos:Concept>
  <skos:Concept rdf:about="http://energy.referencedata.eu/StandardAssetTypeList/B54">
    <skos:inScheme rdf:resource="http://energy.referencedata.eu/StandardAssetTypeList"/>
    <skos:topConceptOf rdf:resource="http://energy.referencedata.eu/StandardAssetTypeList"/>
    <dcterms:identifier>B54</dcterms:identifier>
    <skos:prefLabel>Permanent energy storage</skos:prefLabel>
    <skos:definition xml:lang="en">A resource that is permanently connected to the grid and that may store energy when connected, such as a pumped hydro.</skos:definition>
  </skos:Concept>
  <skos:Concept rdf:about="http://energy.referencedata.eu/StandardAssetTypeList/B55">
    <skos:inScheme rdf:resource="http://energy.referencedata.eu/StandardAssetTypeList"/>
    <skos:topConceptOf rdf:resource="http://energy.referencedata.eu/StandardAssetTypeList"/>
    <dcterms:identifier>B55</dcterms:identifier>
    <skos:prefLabel>Electric vehicle battery</skos:prefLabel>
    <skos:definition xml:lang="en">A resource using electric vehicle batteries, commercial and private. The reason for separating vehicle batteries and non-vehicle batteries is that the vehicle batteries not necessarily is connected to the charger.</skos:definition>
  </skos:Concept>
  <skos:Concept rdf:about="http://energy.referencedata.eu/StandardAssetTypeList/B56">
    <skos:inScheme rdf:resource="http://energy.referencedata.eu/StandardAssetTypeList"/>
    <skos:topConceptOf rdf:resource="http://energy.referencedata.eu/StandardAssetTypeList"/>
    <dcterms:identifier>B56</dcterms:identifier>
    <skos:prefLabel>Heat pump specified</skos:prefLabel>
    <skos:definition xml:lang="en">A heat pump is a device that uses work to transfer heat from a cool space to a warm space by transferring thermal energy using a refrigeration cycle</skos:definition>
  </skos:Concept>
  <skos:Concept rdf:about="http://energy.referencedata.eu/StandardAssetTypeList/B57">
    <skos:inScheme rdf:resource="http://energy.referencedata.eu/StandardAssetTypeList"/>
    <skos:topConceptOf rdf:resource="http://energy.referencedata.eu/StandardAssetTypeList"/>
    <dcterms:identifier>B57</dcterms:identifier>
    <skos:prefLabel>Heat pump electrical</skos:prefLabel>
    <skos:definition xml:lang="en">A heat pump is a device that uses electricity to transfer heat from a cool space to a warm space by transferring thermal energy using a refrigeration cycle.</skos:definition>
  </skos:Concept>
  <skos:Concept rdf:about="http://energy.referencedata.eu/StandardAssetTypeList/B58">
    <skos:inScheme rdf:resource="http://energy.referencedata.eu/StandardAssetTypeList"/>
    <skos:topConceptOf rdf:resource="http://energy.referencedata.eu/StandardAssetTypeList"/>
    <dcterms:identifier>B58</dcterms:identifier>
    <skos:prefLabel>Heat pump absorption</skos:prefLabel>
    <skos:definition xml:lang="en">A heat pump is a device that uses absorption technology to transfer heat from a cool space to a warm space by transferring thermal energy using a refrigeration cycle.</skos:definition>
  </skos:Concept>
  <skos:Concept rdf:about="http://energy.referencedata.eu/StandardAssetTypeList/B59">
    <skos:inScheme rdf:resource="http://energy.referencedata.eu/StandardAssetTypeList"/>
    <skos:topConceptOf rdf:resource="http://energy.referencedata.eu/StandardAssetTypeList"/>
    <dcterms:identifier>B59</dcterms:identifier>
    <skos:prefLabel>Auxiliary power unit</skos:prefLabel>
    <skos:definition xml:lang="en">A technology that provides energy as a backup.</skos:definition>
  </skos:Concept>
  <skos:Concept rdf:about="http://energy.referencedata.eu/StandardAssetTypeList/B60">
    <skos:inScheme rdf:resource="http://energy.referencedata.eu/StandardAssetTypeList"/>
    <skos:topConceptOf rdf:resource="http://energy.referencedata.eu/StandardAssetTypeList"/>
    <dcterms:identifier>B60</dcterms:identifier>
    <skos:prefLabel>Water electrolysis unspecified</skos:prefLabel>
    <skos:definition xml:lang="en">Unspecified water electrolysis. </skos:definition>
  </skos:Concept>
  <skos:Concept rdf:about="http://energy.referencedata.eu/StandardAssetTypeList/B61">
    <skos:inScheme rdf:resource="http://energy.referencedata.eu/StandardAssetTypeList"/>
    <skos:topConceptOf rdf:resource="http://energy.referencedata.eu/StandardAssetTypeList"/>
    <dcterms:identifier>B61</dcterms:identifier>
    <skos:prefLabel>Water electrolysis low temperature unspecified</skos:prefLabel>
    <skos:definition xml:lang="en">Unspecified water electrolysis at low temperature as in an Alkaline or Proto-Exchange Membrane (PEM) fuel cell.</skos:definition>
  </skos:Concept>
  <skos:Concept rdf:about="http://energy.referencedata.eu/StandardAssetTypeList/B62">
    <skos:inScheme rdf:resource="http://energy.referencedata.eu/StandardAssetTypeList"/>
    <skos:topConceptOf rdf:resource="http://energy.referencedata.eu/StandardAssetTypeList"/>
    <dcterms:identifier>B62</dcterms:identifier>
    <skos:prefLabel>Water electrolysis low temperature main product</skos:prefLabel>
    <skos:definition xml:lang="en">Main product water electrolysis at low temperature as in an Alkaline or Proto-Exchange Membrane (PEM) fuel cell.</skos:definition>
  </skos:Concept>
  <skos:Concept rdf:about="http://energy.referencedata.eu/StandardAssetTypeList/B63">
    <skos:inScheme rdf:resource="http://energy.referencedata.eu/StandardAssetTypeList"/>
    <skos:topConceptOf rdf:resource="http://energy.referencedata.eu/StandardAssetTypeList"/>
    <dcterms:identifier>B63</dcterms:identifier>
    <skos:prefLabel>Water electrolysis high temperature unspecified</skos:prefLabel>
    <skos:definition xml:lang="en">Unspecified water electrolysis at high temperature as in a Solid Oxide Electrolysis Cell (SOEC) fuel cell.</skos:definition>
  </skos:Concept>
  <skos:Concept rdf:about="http://energy.referencedata.eu/StandardAssetTypeList/B64">
    <skos:inScheme rdf:resource="http://energy.referencedata.eu/StandardAssetTypeList"/>
    <skos:topConceptOf rdf:resource="http://energy.referencedata.eu/StandardAssetTypeList"/>
    <dcterms:identifier>B64</dcterms:identifier>
    <skos:prefLabel>Steam methane reforming unspecified</skos:prefLabel>
    <skos:definition xml:lang="en">Unspecified methane reforming.</skos:definition>
  </skos:Concept>
  <skos:Concept rdf:about="http://energy.referencedata.eu/StandardAssetTypeList/B65">
    <skos:inScheme rdf:resource="http://energy.referencedata.eu/StandardAssetTypeList"/>
    <skos:topConceptOf rdf:resource="http://energy.referencedata.eu/StandardAssetTypeList"/>
    <dcterms:identifier>B65</dcterms:identifier>
    <skos:prefLabel>Steam methane reforming without CCS/CCU  unspecified</skos:prefLabel>
    <skos:definition xml:lang="en">Main product methane reforming without Carbon Capture and Sequestration (CCS)/Carbon Capture and Use (CCU).  </skos:definition>
  </skos:Concept>
  <skos:Concept rdf:about="http://energy.referencedata.eu/StandardAssetTypeList/B66">
    <skos:inScheme rdf:resource="http://energy.referencedata.eu/StandardAssetTypeList"/>
    <skos:topConceptOf rdf:resource="http://energy.referencedata.eu/StandardAssetTypeList"/>
    <dcterms:identifier>B66</dcterms:identifier>
    <skos:prefLabel>Steam methane reforming with CCS/CCU  unspecified</skos:prefLabel>
    <skos:definition xml:lang="en">Unspecified methane reforming with Carbon Capture and Sequestration (CCS)/Carbon Capture and Use (CCU).    </skos:definition>
  </skos:Concept>
  <skos:Concept rdf:about="http://energy.referencedata.eu/StandardAssetTypeList/B67">
    <skos:inScheme rdf:resource="http://energy.referencedata.eu/StandardAssetTypeList"/>
    <skos:topConceptOf rdf:resource="http://energy.referencedata.eu/StandardAssetTypeList"/>
    <dcterms:identifier>B67</dcterms:identifier>
    <skos:prefLabel>Steam methane reforming with CCS/CCU  main product</skos:prefLabel>
    <skos:definition xml:lang="en">Main product methane reforming with Carbon Capture and Sequestration (CCS)/Carbon Capture and Use (CCU).    </skos:definition>
  </skos:Concept>
  <skos:Concept rdf:about="http://energy.referencedata.eu/StandardAssetTypeList/B68">
    <skos:inScheme rdf:resource="http://energy.referencedata.eu/StandardAssetTypeList"/>
    <skos:topConceptOf rdf:resource="http://energy.referencedata.eu/StandardAssetTypeList"/>
    <dcterms:identifier>B68</dcterms:identifier>
    <skos:prefLabel>Partial oxidation unspecified</skos:prefLabel>
    <skos:definition xml:lang="en">Unspecified partial oxidation.</skos:definition>
  </skos:Concept>
  <skos:Concept rdf:about="http://energy.referencedata.eu/StandardAssetTypeList/B69">
    <skos:inScheme rdf:resource="http://energy.referencedata.eu/StandardAssetTypeList"/>
    <skos:topConceptOf rdf:resource="http://energy.referencedata.eu/StandardAssetTypeList"/>
    <dcterms:identifier>B69</dcterms:identifier>
    <skos:prefLabel>Autothermal reforming unspecified</skos:prefLabel>
    <skos:definition xml:lang="en">Unspecified autothermal reforming.</skos:definition>
  </skos:Concept>
  <skos:Concept rdf:about="http://energy.referencedata.eu/StandardAssetTypeList/B70">
    <skos:inScheme rdf:resource="http://energy.referencedata.eu/StandardAssetTypeList"/>
    <skos:topConceptOf rdf:resource="http://energy.referencedata.eu/StandardAssetTypeList"/>
    <dcterms:identifier>B70</dcterms:identifier>
    <skos:prefLabel>Methanol reforming unspecified</skos:prefLabel>
    <skos:definition xml:lang="en">Unspecified methanol reforming.</skos:definition>
  </skos:Concept>
  <skos:Concept rdf:about="http://energy.referencedata.eu/StandardAssetTypeList/B71">
    <skos:inScheme rdf:resource="http://energy.referencedata.eu/StandardAssetTypeList"/>
    <skos:topConceptOf rdf:resource="http://energy.referencedata.eu/StandardAssetTypeList"/>
    <dcterms:identifier>B71</dcterms:identifier>
    <skos:prefLabel>Ammonia reforming unspecified</skos:prefLabel>
    <skos:definition xml:lang="en">Unspecified ammonia reforming.</skos:definition>
  </skos:Concept>
  <skos:Concept rdf:about="http://energy.referencedata.eu/StandardAssetTypeList/B72">
    <skos:inScheme rdf:resource="http://energy.referencedata.eu/StandardAssetTypeList"/>
    <skos:topConceptOf rdf:resource="http://energy.referencedata.eu/StandardAssetTypeList"/>
    <dcterms:identifier>B72</dcterms:identifier>
    <skos:prefLabel>Ammonia gasification</skos:prefLabel>
    <skos:definition xml:lang="en">Unspecified gasification.</skos:definition>
  </skos:Concept>
  <skos:Concept rdf:about="http://energy.referencedata.eu/StandardAssetTypeList/B73">
    <skos:inScheme rdf:resource="http://energy.referencedata.eu/StandardAssetTypeList"/>
    <skos:topConceptOf rdf:resource="http://energy.referencedata.eu/StandardAssetTypeList"/>
    <dcterms:identifier>B73</dcterms:identifier>
    <skos:prefLabel>Chlor-alkali electrolysis unspecified</skos:prefLabel>
    <skos:definition xml:lang="en">Unspecified alkali electrolysis.</skos:definition>
  </skos:Concept>
  <skos:Concept rdf:about="http://energy.referencedata.eu/StandardAssetTypeList/B74">
    <skos:inScheme rdf:resource="http://energy.referencedata.eu/StandardAssetTypeList"/>
    <skos:topConceptOf rdf:resource="http://energy.referencedata.eu/StandardAssetTypeList"/>
    <dcterms:identifier>B74</dcterms:identifier>
    <skos:prefLabel>Chlor-alkali electrolysis by-product</skos:prefLabel>
    <skos:definition xml:lang="en">Alkali electrolysis product.</skos:definition>
  </skos:Concept>
</rdf:RDF>
