<?xml version='1.0' encoding='UTF-8'?>
<rdf:RDF xmlns:cim="http://iec.ch/TC57/2013/CIM-schema-cim16#" xmlns:rdf="http://www.w3.org/1999/02/22-rdf-syntax-ns#" xmlns:rdfs="http://www.w3.org/2000/01/rdf-schema#" xmlns:dcat="http://www.w3.org/ns/dcat#" xmlns:dc="http://purl.org/dc/elements/1.1/" xmlns:dcterms="http://purl.org/dc/terms/" xmlns:skos="http://www.w3.org/2004/02/skos/core#" xmlns:ecl="urn:entsoe.eu:wgedi:codelists" xmlns:xs="http://www.w3.org/2001/XMLSchema">
  <skos:ConceptScheme rdf:about="http://energy.referencedata.eu/StandardAnalogTypeList">
    <rdf:type rdf:resource="http://www.w3.org/ns/dcat#Dataset"/>
    <dcterms:modified>2023-12-14</dcterms:modified>
    <dcat:version>91</dcat:version>
    <skos:prefLabel>StandardAnalogTypeList</skos:prefLabel>
    <dcterms:identifier>MXM000</dcterms:identifier>
    <skos:definition xml:lang="en">The identification of an analog value.</skos:definition>
  </skos:ConceptScheme>
  <skos:Concept rdf:about="http://energy.referencedata.eu/StandardAnalogTypeList/A01">
    <skos:inScheme rdf:resource="http://energy.referencedata.eu/StandardAnalogTypeList"/>
    <skos:topConceptOf rdf:resource="http://energy.referencedata.eu/StandardAnalogTypeList"/>
    <dcterms:identifier>A01</dcterms:identifier>
    <skos:prefLabel>Flow</skos:prefLabel>
    <skos:definition xml:lang="en">This is the computed flow for the monitored element in the constraint situation ("N situation", "N-1 situation" ...) after the capacity calculation. The flow is expressed in A, %, or MW.</skos:definition>
  </skos:Concept>
  <skos:Concept rdf:about="http://energy.referencedata.eu/StandardAnalogTypeList/A02">
    <skos:inScheme rdf:resource="http://energy.referencedata.eu/StandardAnalogTypeList"/>
    <skos:topConceptOf rdf:resource="http://energy.referencedata.eu/StandardAnalogTypeList"/>
    <dcterms:identifier>A02</dcterms:identifier>
    <skos:prefLabel>Permanent admissible transmission limit (PATL)</skos:prefLabel>
    <skos:definition xml:lang="en">The permanent load of transmission system elements which is allowed for an unlimited period and which does not cause physical damage to the transmission system elements as long as the defined threshold is respected.</skos:definition>
  </skos:Concept>
  <skos:Concept rdf:about="http://energy.referencedata.eu/StandardAnalogTypeList/A03">
    <skos:inScheme rdf:resource="http://energy.referencedata.eu/StandardAnalogTypeList"/>
    <skos:topConceptOf rdf:resource="http://energy.referencedata.eu/StandardAnalogTypeList"/>
    <dcterms:identifier>A03</dcterms:identifier>
    <skos:prefLabel>Flow reliability margin</skos:prefLabel>
    <skos:definition xml:lang="en">This is the flow reliability margin for a given critical network element. The amount of MW or A that is reserved for this critical network element and shall not be used for the computed outage situation, in order to secure the power network.</skos:definition>
  </skos:Concept>
  <skos:Concept rdf:about="http://energy.referencedata.eu/StandardAnalogTypeList/A04">
    <skos:inScheme rdf:resource="http://energy.referencedata.eu/StandardAnalogTypeList"/>
    <skos:topConceptOf rdf:resource="http://energy.referencedata.eu/StandardAnalogTypeList"/>
    <dcterms:identifier>A04</dcterms:identifier>
    <skos:prefLabel>Spanning margin value</skos:prefLabel>
    <skos:definition xml:lang="en">This is the margin that is taken into account when spanning (fall-back process) is applied. Spanning marginal value is an historical based parameter which specifies the amount of MW that reduces the RAM when spanning is applied.</skos:definition>
  </skos:Concept>
  <skos:Concept rdf:about="http://energy.referencedata.eu/StandardAnalogTypeList/A05">
    <skos:inScheme rdf:resource="http://energy.referencedata.eu/StandardAnalogTypeList"/>
    <skos:topConceptOf rdf:resource="http://energy.referencedata.eu/StandardAnalogTypeList"/>
    <dcterms:identifier>A05</dcterms:identifier>
    <skos:prefLabel>Long term allocation margin</skos:prefLabel>
    <skos:definition xml:lang="en">This is the amount of MW that is added to the capacity of the critical network element in order to automatically include the long term allocation domain into the flow based domain.</skos:definition>
  </skos:Concept>
  <skos:Concept rdf:about="http://energy.referencedata.eu/StandardAnalogTypeList/A06">
    <skos:inScheme rdf:resource="http://energy.referencedata.eu/StandardAnalogTypeList"/>
    <skos:topConceptOf rdf:resource="http://energy.referencedata.eu/StandardAnalogTypeList"/>
    <dcterms:identifier>A06</dcterms:identifier>
    <skos:prefLabel>Final adjustment margin value</skos:prefLabel>
    <skos:definition xml:lang="en">This is the margin that is manually added or subtracted to the capacity of the critical network element. A negative value for final adjustment value simulates the effect of an additional margin due to complex remedial actions (RA) which cannot be modeled and so calculated in the flow based parameter calculation. A positive value for FAV as a consequence of the verification phase of the flow based domain, leading to the need to reduce the margin on one or more CBs for system security reasons.</skos:definition>
  </skos:Concept>
  <skos:Concept rdf:about="http://energy.referencedata.eu/StandardAnalogTypeList/A07">
    <skos:inScheme rdf:resource="http://energy.referencedata.eu/StandardAnalogTypeList"/>
    <skos:topConceptOf rdf:resource="http://energy.referencedata.eu/StandardAnalogTypeList"/>
    <dcterms:identifier>A07</dcterms:identifier>
    <skos:prefLabel>Transitory admissible transmission limit (TATL)</skos:prefLabel>
    <skos:definition xml:lang="en">The temporary overload of transmission system elements which is allowed for a limited period and which does not cause physical damage to the transmission system elements as long as the defined duration and thresholds are respected.</skos:definition>
  </skos:Concept>
  <skos:Concept rdf:about="http://energy.referencedata.eu/StandardAnalogTypeList/A08">
    <skos:inScheme rdf:resource="http://energy.referencedata.eu/StandardAnalogTypeList"/>
    <skos:topConceptOf rdf:resource="http://energy.referencedata.eu/StandardAnalogTypeList"/>
    <dcterms:identifier>A08</dcterms:identifier>
    <skos:prefLabel>Long admissible flow</skos:prefLabel>
    <skos:definition xml:lang="en">This is the value, expressed in A or MW, that the overload flow in a network element shall not exceed for a duration no longer than the long duration. The long duration value depends on the TSO network operating rules.</skos:definition>
  </skos:Concept>
  <skos:Concept rdf:about="http://energy.referencedata.eu/StandardAnalogTypeList/A09">
    <skos:inScheme rdf:resource="http://energy.referencedata.eu/StandardAnalogTypeList"/>
    <skos:topConceptOf rdf:resource="http://energy.referencedata.eu/StandardAnalogTypeList"/>
    <dcterms:identifier>A09</dcterms:identifier>
    <skos:prefLabel>Negative Final adjustment margin value</skos:prefLabel>
    <skos:definition xml:lang="en">This is the margin that is manually added to the capacity of the critical network element in order to simulate the effect of an additional margin due to complex remedial actions (RA) which cannot be modeled and so calculated in the flow based parameter calculation.</skos:definition>
  </skos:Concept>
  <skos:Concept rdf:about="http://energy.referencedata.eu/StandardAnalogTypeList/A10">
    <skos:inScheme rdf:resource="http://energy.referencedata.eu/StandardAnalogTypeList"/>
    <skos:topConceptOf rdf:resource="http://energy.referencedata.eu/StandardAnalogTypeList"/>
    <dcterms:identifier>A10</dcterms:identifier>
    <skos:prefLabel>Minimum voltage level</skos:prefLabel>
    <skos:definition xml:lang="en">This is the minimum voltage that can be supported by a network element without involving a risk for the security of supply.</skos:definition>
  </skos:Concept>
  <skos:Concept rdf:about="http://energy.referencedata.eu/StandardAnalogTypeList/A11">
    <skos:inScheme rdf:resource="http://energy.referencedata.eu/StandardAnalogTypeList"/>
    <skos:topConceptOf rdf:resource="http://energy.referencedata.eu/StandardAnalogTypeList"/>
    <dcterms:identifier>A11</dcterms:identifier>
    <skos:prefLabel>Maximum voltage level</skos:prefLabel>
    <skos:definition xml:lang="en">This is the maximum voltage that can be supported by a network element without involving a risk for the security of supply.</skos:definition>
  </skos:Concept>
  <skos:Concept rdf:about="http://energy.referencedata.eu/StandardAnalogTypeList/A12">
    <skos:inScheme rdf:resource="http://energy.referencedata.eu/StandardAnalogTypeList"/>
    <skos:topConceptOf rdf:resource="http://energy.referencedata.eu/StandardAnalogTypeList"/>
    <dcterms:identifier>A12</dcterms:identifier>
    <skos:prefLabel>TATL after automatic RA</skos:prefLabel>
    <skos:definition xml:lang="en">The Transitory admissible transmission limit (TATL) which is allowed after an automatic Remedial Action (RA) has been applied.</skos:definition>
  </skos:Concept>
  <skos:Concept rdf:about="http://energy.referencedata.eu/StandardAnalogTypeList/A13">
    <skos:inScheme rdf:resource="http://energy.referencedata.eu/StandardAnalogTypeList"/>
    <skos:topConceptOf rdf:resource="http://energy.referencedata.eu/StandardAnalogTypeList"/>
    <dcterms:identifier>A13</dcterms:identifier>
    <skos:prefLabel>TATL after curative RA</skos:prefLabel>
    <skos:definition xml:lang="en">The Transitory admissible transmission limit (TATL) which is allowed after a curative Remedial Action (RA) has been applied.</skos:definition>
  </skos:Concept>
  <skos:Concept rdf:about="http://energy.referencedata.eu/StandardAnalogTypeList/A14">
    <skos:inScheme rdf:resource="http://energy.referencedata.eu/StandardAnalogTypeList"/>
    <skos:topConceptOf rdf:resource="http://energy.referencedata.eu/StandardAnalogTypeList"/>
    <dcterms:identifier>A14</dcterms:identifier>
    <skos:prefLabel>Computed Voltage</skos:prefLabel>
    <skos:definition xml:lang="en">This is the computed voltage for a given monitored element.</skos:definition>
  </skos:Concept>
  <skos:Concept rdf:about="http://energy.referencedata.eu/StandardAnalogTypeList/A15">
    <skos:inScheme rdf:resource="http://energy.referencedata.eu/StandardAnalogTypeList"/>
    <skos:topConceptOf rdf:resource="http://energy.referencedata.eu/StandardAnalogTypeList"/>
    <dcterms:identifier>A15</dcterms:identifier>
    <skos:prefLabel>Zero-Balance flow</skos:prefLabel>
    <skos:definition xml:lang="en">This is the amount of power affected by a contingency that reflects a situation with a scheduled exchange of zero.</skos:definition>
  </skos:Concept>
  <skos:Concept rdf:about="http://energy.referencedata.eu/StandardAnalogTypeList/A16">
    <skos:inScheme rdf:resource="http://energy.referencedata.eu/StandardAnalogTypeList"/>
    <skos:topConceptOf rdf:resource="http://energy.referencedata.eu/StandardAnalogTypeList"/>
    <dcterms:identifier>A16</dcterms:identifier>
    <skos:prefLabel>Available margin after remedial actions</skos:prefLabel>
    <skos:definition xml:lang="en">This is the available flow margin adjusted for the consideration of remedial actions in capacity calculation.</skos:definition>
  </skos:Concept>
  <skos:Concept rdf:about="http://energy.referencedata.eu/StandardAnalogTypeList/A17">
    <skos:inScheme rdf:resource="http://energy.referencedata.eu/StandardAnalogTypeList"/>
    <skos:topConceptOf rdf:resource="http://energy.referencedata.eu/StandardAnalogTypeList"/>
    <dcterms:identifier>A17</dcterms:identifier>
    <skos:prefLabel>Loss Factor</skos:prefLabel>
    <skos:definition xml:lang="en">This is the loss factor for an asset.</skos:definition>
  </skos:Concept>
  <skos:Concept rdf:about="http://energy.referencedata.eu/StandardAnalogTypeList/A18">
    <skos:inScheme rdf:resource="http://energy.referencedata.eu/StandardAnalogTypeList"/>
    <skos:topConceptOf rdf:resource="http://energy.referencedata.eu/StandardAnalogTypeList"/>
    <dcterms:identifier>A18</dcterms:identifier>
    <skos:prefLabel>Adjustment for minimum RAM</skos:prefLabel>
    <skos:definition xml:lang="en">This is the adjustment applied to the capacity of a branch to have a minimum RAM (Remaining Available Margin) available for commercial exchanges.</skos:definition>
  </skos:Concept>
  <skos:Concept rdf:about="http://energy.referencedata.eu/StandardAnalogTypeList/A19">
    <skos:inScheme rdf:resource="http://energy.referencedata.eu/StandardAnalogTypeList"/>
    <skos:topConceptOf rdf:resource="http://energy.referencedata.eu/StandardAnalogTypeList"/>
    <dcterms:identifier>A19</dcterms:identifier>
    <skos:prefLabel>Tap changer</skos:prefLabel>
    <skos:definition xml:lang="en">The position of a Tap changer.</skos:definition>
  </skos:Concept>
  <skos:Concept rdf:about="http://energy.referencedata.eu/StandardAnalogTypeList/A20">
    <skos:inScheme rdf:resource="http://energy.referencedata.eu/StandardAnalogTypeList"/>
    <skos:topConceptOf rdf:resource="http://energy.referencedata.eu/StandardAnalogTypeList"/>
    <dcterms:identifier>A20</dcterms:identifier>
    <skos:prefLabel>Regulator mode</skos:prefLabel>
    <skos:definition xml:lang="en">A measurement type indicating the control mode of a regulator, i.e. from voltage regulation to fixed MVAR regulation.</skos:definition>
  </skos:Concept>
  <skos:Concept rdf:about="http://energy.referencedata.eu/StandardAnalogTypeList/A21">
    <skos:inScheme rdf:resource="http://energy.referencedata.eu/StandardAnalogTypeList"/>
    <skos:topConceptOf rdf:resource="http://energy.referencedata.eu/StandardAnalogTypeList"/>
    <dcterms:identifier>A21</dcterms:identifier>
    <skos:prefLabel>Regulator set-point</skos:prefLabel>
    <skos:definition xml:lang="en">The set-point of a regulator. A regulator can be a tap changer, a synchronous machine, a SVC or a shunt.</skos:definition>
  </skos:Concept>
  <skos:Concept rdf:about="http://energy.referencedata.eu/StandardAnalogTypeList/A22">
    <skos:inScheme rdf:resource="http://energy.referencedata.eu/StandardAnalogTypeList"/>
    <skos:topConceptOf rdf:resource="http://energy.referencedata.eu/StandardAnalogTypeList"/>
    <dcterms:identifier>A22</dcterms:identifier>
    <skos:prefLabel>Reference Flow</skos:prefLabel>
    <skos:definition xml:lang="en">This is the amount of power affected by a contingency that reflects a situation with scheduled exchanges from a reference situation.</skos:definition>
  </skos:Concept>
  <skos:Concept rdf:about="http://energy.referencedata.eu/StandardAnalogTypeList/A23">
    <skos:inScheme rdf:resource="http://energy.referencedata.eu/StandardAnalogTypeList"/>
    <skos:topConceptOf rdf:resource="http://energy.referencedata.eu/StandardAnalogTypeList"/>
    <dcterms:identifier>A23</dcterms:identifier>
    <skos:prefLabel>CO2 emission</skos:prefLabel>
    <skos:definition xml:lang="en">This is the CO2 emission from one or several assets.</skos:definition>
  </skos:Concept>
  <skos:Concept rdf:about="http://energy.referencedata.eu/StandardAnalogTypeList/A24">
    <skos:inScheme rdf:resource="http://energy.referencedata.eu/StandardAnalogTypeList"/>
    <skos:topConceptOf rdf:resource="http://energy.referencedata.eu/StandardAnalogTypeList"/>
    <dcterms:identifier>A24</dcterms:identifier>
    <skos:prefLabel>Maximum admissible current (Imax)</skos:prefLabel>
    <skos:definition xml:lang="en">The maximum admissible current of a critical network element or a critical network element and contingency.</skos:definition>
  </skos:Concept>
  <skos:Concept rdf:about="http://energy.referencedata.eu/StandardAnalogTypeList/A25">
    <skos:inScheme rdf:resource="http://energy.referencedata.eu/StandardAnalogTypeList"/>
    <skos:topConceptOf rdf:resource="http://energy.referencedata.eu/StandardAnalogTypeList"/>
    <dcterms:identifier>A25</dcterms:identifier>
    <skos:prefLabel>Individual value adjustment (IVA)</skos:prefLabel>
    <skos:definition xml:lang="en">Individual value adjustment resulting from TSO validation process.
</skos:definition>
  </skos:Concept>
  <skos:Concept rdf:about="http://energy.referencedata.eu/StandardAnalogTypeList/A26">
    <skos:inScheme rdf:resource="http://energy.referencedata.eu/StandardAnalogTypeList"/>
    <skos:topConceptOf rdf:resource="http://energy.referencedata.eu/StandardAnalogTypeList"/>
    <dcterms:identifier>A26</dcterms:identifier>
    <skos:prefLabel>Linear flow approximation (F0)</skos:prefLabel>
    <skos:definition xml:lang="en">The linear approximation of a flow in the reference net position in a situation without any cross-zonal exchanges.</skos:definition>
  </skos:Concept>
  <skos:Concept rdf:about="http://energy.referencedata.eu/StandardAnalogTypeList/A27">
    <skos:inScheme rdf:resource="http://energy.referencedata.eu/StandardAnalogTypeList"/>
    <skos:topConceptOf rdf:resource="http://energy.referencedata.eu/StandardAnalogTypeList"/>
    <dcterms:identifier>A27</dcterms:identifier>
    <skos:prefLabel>Flow without commercial exchanges (F0_Wce)</skos:prefLabel>
    <skos:definition xml:lang="en">Flow per critical network element and contingency without commercial exchanges within a capacity calculation region.</skos:definition>
  </skos:Concept>
  <skos:Concept rdf:about="http://energy.referencedata.eu/StandardAnalogTypeList/A28">
    <skos:inScheme rdf:resource="http://energy.referencedata.eu/StandardAnalogTypeList"/>
    <skos:topConceptOf rdf:resource="http://energy.referencedata.eu/StandardAnalogTypeList"/>
    <dcterms:identifier>A28</dcterms:identifier>
    <skos:prefLabel>Flow without commercial exchanges between areas (F0_all)</skos:prefLabel>
    <skos:definition xml:lang="en">Flow per critical network element and contingency without commercial exchanges between bidding zones within the same or different synchronous areas.</skos:definition>
  </skos:Concept>
  <skos:Concept rdf:about="http://energy.referencedata.eu/StandardAnalogTypeList/A29">
    <skos:inScheme rdf:resource="http://energy.referencedata.eu/StandardAnalogTypeList"/>
    <skos:topConceptOf rdf:resource="http://energy.referencedata.eu/StandardAnalogTypeList"/>
    <dcterms:identifier>A29</dcterms:identifier>
    <skos:prefLabel>Flow due to non-costly remedial actions (F_nrao)</skos:prefLabel>
    <skos:definition xml:lang="en">Expected flow change due to non-costly remedial actions.</skos:definition>
  </skos:Concept>
  <skos:Concept rdf:about="http://energy.referencedata.eu/StandardAnalogTypeList/A30">
    <skos:inScheme rdf:resource="http://energy.referencedata.eu/StandardAnalogTypeList"/>
    <skos:topConceptOf rdf:resource="http://energy.referencedata.eu/StandardAnalogTypeList"/>
    <dcterms:identifier>A30</dcterms:identifier>
    <skos:prefLabel>Flow after long-term nominations (F_LTN)</skos:prefLabel>
    <skos:definition xml:lang="en">Flow after consideration of long-term nominations.</skos:definition>
  </skos:Concept>
  <skos:Concept rdf:about="http://energy.referencedata.eu/StandardAnalogTypeList/A31">
    <skos:inScheme rdf:resource="http://energy.referencedata.eu/StandardAnalogTypeList"/>
    <skos:topConceptOf rdf:resource="http://energy.referencedata.eu/StandardAnalogTypeList"/>
    <dcterms:identifier>A31</dcterms:identifier>
    <skos:prefLabel>Coordinated value adjustment (CVA)</skos:prefLabel>
    <skos:definition xml:lang="en">Coordinated value adjustment resulting from coordinated validation process.</skos:definition>
  </skos:Concept>
  <skos:Concept rdf:about="http://energy.referencedata.eu/StandardAnalogTypeList/A32">
    <skos:inScheme rdf:resource="http://energy.referencedata.eu/StandardAnalogTypeList"/>
    <skos:topConceptOf rdf:resource="http://energy.referencedata.eu/StandardAnalogTypeList"/>
    <dcterms:identifier>A32</dcterms:identifier>
    <skos:prefLabel>Minimum remaining available margin as ratio of maximum allowable power flow (Ramr)</skos:prefLabel>
    <skos:definition xml:lang="en">Percentage of the maximum allowable power flow that needs to be available as minimum Remaining Available Margin. </skos:definition>
  </skos:Concept>
  <skos:Concept rdf:about="http://energy.referencedata.eu/StandardAnalogTypeList/A33">
    <skos:inScheme rdf:resource="http://energy.referencedata.eu/StandardAnalogTypeList"/>
    <skos:topConceptOf rdf:resource="http://energy.referencedata.eu/StandardAnalogTypeList"/>
    <dcterms:identifier>A33</dcterms:identifier>
    <skos:prefLabel>Flows from already allocated cross-zonal capacities (Faac)</skos:prefLabel>
    <skos:definition xml:lang="en">Flows resulting from previously allocated cross-zonal capacities.</skos:definition>
  </skos:Concept>
  <skos:Concept rdf:about="http://energy.referencedata.eu/StandardAnalogTypeList/A34">
    <skos:inScheme rdf:resource="http://energy.referencedata.eu/StandardAnalogTypeList"/>
    <skos:topConceptOf rdf:resource="http://energy.referencedata.eu/StandardAnalogTypeList"/>
    <dcterms:identifier>A34</dcterms:identifier>
    <skos:prefLabel>Flow from remedial action (FRA)</skos:prefLabel>
    <skos:definition xml:lang="en">Flow for increasing the Remaining Available Margin due to remedial action.</skos:definition>
  </skos:Concept>
  <skos:Concept rdf:about="http://energy.referencedata.eu/StandardAnalogTypeList/A35">
    <skos:inScheme rdf:resource="http://energy.referencedata.eu/StandardAnalogTypeList"/>
    <skos:topConceptOf rdf:resource="http://energy.referencedata.eu/StandardAnalogTypeList"/>
    <dcterms:identifier>A35</dcterms:identifier>
    <skos:prefLabel>Assumed external exchanges</skos:prefLabel>
    <skos:definition xml:lang="en">Flow resulting from assumed commercial exchanges outside the region (F_uaf).</skos:definition>
  </skos:Concept>
  <skos:Concept rdf:about="http://energy.referencedata.eu/StandardAnalogTypeList/A36">
    <skos:inScheme rdf:resource="http://energy.referencedata.eu/StandardAnalogTypeList"/>
    <skos:topConceptOf rdf:resource="http://energy.referencedata.eu/StandardAnalogTypeList"/>
    <dcterms:identifier>A36</dcterms:identifier>
    <skos:prefLabel>Minimum remaining available margin target</skos:prefLabel>
    <skos:definition xml:lang="en">Target capacity for exchanges by deducing the exchanges not related to the region.</skos:definition>
  </skos:Concept>
</rdf:RDF>
