<?xml version='1.0' encoding='UTF-8'?>
<rdf:RDF xmlns:cim="http://iec.ch/TC57/2013/CIM-schema-cim16#" xmlns:rdf="http://www.w3.org/1999/02/22-rdf-syntax-ns#" xmlns:rdfs="http://www.w3.org/2000/01/rdf-schema#" xmlns:dcat="http://www.w3.org/ns/dcat#" xmlns:dc="http://purl.org/dc/elements/1.1/" xmlns:dcterms="http://purl.org/dc/terms/" xmlns:skos="http://www.w3.org/2004/02/skos/core#" xmlns:ecl="urn:entsoe.eu:wgedi:codelists" xmlns:xs="http://www.w3.org/2001/XMLSchema">
  <skos:ConceptScheme rdf:about="http://data.europa.eu/energy/StandardStatusTypeList">
    <dcterms:modified>2022-03-31</dcterms:modified>
    <dcat:version>81</dcat:version>
    <skos:prefLabel>StandardStatusTypeList</skos:prefLabel>
    <dcterms:identifier>ET0025</dcterms:identifier>
    <skos:definition xml:lang="en">The condition or position of an object with regard to its standing.</skos:definition>
  </skos:ConceptScheme>
  <skos:Concept rdf:about="http://data.europa.eu/energy/StandardStatusTypeList/A01">
    <skos:inScheme rdf:resource="http://data.europa.eu/energy/StandardStatusTypeList"/>
    <skos:topConceptOf rdf:resource="http://data.europa.eu/energy/StandardStatusTypeList"/>
    <dcterms:identifier>A01</dcterms:identifier>
    <skos:prefLabel>Intermediate</skos:prefLabel>
    <skos:definition xml:lang="en">The document is in a non finalized state.</skos:definition>
  </skos:Concept>
  <skos:Concept rdf:about="http://data.europa.eu/energy/StandardStatusTypeList/A02">
    <skos:inScheme rdf:resource="http://data.europa.eu/energy/StandardStatusTypeList"/>
    <skos:topConceptOf rdf:resource="http://data.europa.eu/energy/StandardStatusTypeList"/>
    <dcterms:identifier>A02</dcterms:identifier>
    <skos:prefLabel>Final</skos:prefLabel>
    <skos:definition xml:lang="en">The document is in a definitive state.</skos:definition>
  </skos:Concept>
  <skos:Concept rdf:about="http://data.europa.eu/energy/StandardStatusTypeList/A03">
    <skos:inScheme rdf:resource="http://data.europa.eu/energy/StandardStatusTypeList"/>
    <skos:topConceptOf rdf:resource="http://data.europa.eu/energy/StandardStatusTypeList"/>
    <dcterms:identifier>A03</dcterms:identifier>
    <skos:prefLabel>Deactivated</skos:prefLabel>
    <skos:definition xml:lang="en">The object being reported has been deactivated.</skos:definition>
  </skos:Concept>
  <skos:Concept rdf:about="http://data.europa.eu/energy/StandardStatusTypeList/A04">
    <skos:inScheme rdf:resource="http://data.europa.eu/energy/StandardStatusTypeList"/>
    <skos:topConceptOf rdf:resource="http://data.europa.eu/energy/StandardStatusTypeList"/>
    <dcterms:identifier>A04</dcterms:identifier>
    <skos:prefLabel>Reactivated</skos:prefLabel>
    <skos:definition xml:lang="en">The object being reported has been reactivated.</skos:definition>
  </skos:Concept>
  <skos:Concept rdf:about="http://data.europa.eu/energy/StandardStatusTypeList/A05">
    <skos:inScheme rdf:resource="http://data.europa.eu/energy/StandardStatusTypeList"/>
    <skos:topConceptOf rdf:resource="http://data.europa.eu/energy/StandardStatusTypeList"/>
    <dcterms:identifier>A05</dcterms:identifier>
    <skos:prefLabel>Active</skos:prefLabel>
    <skos:definition xml:lang="en">The object being reported is currently active.</skos:definition>
  </skos:Concept>
  <skos:Concept rdf:about="http://data.europa.eu/energy/StandardStatusTypeList/A06">
    <skos:inScheme rdf:resource="http://data.europa.eu/energy/StandardStatusTypeList"/>
    <skos:topConceptOf rdf:resource="http://data.europa.eu/energy/StandardStatusTypeList"/>
    <dcterms:identifier>A06</dcterms:identifier>
    <skos:prefLabel>Available</skos:prefLabel>
    <skos:definition xml:lang="en">The volumes (one or more) are available.</skos:definition>
  </skos:Concept>
  <skos:Concept rdf:about="http://data.europa.eu/energy/StandardStatusTypeList/A07">
    <skos:inScheme rdf:resource="http://data.europa.eu/energy/StandardStatusTypeList"/>
    <skos:topConceptOf rdf:resource="http://data.europa.eu/energy/StandardStatusTypeList"/>
    <dcterms:identifier>A07</dcterms:identifier>
    <skos:prefLabel>Activated</skos:prefLabel>
    <skos:definition xml:lang="en">The quantities in the time series have been activated.</skos:definition>
  </skos:Concept>
  <skos:Concept rdf:about="http://data.europa.eu/energy/StandardStatusTypeList/A08">
    <skos:inScheme rdf:resource="http://data.europa.eu/energy/StandardStatusTypeList"/>
    <skos:topConceptOf rdf:resource="http://data.europa.eu/energy/StandardStatusTypeList"/>
    <dcterms:identifier>A08</dcterms:identifier>
    <skos:prefLabel>In process</skos:prefLabel>
    <skos:definition xml:lang="en">The quantities in the time series are in the process of activation (an activation request has been made).</skos:definition>
  </skos:Concept>
  <skos:Concept rdf:about="http://data.europa.eu/energy/StandardStatusTypeList/A09">
    <skos:inScheme rdf:resource="http://data.europa.eu/energy/StandardStatusTypeList"/>
    <skos:topConceptOf rdf:resource="http://data.europa.eu/energy/StandardStatusTypeList"/>
    <dcterms:identifier>A09</dcterms:identifier>
    <skos:prefLabel>Cancelled</skos:prefLabel>
    <skos:definition xml:lang="en">The tender indicated in the time series has been completely cancelled.
In this case the resources are no longer available to all Acquiring System Operators</skos:definition>
  </skos:Concept>
  <skos:Concept rdf:about="http://data.europa.eu/energy/StandardStatusTypeList/A10">
    <skos:inScheme rdf:resource="http://data.europa.eu/energy/StandardStatusTypeList"/>
    <skos:topConceptOf rdf:resource="http://data.europa.eu/energy/StandardStatusTypeList"/>
    <dcterms:identifier>A10</dcterms:identifier>
    <skos:prefLabel>Ordered</skos:prefLabel>
    <skos:definition xml:lang="en">The quantities in the time series are to be activated.</skos:definition>
  </skos:Concept>
  <skos:Concept rdf:about="http://data.europa.eu/energy/StandardStatusTypeList/A11">
    <skos:inScheme rdf:resource="http://data.europa.eu/energy/StandardStatusTypeList"/>
    <skos:topConceptOf rdf:resource="http://data.europa.eu/energy/StandardStatusTypeList"/>
    <dcterms:identifier>A11</dcterms:identifier>
    <skos:prefLabel>Unavailable</skos:prefLabel>
    <skos:definition xml:lang="en">The volumes (one or more) are unavailable.</skos:definition>
  </skos:Concept>
  <skos:Concept rdf:about="http://data.europa.eu/energy/StandardStatusTypeList/A12">
    <skos:inScheme rdf:resource="http://data.europa.eu/energy/StandardStatusTypeList"/>
    <skos:topConceptOf rdf:resource="http://data.europa.eu/energy/StandardStatusTypeList"/>
    <dcterms:identifier>A12</dcterms:identifier>
    <skos:prefLabel>RGCE agreed</skos:prefLabel>
    <skos:definition xml:lang="en">The information has been agreed within the ENTSO-E Regional Group Continental Europe process.</skos:definition>
  </skos:Concept>
  <skos:Concept rdf:about="http://data.europa.eu/energy/StandardStatusTypeList/A13">
    <skos:inScheme rdf:resource="http://data.europa.eu/energy/StandardStatusTypeList"/>
    <skos:topConceptOf rdf:resource="http://data.europa.eu/energy/StandardStatusTypeList"/>
    <dcterms:identifier>A13</dcterms:identifier>
    <skos:prefLabel>Withdrawn</skos:prefLabel>
    <skos:definition xml:lang="en">The information has been withdrawn by the submitter.</skos:definition>
  </skos:Concept>
  <skos:Concept rdf:about="http://data.europa.eu/energy/StandardStatusTypeList/A14">
    <skos:inScheme rdf:resource="http://data.europa.eu/energy/StandardStatusTypeList"/>
    <skos:topConceptOf rdf:resource="http://data.europa.eu/energy/StandardStatusTypeList"/>
    <dcterms:identifier>A14</dcterms:identifier>
    <skos:prefLabel>Creation</skos:prefLabel>
    <skos:definition xml:lang="en">The action requested to be carried out is the creation of a new object.</skos:definition>
  </skos:Concept>
  <skos:Concept rdf:about="http://data.europa.eu/energy/StandardStatusTypeList/A15">
    <skos:inScheme rdf:resource="http://data.europa.eu/energy/StandardStatusTypeList"/>
    <skos:topConceptOf rdf:resource="http://data.europa.eu/energy/StandardStatusTypeList"/>
    <dcterms:identifier>A15</dcterms:identifier>
    <skos:prefLabel>Update</skos:prefLabel>
    <skos:definition xml:lang="en">The action requested to be carried out is the update an existing object.</skos:definition>
  </skos:Concept>
  <skos:Concept rdf:about="http://data.europa.eu/energy/StandardStatusTypeList/A16">
    <skos:inScheme rdf:resource="http://data.europa.eu/energy/StandardStatusTypeList"/>
    <skos:topConceptOf rdf:resource="http://data.europa.eu/energy/StandardStatusTypeList"/>
    <dcterms:identifier>A16</dcterms:identifier>
    <skos:prefLabel>Deactivation</skos:prefLabel>
    <skos:definition xml:lang="en">The action requested to be carried out is to deactivate an existing object.</skos:definition>
  </skos:Concept>
  <skos:Concept rdf:about="http://data.europa.eu/energy/StandardStatusTypeList/A17">
    <skos:inScheme rdf:resource="http://data.europa.eu/energy/StandardStatusTypeList"/>
    <skos:topConceptOf rdf:resource="http://data.europa.eu/energy/StandardStatusTypeList"/>
    <dcterms:identifier>A17</dcterms:identifier>
    <skos:prefLabel>Reactivation</skos:prefLabel>
    <skos:definition xml:lang="en">The action requested to be carried out is to reactivate a previously deactivated object.</skos:definition>
  </skos:Concept>
  <skos:Concept rdf:about="http://data.europa.eu/energy/StandardStatusTypeList/A18">
    <skos:inScheme rdf:resource="http://data.europa.eu/energy/StandardStatusTypeList"/>
    <skos:topConceptOf rdf:resource="http://data.europa.eu/energy/StandardStatusTypeList"/>
    <dcterms:identifier>A18</dcterms:identifier>
    <skos:prefLabel>Preventive</skos:prefLabel>
    <skos:definition xml:lang="en">The remedial action is applied to prevent an outage.</skos:definition>
  </skos:Concept>
  <skos:Concept rdf:about="http://data.europa.eu/energy/StandardStatusTypeList/A19">
    <skos:inScheme rdf:resource="http://data.europa.eu/energy/StandardStatusTypeList"/>
    <skos:topConceptOf rdf:resource="http://data.europa.eu/energy/StandardStatusTypeList"/>
    <dcterms:identifier>A19</dcterms:identifier>
    <skos:prefLabel>Curative</skos:prefLabel>
    <skos:definition xml:lang="en">The remedial action is applied after an outage has occurred, in order to maintain the operational security.</skos:definition>
  </skos:Concept>
  <skos:Concept rdf:about="http://data.europa.eu/energy/StandardStatusTypeList/A20">
    <skos:inScheme rdf:resource="http://data.europa.eu/energy/StandardStatusTypeList"/>
    <skos:topConceptOf rdf:resource="http://data.europa.eu/energy/StandardStatusTypeList"/>
    <dcterms:identifier>A20</dcterms:identifier>
    <skos:prefLabel>Automatic</skos:prefLabel>
    <skos:definition xml:lang="en">The remedial action being described is applied by an automation when an outage occurs.</skos:definition>
  </skos:Concept>
  <skos:Concept rdf:about="http://data.europa.eu/energy/StandardStatusTypeList/A21">
    <skos:inScheme rdf:resource="http://data.europa.eu/energy/StandardStatusTypeList"/>
    <skos:topConceptOf rdf:resource="http://data.europa.eu/energy/StandardStatusTypeList"/>
    <dcterms:identifier>A21</dcterms:identifier>
    <skos:prefLabel>Open</skos:prefLabel>
    <skos:definition xml:lang="en">The action being described consists of disconnecting the network element  to the transmission network.</skos:definition>
  </skos:Concept>
  <skos:Concept rdf:about="http://data.europa.eu/energy/StandardStatusTypeList/A22">
    <skos:inScheme rdf:resource="http://data.europa.eu/energy/StandardStatusTypeList"/>
    <skos:topConceptOf rdf:resource="http://data.europa.eu/energy/StandardStatusTypeList"/>
    <dcterms:identifier>A22</dcterms:identifier>
    <skos:prefLabel>Close</skos:prefLabel>
    <skos:definition xml:lang="en">The action being described consists of connecting the network element  to the transmission network.</skos:definition>
  </skos:Concept>
  <skos:Concept rdf:about="http://data.europa.eu/energy/StandardStatusTypeList/A23">
    <skos:inScheme rdf:resource="http://data.europa.eu/energy/StandardStatusTypeList"/>
    <skos:topConceptOf rdf:resource="http://data.europa.eu/energy/StandardStatusTypeList"/>
    <dcterms:identifier>A23</dcterms:identifier>
    <skos:prefLabel>Stop</skos:prefLabel>
    <skos:definition xml:lang="en">The action being described consists of stopping the production or consumption connected to a network element.</skos:definition>
  </skos:Concept>
  <skos:Concept rdf:about="http://data.europa.eu/energy/StandardStatusTypeList/A24">
    <skos:inScheme rdf:resource="http://data.europa.eu/energy/StandardStatusTypeList"/>
    <skos:topConceptOf rdf:resource="http://data.europa.eu/energy/StandardStatusTypeList"/>
    <dcterms:identifier>A24</dcterms:identifier>
    <skos:prefLabel>Start</skos:prefLabel>
    <skos:definition xml:lang="en">The action being described consists of starting the production or consumption connected to a network element.</skos:definition>
  </skos:Concept>
  <skos:Concept rdf:about="http://data.europa.eu/energy/StandardStatusTypeList/A25">
    <skos:inScheme rdf:resource="http://data.europa.eu/energy/StandardStatusTypeList"/>
    <skos:topConceptOf rdf:resource="http://data.europa.eu/energy/StandardStatusTypeList"/>
    <dcterms:identifier>A25</dcterms:identifier>
    <skos:prefLabel>Relative</skos:prefLabel>
    <skos:definition xml:lang="en">The quantity being described is a relative value to an initial state.</skos:definition>
  </skos:Concept>
  <skos:Concept rdf:about="http://data.europa.eu/energy/StandardStatusTypeList/A26">
    <skos:inScheme rdf:resource="http://data.europa.eu/energy/StandardStatusTypeList"/>
    <skos:topConceptOf rdf:resource="http://data.europa.eu/energy/StandardStatusTypeList"/>
    <dcterms:identifier>A26</dcterms:identifier>
    <skos:prefLabel>Absolute</skos:prefLabel>
    <skos:definition xml:lang="en">The quantity being described is an absolute value.</skos:definition>
  </skos:Concept>
  <skos:Concept rdf:about="http://data.europa.eu/energy/StandardStatusTypeList/A27">
    <skos:inScheme rdf:resource="http://data.europa.eu/energy/StandardStatusTypeList"/>
    <skos:topConceptOf rdf:resource="http://data.europa.eu/energy/StandardStatusTypeList"/>
    <dcterms:identifier>A27</dcterms:identifier>
    <skos:prefLabel>Curative or preventive</skos:prefLabel>
    <skos:definition xml:lang="en">The remedial action can be applied to prevent an outage or after an outage has occurred in order to maintain the operational security.</skos:definition>
  </skos:Concept>
  <skos:Concept rdf:about="http://data.europa.eu/energy/StandardStatusTypeList/A28">
    <skos:inScheme rdf:resource="http://data.europa.eu/energy/StandardStatusTypeList"/>
    <skos:topConceptOf rdf:resource="http://data.europa.eu/energy/StandardStatusTypeList"/>
    <dcterms:identifier>A28</dcterms:identifier>
    <skos:prefLabel>Unshared bid</skos:prefLabel>
    <skos:definition xml:lang="en">Used to indicate that the bid cannot be shared.</skos:definition>
  </skos:Concept>
  <skos:Concept rdf:about="http://data.europa.eu/energy/StandardStatusTypeList/A29">
    <skos:inScheme rdf:resource="http://data.europa.eu/energy/StandardStatusTypeList"/>
    <skos:topConceptOf rdf:resource="http://data.europa.eu/energy/StandardStatusTypeList"/>
    <dcterms:identifier>A29</dcterms:identifier>
    <skos:prefLabel>Pre Processed</skos:prefLabel>
    <skos:definition xml:lang="en">to be process</skos:definition>
  </skos:Concept>
  <skos:Concept rdf:about="http://data.europa.eu/energy/StandardStatusTypeList/A30">
    <skos:inScheme rdf:resource="http://data.europa.eu/energy/StandardStatusTypeList"/>
    <skos:topConceptOf rdf:resource="http://data.europa.eu/energy/StandardStatusTypeList"/>
    <dcterms:identifier>A30</dcterms:identifier>
    <skos:prefLabel>Substituted</skos:prefLabel>
    <skos:definition xml:lang="en">Substituted pre-processing data.</skos:definition>
  </skos:Concept>
  <skos:Concept rdf:about="http://data.europa.eu/energy/StandardStatusTypeList/A31">
    <skos:inScheme rdf:resource="http://data.europa.eu/energy/StandardStatusTypeList"/>
    <skos:topConceptOf rdf:resource="http://data.europa.eu/energy/StandardStatusTypeList"/>
    <dcterms:identifier>A31</dcterms:identifier>
    <skos:prefLabel>Modified</skos:prefLabel>
    <skos:definition xml:lang="en">Modified pre-processing data by RSC or CGMA platform.</skos:definition>
  </skos:Concept>
  <skos:Concept rdf:about="http://data.europa.eu/energy/StandardStatusTypeList/A32">
    <skos:inScheme rdf:resource="http://data.europa.eu/energy/StandardStatusTypeList"/>
    <skos:topConceptOf rdf:resource="http://data.europa.eu/energy/StandardStatusTypeList"/>
    <dcterms:identifier>A32</dcterms:identifier>
    <skos:prefLabel>Result</skos:prefLabel>
    <skos:definition xml:lang="en">Result</skos:definition>
  </skos:Concept>
  <skos:Concept rdf:about="http://data.europa.eu/energy/StandardStatusTypeList/A33">
    <skos:inScheme rdf:resource="http://data.europa.eu/energy/StandardStatusTypeList"/>
    <skos:topConceptOf rdf:resource="http://data.europa.eu/energy/StandardStatusTypeList"/>
    <dcterms:identifier>A33</dcterms:identifier>
    <skos:prefLabel>Not satisfied</skos:prefLabel>
    <skos:definition xml:lang="en">The need described in the time series cannot be satisfied.</skos:definition>
  </skos:Concept>
  <skos:Concept rdf:about="http://data.europa.eu/energy/StandardStatusTypeList/A34">
    <skos:inScheme rdf:resource="http://data.europa.eu/energy/StandardStatusTypeList"/>
    <skos:topConceptOf rdf:resource="http://data.europa.eu/energy/StandardStatusTypeList"/>
    <dcterms:identifier>A34</dcterms:identifier>
    <skos:prefLabel>Rejected</skos:prefLabel>
    <skos:definition xml:lang="en">The document rejected by one or more parties.</skos:definition>
  </skos:Concept>
  <skos:Concept rdf:about="http://data.europa.eu/energy/StandardStatusTypeList/A35">
    <skos:inScheme rdf:resource="http://data.europa.eu/energy/StandardStatusTypeList"/>
    <skos:topConceptOf rdf:resource="http://data.europa.eu/energy/StandardStatusTypeList"/>
    <dcterms:identifier>A35</dcterms:identifier>
    <skos:prefLabel>Preliminary</skos:prefLabel>
    <skos:definition xml:lang="en">Indicative information only for initial planning purposes.</skos:definition>
  </skos:Concept>
  <skos:Concept rdf:about="http://data.europa.eu/energy/StandardStatusTypeList/A36">
    <skos:inScheme rdf:resource="http://data.europa.eu/energy/StandardStatusTypeList"/>
    <skos:topConceptOf rdf:resource="http://data.europa.eu/energy/StandardStatusTypeList"/>
    <dcterms:identifier>A36</dcterms:identifier>
    <skos:prefLabel>Planned</skos:prefLabel>
    <skos:definition xml:lang="en">Is planned.</skos:definition>
  </skos:Concept>
  <skos:Concept rdf:about="http://data.europa.eu/energy/StandardStatusTypeList/A37">
    <skos:inScheme rdf:resource="http://data.europa.eu/energy/StandardStatusTypeList"/>
    <skos:topConceptOf rdf:resource="http://data.europa.eu/energy/StandardStatusTypeList"/>
    <dcterms:identifier>A37</dcterms:identifier>
    <skos:prefLabel>Confirmed</skos:prefLabel>
    <skos:definition xml:lang="en">The status is  confirmed.</skos:definition>
  </skos:Concept>
  <skos:Concept rdf:about="http://data.europa.eu/energy/StandardStatusTypeList/A38">
    <skos:inScheme rdf:resource="http://data.europa.eu/energy/StandardStatusTypeList"/>
    <skos:topConceptOf rdf:resource="http://data.europa.eu/energy/StandardStatusTypeList"/>
    <dcterms:identifier>A38</dcterms:identifier>
    <skos:prefLabel>Shall Be Used</skos:prefLabel>
    <skos:definition xml:lang="en">The object defined in the series shall be used.</skos:definition>
  </skos:Concept>
  <skos:Concept rdf:about="http://data.europa.eu/energy/StandardStatusTypeList/A39">
    <skos:inScheme rdf:resource="http://data.europa.eu/energy/StandardStatusTypeList"/>
    <skos:topConceptOf rdf:resource="http://data.europa.eu/energy/StandardStatusTypeList"/>
    <dcterms:identifier>A39</dcterms:identifier>
    <skos:prefLabel>Could Be Used</skos:prefLabel>
    <skos:definition xml:lang="en">The object defined in the series could be used.</skos:definition>
  </skos:Concept>
  <skos:Concept rdf:about="http://data.europa.eu/energy/StandardStatusTypeList/A40">
    <skos:inScheme rdf:resource="http://data.europa.eu/energy/StandardStatusTypeList"/>
    <skos:topConceptOf rdf:resource="http://data.europa.eu/energy/StandardStatusTypeList"/>
    <dcterms:identifier>A40</dcterms:identifier>
    <skos:prefLabel>Proposed</skos:prefLabel>
    <skos:definition xml:lang="en">The status of the information is proposed.</skos:definition>
  </skos:Concept>
  <skos:Concept rdf:about="http://data.europa.eu/energy/StandardStatusTypeList/A41">
    <skos:inScheme rdf:resource="http://data.europa.eu/energy/StandardStatusTypeList"/>
    <skos:topConceptOf rdf:resource="http://data.europa.eu/energy/StandardStatusTypeList"/>
    <dcterms:identifier>A41</dcterms:identifier>
    <skos:prefLabel>Individual Network Data</skos:prefLabel>
    <skos:definition xml:lang="en">The network data provided in the document or series concerns the the unique TSO area describes by the document or series.</skos:definition>
  </skos:Concept>
  <skos:Concept rdf:about="http://data.europa.eu/energy/StandardStatusTypeList/A42">
    <skos:inScheme rdf:resource="http://data.europa.eu/energy/StandardStatusTypeList"/>
    <skos:topConceptOf rdf:resource="http://data.europa.eu/energy/StandardStatusTypeList"/>
    <dcterms:identifier>A42</dcterms:identifier>
    <skos:prefLabel>Common Network Data</skos:prefLabel>
    <skos:definition xml:lang="en">The network data provided in the document or series concerns the whole area describes by the document or series.</skos:definition>
  </skos:Concept>
  <skos:Concept rdf:about="http://data.europa.eu/energy/StandardStatusTypeList/A43">
    <skos:inScheme rdf:resource="http://data.europa.eu/energy/StandardStatusTypeList"/>
    <skos:topConceptOf rdf:resource="http://data.europa.eu/energy/StandardStatusTypeList"/>
    <dcterms:identifier>A43</dcterms:identifier>
    <skos:prefLabel>Setpoint schedule</skos:prefLabel>
    <skos:definition xml:lang="en">The code for the power setpoint mode of operation of the HVDC link.</skos:definition>
  </skos:Concept>
  <skos:Concept rdf:about="http://data.europa.eu/energy/StandardStatusTypeList/A44">
    <skos:inScheme rdf:resource="http://data.europa.eu/energy/StandardStatusTypeList"/>
    <skos:topConceptOf rdf:resource="http://data.europa.eu/energy/StandardStatusTypeList"/>
    <dcterms:identifier>A44</dcterms:identifier>
    <skos:prefLabel>Proportional external signal</skos:prefLabel>
    <skos:definition xml:lang="en">The code for the proportional external signal mode of operation of the HVDC link.</skos:definition>
  </skos:Concept>
  <skos:Concept rdf:about="http://data.europa.eu/energy/StandardStatusTypeList/A45">
    <skos:inScheme rdf:resource="http://data.europa.eu/energy/StandardStatusTypeList"/>
    <skos:topConceptOf rdf:resource="http://data.europa.eu/energy/StandardStatusTypeList"/>
    <dcterms:identifier>A45</dcterms:identifier>
    <skos:prefLabel>AC emulation</skos:prefLabel>
    <skos:definition xml:lang="en">The code for the AC emulation mode of operation of the HVDC link.</skos:definition>
  </skos:Concept>
  <skos:Concept rdf:about="http://data.europa.eu/energy/StandardStatusTypeList/A46">
    <skos:inScheme rdf:resource="http://data.europa.eu/energy/StandardStatusTypeList"/>
    <skos:topConceptOf rdf:resource="http://data.europa.eu/energy/StandardStatusTypeList"/>
    <dcterms:identifier>A46</dcterms:identifier>
    <skos:prefLabel>Importing element</skos:prefLabel>
    <skos:definition xml:lang="en">An importing network element in which the flow measurement enters.</skos:definition>
  </skos:Concept>
  <skos:Concept rdf:about="http://data.europa.eu/energy/StandardStatusTypeList/A47">
    <skos:inScheme rdf:resource="http://data.europa.eu/energy/StandardStatusTypeList"/>
    <skos:topConceptOf rdf:resource="http://data.europa.eu/energy/StandardStatusTypeList"/>
    <dcterms:identifier>A47</dcterms:identifier>
    <skos:prefLabel>Exporting element</skos:prefLabel>
    <skos:definition xml:lang="en">An exporting network element from which the flow measurement comes out.</skos:definition>
  </skos:Concept>
  <skos:Concept rdf:about="http://data.europa.eu/energy/StandardStatusTypeList/A48">
    <skos:inScheme rdf:resource="http://data.europa.eu/energy/StandardStatusTypeList"/>
    <skos:topConceptOf rdf:resource="http://data.europa.eu/energy/StandardStatusTypeList"/>
    <dcterms:identifier>A48</dcterms:identifier>
    <skos:prefLabel>To be optimized</skos:prefLabel>
    <skos:definition xml:lang="en">Describes an element which needs to be optimized by an optimization process.</skos:definition>
  </skos:Concept>
  <skos:Concept rdf:about="http://data.europa.eu/energy/StandardStatusTypeList/A49">
    <skos:inScheme rdf:resource="http://data.europa.eu/energy/StandardStatusTypeList"/>
    <skos:topConceptOf rdf:resource="http://data.europa.eu/energy/StandardStatusTypeList"/>
    <dcterms:identifier>A49</dcterms:identifier>
    <skos:prefLabel>To be monitored</skos:prefLabel>
    <skos:definition xml:lang="en">Describes an element which needs to be monitored by an optimization process.</skos:definition>
  </skos:Concept>
  <skos:Concept rdf:about="http://data.europa.eu/energy/StandardStatusTypeList/A50">
    <skos:inScheme rdf:resource="http://data.europa.eu/energy/StandardStatusTypeList"/>
    <skos:topConceptOf rdf:resource="http://data.europa.eu/energy/StandardStatusTypeList"/>
    <dcterms:identifier>A50</dcterms:identifier>
    <skos:prefLabel>To be included in capacity calculation</skos:prefLabel>
    <skos:definition xml:lang="en">Describes an element which needs to be taken into account in a capacity calculation process.</skos:definition>
  </skos:Concept>
  <skos:Concept rdf:about="http://data.europa.eu/energy/StandardStatusTypeList/A51">
    <skos:inScheme rdf:resource="http://data.europa.eu/energy/StandardStatusTypeList"/>
    <skos:topConceptOf rdf:resource="http://data.europa.eu/energy/StandardStatusTypeList"/>
    <dcterms:identifier>A51</dcterms:identifier>
    <skos:prefLabel>Relative to previous point in time</skos:prefLabel>
    <skos:definition xml:lang="en">The quantity being described is a relative value to a previous point in time.</skos:definition>
  </skos:Concept>
  <skos:Concept rdf:about="http://data.europa.eu/energy/StandardStatusTypeList/A52">
    <skos:inScheme rdf:resource="http://data.europa.eu/energy/StandardStatusTypeList"/>
    <skos:topConceptOf rdf:resource="http://data.europa.eu/energy/StandardStatusTypeList"/>
    <dcterms:identifier>A52</dcterms:identifier>
    <skos:prefLabel>For flow optimization</skos:prefLabel>
    <skos:definition xml:lang="en">Describes an element which needs to be optimized by a flow optimization process.</skos:definition>
  </skos:Concept>
  <skos:Concept rdf:about="http://data.europa.eu/energy/StandardStatusTypeList/A53">
    <skos:inScheme rdf:resource="http://data.europa.eu/energy/StandardStatusTypeList"/>
    <skos:topConceptOf rdf:resource="http://data.europa.eu/energy/StandardStatusTypeList"/>
    <dcterms:identifier>A53</dcterms:identifier>
    <skos:prefLabel>For voltage optimization</skos:prefLabel>
    <skos:definition xml:lang="en">Describes an element which needs to be optimized by a voltage optimization process.</skos:definition>
  </skos:Concept>
  <skos:Concept rdf:about="http://data.europa.eu/energy/StandardStatusTypeList/A54">
    <skos:inScheme rdf:resource="http://data.europa.eu/energy/StandardStatusTypeList"/>
    <skos:topConceptOf rdf:resource="http://data.europa.eu/energy/StandardStatusTypeList"/>
    <dcterms:identifier>A54</dcterms:identifier>
    <skos:prefLabel>Presolved</skos:prefLabel>
    <skos:definition xml:lang="en">Describes an active constraint that limits the exchanges. It is part of the presolved domain.</skos:definition>
  </skos:Concept>
  <skos:Concept rdf:about="http://data.europa.eu/energy/StandardStatusTypeList/A55">
    <skos:inScheme rdf:resource="http://data.europa.eu/energy/StandardStatusTypeList"/>
    <skos:topConceptOf rdf:resource="http://data.europa.eu/energy/StandardStatusTypeList"/>
    <dcterms:identifier>A55</dcterms:identifier>
    <skos:prefLabel>Not available if linked bid activated</skos:prefLabel>
    <skos:definition xml:lang="en">Bid not available if linked bid activated.</skos:definition>
  </skos:Concept>
  <skos:Concept rdf:about="http://data.europa.eu/energy/StandardStatusTypeList/A56">
    <skos:inScheme rdf:resource="http://data.europa.eu/energy/StandardStatusTypeList"/>
    <skos:topConceptOf rdf:resource="http://data.europa.eu/energy/StandardStatusTypeList"/>
    <dcterms:identifier>A56</dcterms:identifier>
    <skos:prefLabel>Not available if linked bid rejected</skos:prefLabel>
    <skos:definition xml:lang="en">Bid not available if linked bid rejected.</skos:definition>
  </skos:Concept>
  <skos:Concept rdf:about="http://data.europa.eu/energy/StandardStatusTypeList/A57">
    <skos:inScheme rdf:resource="http://data.europa.eu/energy/StandardStatusTypeList"/>
    <skos:topConceptOf rdf:resource="http://data.europa.eu/energy/StandardStatusTypeList"/>
    <dcterms:identifier>A57</dcterms:identifier>
    <skos:prefLabel>Not available for DA if linked bid subject to DA</skos:prefLabel>
    <skos:definition xml:lang="en">Bid not available for direct activation if linked bid subject to direct activation.</skos:definition>
  </skos:Concept>
  <skos:Concept rdf:about="http://data.europa.eu/energy/StandardStatusTypeList/A58">
    <skos:inScheme rdf:resource="http://data.europa.eu/energy/StandardStatusTypeList"/>
    <skos:topConceptOf rdf:resource="http://data.europa.eu/energy/StandardStatusTypeList"/>
    <dcterms:identifier>A58</dcterms:identifier>
    <skos:prefLabel>Not available for DA if linked bid subject to SA</skos:prefLabel>
    <skos:definition xml:lang="en">Bid not available for direct activation if linked bid subject to scheduled activation.</skos:definition>
  </skos:Concept>
  <skos:Concept rdf:about="http://data.europa.eu/energy/StandardStatusTypeList/A59">
    <skos:inScheme rdf:resource="http://data.europa.eu/energy/StandardStatusTypeList"/>
    <skos:topConceptOf rdf:resource="http://data.europa.eu/energy/StandardStatusTypeList"/>
    <dcterms:identifier>A59</dcterms:identifier>
    <skos:prefLabel>Not available if linked bid subject to SA</skos:prefLabel>
    <skos:definition xml:lang="en">Bid not available if linked bid subject to scheduled activation.</skos:definition>
  </skos:Concept>
  <skos:Concept rdf:about="http://data.europa.eu/energy/StandardStatusTypeList/A60">
    <skos:inScheme rdf:resource="http://data.europa.eu/energy/StandardStatusTypeList"/>
    <skos:topConceptOf rdf:resource="http://data.europa.eu/energy/StandardStatusTypeList"/>
    <dcterms:identifier>A60</dcterms:identifier>
    <skos:prefLabel>Not available if linked bid subject to DA</skos:prefLabel>
    <skos:definition xml:lang="en">Bid not available if linked bid subject to direct activation.</skos:definition>
  </skos:Concept>
  <skos:Concept rdf:about="http://data.europa.eu/energy/StandardStatusTypeList/A61">
    <skos:inScheme rdf:resource="http://data.europa.eu/energy/StandardStatusTypeList"/>
    <skos:topConceptOf rdf:resource="http://data.europa.eu/energy/StandardStatusTypeList"/>
    <dcterms:identifier>A61</dcterms:identifier>
    <skos:prefLabel>Primary market</skos:prefLabel>
    <skos:definition xml:lang="en">A value is traded for the first time.</skos:definition>
  </skos:Concept>
  <skos:Concept rdf:about="http://data.europa.eu/energy/StandardStatusTypeList/A62">
    <skos:inScheme rdf:resource="http://data.europa.eu/energy/StandardStatusTypeList"/>
    <skos:topConceptOf rdf:resource="http://data.europa.eu/energy/StandardStatusTypeList"/>
    <dcterms:identifier>A62</dcterms:identifier>
    <skos:prefLabel>Secondary market</skos:prefLabel>
    <skos:definition xml:lang="en">A value is traded for the second or next times between two parties.</skos:definition>
  </skos:Concept>
  <skos:Concept rdf:about="http://data.europa.eu/energy/StandardStatusTypeList/A63">
    <skos:inScheme rdf:resource="http://data.europa.eu/energy/StandardStatusTypeList"/>
    <skos:topConceptOf rdf:resource="http://data.europa.eu/energy/StandardStatusTypeList"/>
    <dcterms:identifier>A63</dcterms:identifier>
    <skos:prefLabel>Interesting</skos:prefLabel>
    <skos:definition xml:lang="en">Describes an asset which is considered as interesting.</skos:definition>
  </skos:Concept>
  <skos:Concept rdf:about="http://data.europa.eu/energy/StandardStatusTypeList/A64">
    <skos:inScheme rdf:resource="http://data.europa.eu/energy/StandardStatusTypeList"/>
    <skos:topConceptOf rdf:resource="http://data.europa.eu/energy/StandardStatusTypeList"/>
    <dcterms:identifier>A64</dcterms:identifier>
    <skos:prefLabel>Relevant</skos:prefLabel>
    <skos:definition xml:lang="en">Describes an asset which is considered as relevant.</skos:definition>
  </skos:Concept>
  <skos:Concept rdf:about="http://data.europa.eu/energy/StandardStatusTypeList/A65">
    <skos:inScheme rdf:resource="http://data.europa.eu/energy/StandardStatusTypeList"/>
    <skos:topConceptOf rdf:resource="http://data.europa.eu/energy/StandardStatusTypeList"/>
    <dcterms:identifier>A65</dcterms:identifier>
    <skos:prefLabel>Conditionally available</skos:prefLabel>
    <skos:definition xml:lang="en">Bid available as long as none of the conditions associated with the linked bids materialise.</skos:definition>
  </skos:Concept>
  <skos:Concept rdf:about="http://data.europa.eu/energy/StandardStatusTypeList/A66">
    <skos:inScheme rdf:resource="http://data.europa.eu/energy/StandardStatusTypeList"/>
    <skos:topConceptOf rdf:resource="http://data.europa.eu/energy/StandardStatusTypeList"/>
    <dcterms:identifier>A66</dcterms:identifier>
    <skos:prefLabel>Conditionally unavailable</skos:prefLabel>
    <skos:definition xml:lang="en">Bid unavailable as long as none of the conditions associated with the linked bids materialise.</skos:definition>
  </skos:Concept>
  <skos:Concept rdf:about="http://data.europa.eu/energy/StandardStatusTypeList/A67">
    <skos:inScheme rdf:resource="http://data.europa.eu/energy/StandardStatusTypeList"/>
    <skos:topConceptOf rdf:resource="http://data.europa.eu/energy/StandardStatusTypeList"/>
    <dcterms:identifier>A67</dcterms:identifier>
    <skos:prefLabel>Available if linked bid activated</skos:prefLabel>
    <skos:definition xml:lang="en">Bid available if linked bid activated.</skos:definition>
  </skos:Concept>
  <skos:Concept rdf:about="http://data.europa.eu/energy/StandardStatusTypeList/A68">
    <skos:inScheme rdf:resource="http://data.europa.eu/energy/StandardStatusTypeList"/>
    <skos:topConceptOf rdf:resource="http://data.europa.eu/energy/StandardStatusTypeList"/>
    <dcterms:identifier>A68</dcterms:identifier>
    <skos:prefLabel>Available if linked bid rejected</skos:prefLabel>
    <skos:definition xml:lang="en">Bid available if linked bid rejected.</skos:definition>
  </skos:Concept>
  <skos:Concept rdf:about="http://data.europa.eu/energy/StandardStatusTypeList/A69">
    <skos:inScheme rdf:resource="http://data.europa.eu/energy/StandardStatusTypeList"/>
    <skos:topConceptOf rdf:resource="http://data.europa.eu/energy/StandardStatusTypeList"/>
    <dcterms:identifier>A69</dcterms:identifier>
    <skos:prefLabel>Available if linked bid subject to SA</skos:prefLabel>
    <skos:definition xml:lang="en">Bid available if linked bid subject to scheduled activation.</skos:definition>
  </skos:Concept>
  <skos:Concept rdf:about="http://data.europa.eu/energy/StandardStatusTypeList/A70">
    <skos:inScheme rdf:resource="http://data.europa.eu/energy/StandardStatusTypeList"/>
    <skos:topConceptOf rdf:resource="http://data.europa.eu/energy/StandardStatusTypeList"/>
    <dcterms:identifier>A70</dcterms:identifier>
    <skos:prefLabel>Available if linked bid subject to DA</skos:prefLabel>
    <skos:definition xml:lang="en">Bid available if linked bid subject to direct activation.</skos:definition>
  </skos:Concept>
  <skos:Concept rdf:about="http://data.europa.eu/energy/StandardStatusTypeList/A71">
    <skos:inScheme rdf:resource="http://data.europa.eu/energy/StandardStatusTypeList"/>
    <skos:topConceptOf rdf:resource="http://data.europa.eu/energy/StandardStatusTypeList"/>
    <dcterms:identifier>A71</dcterms:identifier>
    <skos:prefLabel>Available for DA if linked bid subject to DA</skos:prefLabel>
    <skos:definition xml:lang="en">Bid available for direct activation if linked bid subject to direct activation.</skos:definition>
  </skos:Concept>
  <skos:Concept rdf:about="http://data.europa.eu/energy/StandardStatusTypeList/A72">
    <skos:inScheme rdf:resource="http://data.europa.eu/energy/StandardStatusTypeList"/>
    <skos:topConceptOf rdf:resource="http://data.europa.eu/energy/StandardStatusTypeList"/>
    <dcterms:identifier>A72</dcterms:identifier>
    <skos:prefLabel>Available for DA if linked bid subject to SA</skos:prefLabel>
    <skos:definition xml:lang="en">Bid available for direct activation if linked bid subject to scheduled activation.</skos:definition>
  </skos:Concept>
</rdf:RDF>
