<?xml version='1.0' encoding='UTF-8'?>
<rdf:RDF xmlns:cim="http://iec.ch/TC57/2013/CIM-schema-cim16#" xmlns:rdf="http://www.w3.org/1999/02/22-rdf-syntax-ns#" xmlns:rdfs="http://www.w3.org/2000/01/rdf-schema#" xmlns:dcat="http://www.w3.org/ns/dcat#" xmlns:dc="http://purl.org/dc/elements/1.1/" xmlns:dcterms="http://purl.org/dc/terms/" xmlns:skos="http://www.w3.org/2004/02/skos/core#" xmlns:ecl="urn:entsoe.eu:wgedi:codelists" xmlns:xs="http://www.w3.org/2001/XMLSchema">
  <skos:ConceptScheme rdf:about="http://data.europa.eu/energy/StandardBusinessTypeList">
    <dcterms:modified>2022-03-31</dcterms:modified>
    <dcat:version>81</dcat:version>
    <skos:prefLabel>StandardBusinessTypeList</skos:prefLabel>
    <dcterms:identifier>ET0017</dcterms:identifier>
    <skos:definition xml:lang="en">The exact business nature identifying the principal characteristic of a time series.</skos:definition>
  </skos:ConceptScheme>
  <skos:Concept rdf:about="http://data.europa.eu/energy/StandardBusinessTypeList/A01">
    <skos:inScheme rdf:resource="http://data.europa.eu/energy/StandardBusinessTypeList"/>
    <skos:topConceptOf rdf:resource="http://data.europa.eu/energy/StandardBusinessTypeList"/>
    <dcterms:identifier>A01</dcterms:identifier>
    <skos:prefLabel>Production</skos:prefLabel>
    <skos:definition xml:lang="en">The nature of the business being described is production details.</skos:definition>
  </skos:Concept>
  <skos:Concept rdf:about="http://data.europa.eu/energy/StandardBusinessTypeList/A02">
    <skos:inScheme rdf:resource="http://data.europa.eu/energy/StandardBusinessTypeList"/>
    <skos:topConceptOf rdf:resource="http://data.europa.eu/energy/StandardBusinessTypeList"/>
    <dcterms:identifier>A02</dcterms:identifier>
    <skos:prefLabel>Internal trade</skos:prefLabel>
    <skos:definition xml:lang="en">The nature of the business being described is internal trade details.</skos:definition>
  </skos:Concept>
  <skos:Concept rdf:about="http://data.europa.eu/energy/StandardBusinessTypeList/A03">
    <skos:inScheme rdf:resource="http://data.europa.eu/energy/StandardBusinessTypeList"/>
    <skos:topConceptOf rdf:resource="http://data.europa.eu/energy/StandardBusinessTypeList"/>
    <dcterms:identifier>A03</dcterms:identifier>
    <skos:prefLabel>External trade explicit capacity</skos:prefLabel>
    <skos:definition xml:lang="en">The nature of the business being described is external trade details between two areas with limited capacity requiring a capacity agreement identification.</skos:definition>
  </skos:Concept>
  <skos:Concept rdf:about="http://data.europa.eu/energy/StandardBusinessTypeList/A04">
    <skos:inScheme rdf:resource="http://data.europa.eu/energy/StandardBusinessTypeList"/>
    <skos:topConceptOf rdf:resource="http://data.europa.eu/energy/StandardBusinessTypeList"/>
    <dcterms:identifier>A04</dcterms:identifier>
    <skos:prefLabel>Consumption</skos:prefLabel>
    <skos:definition xml:lang="en">The nature of the business being described is consumption details.</skos:definition>
  </skos:Concept>
  <skos:Concept rdf:about="http://data.europa.eu/energy/StandardBusinessTypeList/A05">
    <skos:inScheme rdf:resource="http://data.europa.eu/energy/StandardBusinessTypeList"/>
    <skos:topConceptOf rdf:resource="http://data.europa.eu/energy/StandardBusinessTypeList"/>
    <dcterms:identifier>A05</dcterms:identifier>
    <skos:prefLabel>External trade total</skos:prefLabel>
    <skos:definition xml:lang="en">The nature of the business being described is external trade total.</skos:definition>
  </skos:Concept>
  <skos:Concept rdf:about="http://data.europa.eu/energy/StandardBusinessTypeList/A06">
    <skos:inScheme rdf:resource="http://data.europa.eu/energy/StandardBusinessTypeList"/>
    <skos:topConceptOf rdf:resource="http://data.europa.eu/energy/StandardBusinessTypeList"/>
    <dcterms:identifier>A06</dcterms:identifier>
    <skos:prefLabel>External trade without explicit capacity</skos:prefLabel>
    <skos:definition xml:lang="en">The nature of the business being described is external trade details between two areas without requiring capacity allocation information.</skos:definition>
  </skos:Concept>
  <skos:Concept rdf:about="http://data.europa.eu/energy/StandardBusinessTypeList/A07">
    <skos:inScheme rdf:resource="http://data.europa.eu/energy/StandardBusinessTypeList"/>
    <skos:topConceptOf rdf:resource="http://data.europa.eu/energy/StandardBusinessTypeList"/>
    <dcterms:identifier>A07</dcterms:identifier>
    <skos:prefLabel>Net Production / Consumption</skos:prefLabel>
    <skos:definition xml:lang="en">Net production/consumption - where signed values will be used. 
With the following rules: In area=Out area, In party=Out party, + means production and - means consumption.</skos:definition>
  </skos:Concept>
  <skos:Concept rdf:about="http://data.europa.eu/energy/StandardBusinessTypeList/A08">
    <skos:inScheme rdf:resource="http://data.europa.eu/energy/StandardBusinessTypeList"/>
    <skos:topConceptOf rdf:resource="http://data.europa.eu/energy/StandardBusinessTypeList"/>
    <dcterms:identifier>A08</dcterms:identifier>
    <skos:prefLabel>Net internal trade</skos:prefLabel>
    <skos:definition xml:lang="en">Net internal trade - where the direction from out party (seller) to in party (buyer) is positive and the opposite direction is negative (with minus signs).</skos:definition>
  </skos:Concept>
  <skos:Concept rdf:about="http://data.europa.eu/energy/StandardBusinessTypeList/A09">
    <skos:inScheme rdf:resource="http://data.europa.eu/energy/StandardBusinessTypeList"/>
    <skos:topConceptOf rdf:resource="http://data.europa.eu/energy/StandardBusinessTypeList"/>
    <dcterms:identifier>A09</dcterms:identifier>
    <skos:prefLabel>IPP (Independent Power Producer)</skos:prefLabel>
    <skos:definition xml:lang="en">A time series concerning the production schedule from an IPP.</skos:definition>
  </skos:Concept>
  <skos:Concept rdf:about="http://data.europa.eu/energy/StandardBusinessTypeList/A10">
    <skos:inScheme rdf:resource="http://data.europa.eu/energy/StandardBusinessTypeList"/>
    <skos:topConceptOf rdf:resource="http://data.europa.eu/energy/StandardBusinessTypeList"/>
    <dcterms:identifier>A10</dcterms:identifier>
    <skos:prefLabel>Tertiary control </skos:prefLabel>
    <skos:definition xml:lang="en">A time series concerning tertiary reserve.</skos:definition>
  </skos:Concept>
  <skos:Concept rdf:about="http://data.europa.eu/energy/StandardBusinessTypeList/A11">
    <skos:inScheme rdf:resource="http://data.europa.eu/energy/StandardBusinessTypeList"/>
    <skos:topConceptOf rdf:resource="http://data.europa.eu/energy/StandardBusinessTypeList"/>
    <dcterms:identifier>A11</dcterms:identifier>
    <skos:prefLabel>Primary control</skos:prefLabel>
    <skos:definition xml:lang="en">A time series concerning primary reserve.</skos:definition>
  </skos:Concept>
  <skos:Concept rdf:about="http://data.europa.eu/energy/StandardBusinessTypeList/A12">
    <skos:inScheme rdf:resource="http://data.europa.eu/energy/StandardBusinessTypeList"/>
    <skos:topConceptOf rdf:resource="http://data.europa.eu/energy/StandardBusinessTypeList"/>
    <dcterms:identifier>A12</dcterms:identifier>
    <skos:prefLabel>Secondary control</skos:prefLabel>
    <skos:definition xml:lang="en">A time series concerning secondary reserve.</skos:definition>
  </skos:Concept>
  <skos:Concept rdf:about="http://data.europa.eu/energy/StandardBusinessTypeList/A13">
    <skos:inScheme rdf:resource="http://data.europa.eu/energy/StandardBusinessTypeList"/>
    <skos:topConceptOf rdf:resource="http://data.europa.eu/energy/StandardBusinessTypeList"/>
    <dcterms:identifier>A13</dcterms:identifier>
    <skos:prefLabel>Load profile</skos:prefLabel>
    <skos:definition xml:lang="en">A time series concerning a load profile as calculated by a metered data aggregator.</skos:definition>
  </skos:Concept>
  <skos:Concept rdf:about="http://data.europa.eu/energy/StandardBusinessTypeList/A14">
    <skos:inScheme rdf:resource="http://data.europa.eu/energy/StandardBusinessTypeList"/>
    <skos:topConceptOf rdf:resource="http://data.europa.eu/energy/StandardBusinessTypeList"/>
    <dcterms:identifier>A14</dcterms:identifier>
    <skos:prefLabel>Aggregated energy data</skos:prefLabel>
    <skos:definition xml:lang="en">A time series concerning adjusted metered readings received from a metered data collector and aggregated and validated by a metered data aggregator.</skos:definition>
  </skos:Concept>
  <skos:Concept rdf:about="http://data.europa.eu/energy/StandardBusinessTypeList/A15">
    <skos:inScheme rdf:resource="http://data.europa.eu/energy/StandardBusinessTypeList"/>
    <skos:topConceptOf rdf:resource="http://data.europa.eu/energy/StandardBusinessTypeList"/>
    <dcterms:identifier>A15</dcterms:identifier>
    <skos:prefLabel>Losses</skos:prefLabel>
    <skos:definition xml:lang="en">A time series concerning losses that have been calculated for a tieline or an area.</skos:definition>
  </skos:Concept>
  <skos:Concept rdf:about="http://data.europa.eu/energy/StandardBusinessTypeList/A16">
    <skos:inScheme rdf:resource="http://data.europa.eu/energy/StandardBusinessTypeList"/>
    <skos:topConceptOf rdf:resource="http://data.europa.eu/energy/StandardBusinessTypeList"/>
    <dcterms:identifier>A16</dcterms:identifier>
    <skos:prefLabel>Transits (CBT)</skos:prefLabel>
    <skos:definition xml:lang="en">A time series concerning inter area transit flows determined for CBT requirements.</skos:definition>
  </skos:Concept>
  <skos:Concept rdf:about="http://data.europa.eu/energy/StandardBusinessTypeList/A17">
    <skos:inScheme rdf:resource="http://data.europa.eu/energy/StandardBusinessTypeList"/>
    <skos:topConceptOf rdf:resource="http://data.europa.eu/energy/StandardBusinessTypeList"/>
    <dcterms:identifier>A17</dcterms:identifier>
    <skos:prefLabel>Settlement deviation</skos:prefLabel>
    <skos:definition xml:lang="en">A time series concerning the imbalance energy calculated by an imbalance settlement responsible.</skos:definition>
  </skos:Concept>
  <skos:Concept rdf:about="http://data.europa.eu/energy/StandardBusinessTypeList/A18">
    <skos:inScheme rdf:resource="http://data.europa.eu/energy/StandardBusinessTypeList"/>
    <skos:topConceptOf rdf:resource="http://data.europa.eu/energy/StandardBusinessTypeList"/>
    <dcterms:identifier>A18</dcterms:identifier>
    <skos:prefLabel>Technical constraint deviation</skos:prefLabel>
    <skos:definition xml:lang="en">A time series defining the imbalance between schedules accepted by the system operator due to technical constraints and schedules declared by the balance responsible party.</skos:definition>
  </skos:Concept>
  <skos:Concept rdf:about="http://data.europa.eu/energy/StandardBusinessTypeList/A19">
    <skos:inScheme rdf:resource="http://data.europa.eu/energy/StandardBusinessTypeList"/>
    <skos:topConceptOf rdf:resource="http://data.europa.eu/energy/StandardBusinessTypeList"/>
    <dcterms:identifier>A19</dcterms:identifier>
    <skos:prefLabel>Balance energy deviation</skos:prefLabel>
    <skos:definition xml:lang="en">A time series defining the imbalance between the schedule of a balance responsible party that has been corrected by the system operator after using balance energy bids and the schedule that was accepted by the system operator due to technical constraints.</skos:definition>
  </skos:Concept>
  <skos:Concept rdf:about="http://data.europa.eu/energy/StandardBusinessTypeList/A20">
    <skos:inScheme rdf:resource="http://data.europa.eu/energy/StandardBusinessTypeList"/>
    <skos:topConceptOf rdf:resource="http://data.europa.eu/energy/StandardBusinessTypeList"/>
    <dcterms:identifier>A20</dcterms:identifier>
    <skos:prefLabel>Imbalance volume</skos:prefLabel>
    <skos:definition xml:lang="en">A time series defining the imbalance between the actual meter readings and the schedule of the balance responsible party corrected by the system operator after using balance energy bids.</skos:definition>
  </skos:Concept>
  <skos:Concept rdf:about="http://data.europa.eu/energy/StandardBusinessTypeList/A21">
    <skos:inScheme rdf:resource="http://data.europa.eu/energy/StandardBusinessTypeList"/>
    <skos:topConceptOf rdf:resource="http://data.europa.eu/energy/StandardBusinessTypeList"/>
    <dcterms:identifier>A21</dcterms:identifier>
    <skos:prefLabel>Unintended energy</skos:prefLabel>
    <skos:definition xml:lang="en">A timeseries concerning the volume of an unintended cross-border exchange of energy.</skos:definition>
  </skos:Concept>
  <skos:Concept rdf:about="http://data.europa.eu/energy/StandardBusinessTypeList/A22">
    <skos:inScheme rdf:resource="http://data.europa.eu/energy/StandardBusinessTypeList"/>
    <skos:topConceptOf rdf:resource="http://data.europa.eu/energy/StandardBusinessTypeList"/>
    <dcterms:identifier>A22</dcterms:identifier>
    <skos:prefLabel>Frequency control</skos:prefLabel>
    <skos:definition xml:lang="en">A time series concerning primary and secondary reserve.</skos:definition>
  </skos:Concept>
  <skos:Concept rdf:about="http://data.europa.eu/energy/StandardBusinessTypeList/A23">
    <skos:inScheme rdf:resource="http://data.europa.eu/energy/StandardBusinessTypeList"/>
    <skos:topConceptOf rdf:resource="http://data.europa.eu/energy/StandardBusinessTypeList"/>
    <dcterms:identifier>A23</dcterms:identifier>
    <skos:prefLabel>Balance management</skos:prefLabel>
    <skos:definition xml:lang="en">A time series concerning energy balancing services.</skos:definition>
  </skos:Concept>
  <skos:Concept rdf:about="http://data.europa.eu/energy/StandardBusinessTypeList/A24">
    <skos:inScheme rdf:resource="http://data.europa.eu/energy/StandardBusinessTypeList"/>
    <skos:topConceptOf rdf:resource="http://data.europa.eu/energy/StandardBusinessTypeList"/>
    <dcterms:identifier>A24</dcterms:identifier>
    <skos:prefLabel>Total trade</skos:prefLabel>
    <skos:definition xml:lang="en">A time series concerning the total of both the internal and external trades.</skos:definition>
  </skos:Concept>
  <skos:Concept rdf:about="http://data.europa.eu/energy/StandardBusinessTypeList/A25">
    <skos:inScheme rdf:resource="http://data.europa.eu/energy/StandardBusinessTypeList"/>
    <skos:topConceptOf rdf:resource="http://data.europa.eu/energy/StandardBusinessTypeList"/>
    <dcterms:identifier>A25</dcterms:identifier>
    <skos:prefLabel>General Capacity Information</skos:prefLabel>
    <skos:definition xml:lang="en">A time series providing the total capacity available on a TSO border.</skos:definition>
  </skos:Concept>
  <skos:Concept rdf:about="http://data.europa.eu/energy/StandardBusinessTypeList/A26">
    <skos:inScheme rdf:resource="http://data.europa.eu/energy/StandardBusinessTypeList"/>
    <skos:topConceptOf rdf:resource="http://data.europa.eu/energy/StandardBusinessTypeList"/>
    <dcterms:identifier>A26</dcterms:identifier>
    <skos:prefLabel>Available transfer capacity (ATC)</skos:prefLabel>
    <skos:definition xml:lang="en">Available transfer capacity for cross-border exchanges.</skos:definition>
  </skos:Concept>
  <skos:Concept rdf:about="http://data.europa.eu/energy/StandardBusinessTypeList/A27">
    <skos:inScheme rdf:resource="http://data.europa.eu/energy/StandardBusinessTypeList"/>
    <skos:topConceptOf rdf:resource="http://data.europa.eu/energy/StandardBusinessTypeList"/>
    <dcterms:identifier>A27</dcterms:identifier>
    <skos:prefLabel>Net transfer capacity (NTC)</skos:prefLabel>
    <skos:definition xml:lang="en">Net transfer capacity for cross-border exchanges.</skos:definition>
  </skos:Concept>
  <skos:Concept rdf:about="http://data.europa.eu/energy/StandardBusinessTypeList/A28">
    <skos:inScheme rdf:resource="http://data.europa.eu/energy/StandardBusinessTypeList"/>
    <skos:topConceptOf rdf:resource="http://data.europa.eu/energy/StandardBusinessTypeList"/>
    <dcterms:identifier>A28</dcterms:identifier>
    <skos:prefLabel>Control Area Program</skos:prefLabel>
    <skos:definition xml:lang="en">A time series providing the total exchanges between two TSOs (including the commercial transactions, the compensation program and the losses compensation program). 
Note this definition might change when UCTE brings forward its coding requirements.</skos:definition>
  </skos:Concept>
  <skos:Concept rdf:about="http://data.europa.eu/energy/StandardBusinessTypeList/A29">
    <skos:inScheme rdf:resource="http://data.europa.eu/energy/StandardBusinessTypeList"/>
    <skos:topConceptOf rdf:resource="http://data.europa.eu/energy/StandardBusinessTypeList"/>
    <dcterms:identifier>A29</dcterms:identifier>
    <skos:prefLabel>Already allocated capacity (AAC)</skos:prefLabel>
    <skos:definition xml:lang="en">The already allocated capacity is the total amount of allocated transmission rights.</skos:definition>
  </skos:Concept>
  <skos:Concept rdf:about="http://data.europa.eu/energy/StandardBusinessTypeList/A30">
    <skos:inScheme rdf:resource="http://data.europa.eu/energy/StandardBusinessTypeList"/>
    <skos:topConceptOf rdf:resource="http://data.europa.eu/energy/StandardBusinessTypeList"/>
    <dcterms:identifier>A30</dcterms:identifier>
    <skos:prefLabel>Internal inter area trade</skos:prefLabel>
    <skos:definition xml:lang="en">A trade that occurs between internal areas within a market balance area.</skos:definition>
  </skos:Concept>
  <skos:Concept rdf:about="http://data.europa.eu/energy/StandardBusinessTypeList/A31">
    <skos:inScheme rdf:resource="http://data.europa.eu/energy/StandardBusinessTypeList"/>
    <skos:topConceptOf rdf:resource="http://data.europa.eu/energy/StandardBusinessTypeList"/>
    <dcterms:identifier>A31</dcterms:identifier>
    <skos:prefLabel>Offered Capacity</skos:prefLabel>
    <skos:definition xml:lang="en">The time series provides the offered capacity.</skos:definition>
  </skos:Concept>
  <skos:Concept rdf:about="http://data.europa.eu/energy/StandardBusinessTypeList/A32">
    <skos:inScheme rdf:resource="http://data.europa.eu/energy/StandardBusinessTypeList"/>
    <skos:topConceptOf rdf:resource="http://data.europa.eu/energy/StandardBusinessTypeList"/>
    <dcterms:identifier>A32</dcterms:identifier>
    <skos:prefLabel>Capacity transfer notification</skos:prefLabel>
    <skos:definition xml:lang="en">The time series provides information concerning the notification of the transfer of capacity to another market participant.</skos:definition>
  </skos:Concept>
  <skos:Concept rdf:about="http://data.europa.eu/energy/StandardBusinessTypeList/A33">
    <skos:inScheme rdf:resource="http://data.europa.eu/energy/StandardBusinessTypeList"/>
    <skos:topConceptOf rdf:resource="http://data.europa.eu/energy/StandardBusinessTypeList"/>
    <dcterms:identifier>A33</dcterms:identifier>
    <skos:prefLabel>Authorised AAC</skos:prefLabel>
    <skos:definition xml:lang="en">The time series in question provides the amount of transmission capacity rights to be nominated.</skos:definition>
  </skos:Concept>
  <skos:Concept rdf:about="http://data.europa.eu/energy/StandardBusinessTypeList/A34">
    <skos:inScheme rdf:resource="http://data.europa.eu/energy/StandardBusinessTypeList"/>
    <skos:topConceptOf rdf:resource="http://data.europa.eu/energy/StandardBusinessTypeList"/>
    <dcterms:identifier>A34</dcterms:identifier>
    <skos:prefLabel>Capacity rights</skos:prefLabel>
    <skos:definition xml:lang="en">The time series in question provides the capacity rights allocated for a given border.</skos:definition>
  </skos:Concept>
  <skos:Concept rdf:about="http://data.europa.eu/energy/StandardBusinessTypeList/A35">
    <skos:inScheme rdf:resource="http://data.europa.eu/energy/StandardBusinessTypeList"/>
    <skos:topConceptOf rdf:resource="http://data.europa.eu/energy/StandardBusinessTypeList"/>
    <dcterms:identifier>A35</dcterms:identifier>
    <skos:prefLabel>Minimum authorised AAC</skos:prefLabel>
    <skos:definition xml:lang="en">The time series in question provides the minimum amount of transmission capacity rights to be nominated.</skos:definition>
  </skos:Concept>
  <skos:Concept rdf:about="http://data.europa.eu/energy/StandardBusinessTypeList/A36">
    <skos:inScheme rdf:resource="http://data.europa.eu/energy/StandardBusinessTypeList"/>
    <skos:topConceptOf rdf:resource="http://data.europa.eu/energy/StandardBusinessTypeList"/>
    <dcterms:identifier>A36</dcterms:identifier>
    <skos:prefLabel>Maximum authorised AAC</skos:prefLabel>
    <skos:definition xml:lang="en">The time series in question provides the maximum amount of transmission capacity rights to be nominated.</skos:definition>
  </skos:Concept>
  <skos:Concept rdf:about="http://data.europa.eu/energy/StandardBusinessTypeList/A37">
    <skos:inScheme rdf:resource="http://data.europa.eu/energy/StandardBusinessTypeList"/>
    <skos:topConceptOf rdf:resource="http://data.europa.eu/energy/StandardBusinessTypeList"/>
    <dcterms:identifier>A37</dcterms:identifier>
    <skos:prefLabel>Installed generation</skos:prefLabel>
    <skos:definition xml:lang="en">The time series in question provides the installed generation.</skos:definition>
  </skos:Concept>
  <skos:Concept rdf:about="http://data.europa.eu/energy/StandardBusinessTypeList/A38">
    <skos:inScheme rdf:resource="http://data.europa.eu/energy/StandardBusinessTypeList"/>
    <skos:topConceptOf rdf:resource="http://data.europa.eu/energy/StandardBusinessTypeList"/>
    <dcterms:identifier>A38</dcterms:identifier>
    <skos:prefLabel>Available generation</skos:prefLabel>
    <skos:definition xml:lang="en">The time series in question provides the available generation.</skos:definition>
  </skos:Concept>
  <skos:Concept rdf:about="http://data.europa.eu/energy/StandardBusinessTypeList/A40">
    <skos:inScheme rdf:resource="http://data.europa.eu/energy/StandardBusinessTypeList"/>
    <skos:topConceptOf rdf:resource="http://data.europa.eu/energy/StandardBusinessTypeList"/>
    <dcterms:identifier>A40</dcterms:identifier>
    <skos:prefLabel>Interconnection Trade Responsible Designation</skos:prefLabel>
    <skos:definition xml:lang="en">The Time series in question provides the designation of the ITR that may nominate the capacity in question.</skos:definition>
  </skos:Concept>
  <skos:Concept rdf:about="http://data.europa.eu/energy/StandardBusinessTypeList/A41">
    <skos:inScheme rdf:resource="http://data.europa.eu/energy/StandardBusinessTypeList"/>
    <skos:topConceptOf rdf:resource="http://data.europa.eu/energy/StandardBusinessTypeList"/>
    <dcterms:identifier>A41</dcterms:identifier>
    <skos:prefLabel>Released AAC</skos:prefLabel>
    <skos:definition xml:lang="en">The already allocated capacity (AAC) that has been released for resale.</skos:definition>
  </skos:Concept>
  <skos:Concept rdf:about="http://data.europa.eu/energy/StandardBusinessTypeList/A42">
    <skos:inScheme rdf:resource="http://data.europa.eu/energy/StandardBusinessTypeList"/>
    <skos:topConceptOf rdf:resource="http://data.europa.eu/energy/StandardBusinessTypeList"/>
    <dcterms:identifier>A42</dcterms:identifier>
    <skos:prefLabel>Requested capacity (with price)</skos:prefLabel>
    <skos:definition xml:lang="en">The time series in question provides information concerning the requested capacity including price information.</skos:definition>
  </skos:Concept>
  <skos:Concept rdf:about="http://data.europa.eu/energy/StandardBusinessTypeList/A43">
    <skos:inScheme rdf:resource="http://data.europa.eu/energy/StandardBusinessTypeList"/>
    <skos:topConceptOf rdf:resource="http://data.europa.eu/energy/StandardBusinessTypeList"/>
    <dcterms:identifier>A43</dcterms:identifier>
    <skos:prefLabel>Requested capacity (without price)</skos:prefLabel>
    <skos:definition xml:lang="en">The time series in question provides information concerning the requested capacity but excludes price information.</skos:definition>
  </skos:Concept>
  <skos:Concept rdf:about="http://data.europa.eu/energy/StandardBusinessTypeList/A44">
    <skos:inScheme rdf:resource="http://data.europa.eu/energy/StandardBusinessTypeList"/>
    <skos:topConceptOf rdf:resource="http://data.europa.eu/energy/StandardBusinessTypeList"/>
    <dcterms:identifier>A44</dcterms:identifier>
    <skos:prefLabel>Compensation program</skos:prefLabel>
    <skos:definition xml:lang="en">Compensation of unintentional deviation is performed by exporting to / importing from the interconnected system during the compensation period by means of schedules as calculated during the accounting of unintentional deviations.</skos:definition>
  </skos:Concept>
  <skos:Concept rdf:about="http://data.europa.eu/energy/StandardBusinessTypeList/A45">
    <skos:inScheme rdf:resource="http://data.europa.eu/energy/StandardBusinessTypeList"/>
    <skos:topConceptOf rdf:resource="http://data.europa.eu/energy/StandardBusinessTypeList"/>
    <dcterms:identifier>A45</dcterms:identifier>
    <skos:prefLabel>Schedule activated reserves</skos:prefLabel>
    <skos:definition xml:lang="en">The cross border or internal reserves that are to be activated through schedule nomination.</skos:definition>
  </skos:Concept>
  <skos:Concept rdf:about="http://data.europa.eu/energy/StandardBusinessTypeList/A46">
    <skos:inScheme rdf:resource="http://data.europa.eu/energy/StandardBusinessTypeList"/>
    <skos:topConceptOf rdf:resource="http://data.europa.eu/energy/StandardBusinessTypeList"/>
    <dcterms:identifier>A46</dcterms:identifier>
    <skos:prefLabel>System Operator redispatching</skos:prefLabel>
    <skos:definition xml:lang="en">The cross border redispatching between System Operators that are to be activated through schedule nomination.</skos:definition>
  </skos:Concept>
  <skos:Concept rdf:about="http://data.europa.eu/energy/StandardBusinessTypeList/A47">
    <skos:inScheme rdf:resource="http://data.europa.eu/energy/StandardBusinessTypeList"/>
    <skos:topConceptOf rdf:resource="http://data.europa.eu/energy/StandardBusinessTypeList"/>
    <dcterms:identifier>A47</dcterms:identifier>
    <skos:prefLabel>Market capacity price</skos:prefLabel>
    <skos:definition xml:lang="en">The price of the capacity offered on a given market.</skos:definition>
  </skos:Concept>
  <skos:Concept rdf:about="http://data.europa.eu/energy/StandardBusinessTypeList/A48">
    <skos:inScheme rdf:resource="http://data.europa.eu/energy/StandardBusinessTypeList"/>
    <skos:topConceptOf rdf:resource="http://data.europa.eu/energy/StandardBusinessTypeList"/>
    <dcterms:identifier>A48</dcterms:identifier>
    <skos:prefLabel>Market capacity price differential</skos:prefLabel>
    <skos:definition xml:lang="en">The difference between the price of capacity in a Market Balance Area receiving the capacity (In Area) and the price of capacity in a Market Balance Area providing the capacity (Out Area), i.e. In Area Price - Out Area price.</skos:definition>
  </skos:Concept>
  <skos:Concept rdf:about="http://data.europa.eu/energy/StandardBusinessTypeList/A49">
    <skos:inScheme rdf:resource="http://data.europa.eu/energy/StandardBusinessTypeList"/>
    <skos:topConceptOf rdf:resource="http://data.europa.eu/energy/StandardBusinessTypeList"/>
    <dcterms:identifier>A49</dcterms:identifier>
    <skos:prefLabel>Inflow</skos:prefLabel>
    <skos:definition xml:lang="en">The volume of water that flows into a reservoir in a given interval.</skos:definition>
  </skos:Concept>
  <skos:Concept rdf:about="http://data.europa.eu/energy/StandardBusinessTypeList/A50">
    <skos:inScheme rdf:resource="http://data.europa.eu/energy/StandardBusinessTypeList"/>
    <skos:topConceptOf rdf:resource="http://data.europa.eu/energy/StandardBusinessTypeList"/>
    <dcterms:identifier>A50</dcterms:identifier>
    <skos:prefLabel>Water extraction</skos:prefLabel>
    <skos:definition xml:lang="en">The volume of water that can be extracted from a reservoir in a given interval.</skos:definition>
  </skos:Concept>
  <skos:Concept rdf:about="http://data.europa.eu/energy/StandardBusinessTypeList/A51">
    <skos:inScheme rdf:resource="http://data.europa.eu/energy/StandardBusinessTypeList"/>
    <skos:topConceptOf rdf:resource="http://data.europa.eu/energy/StandardBusinessTypeList"/>
    <dcterms:identifier>A51</dcterms:identifier>
    <skos:prefLabel>Turbined water</skos:prefLabel>
    <skos:definition xml:lang="en">The volume of water that can be turbined in a plant in a given interval.</skos:definition>
  </skos:Concept>
  <skos:Concept rdf:about="http://data.europa.eu/energy/StandardBusinessTypeList/A52">
    <skos:inScheme rdf:resource="http://data.europa.eu/energy/StandardBusinessTypeList"/>
    <skos:topConceptOf rdf:resource="http://data.europa.eu/energy/StandardBusinessTypeList"/>
    <dcterms:identifier>A52</dcterms:identifier>
    <skos:prefLabel>Water spillage</skos:prefLabel>
    <skos:definition xml:lang="en">The volume of water that is not turbined going through the spillway in a given interval.</skos:definition>
  </skos:Concept>
  <skos:Concept rdf:about="http://data.europa.eu/energy/StandardBusinessTypeList/A53">
    <skos:inScheme rdf:resource="http://data.europa.eu/energy/StandardBusinessTypeList"/>
    <skos:topConceptOf rdf:resource="http://data.europa.eu/energy/StandardBusinessTypeList"/>
    <dcterms:identifier>A53</dcterms:identifier>
    <skos:prefLabel>Planned maintenance</skos:prefLabel>
    <skos:definition xml:lang="en">Maintenance has been planned for the object in question with a forecast ending date.</skos:definition>
  </skos:Concept>
  <skos:Concept rdf:about="http://data.europa.eu/energy/StandardBusinessTypeList/A54">
    <skos:inScheme rdf:resource="http://data.europa.eu/energy/StandardBusinessTypeList"/>
    <skos:topConceptOf rdf:resource="http://data.europa.eu/energy/StandardBusinessTypeList"/>
    <dcterms:identifier>A54</dcterms:identifier>
    <skos:prefLabel>Unplanned outage</skos:prefLabel>
    <skos:definition xml:lang="en">An unplanned outage has occurred on the object in question.</skos:definition>
  </skos:Concept>
  <skos:Concept rdf:about="http://data.europa.eu/energy/StandardBusinessTypeList/A55">
    <skos:inScheme rdf:resource="http://data.europa.eu/energy/StandardBusinessTypeList"/>
    <skos:topConceptOf rdf:resource="http://data.europa.eu/energy/StandardBusinessTypeList"/>
    <dcterms:identifier>A55</dcterms:identifier>
    <skos:prefLabel>Use it Or Sell it (UIOSI) pricing</skos:prefLabel>
    <skos:definition xml:lang="en">The time series provides information on the capacity resold in the "use it or sell it" process and its corresponding price.</skos:definition>
  </skos:Concept>
  <skos:Concept rdf:about="http://data.europa.eu/energy/StandardBusinessTypeList/A56">
    <skos:inScheme rdf:resource="http://data.europa.eu/energy/StandardBusinessTypeList"/>
    <skos:topConceptOf rdf:resource="http://data.europa.eu/energy/StandardBusinessTypeList"/>
    <dcterms:identifier>A56</dcterms:identifier>
    <skos:prefLabel>Compensation for auction cancellation where capacity is for resale</skos:prefLabel>
    <skos:definition xml:lang="en">The time series provides information on the compensation of the capacity for resale following an auction cancellation.</skos:definition>
  </skos:Concept>
  <skos:Concept rdf:about="http://data.europa.eu/energy/StandardBusinessTypeList/A57">
    <skos:inScheme rdf:resource="http://data.europa.eu/energy/StandardBusinessTypeList"/>
    <skos:topConceptOf rdf:resource="http://data.europa.eu/energy/StandardBusinessTypeList"/>
    <dcterms:identifier>A57</dcterms:identifier>
    <skos:prefLabel>Resale pricing</skos:prefLabel>
    <skos:definition xml:lang="en">For each Physical Transmission Rights holder, this document contains the resold capacity and its corresponding price.</skos:definition>
  </skos:Concept>
  <skos:Concept rdf:about="http://data.europa.eu/energy/StandardBusinessTypeList/A58">
    <skos:inScheme rdf:resource="http://data.europa.eu/energy/StandardBusinessTypeList"/>
    <skos:topConceptOf rdf:resource="http://data.europa.eu/energy/StandardBusinessTypeList"/>
    <dcterms:identifier>A58</dcterms:identifier>
    <skos:prefLabel>Curtailed capacity compensation</skos:prefLabel>
    <skos:definition xml:lang="en">The time series provides information to compensate a party when curtailment is applied on the capacity obtained in a previous auction, resale or transfer.</skos:definition>
  </skos:Concept>
  <skos:Concept rdf:about="http://data.europa.eu/energy/StandardBusinessTypeList/A59">
    <skos:inScheme rdf:resource="http://data.europa.eu/energy/StandardBusinessTypeList"/>
    <skos:topConceptOf rdf:resource="http://data.europa.eu/energy/StandardBusinessTypeList"/>
    <dcterms:identifier>A59</dcterms:identifier>
    <skos:prefLabel>Use it Or Sell it (UIOSI) compensation</skos:prefLabel>
    <skos:definition xml:lang="en">The time series provides information on the compensation for the capacity following an auction cancellation.</skos:definition>
  </skos:Concept>
  <skos:Concept rdf:about="http://data.europa.eu/energy/StandardBusinessTypeList/A60">
    <skos:inScheme rdf:resource="http://data.europa.eu/energy/StandardBusinessTypeList"/>
    <skos:topConceptOf rdf:resource="http://data.europa.eu/energy/StandardBusinessTypeList"/>
    <dcterms:identifier>A60</dcterms:identifier>
    <skos:prefLabel>Minimum possible</skos:prefLabel>
    <skos:definition xml:lang="en">The time series provides a schedule of minimum possible values for a Resource Object. The nature of the flow could be defined by the attribute Direction.</skos:definition>
  </skos:Concept>
  <skos:Concept rdf:about="http://data.europa.eu/energy/StandardBusinessTypeList/A61">
    <skos:inScheme rdf:resource="http://data.europa.eu/energy/StandardBusinessTypeList"/>
    <skos:topConceptOf rdf:resource="http://data.europa.eu/energy/StandardBusinessTypeList"/>
    <dcterms:identifier>A61</dcterms:identifier>
    <skos:prefLabel>Maximum available</skos:prefLabel>
    <skos:definition xml:lang="en">The time series provides a schedule of maximum available values for a Resource Object. The nature of the flow could be defined by the attribute Direction.</skos:definition>
  </skos:Concept>
  <skos:Concept rdf:about="http://data.europa.eu/energy/StandardBusinessTypeList/A62">
    <skos:inScheme rdf:resource="http://data.europa.eu/energy/StandardBusinessTypeList"/>
    <skos:topConceptOf rdf:resource="http://data.europa.eu/energy/StandardBusinessTypeList"/>
    <dcterms:identifier>A62</dcterms:identifier>
    <skos:prefLabel>Spot price</skos:prefLabel>
    <skos:definition xml:lang="en">The time series provides the market spot prices from an auction.</skos:definition>
  </skos:Concept>
  <skos:Concept rdf:about="http://data.europa.eu/energy/StandardBusinessTypeList/A63">
    <skos:inScheme rdf:resource="http://data.europa.eu/energy/StandardBusinessTypeList"/>
    <skos:topConceptOf rdf:resource="http://data.europa.eu/energy/StandardBusinessTypeList"/>
    <dcterms:identifier>A63</dcterms:identifier>
    <skos:prefLabel>Minimum ATC</skos:prefLabel>
    <skos:definition xml:lang="en">The Available Transmission Capacity that must be guaranteed because of regulatory constraints.</skos:definition>
  </skos:Concept>
  <skos:Concept rdf:about="http://data.europa.eu/energy/StandardBusinessTypeList/A64">
    <skos:inScheme rdf:resource="http://data.europa.eu/energy/StandardBusinessTypeList"/>
    <skos:topConceptOf rdf:resource="http://data.europa.eu/energy/StandardBusinessTypeList"/>
    <dcterms:identifier>A64</dcterms:identifier>
    <skos:prefLabel>Meter Measurement data </skos:prefLabel>
    <skos:definition xml:lang="en">The data as provided for a meter measurement source.</skos:definition>
  </skos:Concept>
  <skos:Concept rdf:about="http://data.europa.eu/energy/StandardBusinessTypeList/A65">
    <skos:inScheme rdf:resource="http://data.europa.eu/energy/StandardBusinessTypeList"/>
    <skos:topConceptOf rdf:resource="http://data.europa.eu/energy/StandardBusinessTypeList"/>
    <dcterms:identifier>A65</dcterms:identifier>
    <skos:prefLabel>Accounting Point Relevant data </skos:prefLabel>
    <skos:definition xml:lang="en">The metered data that is to be considered relevant for accounting purposes.</skos:definition>
  </skos:Concept>
  <skos:Concept rdf:about="http://data.europa.eu/energy/StandardBusinessTypeList/A66">
    <skos:inScheme rdf:resource="http://data.europa.eu/energy/StandardBusinessTypeList"/>
    <skos:topConceptOf rdf:resource="http://data.europa.eu/energy/StandardBusinessTypeList"/>
    <dcterms:identifier>A66</dcterms:identifier>
    <skos:prefLabel>Energy flow</skos:prefLabel>
    <skos:definition xml:lang="en">Energy flow information.</skos:definition>
  </skos:Concept>
  <skos:Concept rdf:about="http://data.europa.eu/energy/StandardBusinessTypeList/A67">
    <skos:inScheme rdf:resource="http://data.europa.eu/energy/StandardBusinessTypeList"/>
    <skos:topConceptOf rdf:resource="http://data.europa.eu/energy/StandardBusinessTypeList"/>
    <dcterms:identifier>A67</dcterms:identifier>
    <skos:prefLabel>Power plant energy Schedule</skos:prefLabel>
    <skos:definition xml:lang="en">Energy flow scheduled for a power plant.</skos:definition>
  </skos:Concept>
  <skos:Concept rdf:about="http://data.europa.eu/energy/StandardBusinessTypeList/A68">
    <skos:inScheme rdf:resource="http://data.europa.eu/energy/StandardBusinessTypeList"/>
    <skos:topConceptOf rdf:resource="http://data.europa.eu/energy/StandardBusinessTypeList"/>
    <dcterms:identifier>A68</dcterms:identifier>
    <skos:prefLabel>Compensation Requirements for the compensation period</skos:prefLabel>
    <skos:definition xml:lang="en">The time series provides the compensation requirements for a given compensation period.</skos:definition>
  </skos:Concept>
  <skos:Concept rdf:about="http://data.europa.eu/energy/StandardBusinessTypeList/A69">
    <skos:inScheme rdf:resource="http://data.europa.eu/energy/StandardBusinessTypeList"/>
    <skos:topConceptOf rdf:resource="http://data.europa.eu/energy/StandardBusinessTypeList"/>
    <dcterms:identifier>A69</dcterms:identifier>
    <skos:prefLabel>Market coupling results</skos:prefLabel>
    <skos:definition xml:lang="en">The time series provides the results of a market coupling auction.</skos:definition>
  </skos:Concept>
  <skos:Concept rdf:about="http://data.europa.eu/energy/StandardBusinessTypeList/A70">
    <skos:inScheme rdf:resource="http://data.europa.eu/energy/StandardBusinessTypeList"/>
    <skos:topConceptOf rdf:resource="http://data.europa.eu/energy/StandardBusinessTypeList"/>
    <dcterms:identifier>A70</dcterms:identifier>
    <skos:prefLabel>Production, unavailable</skos:prefLabel>
    <skos:definition xml:lang="en">Production capacity that normally would be available, but due to maintenance or similar is temporarily unavailable.</skos:definition>
  </skos:Concept>
  <skos:Concept rdf:about="http://data.europa.eu/energy/StandardBusinessTypeList/A71">
    <skos:inScheme rdf:resource="http://data.europa.eu/energy/StandardBusinessTypeList"/>
    <skos:topConceptOf rdf:resource="http://data.europa.eu/energy/StandardBusinessTypeList"/>
    <dcterms:identifier>A71</dcterms:identifier>
    <skos:prefLabel>Supplementary available generation</skos:prefLabel>
    <skos:definition xml:lang="en">The supplementary generation that is available.</skos:definition>
  </skos:Concept>
  <skos:Concept rdf:about="http://data.europa.eu/energy/StandardBusinessTypeList/A72">
    <skos:inScheme rdf:resource="http://data.europa.eu/energy/StandardBusinessTypeList"/>
    <skos:topConceptOf rdf:resource="http://data.europa.eu/energy/StandardBusinessTypeList"/>
    <dcterms:identifier>A72</dcterms:identifier>
    <skos:prefLabel>Interruptible consumption</skos:prefLabel>
    <skos:definition xml:lang="en">The consumption that may be interrupted on request.</skos:definition>
  </skos:Concept>
  <skos:Concept rdf:about="http://data.europa.eu/energy/StandardBusinessTypeList/A73">
    <skos:inScheme rdf:resource="http://data.europa.eu/energy/StandardBusinessTypeList"/>
    <skos:topConceptOf rdf:resource="http://data.europa.eu/energy/StandardBusinessTypeList"/>
    <dcterms:identifier>A73</dcterms:identifier>
    <skos:prefLabel>Summarised Market Balance Area Schedule</skos:prefLabel>
    <skos:definition xml:lang="en">A time series providing the total exchanges based on commercial transactions between two Market Balance Areas.</skos:definition>
  </skos:Concept>
  <skos:Concept rdf:about="http://data.europa.eu/energy/StandardBusinessTypeList/A74">
    <skos:inScheme rdf:resource="http://data.europa.eu/energy/StandardBusinessTypeList"/>
    <skos:topConceptOf rdf:resource="http://data.europa.eu/energy/StandardBusinessTypeList"/>
    <dcterms:identifier>A74</dcterms:identifier>
    <skos:prefLabel>Load Frequency Control Program Schedule</skos:prefLabel>
    <skos:definition xml:lang="en">A time series providing the schedule information for the Load Frequency Control Program.</skos:definition>
  </skos:Concept>
  <skos:Concept rdf:about="http://data.europa.eu/energy/StandardBusinessTypeList/A75">
    <skos:inScheme rdf:resource="http://data.europa.eu/energy/StandardBusinessTypeList"/>
    <skos:topConceptOf rdf:resource="http://data.europa.eu/energy/StandardBusinessTypeList"/>
    <dcterms:identifier>A75</dcterms:identifier>
    <skos:prefLabel>Timeframe Independent Schedule</skos:prefLabel>
    <skos:definition xml:lang="en">A time series providing the total exchanges of Timeframe Independent Schedules between two System Operators.</skos:definition>
  </skos:Concept>
  <skos:Concept rdf:about="http://data.europa.eu/energy/StandardBusinessTypeList/A76">
    <skos:inScheme rdf:resource="http://data.europa.eu/energy/StandardBusinessTypeList"/>
    <skos:topConceptOf rdf:resource="http://data.europa.eu/energy/StandardBusinessTypeList"/>
    <dcterms:identifier>A76</dcterms:identifier>
    <skos:prefLabel>Consumption curtailment</skos:prefLabel>
    <skos:definition xml:lang="en">A time series providing the amount of voluntary consumption curtailed by the energy supplier of an end-consumer.</skos:definition>
  </skos:Concept>
  <skos:Concept rdf:about="http://data.europa.eu/energy/StandardBusinessTypeList/A77">
    <skos:inScheme rdf:resource="http://data.europa.eu/energy/StandardBusinessTypeList"/>
    <skos:topConceptOf rdf:resource="http://data.europa.eu/energy/StandardBusinessTypeList"/>
    <dcterms:identifier>A77</dcterms:identifier>
    <skos:prefLabel>Production, dispatchable</skos:prefLabel>
    <skos:definition xml:lang="en">The nature of the business being described is dispatchable production details, i.e. generation output that can be changed by a request (activation order) of the TSO according with the applicable Market Rules. </skos:definition>
  </skos:Concept>
  <skos:Concept rdf:about="http://data.europa.eu/energy/StandardBusinessTypeList/A78">
    <skos:inScheme rdf:resource="http://data.europa.eu/energy/StandardBusinessTypeList"/>
    <skos:topConceptOf rdf:resource="http://data.europa.eu/energy/StandardBusinessTypeList"/>
    <dcterms:identifier>A78</dcterms:identifier>
    <skos:prefLabel>Consumption, dispatchable</skos:prefLabel>
    <skos:definition xml:lang="en">The nature of the business being described is dispatchable consumption details, i.e. consumption output that can be changed by a request (activation order) of the TSO according with the applicable Market Rules. </skos:definition>
  </skos:Concept>
  <skos:Concept rdf:about="http://data.europa.eu/energy/StandardBusinessTypeList/A79">
    <skos:inScheme rdf:resource="http://data.europa.eu/energy/StandardBusinessTypeList"/>
    <skos:topConceptOf rdf:resource="http://data.europa.eu/energy/StandardBusinessTypeList"/>
    <dcterms:identifier>A79</dcterms:identifier>
    <skos:prefLabel>Production, non-dispatchable</skos:prefLabel>
    <skos:definition xml:lang="en">The nature of the business being described is non-dispatchable production details, i.e. generation output that cannot be modified by an activation order.</skos:definition>
  </skos:Concept>
  <skos:Concept rdf:about="http://data.europa.eu/energy/StandardBusinessTypeList/A80">
    <skos:inScheme rdf:resource="http://data.europa.eu/energy/StandardBusinessTypeList"/>
    <skos:topConceptOf rdf:resource="http://data.europa.eu/energy/StandardBusinessTypeList"/>
    <dcterms:identifier>A80</dcterms:identifier>
    <skos:prefLabel>Consumption, non-dispatchable</skos:prefLabel>
    <skos:definition xml:lang="en">The nature of the business being described is non-dispatchable consumption details, i.e. consumption output that cannot be modified by an activation order.</skos:definition>
  </skos:Concept>
  <skos:Concept rdf:about="http://data.europa.eu/energy/StandardBusinessTypeList/A81">
    <skos:inScheme rdf:resource="http://data.europa.eu/energy/StandardBusinessTypeList"/>
    <skos:topConceptOf rdf:resource="http://data.europa.eu/energy/StandardBusinessTypeList"/>
    <dcterms:identifier>A81</dcterms:identifier>
    <skos:prefLabel>Total Transfer Capacity (TTC)</skos:prefLabel>
    <skos:definition xml:lang="en">The Total Transfer Capacity is the maximum exchange program between two areas compatible with operational security standards applicable at each system if future network conditions, generation and load patterns were perfectly known in advance.</skos:definition>
  </skos:Concept>
  <skos:Concept rdf:about="http://data.europa.eu/energy/StandardBusinessTypeList/A82">
    <skos:inScheme rdf:resource="http://data.europa.eu/energy/StandardBusinessTypeList"/>
    <skos:topConceptOf rdf:resource="http://data.europa.eu/energy/StandardBusinessTypeList"/>
    <dcterms:identifier>A82</dcterms:identifier>
    <skos:prefLabel>Mutual Emergency Assistance Service (MEAS) </skos:prefLabel>
    <skos:definition xml:lang="en">The cross border Mutual Emergency Assistance Service between System Operators that are to be activated through schedule nomination.</skos:definition>
  </skos:Concept>
  <skos:Concept rdf:about="http://data.europa.eu/energy/StandardBusinessTypeList/A83">
    <skos:inScheme rdf:resource="http://data.europa.eu/energy/StandardBusinessTypeList"/>
    <skos:topConceptOf rdf:resource="http://data.europa.eu/energy/StandardBusinessTypeList"/>
    <dcterms:identifier>A83</dcterms:identifier>
    <skos:prefLabel>Auction cancelation </skos:prefLabel>
    <skos:definition xml:lang="en">The time series covers auction cancellation right.</skos:definition>
  </skos:Concept>
  <skos:Concept rdf:about="http://data.europa.eu/energy/StandardBusinessTypeList/A84">
    <skos:inScheme rdf:resource="http://data.europa.eu/energy/StandardBusinessTypeList"/>
    <skos:topConceptOf rdf:resource="http://data.europa.eu/energy/StandardBusinessTypeList"/>
    <dcterms:identifier>A84</dcterms:identifier>
    <skos:prefLabel>Nomination curtailment</skos:prefLabel>
    <skos:definition xml:lang="en">The time series covers nomination curtailment rights </skos:definition>
  </skos:Concept>
  <skos:Concept rdf:about="http://data.europa.eu/energy/StandardBusinessTypeList/A85">
    <skos:inScheme rdf:resource="http://data.europa.eu/energy/StandardBusinessTypeList"/>
    <skos:topConceptOf rdf:resource="http://data.europa.eu/energy/StandardBusinessTypeList"/>
    <dcterms:identifier>A85</dcterms:identifier>
    <skos:prefLabel>Internal redispatch</skos:prefLabel>
    <skos:definition xml:lang="en">Redispatch to relieve Market Balance Area internal congestion.</skos:definition>
  </skos:Concept>
  <skos:Concept rdf:about="http://data.europa.eu/energy/StandardBusinessTypeList/A86">
    <skos:inScheme rdf:resource="http://data.europa.eu/energy/StandardBusinessTypeList"/>
    <skos:topConceptOf rdf:resource="http://data.europa.eu/energy/StandardBusinessTypeList"/>
    <dcterms:identifier>A86</dcterms:identifier>
    <skos:prefLabel>Control area balance energy</skos:prefLabel>
    <skos:definition xml:lang="en">A sum of secondary, tertiary control as well as other energy that was used to balance a control area.</skos:definition>
  </skos:Concept>
  <skos:Concept rdf:about="http://data.europa.eu/energy/StandardBusinessTypeList/A87">
    <skos:inScheme rdf:resource="http://data.europa.eu/energy/StandardBusinessTypeList"/>
    <skos:topConceptOf rdf:resource="http://data.europa.eu/energy/StandardBusinessTypeList"/>
    <dcterms:identifier>A87</dcterms:identifier>
    <skos:prefLabel>Balancing energy price</skos:prefLabel>
    <skos:definition xml:lang="en">Price of energy used to balance.</skos:definition>
  </skos:Concept>
  <skos:Concept rdf:about="http://data.europa.eu/energy/StandardBusinessTypeList/A88">
    <skos:inScheme rdf:resource="http://data.europa.eu/energy/StandardBusinessTypeList"/>
    <skos:topConceptOf rdf:resource="http://data.europa.eu/energy/StandardBusinessTypeList"/>
    <dcterms:identifier>A88</dcterms:identifier>
    <skos:prefLabel>Economised secondary reserve</skos:prefLabel>
    <skos:definition xml:lang="en">The activated secondary reserve that had been economised due to pooled reserve management.</skos:definition>
  </skos:Concept>
  <skos:Concept rdf:about="http://data.europa.eu/energy/StandardBusinessTypeList/A89">
    <skos:inScheme rdf:resource="http://data.europa.eu/energy/StandardBusinessTypeList"/>
    <skos:topConceptOf rdf:resource="http://data.europa.eu/energy/StandardBusinessTypeList"/>
    <dcterms:identifier>A89</dcterms:identifier>
    <skos:prefLabel>Spinning reserve</skos:prefLabel>
    <skos:definition xml:lang="en">The extra generating capacity that is available by increasing the production of generators that are already connected to the power system.</skos:definition>
  </skos:Concept>
  <skos:Concept rdf:about="http://data.europa.eu/energy/StandardBusinessTypeList/A90">
    <skos:inScheme rdf:resource="http://data.europa.eu/energy/StandardBusinessTypeList"/>
    <skos:topConceptOf rdf:resource="http://data.europa.eu/energy/StandardBusinessTypeList"/>
    <dcterms:identifier>A90</dcterms:identifier>
    <skos:prefLabel>Solar</skos:prefLabel>
    <skos:definition xml:lang="en">The business being described concerns solar power.</skos:definition>
  </skos:Concept>
  <skos:Concept rdf:about="http://data.europa.eu/energy/StandardBusinessTypeList/A91">
    <skos:inScheme rdf:resource="http://data.europa.eu/energy/StandardBusinessTypeList"/>
    <skos:topConceptOf rdf:resource="http://data.europa.eu/energy/StandardBusinessTypeList"/>
    <dcterms:identifier>A91</dcterms:identifier>
    <skos:prefLabel>positive forecast margin</skos:prefLabel>
    <skos:definition xml:lang="en">The business being described concerns a positive forecast margin.</skos:definition>
  </skos:Concept>
  <skos:Concept rdf:about="http://data.europa.eu/energy/StandardBusinessTypeList/A92">
    <skos:inScheme rdf:resource="http://data.europa.eu/energy/StandardBusinessTypeList"/>
    <skos:topConceptOf rdf:resource="http://data.europa.eu/energy/StandardBusinessTypeList"/>
    <dcterms:identifier>A92</dcterms:identifier>
    <skos:prefLabel>Negative forecast margin</skos:prefLabel>
    <skos:definition xml:lang="en">The business being described concerns a negative forecast margin.</skos:definition>
  </skos:Concept>
  <skos:Concept rdf:about="http://data.europa.eu/energy/StandardBusinessTypeList/A93">
    <skos:inScheme rdf:resource="http://data.europa.eu/energy/StandardBusinessTypeList"/>
    <skos:topConceptOf rdf:resource="http://data.europa.eu/energy/StandardBusinessTypeList"/>
    <dcterms:identifier>A93</dcterms:identifier>
    <skos:prefLabel>Wind generation</skos:prefLabel>
    <skos:definition xml:lang="en">The business being described concerns wind generation.</skos:definition>
  </skos:Concept>
  <skos:Concept rdf:about="http://data.europa.eu/energy/StandardBusinessTypeList/A94">
    <skos:inScheme rdf:resource="http://data.europa.eu/energy/StandardBusinessTypeList"/>
    <skos:topConceptOf rdf:resource="http://data.europa.eu/energy/StandardBusinessTypeList"/>
    <dcterms:identifier>A94</dcterms:identifier>
    <skos:prefLabel>Solar generation</skos:prefLabel>
    <skos:definition xml:lang="en">The business being described concerns solar generation.</skos:definition>
  </skos:Concept>
  <skos:Concept rdf:about="http://data.europa.eu/energy/StandardBusinessTypeList/A95">
    <skos:inScheme rdf:resource="http://data.europa.eu/energy/StandardBusinessTypeList"/>
    <skos:topConceptOf rdf:resource="http://data.europa.eu/energy/StandardBusinessTypeList"/>
    <dcterms:identifier>A95</dcterms:identifier>
    <skos:prefLabel>Frequency containment reserve</skos:prefLabel>
    <skos:definition xml:lang="en">The business being described concerns frequency containment reserve.</skos:definition>
  </skos:Concept>
  <skos:Concept rdf:about="http://data.europa.eu/energy/StandardBusinessTypeList/A96">
    <skos:inScheme rdf:resource="http://data.europa.eu/energy/StandardBusinessTypeList"/>
    <skos:topConceptOf rdf:resource="http://data.europa.eu/energy/StandardBusinessTypeList"/>
    <dcterms:identifier>A96</dcterms:identifier>
    <skos:prefLabel>Automatic frequency restoration reserve</skos:prefLabel>
    <skos:definition xml:lang="en">The business being described concerns automatic frequency restoration reserve.</skos:definition>
  </skos:Concept>
  <skos:Concept rdf:about="http://data.europa.eu/energy/StandardBusinessTypeList/A97">
    <skos:inScheme rdf:resource="http://data.europa.eu/energy/StandardBusinessTypeList"/>
    <skos:topConceptOf rdf:resource="http://data.europa.eu/energy/StandardBusinessTypeList"/>
    <dcterms:identifier>A97</dcterms:identifier>
    <skos:prefLabel>Manual frequency restoration reserve</skos:prefLabel>
    <skos:definition xml:lang="en">The business being described concerns manual frequency restoration reserve.</skos:definition>
  </skos:Concept>
  <skos:Concept rdf:about="http://data.europa.eu/energy/StandardBusinessTypeList/A98">
    <skos:inScheme rdf:resource="http://data.europa.eu/energy/StandardBusinessTypeList"/>
    <skos:topConceptOf rdf:resource="http://data.europa.eu/energy/StandardBusinessTypeList"/>
    <dcterms:identifier>A98</dcterms:identifier>
    <skos:prefLabel>Replacement reserve</skos:prefLabel>
    <skos:definition xml:lang="en">The business being described concerns replacement reserve.</skos:definition>
  </skos:Concept>
  <skos:Concept rdf:about="http://data.europa.eu/energy/StandardBusinessTypeList/A99">
    <skos:inScheme rdf:resource="http://data.europa.eu/energy/StandardBusinessTypeList"/>
    <skos:topConceptOf rdf:resource="http://data.europa.eu/energy/StandardBusinessTypeList"/>
    <dcterms:identifier>A99</dcterms:identifier>
    <skos:prefLabel>Financial information</skos:prefLabel>
    <skos:definition xml:lang="en">The business being described concerns financial information.</skos:definition>
  </skos:Concept>
  <skos:Concept rdf:about="http://data.europa.eu/energy/StandardBusinessTypeList/B01">
    <skos:inScheme rdf:resource="http://data.europa.eu/energy/StandardBusinessTypeList"/>
    <skos:topConceptOf rdf:resource="http://data.europa.eu/energy/StandardBusinessTypeList"/>
    <dcterms:identifier>B01</dcterms:identifier>
    <skos:prefLabel>Interconnector network evolution</skos:prefLabel>
    <skos:definition xml:lang="en">The business being described concerns interconnector network evolution.</skos:definition>
  </skos:Concept>
  <skos:Concept rdf:about="http://data.europa.eu/energy/StandardBusinessTypeList/B02">
    <skos:inScheme rdf:resource="http://data.europa.eu/energy/StandardBusinessTypeList"/>
    <skos:topConceptOf rdf:resource="http://data.europa.eu/energy/StandardBusinessTypeList"/>
    <dcterms:identifier>B02</dcterms:identifier>
    <skos:prefLabel>Interconnector network dismantling</skos:prefLabel>
    <skos:definition xml:lang="en">The business being described concerns interconnector network dismantling.</skos:definition>
  </skos:Concept>
  <skos:Concept rdf:about="http://data.europa.eu/energy/StandardBusinessTypeList/B03">
    <skos:inScheme rdf:resource="http://data.europa.eu/energy/StandardBusinessTypeList"/>
    <skos:topConceptOf rdf:resource="http://data.europa.eu/energy/StandardBusinessTypeList"/>
    <dcterms:identifier>B03</dcterms:identifier>
    <skos:prefLabel>Counter trade</skos:prefLabel>
    <skos:definition xml:lang="en">The business being described concerns counter trades.</skos:definition>
  </skos:Concept>
  <skos:Concept rdf:about="http://data.europa.eu/energy/StandardBusinessTypeList/B04">
    <skos:inScheme rdf:resource="http://data.europa.eu/energy/StandardBusinessTypeList"/>
    <skos:topConceptOf rdf:resource="http://data.europa.eu/energy/StandardBusinessTypeList"/>
    <dcterms:identifier>B04</dcterms:identifier>
    <skos:prefLabel>Congestion costs</skos:prefLabel>
    <skos:definition xml:lang="en">The business being described concerns congestion costs.</skos:definition>
  </skos:Concept>
  <skos:Concept rdf:about="http://data.europa.eu/energy/StandardBusinessTypeList/B05">
    <skos:inScheme rdf:resource="http://data.europa.eu/energy/StandardBusinessTypeList"/>
    <skos:topConceptOf rdf:resource="http://data.europa.eu/energy/StandardBusinessTypeList"/>
    <dcterms:identifier>B05</dcterms:identifier>
    <skos:prefLabel>Capacity allocated (including price)</skos:prefLabel>
    <skos:definition xml:lang="en">The business being described concerns capacity allocation and includes price information.</skos:definition>
  </skos:Concept>
  <skos:Concept rdf:about="http://data.europa.eu/energy/StandardBusinessTypeList/B06">
    <skos:inScheme rdf:resource="http://data.europa.eu/energy/StandardBusinessTypeList"/>
    <skos:topConceptOf rdf:resource="http://data.europa.eu/energy/StandardBusinessTypeList"/>
    <dcterms:identifier>B06</dcterms:identifier>
    <skos:prefLabel>DC link constraint</skos:prefLabel>
    <skos:definition xml:lang="en">The business being described concerns DC link constraints.</skos:definition>
  </skos:Concept>
  <skos:Concept rdf:about="http://data.europa.eu/energy/StandardBusinessTypeList/B07">
    <skos:inScheme rdf:resource="http://data.europa.eu/energy/StandardBusinessTypeList"/>
    <skos:topConceptOf rdf:resource="http://data.europa.eu/energy/StandardBusinessTypeList"/>
    <dcterms:identifier>B07</dcterms:identifier>
    <skos:prefLabel>Auction revenue</skos:prefLabel>
    <skos:definition xml:lang="en">The business being described concerns auction revenue.</skos:definition>
  </skos:Concept>
  <skos:Concept rdf:about="http://data.europa.eu/energy/StandardBusinessTypeList/B08">
    <skos:inScheme rdf:resource="http://data.europa.eu/energy/StandardBusinessTypeList"/>
    <skos:topConceptOf rdf:resource="http://data.europa.eu/energy/StandardBusinessTypeList"/>
    <dcterms:identifier>B08</dcterms:identifier>
    <skos:prefLabel>Total nominated capacity</skos:prefLabel>
    <skos:definition xml:lang="en">The business being described concerns the total nominated capacity.</skos:definition>
  </skos:Concept>
  <skos:Concept rdf:about="http://data.europa.eu/energy/StandardBusinessTypeList/B09">
    <skos:inScheme rdf:resource="http://data.europa.eu/energy/StandardBusinessTypeList"/>
    <skos:topConceptOf rdf:resource="http://data.europa.eu/energy/StandardBusinessTypeList"/>
    <dcterms:identifier>B09</dcterms:identifier>
    <skos:prefLabel>Net position</skos:prefLabel>
    <skos:definition xml:lang="en">The business being described concerns net position.</skos:definition>
  </skos:Concept>
  <skos:Concept rdf:about="http://data.europa.eu/energy/StandardBusinessTypeList/B10">
    <skos:inScheme rdf:resource="http://data.europa.eu/energy/StandardBusinessTypeList"/>
    <skos:topConceptOf rdf:resource="http://data.europa.eu/energy/StandardBusinessTypeList"/>
    <dcterms:identifier>B10</dcterms:identifier>
    <skos:prefLabel>Congestion income</skos:prefLabel>
    <skos:definition xml:lang="en">The business being described concerns congestion income.</skos:definition>
  </skos:Concept>
  <skos:Concept rdf:about="http://data.europa.eu/energy/StandardBusinessTypeList/B11">
    <skos:inScheme rdf:resource="http://data.europa.eu/energy/StandardBusinessTypeList"/>
    <skos:topConceptOf rdf:resource="http://data.europa.eu/energy/StandardBusinessTypeList"/>
    <dcterms:identifier>B11</dcterms:identifier>
    <skos:prefLabel>Production unit</skos:prefLabel>
    <skos:definition xml:lang="en">The business being described concerns a production unit.</skos:definition>
  </skos:Concept>
  <skos:Concept rdf:about="http://data.europa.eu/energy/StandardBusinessTypeList/B12">
    <skos:inScheme rdf:resource="http://data.europa.eu/energy/StandardBusinessTypeList"/>
    <skos:topConceptOf rdf:resource="http://data.europa.eu/energy/StandardBusinessTypeList"/>
    <dcterms:identifier>B12</dcterms:identifier>
    <skos:prefLabel>Rounded market coupling results</skos:prefLabel>
    <skos:definition xml:lang="en">Rounded outputs of the market coupling to be sent to TSOs and Market Participants.</skos:definition>
  </skos:Concept>
  <skos:Concept rdf:about="http://data.europa.eu/energy/StandardBusinessTypeList/B13">
    <skos:inScheme rdf:resource="http://data.europa.eu/energy/StandardBusinessTypeList"/>
    <skos:topConceptOf rdf:resource="http://data.europa.eu/energy/StandardBusinessTypeList"/>
    <dcterms:identifier>B13</dcterms:identifier>
    <skos:prefLabel>Allocation Revenue</skos:prefLabel>
    <skos:definition xml:lang="en">The time series provides information on the revenue generated by the allocations.</skos:definition>
  </skos:Concept>
  <skos:Concept rdf:about="http://data.europa.eu/energy/StandardBusinessTypeList/B14">
    <skos:inScheme rdf:resource="http://data.europa.eu/energy/StandardBusinessTypeList"/>
    <skos:topConceptOf rdf:resource="http://data.europa.eu/energy/StandardBusinessTypeList"/>
    <dcterms:identifier>B14</dcterms:identifier>
    <skos:prefLabel>Production deviation</skos:prefLabel>
    <skos:definition xml:lang="en">A time series concerning the imbalance energy between the metered production and the schedules calculated by an imbalance settlement responsible.</skos:definition>
  </skos:Concept>
  <skos:Concept rdf:about="http://data.europa.eu/energy/StandardBusinessTypeList/B15">
    <skos:inScheme rdf:resource="http://data.europa.eu/energy/StandardBusinessTypeList"/>
    <skos:topConceptOf rdf:resource="http://data.europa.eu/energy/StandardBusinessTypeList"/>
    <dcterms:identifier>B15</dcterms:identifier>
    <skos:prefLabel>Consumption deviation</skos:prefLabel>
    <skos:definition xml:lang="en">A time series concerning the imbalance energy between  metered consumption and the forecasted consumption calculated by an imbalance settlement responsible.</skos:definition>
  </skos:Concept>
  <skos:Concept rdf:about="http://data.europa.eu/energy/StandardBusinessTypeList/B16">
    <skos:inScheme rdf:resource="http://data.europa.eu/energy/StandardBusinessTypeList"/>
    <skos:topConceptOf rdf:resource="http://data.europa.eu/energy/StandardBusinessTypeList"/>
    <dcterms:identifier>B16</dcterms:identifier>
    <skos:prefLabel>Transmission asset</skos:prefLabel>
    <skos:definition xml:lang="en">The business being described concerns a transmission asset.</skos:definition>
  </skos:Concept>
  <skos:Concept rdf:about="http://data.europa.eu/energy/StandardBusinessTypeList/B17">
    <skos:inScheme rdf:resource="http://data.europa.eu/energy/StandardBusinessTypeList"/>
    <skos:topConceptOf rdf:resource="http://data.europa.eu/energy/StandardBusinessTypeList"/>
    <dcterms:identifier>B17</dcterms:identifier>
    <skos:prefLabel>Consumption unit</skos:prefLabel>
    <skos:definition xml:lang="en">The business being described concerns a consumption unit.</skos:definition>
  </skos:Concept>
  <skos:Concept rdf:about="http://data.europa.eu/energy/StandardBusinessTypeList/B18">
    <skos:inScheme rdf:resource="http://data.europa.eu/energy/StandardBusinessTypeList"/>
    <skos:topConceptOf rdf:resource="http://data.europa.eu/energy/StandardBusinessTypeList"/>
    <dcterms:identifier>B18</dcterms:identifier>
    <skos:prefLabel>In-feed ATC</skos:prefLabel>
    <skos:definition xml:lang="en">Available Transfer Capacity at the in-feed side of a DC tieline.</skos:definition>
  </skos:Concept>
  <skos:Concept rdf:about="http://data.europa.eu/energy/StandardBusinessTypeList/B19">
    <skos:inScheme rdf:resource="http://data.europa.eu/energy/StandardBusinessTypeList"/>
    <skos:topConceptOf rdf:resource="http://data.europa.eu/energy/StandardBusinessTypeList"/>
    <dcterms:identifier>B19</dcterms:identifier>
    <skos:prefLabel>Out-feed ATC</skos:prefLabel>
    <skos:definition xml:lang="en">Available Transfer Capacity at the out-feed side of a DC tieline.</skos:definition>
  </skos:Concept>
  <skos:Concept rdf:about="http://data.europa.eu/energy/StandardBusinessTypeList/B20">
    <skos:inScheme rdf:resource="http://data.europa.eu/energy/StandardBusinessTypeList"/>
    <skos:topConceptOf rdf:resource="http://data.europa.eu/energy/StandardBusinessTypeList"/>
    <dcterms:identifier>B20</dcterms:identifier>
    <skos:prefLabel>Balance up regulation price</skos:prefLabel>
    <skos:definition xml:lang="en">A time series concerning balance regulation market prices for up regulation.</skos:definition>
  </skos:Concept>
  <skos:Concept rdf:about="http://data.europa.eu/energy/StandardBusinessTypeList/B21">
    <skos:inScheme rdf:resource="http://data.europa.eu/energy/StandardBusinessTypeList"/>
    <skos:topConceptOf rdf:resource="http://data.europa.eu/energy/StandardBusinessTypeList"/>
    <dcterms:identifier>B21</dcterms:identifier>
    <skos:prefLabel>Balance down regulation price</skos:prefLabel>
    <skos:definition xml:lang="en">A time series concerning balance regulation market prices for down regulation.</skos:definition>
  </skos:Concept>
  <skos:Concept rdf:about="http://data.europa.eu/energy/StandardBusinessTypeList/B22">
    <skos:inScheme rdf:resource="http://data.europa.eu/energy/StandardBusinessTypeList"/>
    <skos:topConceptOf rdf:resource="http://data.europa.eu/energy/StandardBusinessTypeList"/>
    <dcterms:identifier>B22</dcterms:identifier>
    <skos:prefLabel>Main direction</skos:prefLabel>
    <skos:definition xml:lang="en">A time series concerning the direction of balance regulations.</skos:definition>
  </skos:Concept>
  <skos:Concept rdf:about="http://data.europa.eu/energy/StandardBusinessTypeList/B23">
    <skos:inScheme rdf:resource="http://data.europa.eu/energy/StandardBusinessTypeList"/>
    <skos:topConceptOf rdf:resource="http://data.europa.eu/energy/StandardBusinessTypeList"/>
    <dcterms:identifier>B23</dcterms:identifier>
    <skos:prefLabel>Consumption imbalance price</skos:prefLabel>
    <skos:definition xml:lang="en">A time series concerning imbalance prices for consumption.</skos:definition>
  </skos:Concept>
  <skos:Concept rdf:about="http://data.europa.eu/energy/StandardBusinessTypeList/B24">
    <skos:inScheme rdf:resource="http://data.europa.eu/energy/StandardBusinessTypeList"/>
    <skos:topConceptOf rdf:resource="http://data.europa.eu/energy/StandardBusinessTypeList"/>
    <dcterms:identifier>B24</dcterms:identifier>
    <skos:prefLabel>Production sales imbalance price</skos:prefLabel>
    <skos:definition xml:lang="en">A time series concerning imbalance prices for production sales.</skos:definition>
  </skos:Concept>
  <skos:Concept rdf:about="http://data.europa.eu/energy/StandardBusinessTypeList/B25">
    <skos:inScheme rdf:resource="http://data.europa.eu/energy/StandardBusinessTypeList"/>
    <skos:topConceptOf rdf:resource="http://data.europa.eu/energy/StandardBusinessTypeList"/>
    <dcterms:identifier>B25</dcterms:identifier>
    <skos:prefLabel>Production purchase imbalance price</skos:prefLabel>
    <skos:definition xml:lang="en">A time series concerning imbalance prices for production purchase.</skos:definition>
  </skos:Concept>
  <skos:Concept rdf:about="http://data.europa.eu/energy/StandardBusinessTypeList/B26">
    <skos:inScheme rdf:resource="http://data.europa.eu/energy/StandardBusinessTypeList"/>
    <skos:topConceptOf rdf:resource="http://data.europa.eu/energy/StandardBusinessTypeList"/>
    <dcterms:identifier>B26</dcterms:identifier>
    <skos:prefLabel>Average balance price between MBAs</skos:prefLabel>
    <skos:definition xml:lang="en">A time series concerning the average prices between Market Balance Areas.</skos:definition>
  </skos:Concept>
  <skos:Concept rdf:about="http://data.europa.eu/energy/StandardBusinessTypeList/B27">
    <skos:inScheme rdf:resource="http://data.europa.eu/energy/StandardBusinessTypeList"/>
    <skos:topConceptOf rdf:resource="http://data.europa.eu/energy/StandardBusinessTypeList"/>
    <dcterms:identifier>B27</dcterms:identifier>
    <skos:prefLabel>Pumped</skos:prefLabel>
    <skos:definition xml:lang="en">A time series concerning the electricity consumption related to pumping.</skos:definition>
  </skos:Concept>
  <skos:Concept rdf:about="http://data.europa.eu/energy/StandardBusinessTypeList/B28">
    <skos:inScheme rdf:resource="http://data.europa.eu/energy/StandardBusinessTypeList"/>
    <skos:topConceptOf rdf:resource="http://data.europa.eu/energy/StandardBusinessTypeList"/>
    <dcterms:identifier>B28</dcterms:identifier>
    <skos:prefLabel>Large installation consumption</skos:prefLabel>
    <skos:definition xml:lang="en">A time series concerning consumption from large installation.</skos:definition>
  </skos:Concept>
  <skos:Concept rdf:about="http://data.europa.eu/energy/StandardBusinessTypeList/B29">
    <skos:inScheme rdf:resource="http://data.europa.eu/energy/StandardBusinessTypeList"/>
    <skos:topConceptOf rdf:resource="http://data.europa.eu/energy/StandardBusinessTypeList"/>
    <dcterms:identifier>B29</dcterms:identifier>
    <skos:prefLabel>Metering Grid Area (MGA) imbalance</skos:prefLabel>
    <skos:definition xml:lang="en">A time series concerning imbalance between reported consumption, production and exchange in a Metering Grid Area.</skos:definition>
  </skos:Concept>
  <skos:Concept rdf:about="http://data.europa.eu/energy/StandardBusinessTypeList/B30">
    <skos:inScheme rdf:resource="http://data.europa.eu/energy/StandardBusinessTypeList"/>
    <skos:topConceptOf rdf:resource="http://data.europa.eu/energy/StandardBusinessTypeList"/>
    <dcterms:identifier>B30</dcterms:identifier>
    <skos:prefLabel>HVDC Link settings</skos:prefLabel>
    <skos:definition xml:lang="en">The time series in question provides HVDC Link settings.</skos:definition>
  </skos:Concept>
  <skos:Concept rdf:about="http://data.europa.eu/energy/StandardBusinessTypeList/B31">
    <skos:inScheme rdf:resource="http://data.europa.eu/energy/StandardBusinessTypeList"/>
    <skos:topConceptOf rdf:resource="http://data.europa.eu/energy/StandardBusinessTypeList"/>
    <dcterms:identifier>B31</dcterms:identifier>
    <skos:prefLabel>Transmission Reliability Margin (TRM)</skos:prefLabel>
    <skos:definition xml:lang="en">A time series concerning Transmission Reliability Margin (TRM).</skos:definition>
  </skos:Concept>
  <skos:Concept rdf:about="http://data.europa.eu/energy/StandardBusinessTypeList/B32">
    <skos:inScheme rdf:resource="http://data.europa.eu/energy/StandardBusinessTypeList"/>
    <skos:topConceptOf rdf:resource="http://data.europa.eu/energy/StandardBusinessTypeList"/>
    <dcterms:identifier>B32</dcterms:identifier>
    <skos:prefLabel>Imbalance component for a pool</skos:prefLabel>
    <skos:definition xml:lang="en">This information is used to provide to a pool manager the combined imbalance of all the pool participants.</skos:definition>
  </skos:Concept>
  <skos:Concept rdf:about="http://data.europa.eu/energy/StandardBusinessTypeList/B33">
    <skos:inScheme rdf:resource="http://data.europa.eu/energy/StandardBusinessTypeList"/>
    <skos:topConceptOf rdf:resource="http://data.europa.eu/energy/StandardBusinessTypeList"/>
    <dcterms:identifier>B33</dcterms:identifier>
    <skos:prefLabel>Area Control error (ACE)</skos:prefLabel>
    <skos:definition xml:lang="en">The sum of the instantaneous difference between the actual and the set-point value of the measured total power value and Control Program including Virtual Tie-Lines for the power interchange of a LFC Area or a LFC Block and the frequency bias given by the product of the K-Factor of the LFC Area or the LFC Block and the Frequency Deviation.</skos:definition>
  </skos:Concept>
  <skos:Concept rdf:about="http://data.europa.eu/energy/StandardBusinessTypeList/B34">
    <skos:inScheme rdf:resource="http://data.europa.eu/energy/StandardBusinessTypeList"/>
    <skos:topConceptOf rdf:resource="http://data.europa.eu/energy/StandardBusinessTypeList"/>
    <dcterms:identifier>B34</dcterms:identifier>
    <skos:prefLabel>Area Control Error after Imbalance Netting</skos:prefLabel>
    <skos:definition xml:lang="en">A time series concerning the Area Control Error after applying the  imbalance netting energy correction.</skos:definition>
  </skos:Concept>
  <skos:Concept rdf:about="http://data.europa.eu/energy/StandardBusinessTypeList/B35">
    <skos:inScheme rdf:resource="http://data.europa.eu/energy/StandardBusinessTypeList"/>
    <skos:topConceptOf rdf:resource="http://data.europa.eu/energy/StandardBusinessTypeList"/>
    <dcterms:identifier>B35</dcterms:identifier>
    <skos:prefLabel>Implicit and explicit trade total</skos:prefLabel>
    <skos:definition xml:lang="en">The sum of cross border schedules based on implicit and explicit trades including long term, yearly, monthly, weekly, daily processes. </skos:definition>
  </skos:Concept>
  <skos:Concept rdf:about="http://data.europa.eu/energy/StandardBusinessTypeList/B36">
    <skos:inScheme rdf:resource="http://data.europa.eu/energy/StandardBusinessTypeList"/>
    <skos:topConceptOf rdf:resource="http://data.europa.eu/energy/StandardBusinessTypeList"/>
    <dcterms:identifier>B36</dcterms:identifier>
    <skos:prefLabel>Production units own consumption</skos:prefLabel>
    <skos:definition xml:lang="en">The consumption of one or more production units.</skos:definition>
  </skos:Concept>
  <skos:Concept rdf:about="http://data.europa.eu/energy/StandardBusinessTypeList/B37">
    <skos:inScheme rdf:resource="http://data.europa.eu/energy/StandardBusinessTypeList"/>
    <skos:topConceptOf rdf:resource="http://data.europa.eu/energy/StandardBusinessTypeList"/>
    <dcterms:identifier>B37</dcterms:identifier>
    <skos:prefLabel>Constraint situation</skos:prefLabel>
    <skos:definition xml:lang="en">The timeseries describes the constraint situation for a given TimeInterval.
A constraint situation can be: 
- composed of a list of network elements in outage associated for each outage to a list of network elements on which remedial actions have been carried out accordingly to contingency process 
- or it can be an external constraint.</skos:definition>
  </skos:Concept>
  <skos:Concept rdf:about="http://data.europa.eu/energy/StandardBusinessTypeList/B38">
    <skos:inScheme rdf:resource="http://data.europa.eu/energy/StandardBusinessTypeList"/>
    <skos:topConceptOf rdf:resource="http://data.europa.eu/energy/StandardBusinessTypeList"/>
    <dcterms:identifier>B38</dcterms:identifier>
    <skos:prefLabel>Initial domain</skos:prefLabel>
    <skos:definition xml:lang="en">The timeseries describe the full flow based domain for a given TimeInterval. 
Critical network elements are displayed in details and their impact on the market is quantified.</skos:definition>
  </skos:Concept>
  <skos:Concept rdf:about="http://data.europa.eu/energy/StandardBusinessTypeList/B39">
    <skos:inScheme rdf:resource="http://data.europa.eu/energy/StandardBusinessTypeList"/>
    <skos:topConceptOf rdf:resource="http://data.europa.eu/energy/StandardBusinessTypeList"/>
    <dcterms:identifier>B39</dcterms:identifier>
    <skos:prefLabel>Flow based domain adjusted to long term schedules</skos:prefLabel>
    <skos:definition xml:lang="en">The timeseries describe the full flow based domain for a given TimeInterval adjusted to the latest update of the schedules. 
Critical network elements are displayed in details and their impact on the market is quantified.</skos:definition>
  </skos:Concept>
  <skos:Concept rdf:about="http://data.europa.eu/energy/StandardBusinessTypeList/B40">
    <skos:inScheme rdf:resource="http://data.europa.eu/energy/StandardBusinessTypeList"/>
    <skos:topConceptOf rdf:resource="http://data.europa.eu/energy/StandardBusinessTypeList"/>
    <dcterms:identifier>B40</dcterms:identifier>
    <skos:prefLabel>Network element constraint</skos:prefLabel>
    <skos:definition xml:lang="en">The timeSeries describes limiting elements which are overloaded.</skos:definition>
  </skos:Concept>
  <skos:Concept rdf:about="http://data.europa.eu/energy/StandardBusinessTypeList/B41">
    <skos:inScheme rdf:resource="http://data.europa.eu/energy/StandardBusinessTypeList"/>
    <skos:topConceptOf rdf:resource="http://data.europa.eu/energy/StandardBusinessTypeList"/>
    <dcterms:identifier>B41</dcterms:identifier>
    <skos:prefLabel>Calculation opposition (Red Flag)</skos:prefLabel>
    <skos:definition xml:lang="en">The timeSeries describes a party who is opposed to the calculation result and imposes its transfer capacity value.</skos:definition>
  </skos:Concept>
  <skos:Concept rdf:about="http://data.europa.eu/energy/StandardBusinessTypeList/B42">
    <skos:inScheme rdf:resource="http://data.europa.eu/energy/StandardBusinessTypeList"/>
    <skos:topConceptOf rdf:resource="http://data.europa.eu/energy/StandardBusinessTypeList"/>
    <dcterms:identifier>B42</dcterms:identifier>
    <skos:prefLabel>Base case proportional shift key</skos:prefLabel>
    <skos:definition xml:lang="en">The GSK or LSK are proportional to the base case generation or load.</skos:definition>
  </skos:Concept>
  <skos:Concept rdf:about="http://data.europa.eu/energy/StandardBusinessTypeList/B43">
    <skos:inScheme rdf:resource="http://data.europa.eu/energy/StandardBusinessTypeList"/>
    <skos:topConceptOf rdf:resource="http://data.europa.eu/energy/StandardBusinessTypeList"/>
    <dcterms:identifier>B43</dcterms:identifier>
    <skos:prefLabel>Proportional to participation factors shift key</skos:prefLabel>
    <skos:definition xml:lang="en">The GSK or LSK are proportional to the participation factors.</skos:definition>
  </skos:Concept>
  <skos:Concept rdf:about="http://data.europa.eu/energy/StandardBusinessTypeList/B44">
    <skos:inScheme rdf:resource="http://data.europa.eu/energy/StandardBusinessTypeList"/>
    <skos:topConceptOf rdf:resource="http://data.europa.eu/energy/StandardBusinessTypeList"/>
    <dcterms:identifier>B44</dcterms:identifier>
    <skos:prefLabel>Proportional to the remaining capacity shift key</skos:prefLabel>
    <skos:definition xml:lang="en">The GSK is proportional to the remaining available capacity.</skos:definition>
  </skos:Concept>
  <skos:Concept rdf:about="http://data.europa.eu/energy/StandardBusinessTypeList/B45">
    <skos:inScheme rdf:resource="http://data.europa.eu/energy/StandardBusinessTypeList"/>
    <skos:topConceptOf rdf:resource="http://data.europa.eu/energy/StandardBusinessTypeList"/>
    <dcterms:identifier>B45</dcterms:identifier>
    <skos:prefLabel>Merit order shift key</skos:prefLabel>
    <skos:definition xml:lang="en">The GSK is proportional to a merit order list.</skos:definition>
  </skos:Concept>
  <skos:Concept rdf:about="http://data.europa.eu/energy/StandardBusinessTypeList/B46">
    <skos:inScheme rdf:resource="http://data.europa.eu/energy/StandardBusinessTypeList"/>
    <skos:topConceptOf rdf:resource="http://data.europa.eu/energy/StandardBusinessTypeList"/>
    <dcterms:identifier>B46</dcterms:identifier>
    <skos:prefLabel>Wind speed</skos:prefLabel>
    <skos:definition xml:lang="en">The TimeSeries provides information on the wind speed.</skos:definition>
  </skos:Concept>
  <skos:Concept rdf:about="http://data.europa.eu/energy/StandardBusinessTypeList/B47">
    <skos:inScheme rdf:resource="http://data.europa.eu/energy/StandardBusinessTypeList"/>
    <skos:topConceptOf rdf:resource="http://data.europa.eu/energy/StandardBusinessTypeList"/>
    <dcterms:identifier>B47</dcterms:identifier>
    <skos:prefLabel>Wind direction</skos:prefLabel>
    <skos:definition xml:lang="en">The TimeSeries provides information on the wind direction.</skos:definition>
  </skos:Concept>
  <skos:Concept rdf:about="http://data.europa.eu/energy/StandardBusinessTypeList/B48">
    <skos:inScheme rdf:resource="http://data.europa.eu/energy/StandardBusinessTypeList"/>
    <skos:topConceptOf rdf:resource="http://data.europa.eu/energy/StandardBusinessTypeList"/>
    <dcterms:identifier>B48</dcterms:identifier>
    <skos:prefLabel>Solar irradiance</skos:prefLabel>
    <skos:definition xml:lang="en">The TimeSeries provides information on the power per unit area produced by the sun in the form of electromagnetic radiation.</skos:definition>
  </skos:Concept>
  <skos:Concept rdf:about="http://data.europa.eu/energy/StandardBusinessTypeList/B49">
    <skos:inScheme rdf:resource="http://data.europa.eu/energy/StandardBusinessTypeList"/>
    <skos:topConceptOf rdf:resource="http://data.europa.eu/energy/StandardBusinessTypeList"/>
    <dcterms:identifier>B49</dcterms:identifier>
    <skos:prefLabel>Air temperature</skos:prefLabel>
    <skos:definition xml:lang="en">The TimeSeries provides information on the air temperature.</skos:definition>
  </skos:Concept>
  <skos:Concept rdf:about="http://data.europa.eu/energy/StandardBusinessTypeList/B50">
    <skos:inScheme rdf:resource="http://data.europa.eu/energy/StandardBusinessTypeList"/>
    <skos:topConceptOf rdf:resource="http://data.europa.eu/energy/StandardBusinessTypeList"/>
    <dcterms:identifier>B50</dcterms:identifier>
    <skos:prefLabel>Cloudiness</skos:prefLabel>
    <skos:definition xml:lang="en">The TimeSeries provides information on the cloudiness, i.e. the level of coverage of the sky with clouds.</skos:definition>
  </skos:Concept>
  <skos:Concept rdf:about="http://data.europa.eu/energy/StandardBusinessTypeList/B51">
    <skos:inScheme rdf:resource="http://data.europa.eu/energy/StandardBusinessTypeList"/>
    <skos:topConceptOf rdf:resource="http://data.europa.eu/energy/StandardBusinessTypeList"/>
    <dcterms:identifier>B51</dcterms:identifier>
    <skos:prefLabel>Air humidity</skos:prefLabel>
    <skos:definition xml:lang="en">The TimeSeries provides information on the level of humidity of the air.</skos:definition>
  </skos:Concept>
  <skos:Concept rdf:about="http://data.europa.eu/energy/StandardBusinessTypeList/B52">
    <skos:inScheme rdf:resource="http://data.europa.eu/energy/StandardBusinessTypeList"/>
    <skos:topConceptOf rdf:resource="http://data.europa.eu/energy/StandardBusinessTypeList"/>
    <dcterms:identifier>B52</dcterms:identifier>
    <skos:prefLabel>Atmospheric pressure</skos:prefLabel>
    <skos:definition xml:lang="en">The TimeSeries provides information on the atmospheric pressure.</skos:definition>
  </skos:Concept>
  <skos:Concept rdf:about="http://data.europa.eu/energy/StandardBusinessTypeList/B53">
    <skos:inScheme rdf:resource="http://data.europa.eu/energy/StandardBusinessTypeList"/>
    <skos:topConceptOf rdf:resource="http://data.europa.eu/energy/StandardBusinessTypeList"/>
    <dcterms:identifier>B53</dcterms:identifier>
    <skos:prefLabel>Precipitation</skos:prefLabel>
    <skos:definition xml:lang="en">The TimeSeries provides information on the amount of rain, snow, etc. that falls on the ground.</skos:definition>
  </skos:Concept>
  <skos:Concept rdf:about="http://data.europa.eu/energy/StandardBusinessTypeList/B54">
    <skos:inScheme rdf:resource="http://data.europa.eu/energy/StandardBusinessTypeList"/>
    <skos:topConceptOf rdf:resource="http://data.europa.eu/energy/StandardBusinessTypeList"/>
    <dcterms:identifier>B54</dcterms:identifier>
    <skos:prefLabel>Network constraint situation that constraints the market</skos:prefLabel>
    <skos:definition xml:lang="en">The TimeSeries describes the network elements, that constraints the market, to be taken into account to simulate a network constraint during the network load flow studies. The network situation includes the contingencies, the remedial actions, the monitored network elements and the potential additional constraints.</skos:definition>
  </skos:Concept>
  <skos:Concept rdf:about="http://data.europa.eu/energy/StandardBusinessTypeList/B55">
    <skos:inScheme rdf:resource="http://data.europa.eu/energy/StandardBusinessTypeList"/>
    <skos:topConceptOf rdf:resource="http://data.europa.eu/energy/StandardBusinessTypeList"/>
    <dcterms:identifier>B55</dcterms:identifier>
    <skos:prefLabel>Contingency</skos:prefLabel>
    <skos:definition xml:lang="en">The TimeSeries describes the network elements part of the contingency to be simulated for a given TimeInterval.</skos:definition>
  </skos:Concept>
  <skos:Concept rdf:about="http://data.europa.eu/energy/StandardBusinessTypeList/B56">
    <skos:inScheme rdf:resource="http://data.europa.eu/energy/StandardBusinessTypeList"/>
    <skos:topConceptOf rdf:resource="http://data.europa.eu/energy/StandardBusinessTypeList"/>
    <dcterms:identifier>B56</dcterms:identifier>
    <skos:prefLabel>Remedial Action</skos:prefLabel>
    <skos:definition xml:lang="en">The TimeSeries describes a set of remedial actions for a given TimeInterval.</skos:definition>
  </skos:Concept>
  <skos:Concept rdf:about="http://data.europa.eu/energy/StandardBusinessTypeList/B57">
    <skos:inScheme rdf:resource="http://data.europa.eu/energy/StandardBusinessTypeList"/>
    <skos:topConceptOf rdf:resource="http://data.europa.eu/energy/StandardBusinessTypeList"/>
    <dcterms:identifier>B57</dcterms:identifier>
    <skos:prefLabel>Monitored Network Element</skos:prefLabel>
    <skos:definition xml:lang="en">The TimeSeries describes the network elements to be monitored during the network load flow studies.</skos:definition>
  </skos:Concept>
  <skos:Concept rdf:about="http://data.europa.eu/energy/StandardBusinessTypeList/B58">
    <skos:inScheme rdf:resource="http://data.europa.eu/energy/StandardBusinessTypeList"/>
    <skos:topConceptOf rdf:resource="http://data.europa.eu/energy/StandardBusinessTypeList"/>
    <dcterms:identifier>B58</dcterms:identifier>
    <skos:prefLabel>Busbar</skos:prefLabel>
    <skos:definition xml:lang="en">The TimeSeries describes the network elements that composed a busbar.</skos:definition>
  </skos:Concept>
  <skos:Concept rdf:about="http://data.europa.eu/energy/StandardBusinessTypeList/B59">
    <skos:inScheme rdf:resource="http://data.europa.eu/energy/StandardBusinessTypeList"/>
    <skos:topConceptOf rdf:resource="http://data.europa.eu/energy/StandardBusinessTypeList"/>
    <dcterms:identifier>B59</dcterms:identifier>
    <skos:prefLabel>Network Element</skos:prefLabel>
    <skos:definition xml:lang="en">The TimeSeries describes network elements.</skos:definition>
  </skos:Concept>
  <skos:Concept rdf:about="http://data.europa.eu/energy/StandardBusinessTypeList/B60">
    <skos:inScheme rdf:resource="http://data.europa.eu/energy/StandardBusinessTypeList"/>
    <skos:topConceptOf rdf:resource="http://data.europa.eu/energy/StandardBusinessTypeList"/>
    <dcterms:identifier>B60</dcterms:identifier>
    <skos:prefLabel>SPS</skos:prefLabel>
    <skos:definition xml:lang="en">The TimeSeries describes the network elements managed by a Special Protection System (automation).</skos:definition>
  </skos:Concept>
  <skos:Concept rdf:about="http://data.europa.eu/energy/StandardBusinessTypeList/B61">
    <skos:inScheme rdf:resource="http://data.europa.eu/energy/StandardBusinessTypeList"/>
    <skos:topConceptOf rdf:resource="http://data.europa.eu/energy/StandardBusinessTypeList"/>
    <dcterms:identifier>B61</dcterms:identifier>
    <skos:prefLabel>Aggregated netted external market schedule</skos:prefLabel>
    <skos:definition xml:lang="en">The aggregated netted external market schedules for a given border.</skos:definition>
  </skos:Concept>
  <skos:Concept rdf:about="http://data.europa.eu/energy/StandardBusinessTypeList/B62">
    <skos:inScheme rdf:resource="http://data.europa.eu/energy/StandardBusinessTypeList"/>
    <skos:topConceptOf rdf:resource="http://data.europa.eu/energy/StandardBusinessTypeList"/>
    <dcterms:identifier>B62</dcterms:identifier>
    <skos:prefLabel>Aggregated netted external TSO schedule</skos:prefLabel>
    <skos:definition xml:lang="en">The aggregated netted external TSO schedules for a given border.</skos:definition>
  </skos:Concept>
  <skos:Concept rdf:about="http://data.europa.eu/energy/StandardBusinessTypeList/B63">
    <skos:inScheme rdf:resource="http://data.europa.eu/energy/StandardBusinessTypeList"/>
    <skos:topConceptOf rdf:resource="http://data.europa.eu/energy/StandardBusinessTypeList"/>
    <dcterms:identifier>B63</dcterms:identifier>
    <skos:prefLabel>Aggregated netted external schedule</skos:prefLabel>
    <skos:definition xml:lang="en">The aggregated netted external schedules for a given border.</skos:definition>
  </skos:Concept>
  <skos:Concept rdf:about="http://data.europa.eu/energy/StandardBusinessTypeList/B64">
    <skos:inScheme rdf:resource="http://data.europa.eu/energy/StandardBusinessTypeList"/>
    <skos:topConceptOf rdf:resource="http://data.europa.eu/energy/StandardBusinessTypeList"/>
    <dcterms:identifier>B64</dcterms:identifier>
    <skos:prefLabel>Netted area AC position</skos:prefLabel>
    <skos:definition xml:lang="en">The AC position for a given area.</skos:definition>
  </skos:Concept>
  <skos:Concept rdf:about="http://data.europa.eu/energy/StandardBusinessTypeList/B65">
    <skos:inScheme rdf:resource="http://data.europa.eu/energy/StandardBusinessTypeList"/>
    <skos:topConceptOf rdf:resource="http://data.europa.eu/energy/StandardBusinessTypeList"/>
    <dcterms:identifier>B65</dcterms:identifier>
    <skos:prefLabel>Netted area position</skos:prefLabel>
    <skos:definition xml:lang="en">The netted aggregation of all AC external schedules of an area plus the aggregated External Netted Schedules of related HVDC links of an area.</skos:definition>
  </skos:Concept>
  <skos:Concept rdf:about="http://data.europa.eu/energy/StandardBusinessTypeList/B66">
    <skos:inScheme rdf:resource="http://data.europa.eu/energy/StandardBusinessTypeList"/>
    <skos:topConceptOf rdf:resource="http://data.europa.eu/energy/StandardBusinessTypeList"/>
    <dcterms:identifier>B66</dcterms:identifier>
    <skos:prefLabel>Interconnection shift key</skos:prefLabel>
    <skos:definition xml:lang="en">The shift key series describes the amount of power to be shifted from a border area.
</skos:definition>
  </skos:Concept>
  <skos:Concept rdf:about="http://data.europa.eu/energy/StandardBusinessTypeList/B67">
    <skos:inScheme rdf:resource="http://data.europa.eu/energy/StandardBusinessTypeList"/>
    <skos:topConceptOf rdf:resource="http://data.europa.eu/energy/StandardBusinessTypeList"/>
    <dcterms:identifier>B67</dcterms:identifier>
    <skos:prefLabel>DC flow with losses</skos:prefLabel>
    <skos:definition xml:lang="en">DC flow with losses refers to the values at the importing end of the DC line.</skos:definition>
  </skos:Concept>
  <skos:Concept rdf:about="http://data.europa.eu/energy/StandardBusinessTypeList/B68">
    <skos:inScheme rdf:resource="http://data.europa.eu/energy/StandardBusinessTypeList"/>
    <skos:topConceptOf rdf:resource="http://data.europa.eu/energy/StandardBusinessTypeList"/>
    <dcterms:identifier>B68</dcterms:identifier>
    <skos:prefLabel>DC flow without losses</skos:prefLabel>
    <skos:definition xml:lang="en">DC flow without losses refers to the values at the exporting end of the DC line.</skos:definition>
  </skos:Concept>
  <skos:Concept rdf:about="http://data.europa.eu/energy/StandardBusinessTypeList/B69">
    <skos:inScheme rdf:resource="http://data.europa.eu/energy/StandardBusinessTypeList"/>
    <skos:topConceptOf rdf:resource="http://data.europa.eu/energy/StandardBusinessTypeList"/>
    <dcterms:identifier>B69</dcterms:identifier>
    <skos:prefLabel>minimum value of netted area position</skos:prefLabel>
    <skos:definition xml:lang="en">That value which a netted area position must not fall below for a given area.</skos:definition>
  </skos:Concept>
  <skos:Concept rdf:about="http://data.europa.eu/energy/StandardBusinessTypeList/B70">
    <skos:inScheme rdf:resource="http://data.europa.eu/energy/StandardBusinessTypeList"/>
    <skos:topConceptOf rdf:resource="http://data.europa.eu/energy/StandardBusinessTypeList"/>
    <dcterms:identifier>B70</dcterms:identifier>
    <skos:prefLabel>maximum value of netted area position</skos:prefLabel>
    <skos:definition xml:lang="en">That value which a netted area position must not exceed for a given optimisation area. </skos:definition>
  </skos:Concept>
  <skos:Concept rdf:about="http://data.europa.eu/energy/StandardBusinessTypeList/B71">
    <skos:inScheme rdf:resource="http://data.europa.eu/energy/StandardBusinessTypeList"/>
    <skos:topConceptOf rdf:resource="http://data.europa.eu/energy/StandardBusinessTypeList"/>
    <dcterms:identifier>B71</dcterms:identifier>
    <skos:prefLabel>maximum value of DC flow</skos:prefLabel>
    <skos:definition xml:lang="en">That value which a balanced DC flow must not exceed for a given DC line on exporting end. When aligning DC flows CGMA algorithm will respect this constraint.</skos:definition>
  </skos:Concept>
  <skos:Concept rdf:about="http://data.europa.eu/energy/StandardBusinessTypeList/B72">
    <skos:inScheme rdf:resource="http://data.europa.eu/energy/StandardBusinessTypeList"/>
    <skos:topConceptOf rdf:resource="http://data.europa.eu/energy/StandardBusinessTypeList"/>
    <dcterms:identifier>B72</dcterms:identifier>
    <skos:prefLabel>minimum value of DC flow</skos:prefLabel>
    <skos:definition xml:lang="en">That value which a balanced DC flow must not fall below for a given DC line on exporting end. Currently this business type is only included for consistency reasons. It is always set to 0. This constraint might, however, be used in future. When aligning DC flows the CGMA algorithm will respect this constraint.</skos:definition>
  </skos:Concept>
  <skos:Concept rdf:about="http://data.europa.eu/energy/StandardBusinessTypeList/B73">
    <skos:inScheme rdf:resource="http://data.europa.eu/energy/StandardBusinessTypeList"/>
    <skos:topConceptOf rdf:resource="http://data.europa.eu/energy/StandardBusinessTypeList"/>
    <dcterms:identifier>B73</dcterms:identifier>
    <skos:prefLabel>indicative AC flow</skos:prefLabel>
    <skos:definition xml:lang="en">It is the hypothetical flow on the aggregate of all AC tie lines of an electrical border between two optimisation areas. It results from the adjustments to the preliminary netted area positions of all optimisation areas made by the CGMA algorithm. Indicative AC flows are an artefact of the CGMA algorithm, and do not correspond to physical flows</skos:definition>
  </skos:Concept>
  <skos:Concept rdf:about="http://data.europa.eu/energy/StandardBusinessTypeList/B74">
    <skos:inScheme rdf:resource="http://data.europa.eu/energy/StandardBusinessTypeList"/>
    <skos:topConceptOf rdf:resource="http://data.europa.eu/energy/StandardBusinessTypeList"/>
    <dcterms:identifier>B74</dcterms:identifier>
    <skos:prefLabel>Offer</skos:prefLabel>
    <skos:definition xml:lang="en">The time series provides an offer to provide reserves. </skos:definition>
  </skos:Concept>
  <skos:Concept rdf:about="http://data.europa.eu/energy/StandardBusinessTypeList/B75">
    <skos:inScheme rdf:resource="http://data.europa.eu/energy/StandardBusinessTypeList"/>
    <skos:topConceptOf rdf:resource="http://data.europa.eu/energy/StandardBusinessTypeList"/>
    <dcterms:identifier>B75</dcterms:identifier>
    <skos:prefLabel>Need</skos:prefLabel>
    <skos:definition xml:lang="en">The time series provides a requirement for reserves.
</skos:definition>
  </skos:Concept>
  <skos:Concept rdf:about="http://data.europa.eu/energy/StandardBusinessTypeList/B76">
    <skos:inScheme rdf:resource="http://data.europa.eu/energy/StandardBusinessTypeList"/>
    <skos:topConceptOf rdf:resource="http://data.europa.eu/energy/StandardBusinessTypeList"/>
    <dcterms:identifier>B76</dcterms:identifier>
    <skos:prefLabel>Opportunity costs or benefits</skos:prefLabel>
    <skos:definition xml:lang="en">The time series describes any opportunity costs or benefits.</skos:definition>
  </skos:Concept>
  <skos:Concept rdf:about="http://data.europa.eu/energy/StandardBusinessTypeList/B77">
    <skos:inScheme rdf:resource="http://data.europa.eu/energy/StandardBusinessTypeList"/>
    <skos:topConceptOf rdf:resource="http://data.europa.eu/energy/StandardBusinessTypeList"/>
    <dcterms:identifier>B77</dcterms:identifier>
    <skos:prefLabel>Financial compensation or penalties</skos:prefLabel>
    <skos:definition xml:lang="en">The time series describes any financial compensation or penalties</skos:definition>
  </skos:Concept>
  <skos:Concept rdf:about="http://data.europa.eu/energy/StandardBusinessTypeList/B78">
    <skos:inScheme rdf:resource="http://data.europa.eu/energy/StandardBusinessTypeList"/>
    <skos:topConceptOf rdf:resource="http://data.europa.eu/energy/StandardBusinessTypeList"/>
    <dcterms:identifier>B78</dcterms:identifier>
    <skos:prefLabel>Global radiation</skos:prefLabel>
    <skos:definition xml:lang="en">The total short-wave radiation from the Global radiation is the total short-wave radiation from the sky falling onto a horizontal surface on the ground. It includes both the direct solar radiation and the diffuse radiation resulting from reflected or scattered sunlight.</skos:definition>
  </skos:Concept>
  <skos:Concept rdf:about="http://data.europa.eu/energy/StandardBusinessTypeList/B79">
    <skos:inScheme rdf:resource="http://data.europa.eu/energy/StandardBusinessTypeList"/>
    <skos:topConceptOf rdf:resource="http://data.europa.eu/energy/StandardBusinessTypeList"/>
    <dcterms:identifier>B79</dcterms:identifier>
    <skos:prefLabel>Diffuse radiation</skos:prefLabel>
    <skos:definition xml:lang="en">Radiation resulting from reflected or scattered sunlight.</skos:definition>
  </skos:Concept>
  <skos:Concept rdf:about="http://data.europa.eu/energy/StandardBusinessTypeList/B80">
    <skos:inScheme rdf:resource="http://data.europa.eu/energy/StandardBusinessTypeList"/>
    <skos:topConceptOf rdf:resource="http://data.europa.eu/energy/StandardBusinessTypeList"/>
    <dcterms:identifier>B80</dcterms:identifier>
    <skos:prefLabel>Direct solar radiation</skos:prefLabel>
    <skos:definition xml:lang="en">Radiation resulting from direct sunlight</skos:definition>
  </skos:Concept>
  <skos:Concept rdf:about="http://data.europa.eu/energy/StandardBusinessTypeList/B81">
    <skos:inScheme rdf:resource="http://data.europa.eu/energy/StandardBusinessTypeList"/>
    <skos:topConceptOf rdf:resource="http://data.europa.eu/energy/StandardBusinessTypeList"/>
    <dcterms:identifier>B81</dcterms:identifier>
    <skos:prefLabel>Outage (OUT)</skos:prefLabel>
    <skos:definition xml:lang="en">Outage process: Element is out of operation due to planned maintenance or due to an unplanned/forced outage. Outage may be used as a synonym for unavailability. </skos:definition>
  </skos:Concept>
  <skos:Concept rdf:about="http://data.europa.eu/energy/StandardBusinessTypeList/B82">
    <skos:inScheme rdf:resource="http://data.europa.eu/energy/StandardBusinessTypeList"/>
    <skos:topConceptOf rdf:resource="http://data.europa.eu/energy/StandardBusinessTypeList"/>
    <dcterms:identifier>B82</dcterms:identifier>
    <skos:prefLabel>Special switching state (SSS)</skos:prefLabel>
    <skos:definition xml:lang="en">Outage Process: This state applies to grid elements which are in operation in an exceptional state (e.g. separated nodes operation).</skos:definition>
  </skos:Concept>
  <skos:Concept rdf:about="http://data.europa.eu/energy/StandardBusinessTypeList/B83">
    <skos:inScheme rdf:resource="http://data.europa.eu/energy/StandardBusinessTypeList"/>
    <skos:topConceptOf rdf:resource="http://data.europa.eu/energy/StandardBusinessTypeList"/>
    <dcterms:identifier>B83</dcterms:identifier>
    <skos:prefLabel>Testing (TEST)</skos:prefLabel>
    <skos:definition xml:lang="en">Outage process: TESTING means any element status is possible - ON or OUT. This status applies either between first connection and final commissioning of the relevant asset, or directly following maintenance of the relevant asset.</skos:definition>
  </skos:Concept>
  <skos:Concept rdf:about="http://data.europa.eu/energy/StandardBusinessTypeList/B84">
    <skos:inScheme rdf:resource="http://data.europa.eu/energy/StandardBusinessTypeList"/>
    <skos:topConceptOf rdf:resource="http://data.europa.eu/energy/StandardBusinessTypeList"/>
    <dcterms:identifier>B84</dcterms:identifier>
    <skos:prefLabel>Auxiliary busbar operation</skos:prefLabel>
    <skos:definition xml:lang="en">Outage process: Element is in operation but connected via auxiliary busbar</skos:definition>
  </skos:Concept>
  <skos:Concept rdf:about="http://data.europa.eu/energy/StandardBusinessTypeList/B85">
    <skos:inScheme rdf:resource="http://data.europa.eu/energy/StandardBusinessTypeList"/>
    <skos:topConceptOf rdf:resource="http://data.europa.eu/energy/StandardBusinessTypeList"/>
    <dcterms:identifier>B85</dcterms:identifier>
    <skos:prefLabel>Automatic reclosing</skos:prefLabel>
    <skos:definition xml:lang="en">Outage process: Protection function Automatic reclosing is switched off for electric line</skos:definition>
  </skos:Concept>
  <skos:Concept rdf:about="http://data.europa.eu/energy/StandardBusinessTypeList/B86">
    <skos:inScheme rdf:resource="http://data.europa.eu/energy/StandardBusinessTypeList"/>
    <skos:topConceptOf rdf:resource="http://data.europa.eu/energy/StandardBusinessTypeList"/>
    <dcterms:identifier>B86</dcterms:identifier>
    <skos:prefLabel>Busbar protection</skos:prefLabel>
    <skos:definition xml:lang="en">Protection function busbar protection is switched off</skos:definition>
  </skos:Concept>
  <skos:Concept rdf:about="http://data.europa.eu/energy/StandardBusinessTypeList/B87">
    <skos:inScheme rdf:resource="http://data.europa.eu/energy/StandardBusinessTypeList"/>
    <skos:topConceptOf rdf:resource="http://data.europa.eu/energy/StandardBusinessTypeList"/>
    <dcterms:identifier>B87</dcterms:identifier>
    <skos:prefLabel>Phase Shift Angle</skos:prefLabel>
    <skos:definition xml:lang="en">The maximum phase shift angle allowed between two network elements. </skos:definition>
  </skos:Concept>
  <skos:Concept rdf:about="http://data.europa.eu/energy/StandardBusinessTypeList/B88">
    <skos:inScheme rdf:resource="http://data.europa.eu/energy/StandardBusinessTypeList"/>
    <skos:topConceptOf rdf:resource="http://data.europa.eu/energy/StandardBusinessTypeList"/>
    <dcterms:identifier>B88</dcterms:identifier>
    <skos:prefLabel>Base Case Network Situation</skos:prefLabel>
    <skos:definition xml:lang="en">The TimeSeries describes the network elements to be taken into account to simulate a base case network situation during the network load flow studies, without any contingency.</skos:definition>
  </skos:Concept>
  <skos:Concept rdf:about="http://data.europa.eu/energy/StandardBusinessTypeList/B89">
    <skos:inScheme rdf:resource="http://data.europa.eu/energy/StandardBusinessTypeList"/>
    <skos:topConceptOf rdf:resource="http://data.europa.eu/energy/StandardBusinessTypeList"/>
    <dcterms:identifier>B89</dcterms:identifier>
    <skos:prefLabel>Inter-TSO assistance</skos:prefLabel>
    <skos:definition xml:lang="en">Cross border assistance schedule between TSOs not interconnected directly. </skos:definition>
  </skos:Concept>
  <skos:Concept rdf:about="http://data.europa.eu/energy/StandardBusinessTypeList/B90">
    <skos:inScheme rdf:resource="http://data.europa.eu/energy/StandardBusinessTypeList"/>
    <skos:topConceptOf rdf:resource="http://data.europa.eu/energy/StandardBusinessTypeList"/>
    <dcterms:identifier>B90</dcterms:identifier>
    <skos:prefLabel>FlexibleNeed</skos:prefLabel>
    <skos:definition xml:lang="en">The business type indicates that the need is optional.</skos:definition>
  </skos:Concept>
  <skos:Concept rdf:about="http://data.europa.eu/energy/StandardBusinessTypeList/B91">
    <skos:inScheme rdf:resource="http://data.europa.eu/energy/StandardBusinessTypeList"/>
    <skos:topConceptOf rdf:resource="http://data.europa.eu/energy/StandardBusinessTypeList"/>
    <dcterms:identifier>B91</dcterms:identifier>
    <skos:prefLabel>GLSK Limitation</skos:prefLabel>
    <skos:definition xml:lang="en">A constraint related to a GLSK maximum or minimum limitation in the production or/and consumption shift.</skos:definition>
  </skos:Concept>
  <skos:Concept rdf:about="http://data.europa.eu/energy/StandardBusinessTypeList/B92">
    <skos:inScheme rdf:resource="http://data.europa.eu/energy/StandardBusinessTypeList"/>
    <skos:topConceptOf rdf:resource="http://data.europa.eu/energy/StandardBusinessTypeList"/>
    <dcterms:identifier>B92</dcterms:identifier>
    <skos:prefLabel>Capacity ramping limitation</skos:prefLabel>
    <skos:definition xml:lang="en">A constraint related to a ramping limitation on the capacity offered at a given border.</skos:definition>
  </skos:Concept>
  <skos:Concept rdf:about="http://data.europa.eu/energy/StandardBusinessTypeList/B93">
    <skos:inScheme rdf:resource="http://data.europa.eu/energy/StandardBusinessTypeList"/>
    <skos:topConceptOf rdf:resource="http://data.europa.eu/energy/StandardBusinessTypeList"/>
    <dcterms:identifier>B93</dcterms:identifier>
    <skos:prefLabel>interconnector capacity</skos:prefLabel>
    <skos:definition xml:lang="en">The maximum capacity that can be exchanged on an interconnector, excluding external factor on both ends. </skos:definition>
  </skos:Concept>
  <skos:Concept rdf:about="http://data.europa.eu/energy/StandardBusinessTypeList/B94">
    <skos:inScheme rdf:resource="http://data.europa.eu/energy/StandardBusinessTypeList"/>
    <skos:topConceptOf rdf:resource="http://data.europa.eu/energy/StandardBusinessTypeList"/>
    <dcterms:identifier>B94</dcterms:identifier>
    <skos:prefLabel>Must Run</skos:prefLabel>
    <skos:definition xml:lang="en">A time series concerning must run generation.</skos:definition>
  </skos:Concept>
  <skos:Concept rdf:about="http://data.europa.eu/energy/StandardBusinessTypeList/B95">
    <skos:inScheme rdf:resource="http://data.europa.eu/energy/StandardBusinessTypeList"/>
    <skos:topConceptOf rdf:resource="http://data.europa.eu/energy/StandardBusinessTypeList"/>
    <dcterms:identifier>B95</dcterms:identifier>
    <skos:prefLabel>Procured capacity</skos:prefLabel>
    <skos:definition xml:lang="en">An accepted offer of balancing capacity.</skos:definition>
  </skos:Concept>
  <skos:Concept rdf:about="http://data.europa.eu/energy/StandardBusinessTypeList/B96">
    <skos:inScheme rdf:resource="http://data.europa.eu/energy/StandardBusinessTypeList"/>
    <skos:topConceptOf rdf:resource="http://data.europa.eu/energy/StandardBusinessTypeList"/>
    <dcterms:identifier>B96</dcterms:identifier>
    <skos:prefLabel>Used capacity</skos:prefLabel>
    <skos:definition xml:lang="en">The used cross-zonal balancing capacity.</skos:definition>
  </skos:Concept>
  <skos:Concept rdf:about="http://data.europa.eu/energy/StandardBusinessTypeList/B97">
    <skos:inScheme rdf:resource="http://data.europa.eu/energy/StandardBusinessTypeList"/>
    <skos:topConceptOf rdf:resource="http://data.europa.eu/energy/StandardBusinessTypeList"/>
    <dcterms:identifier>B97</dcterms:identifier>
    <skos:prefLabel>Estimated costs</skos:prefLabel>
    <skos:definition xml:lang="en">Estimated costs of the process.</skos:definition>
  </skos:Concept>
  <skos:Concept rdf:about="http://data.europa.eu/energy/StandardBusinessTypeList/B98">
    <skos:inScheme rdf:resource="http://data.europa.eu/energy/StandardBusinessTypeList"/>
    <skos:topConceptOf rdf:resource="http://data.europa.eu/energy/StandardBusinessTypeList"/>
    <dcterms:identifier>B98</dcterms:identifier>
    <skos:prefLabel>Estimated benefits</skos:prefLabel>
    <skos:definition xml:lang="en">Estimated benefits of the process.</skos:definition>
  </skos:Concept>
  <skos:Concept rdf:about="http://data.europa.eu/energy/StandardBusinessTypeList/B99">
    <skos:inScheme rdf:resource="http://data.europa.eu/energy/StandardBusinessTypeList"/>
    <skos:topConceptOf rdf:resource="http://data.europa.eu/energy/StandardBusinessTypeList"/>
    <dcterms:identifier>B99</dcterms:identifier>
    <skos:prefLabel>Load Shedding</skos:prefLabel>
    <skos:definition xml:lang="en">A time series concerning a load shedding used to avoid failure of the power system.</skos:definition>
  </skos:Concept>
  <skos:Concept rdf:about="http://data.europa.eu/energy/StandardBusinessTypeList/C01">
    <skos:inScheme rdf:resource="http://data.europa.eu/energy/StandardBusinessTypeList"/>
    <skos:topConceptOf rdf:resource="http://data.europa.eu/energy/StandardBusinessTypeList"/>
    <dcterms:identifier>C01</dcterms:identifier>
    <skos:prefLabel>Remaining Capacity</skos:prefLabel>
    <skos:definition xml:lang="en">A time series concerning the remaining capacity.</skos:definition>
  </skos:Concept>
  <skos:Concept rdf:about="http://data.europa.eu/energy/StandardBusinessTypeList/C02">
    <skos:inScheme rdf:resource="http://data.europa.eu/energy/StandardBusinessTypeList"/>
    <skos:topConceptOf rdf:resource="http://data.europa.eu/energy/StandardBusinessTypeList"/>
    <dcterms:identifier>C02</dcterms:identifier>
    <skos:prefLabel>Indicator of generation capacity adequacy</skos:prefLabel>
    <skos:definition xml:lang="en">Indicator of adequacy, it indicates if there is final generation remaining capacity after SMTA calculation.</skos:definition>
  </skos:Concept>
  <skos:Concept rdf:about="http://data.europa.eu/energy/StandardBusinessTypeList/C03">
    <skos:inScheme rdf:resource="http://data.europa.eu/energy/StandardBusinessTypeList"/>
    <skos:topConceptOf rdf:resource="http://data.europa.eu/energy/StandardBusinessTypeList"/>
    <dcterms:identifier>C03</dcterms:identifier>
    <skos:prefLabel>Income from price divergence without congestions</skos:prefLabel>
    <skos:definition xml:lang="en">The time series describes income due to price divergence without congestion between bidding zones.</skos:definition>
  </skos:Concept>
  <skos:Concept rdf:about="http://data.europa.eu/energy/StandardBusinessTypeList/C04">
    <skos:inScheme rdf:resource="http://data.europa.eu/energy/StandardBusinessTypeList"/>
    <skos:topConceptOf rdf:resource="http://data.europa.eu/energy/StandardBusinessTypeList"/>
    <dcterms:identifier>C04</dcterms:identifier>
    <skos:prefLabel>Push-button</skos:prefLabel>
    <skos:definition xml:lang="en">The cross-border Push-button service between System Operators.</skos:definition>
  </skos:Concept>
  <skos:Concept rdf:about="http://data.europa.eu/energy/StandardBusinessTypeList/C05">
    <skos:inScheme rdf:resource="http://data.europa.eu/energy/StandardBusinessTypeList"/>
    <skos:topConceptOf rdf:resource="http://data.europa.eu/energy/StandardBusinessTypeList"/>
    <dcterms:identifier>C05</dcterms:identifier>
    <skos:prefLabel>Intertripping</skos:prefLabel>
    <skos:definition xml:lang="en">The cross-border Intertripping service between System Operators.</skos:definition>
  </skos:Concept>
  <skos:Concept rdf:about="http://data.europa.eu/energy/StandardBusinessTypeList/C06">
    <skos:inScheme rdf:resource="http://data.europa.eu/energy/StandardBusinessTypeList"/>
    <skos:topConceptOf rdf:resource="http://data.europa.eu/energy/StandardBusinessTypeList"/>
    <dcterms:identifier>C06</dcterms:identifier>
    <skos:prefLabel>Emergency instruction</skos:prefLabel>
    <skos:definition xml:lang="en">The cross-border Emergency instruction service between System Operators.</skos:definition>
  </skos:Concept>
  <skos:Concept rdf:about="http://data.europa.eu/energy/StandardBusinessTypeList/C07">
    <skos:inScheme rdf:resource="http://data.europa.eu/energy/StandardBusinessTypeList"/>
    <skos:topConceptOf rdf:resource="http://data.europa.eu/energy/StandardBusinessTypeList"/>
    <dcterms:identifier>C07</dcterms:identifier>
    <skos:prefLabel>Ramp management</skos:prefLabel>
    <skos:definition xml:lang="en">The schedule resulting from cross-border Ramp management service between System Operators.</skos:definition>
  </skos:Concept>
  <skos:Concept rdf:about="http://data.europa.eu/energy/StandardBusinessTypeList/C08">
    <skos:inScheme rdf:resource="http://data.europa.eu/energy/StandardBusinessTypeList"/>
    <skos:topConceptOf rdf:resource="http://data.europa.eu/energy/StandardBusinessTypeList"/>
    <dcterms:identifier>C08</dcterms:identifier>
    <skos:prefLabel>Profile smoothing</skos:prefLabel>
    <skos:definition xml:lang="en">The schedule resulting from cross-border Profile smoothing service between System Operators.</skos:definition>
  </skos:Concept>
  <skos:Concept rdf:about="http://data.europa.eu/energy/StandardBusinessTypeList/C09">
    <skos:inScheme rdf:resource="http://data.europa.eu/energy/StandardBusinessTypeList"/>
    <skos:topConceptOf rdf:resource="http://data.europa.eu/energy/StandardBusinessTypeList"/>
    <dcterms:identifier>C09</dcterms:identifier>
    <skos:prefLabel>Emergency reallocation deselection</skos:prefLabel>
    <skos:definition xml:lang="en">The schedule resulting from cross-border Emergency reallocation deselection service between System Operators.</skos:definition>
  </skos:Concept>
  <skos:Concept rdf:about="http://data.europa.eu/energy/StandardBusinessTypeList/C10">
    <skos:inScheme rdf:resource="http://data.europa.eu/energy/StandardBusinessTypeList"/>
    <skos:topConceptOf rdf:resource="http://data.europa.eu/energy/StandardBusinessTypeList"/>
    <dcterms:identifier>C10</dcterms:identifier>
    <skos:prefLabel>SO-SO-trade</skos:prefLabel>
    <skos:definition xml:lang="en">The generic cross border trade between System Operators.</skos:definition>
  </skos:Concept>
  <skos:Concept rdf:about="http://data.europa.eu/energy/StandardBusinessTypeList/C11">
    <skos:inScheme rdf:resource="http://data.europa.eu/energy/StandardBusinessTypeList"/>
    <skos:topConceptOf rdf:resource="http://data.europa.eu/energy/StandardBusinessTypeList"/>
    <dcterms:identifier>C11</dcterms:identifier>
    <skos:prefLabel>Production reduction</skos:prefLabel>
    <skos:definition xml:lang="en">A time series providing the volume of production reduced by an energy provider / producer / supplier.</skos:definition>
  </skos:Concept>
  <skos:Concept rdf:about="http://data.europa.eu/energy/StandardBusinessTypeList/C12">
    <skos:inScheme rdf:resource="http://data.europa.eu/energy/StandardBusinessTypeList"/>
    <skos:topConceptOf rdf:resource="http://data.europa.eu/energy/StandardBusinessTypeList"/>
    <dcterms:identifier>C12</dcterms:identifier>
    <skos:prefLabel>Maximum power exchange</skos:prefLabel>
    <skos:definition xml:lang="en">The timeseries provides the maximum admissible power flow between two bidding zones respecting operational security limits taking into account N-1 criterion.</skos:definition>
  </skos:Concept>
  <skos:Concept rdf:about="http://data.europa.eu/energy/StandardBusinessTypeList/C13">
    <skos:inScheme rdf:resource="http://data.europa.eu/energy/StandardBusinessTypeList"/>
    <skos:topConceptOf rdf:resource="http://data.europa.eu/energy/StandardBusinessTypeList"/>
    <dcterms:identifier>C13</dcterms:identifier>
    <skos:prefLabel>Maximum power exchange after remedial actions</skos:prefLabel>
    <skos:definition xml:lang="en">The timeseries provides the maximum admissible power flow between two bidding zones after remedial actions.</skos:definition>
  </skos:Concept>
  <skos:Concept rdf:about="http://data.europa.eu/energy/StandardBusinessTypeList/C14">
    <skos:inScheme rdf:resource="http://data.europa.eu/energy/StandardBusinessTypeList"/>
    <skos:topConceptOf rdf:resource="http://data.europa.eu/energy/StandardBusinessTypeList"/>
    <dcterms:identifier>C14</dcterms:identifier>
    <skos:prefLabel>Network constraint situation that cannot limit the market</skos:prefLabel>
    <skos:definition xml:lang="en">The TimeSeries describes the network elements, that cannot limit the market, to be taken into account to simulate a network constraint during the network load flow studies. The network situation includes the contingencies, the remedial actions, the monitored network elements and the potential additional constraints.</skos:definition>
  </skos:Concept>
  <skos:Concept rdf:about="http://data.europa.eu/energy/StandardBusinessTypeList/C15">
    <skos:inScheme rdf:resource="http://data.europa.eu/energy/StandardBusinessTypeList"/>
    <skos:topConceptOf rdf:resource="http://data.europa.eu/energy/StandardBusinessTypeList"/>
    <dcterms:identifier>C15</dcterms:identifier>
    <skos:prefLabel>Flat participation for all generators or loads</skos:prefLabel>
    <skos:definition xml:lang="en">Flat GSK factors of all generators or loads, independently of the size.</skos:definition>
  </skos:Concept>
  <skos:Concept rdf:about="http://data.europa.eu/energy/StandardBusinessTypeList/C16">
    <skos:inScheme rdf:resource="http://data.europa.eu/energy/StandardBusinessTypeList"/>
    <skos:topConceptOf rdf:resource="http://data.europa.eu/energy/StandardBusinessTypeList"/>
    <dcterms:identifier>C16</dcterms:identifier>
    <skos:prefLabel>Proportional to installed capacity of generators</skos:prefLabel>
    <skos:definition xml:lang="en">Generators participate relative to their maximum (installed) capacity (MW).</skos:definition>
  </skos:Concept>
  <skos:Concept rdf:about="http://data.europa.eu/energy/StandardBusinessTypeList/C17">
    <skos:inScheme rdf:resource="http://data.europa.eu/energy/StandardBusinessTypeList"/>
    <skos:topConceptOf rdf:resource="http://data.europa.eu/energy/StandardBusinessTypeList"/>
    <dcterms:identifier>C17</dcterms:identifier>
    <skos:prefLabel>Market price and total volume</skos:prefLabel>
    <skos:definition xml:lang="en">A time series concerning market price and total volume.</skos:definition>
  </skos:Concept>
  <skos:Concept rdf:about="http://data.europa.eu/energy/StandardBusinessTypeList/C18">
    <skos:inScheme rdf:resource="http://data.europa.eu/energy/StandardBusinessTypeList"/>
    <skos:topConceptOf rdf:resource="http://data.europa.eu/energy/StandardBusinessTypeList"/>
    <dcterms:identifier>C18</dcterms:identifier>
    <skos:prefLabel>Import price</skos:prefLabel>
    <skos:definition xml:lang="en">A time series concerning import price (the volume-weighted price average of all accepted bids).</skos:definition>
  </skos:Concept>
  <skos:Concept rdf:about="http://data.europa.eu/energy/StandardBusinessTypeList/C19">
    <skos:inScheme rdf:resource="http://data.europa.eu/energy/StandardBusinessTypeList"/>
    <skos:topConceptOf rdf:resource="http://data.europa.eu/energy/StandardBusinessTypeList"/>
    <dcterms:identifier>C19</dcterms:identifier>
    <skos:prefLabel>Capacity allocated (excluding price)</skos:prefLabel>
    <skos:definition xml:lang="en">The business being described concerns capacity allocation and excludes price information.</skos:definition>
  </skos:Concept>
  <skos:Concept rdf:about="http://data.europa.eu/energy/StandardBusinessTypeList/C20">
    <skos:inScheme rdf:resource="http://data.europa.eu/energy/StandardBusinessTypeList"/>
    <skos:topConceptOf rdf:resource="http://data.europa.eu/energy/StandardBusinessTypeList"/>
    <dcterms:identifier>C20</dcterms:identifier>
    <skos:prefLabel>Common Grid Model Equipment</skos:prefLabel>
    <skos:definition xml:lang="en">The timeseries provides equipment related to the Common Grid Model (CGM).</skos:definition>
  </skos:Concept>
  <skos:Concept rdf:about="http://data.europa.eu/energy/StandardBusinessTypeList/C21">
    <skos:inScheme rdf:resource="http://data.europa.eu/energy/StandardBusinessTypeList"/>
    <skos:topConceptOf rdf:resource="http://data.europa.eu/energy/StandardBusinessTypeList"/>
    <dcterms:identifier>C21</dcterms:identifier>
    <skos:prefLabel>Exchanged balancing reserve capacity</skos:prefLabel>
    <skos:definition xml:lang="en">The balancing reserve capacity exchanged between areas.</skos:definition>
  </skos:Concept>
  <skos:Concept rdf:about="http://data.europa.eu/energy/StandardBusinessTypeList/C22">
    <skos:inScheme rdf:resource="http://data.europa.eu/energy/StandardBusinessTypeList"/>
    <skos:topConceptOf rdf:resource="http://data.europa.eu/energy/StandardBusinessTypeList"/>
    <dcterms:identifier>C22</dcterms:identifier>
    <skos:prefLabel>Shared balancing reserve capacity</skos:prefLabel>
    <skos:definition xml:lang="en">The balancing reserve capacity shared between areas.</skos:definition>
  </skos:Concept>
  <skos:Concept rdf:about="http://data.europa.eu/energy/StandardBusinessTypeList/C23">
    <skos:inScheme rdf:resource="http://data.europa.eu/energy/StandardBusinessTypeList"/>
    <skos:topConceptOf rdf:resource="http://data.europa.eu/energy/StandardBusinessTypeList"/>
    <dcterms:identifier>C23</dcterms:identifier>
    <skos:prefLabel>Share of reserve capacity</skos:prefLabel>
    <skos:definition xml:lang="en">A time series concerning the share of reserve capacity.</skos:definition>
  </skos:Concept>
  <skos:Concept rdf:about="http://data.europa.eu/energy/StandardBusinessTypeList/C24">
    <skos:inScheme rdf:resource="http://data.europa.eu/energy/StandardBusinessTypeList"/>
    <skos:topConceptOf rdf:resource="http://data.europa.eu/energy/StandardBusinessTypeList"/>
    <dcterms:identifier>C24</dcterms:identifier>
    <skos:prefLabel>Actual reserve capacity</skos:prefLabel>
    <skos:definition xml:lang="en">A timeseries concerning actual reserve capacity.</skos:definition>
  </skos:Concept>
  <skos:Concept rdf:about="http://data.europa.eu/energy/StandardBusinessTypeList/C25">
    <skos:inScheme rdf:resource="http://data.europa.eu/energy/StandardBusinessTypeList"/>
    <skos:topConceptOf rdf:resource="http://data.europa.eu/energy/StandardBusinessTypeList"/>
    <dcterms:identifier>C25</dcterms:identifier>
    <skos:prefLabel>K-factor</skos:prefLabel>
    <skos:definition xml:lang="en">K-factor as stated in the SO GL Art. 2 (45). It is also known as Frequency Bias.</skos:definition>
  </skos:Concept>
  <skos:Concept rdf:about="http://data.europa.eu/energy/StandardBusinessTypeList/C26">
    <skos:inScheme rdf:resource="http://data.europa.eu/energy/StandardBusinessTypeList"/>
    <skos:topConceptOf rdf:resource="http://data.europa.eu/energy/StandardBusinessTypeList"/>
    <dcterms:identifier>C26</dcterms:identifier>
    <skos:prefLabel>Frequency Containment Reserve-Normal (FCR-N)</skos:prefLabel>
    <skos:definition xml:lang="en">FCR-N is a reserve that is automatically activated in both directions around a set point when the frequency varies between 50.10 Hz and 49.90 Hz after an imbalance.</skos:definition>
  </skos:Concept>
  <skos:Concept rdf:about="http://data.europa.eu/energy/StandardBusinessTypeList/C27">
    <skos:inScheme rdf:resource="http://data.europa.eu/energy/StandardBusinessTypeList"/>
    <skos:topConceptOf rdf:resource="http://data.europa.eu/energy/StandardBusinessTypeList"/>
    <dcterms:identifier>C27</dcterms:identifier>
    <skos:prefLabel>Frequency Containment Reserve-Disturbance (FCR-D)</skos:prefLabel>
    <skos:definition xml:lang="en">FCR-D is a reserve that is automatically activated when the frequency falls below 49.90 Hz or rises above 50.1 Hz after an imbalance.</skos:definition>
  </skos:Concept>
  <skos:Concept rdf:about="http://data.europa.eu/energy/StandardBusinessTypeList/C28">
    <skos:inScheme rdf:resource="http://data.europa.eu/energy/StandardBusinessTypeList"/>
    <skos:topConceptOf rdf:resource="http://data.europa.eu/energy/StandardBusinessTypeList"/>
    <dcterms:identifier>C28</dcterms:identifier>
    <skos:prefLabel>Internal trade difference</skos:prefLabel>
    <skos:definition xml:lang="en">A time series concerning internal trade difference, within an area, such as a Bidding Zone or Scheduling Area. The internal trade difference is the difference between trades reported from an out party (seller) and an in party (buyer). </skos:definition>
  </skos:Concept>
  <skos:Concept rdf:about="http://data.europa.eu/energy/StandardBusinessTypeList/C29">
    <skos:inScheme rdf:resource="http://data.europa.eu/energy/StandardBusinessTypeList"/>
    <skos:topConceptOf rdf:resource="http://data.europa.eu/energy/StandardBusinessTypeList"/>
    <dcterms:identifier>C29</dcterms:identifier>
    <skos:prefLabel>Small scale production</skos:prefLabel>
    <skos:definition xml:lang="en">Production from small scale production plants.</skos:definition>
  </skos:Concept>
  <skos:Concept rdf:about="http://data.europa.eu/energy/StandardBusinessTypeList/C30">
    <skos:inScheme rdf:resource="http://data.europa.eu/energy/StandardBusinessTypeList"/>
    <skos:topConceptOf rdf:resource="http://data.europa.eu/energy/StandardBusinessTypeList"/>
    <dcterms:identifier>C30</dcterms:identifier>
    <skos:prefLabel>System price</skos:prefLabel>
    <skos:definition xml:lang="en">The system price is an unconstrained market clearing reference price. It is calculated without any congestion restrictions by setting capacities to infinity.</skos:definition>
  </skos:Concept>
  <skos:Concept rdf:about="http://data.europa.eu/energy/StandardBusinessTypeList/C31">
    <skos:inScheme rdf:resource="http://data.europa.eu/energy/StandardBusinessTypeList"/>
    <skos:topConceptOf rdf:resource="http://data.europa.eu/energy/StandardBusinessTypeList"/>
    <dcterms:identifier>C31</dcterms:identifier>
    <skos:prefLabel>Wind gust</skos:prefLabel>
    <skos:definition xml:lang="en">An increase in the speed of the wind lasting for a short period.</skos:definition>
  </skos:Concept>
  <skos:Concept rdf:about="http://data.europa.eu/energy/StandardBusinessTypeList/C32">
    <skos:inScheme rdf:resource="http://data.europa.eu/energy/StandardBusinessTypeList"/>
    <skos:topConceptOf rdf:resource="http://data.europa.eu/energy/StandardBusinessTypeList"/>
    <dcterms:identifier>C32</dcterms:identifier>
    <skos:prefLabel>Area imbalance</skos:prefLabel>
    <skos:definition xml:lang="en">A time series concerning imbalance between planned consumption, production and exchange in an Area.</skos:definition>
  </skos:Concept>
  <skos:Concept rdf:about="http://data.europa.eu/energy/StandardBusinessTypeList/C33">
    <skos:inScheme rdf:resource="http://data.europa.eu/energy/StandardBusinessTypeList"/>
    <skos:topConceptOf rdf:resource="http://data.europa.eu/energy/StandardBusinessTypeList"/>
    <dcterms:identifier>C33</dcterms:identifier>
    <skos:prefLabel>Unintended energy price</skos:prefLabel>
    <skos:definition xml:lang="en">A timeseries concerning the price of the unintended cross-border exchange of energy.</skos:definition>
  </skos:Concept>
  <skos:Concept rdf:about="http://data.europa.eu/energy/StandardBusinessTypeList/C34">
    <skos:inScheme rdf:resource="http://data.europa.eu/energy/StandardBusinessTypeList"/>
    <skos:topConceptOf rdf:resource="http://data.europa.eu/energy/StandardBusinessTypeList"/>
    <dcterms:identifier>C34</dcterms:identifier>
    <skos:prefLabel>Frequency containment process energy</skos:prefLabel>
    <skos:definition xml:lang="en">A timeseries containing the volume of energy resulting from the frequency containment process.</skos:definition>
  </skos:Concept>
  <skos:Concept rdf:about="http://data.europa.eu/energy/StandardBusinessTypeList/C35">
    <skos:inScheme rdf:resource="http://data.europa.eu/energy/StandardBusinessTypeList"/>
    <skos:topConceptOf rdf:resource="http://data.europa.eu/energy/StandardBusinessTypeList"/>
    <dcterms:identifier>C35</dcterms:identifier>
    <skos:prefLabel>Frequency containment process energy price</skos:prefLabel>
    <skos:definition xml:lang="en">A timeseries containing the energy price from the frequency containment process.</skos:definition>
  </skos:Concept>
  <skos:Concept rdf:about="http://data.europa.eu/energy/StandardBusinessTypeList/C36">
    <skos:inScheme rdf:resource="http://data.europa.eu/energy/StandardBusinessTypeList"/>
    <skos:topConceptOf rdf:resource="http://data.europa.eu/energy/StandardBusinessTypeList"/>
    <dcterms:identifier>C36</dcterms:identifier>
    <skos:prefLabel>Ramping period energy</skos:prefLabel>
    <skos:definition xml:lang="en">A timeseries containing the volume of energy exchanged as a result of ramping between different ANES values.</skos:definition>
  </skos:Concept>
  <skos:Concept rdf:about="http://data.europa.eu/energy/StandardBusinessTypeList/C37">
    <skos:inScheme rdf:resource="http://data.europa.eu/energy/StandardBusinessTypeList"/>
    <skos:topConceptOf rdf:resource="http://data.europa.eu/energy/StandardBusinessTypeList"/>
    <dcterms:identifier>C37</dcterms:identifier>
    <skos:prefLabel>Ramping period energy price</skos:prefLabel>
    <skos:definition xml:lang="en">A timeseries containing the price of the energy exchanged as a result of ramping between different ANES values.</skos:definition>
  </skos:Concept>
  <skos:Concept rdf:about="http://data.europa.eu/energy/StandardBusinessTypeList/C38">
    <skos:inScheme rdf:resource="http://data.europa.eu/energy/StandardBusinessTypeList"/>
    <skos:topConceptOf rdf:resource="http://data.europa.eu/energy/StandardBusinessTypeList"/>
    <dcterms:identifier>C38</dcterms:identifier>
    <skos:prefLabel>Frequency deviation</skos:prefLabel>
    <skos:definition xml:lang="en">A timeseries concerning the difference between the actual and the nominal frequency of a synchronous area.</skos:definition>
  </skos:Concept>
  <skos:Concept rdf:about="http://data.europa.eu/energy/StandardBusinessTypeList/C39">
    <skos:inScheme rdf:resource="http://data.europa.eu/energy/StandardBusinessTypeList"/>
    <skos:topConceptOf rdf:resource="http://data.europa.eu/energy/StandardBusinessTypeList"/>
    <dcterms:identifier>C39</dcterms:identifier>
    <skos:prefLabel>Day-Ahead market price</skos:prefLabel>
    <skos:definition xml:lang="en">A timeseries concerning Day-Ahead market prices.</skos:definition>
  </skos:Concept>
  <skos:Concept rdf:about="http://data.europa.eu/energy/StandardBusinessTypeList/C40">
    <skos:inScheme rdf:resource="http://data.europa.eu/energy/StandardBusinessTypeList"/>
    <skos:topConceptOf rdf:resource="http://data.europa.eu/energy/StandardBusinessTypeList"/>
    <dcterms:identifier>C40</dcterms:identifier>
    <skos:prefLabel>Conditional bid</skos:prefLabel>
    <skos:definition xml:lang="en">Standard product bid that is conditional on bids submitted outside of common platform.</skos:definition>
  </skos:Concept>
  <skos:Concept rdf:about="http://data.europa.eu/energy/StandardBusinessTypeList/C41">
    <skos:inScheme rdf:resource="http://data.europa.eu/energy/StandardBusinessTypeList"/>
    <skos:topConceptOf rdf:resource="http://data.europa.eu/energy/StandardBusinessTypeList"/>
    <dcterms:identifier>C41</dcterms:identifier>
    <skos:prefLabel>Thermal limit</skos:prefLabel>
    <skos:definition xml:lang="en">The current causing a given network element to work outside of the range of safe operating temperatures.</skos:definition>
  </skos:Concept>
  <skos:Concept rdf:about="http://data.europa.eu/energy/StandardBusinessTypeList/C42">
    <skos:inScheme rdf:resource="http://data.europa.eu/energy/StandardBusinessTypeList"/>
    <skos:topConceptOf rdf:resource="http://data.europa.eu/energy/StandardBusinessTypeList"/>
    <dcterms:identifier>C42</dcterms:identifier>
    <skos:prefLabel>Frequency Limit</skos:prefLabel>
    <skos:definition xml:lang="en">A constraint related to the containment of frequency deviations within a given area.</skos:definition>
  </skos:Concept>
  <skos:Concept rdf:about="http://data.europa.eu/energy/StandardBusinessTypeList/C43">
    <skos:inScheme rdf:resource="http://data.europa.eu/energy/StandardBusinessTypeList"/>
    <skos:topConceptOf rdf:resource="http://data.europa.eu/energy/StandardBusinessTypeList"/>
    <dcterms:identifier>C43</dcterms:identifier>
    <skos:prefLabel>Voltage limit</skos:prefLabel>
    <skos:definition xml:lang="en">The maximum or minimum permissible voltage within normal operation state of a given network element.</skos:definition>
  </skos:Concept>
  <skos:Concept rdf:about="http://data.europa.eu/energy/StandardBusinessTypeList/C44">
    <skos:inScheme rdf:resource="http://data.europa.eu/energy/StandardBusinessTypeList"/>
    <skos:topConceptOf rdf:resource="http://data.europa.eu/energy/StandardBusinessTypeList"/>
    <dcterms:identifier>C44</dcterms:identifier>
    <skos:prefLabel>Current limit</skos:prefLabel>
    <skos:definition xml:lang="en">The maximum permissible current within normal operation state of a given network element.</skos:definition>
  </skos:Concept>
  <skos:Concept rdf:about="http://data.europa.eu/energy/StandardBusinessTypeList/C45">
    <skos:inScheme rdf:resource="http://data.europa.eu/energy/StandardBusinessTypeList"/>
    <skos:topConceptOf rdf:resource="http://data.europa.eu/energy/StandardBusinessTypeList"/>
    <dcterms:identifier>C45</dcterms:identifier>
    <skos:prefLabel>Short circuit current limit</skos:prefLabel>
    <skos:definition xml:lang="en">The maximum permissible short-circuit current within normal operation state of a given network element.</skos:definition>
  </skos:Concept>
  <skos:Concept rdf:about="http://data.europa.eu/energy/StandardBusinessTypeList/C46">
    <skos:inScheme rdf:resource="http://data.europa.eu/energy/StandardBusinessTypeList"/>
    <skos:topConceptOf rdf:resource="http://data.europa.eu/energy/StandardBusinessTypeList"/>
    <dcterms:identifier>C46</dcterms:identifier>
    <skos:prefLabel>Dynamic stability limit</skos:prefLabel>
    <skos:definition xml:lang="en">A maximum permissible load ensuring the control of oscillations in the grid and avoiding the loss of synchronism.</skos:definition>
  </skos:Concept>
  <skos:Concept rdf:about="http://data.europa.eu/energy/StandardBusinessTypeList/C47">
    <skos:inScheme rdf:resource="http://data.europa.eu/energy/StandardBusinessTypeList"/>
    <skos:topConceptOf rdf:resource="http://data.europa.eu/energy/StandardBusinessTypeList"/>
    <dcterms:identifier>C47</dcterms:identifier>
    <skos:prefLabel>Disconnection</skos:prefLabel>
    <skos:definition xml:lang="en">A timeseries describing disconnection of a TSO from a common platform.</skos:definition>
  </skos:Concept>
  <skos:Concept rdf:about="http://data.europa.eu/energy/StandardBusinessTypeList/C48">
    <skos:inScheme rdf:resource="http://data.europa.eu/energy/StandardBusinessTypeList"/>
    <skos:topConceptOf rdf:resource="http://data.europa.eu/energy/StandardBusinessTypeList"/>
    <dcterms:identifier>C48</dcterms:identifier>
    <skos:prefLabel>Intended energy with positive price</skos:prefLabel>
    <skos:definition xml:lang="en">A timeseries concerning the amount of intended energy with prices higher than zero (and including zero).</skos:definition>
  </skos:Concept>
  <skos:Concept rdf:about="http://data.europa.eu/energy/StandardBusinessTypeList/C49">
    <skos:inScheme rdf:resource="http://data.europa.eu/energy/StandardBusinessTypeList"/>
    <skos:topConceptOf rdf:resource="http://data.europa.eu/energy/StandardBusinessTypeList"/>
    <dcterms:identifier>C49</dcterms:identifier>
    <skos:prefLabel>Intended energy with negative price</skos:prefLabel>
    <skos:definition xml:lang="en">A timeseries concerning the amount of intended energy with prices lower than zero (excluding zero).</skos:definition>
  </skos:Concept>
  <skos:Concept rdf:about="http://data.europa.eu/energy/StandardBusinessTypeList/C50">
    <skos:inScheme rdf:resource="http://data.europa.eu/energy/StandardBusinessTypeList"/>
    <skos:topConceptOf rdf:resource="http://data.europa.eu/energy/StandardBusinessTypeList"/>
    <dcterms:identifier>C50</dcterms:identifier>
    <skos:prefLabel>Decopuling</skos:prefLabel>
    <skos:definition xml:lang="en">A time series describing decoupling of an area.</skos:definition>
  </skos:Concept>
  <skos:Concept rdf:about="http://data.europa.eu/energy/StandardBusinessTypeList/C51">
    <skos:inScheme rdf:resource="http://data.europa.eu/energy/StandardBusinessTypeList"/>
    <skos:topConceptOf rdf:resource="http://data.europa.eu/energy/StandardBusinessTypeList"/>
    <dcterms:identifier>C51</dcterms:identifier>
    <skos:prefLabel>Resource capacity unit</skos:prefLabel>
    <skos:definition xml:lang="en">A timeseries containing information about resource capacity units.</skos:definition>
  </skos:Concept>
  <skos:Concept rdf:about="http://data.europa.eu/energy/StandardBusinessTypeList/C52">
    <skos:inScheme rdf:resource="http://data.europa.eu/energy/StandardBusinessTypeList"/>
    <skos:topConceptOf rdf:resource="http://data.europa.eu/energy/StandardBusinessTypeList"/>
    <dcterms:identifier>C52</dcterms:identifier>
    <skos:prefLabel>Resource entry capacity data</skos:prefLabel>
    <skos:definition xml:lang="en">A timeseries containing the resource capacity that can be allocated to an eligible resource capacity operator from another area.</skos:definition>
  </skos:Concept>
  <skos:Concept rdf:about="http://data.europa.eu/energy/StandardBusinessTypeList/C53">
    <skos:inScheme rdf:resource="http://data.europa.eu/energy/StandardBusinessTypeList"/>
    <skos:topConceptOf rdf:resource="http://data.europa.eu/energy/StandardBusinessTypeList"/>
    <dcterms:identifier>C53</dcterms:identifier>
    <skos:prefLabel>Resource capacity obligation data</skos:prefLabel>
    <skos:definition xml:lang="en">A timeseries containing the resource capacity operator obligation to guarantee delivery.</skos:definition>
  </skos:Concept>
  <skos:Concept rdf:about="http://data.europa.eu/energy/StandardBusinessTypeList/C54">
    <skos:inScheme rdf:resource="http://data.europa.eu/energy/StandardBusinessTypeList"/>
    <skos:topConceptOf rdf:resource="http://data.europa.eu/energy/StandardBusinessTypeList"/>
    <dcterms:identifier>C54</dcterms:identifier>
    <skos:prefLabel>Available energy</skos:prefLabel>
    <skos:definition xml:lang="en">A timeseries concerning the available energy.</skos:definition>
  </skos:Concept>
  <skos:Concept rdf:about="http://data.europa.eu/energy/StandardBusinessTypeList/C55">
    <skos:inScheme rdf:resource="http://data.europa.eu/energy/StandardBusinessTypeList"/>
    <skos:topConceptOf rdf:resource="http://data.europa.eu/energy/StandardBusinessTypeList"/>
    <dcterms:identifier>C55</dcterms:identifier>
    <skos:prefLabel>Production curtailment</skos:prefLabel>
    <skos:definition xml:lang="en">A timeseries concerning the curtailment of production.</skos:definition>
  </skos:Concept>
  <skos:Concept rdf:about="http://data.europa.eu/energy/StandardBusinessTypeList/C56">
    <skos:inScheme rdf:resource="http://data.europa.eu/energy/StandardBusinessTypeList"/>
    <skos:topConceptOf rdf:resource="http://data.europa.eu/energy/StandardBusinessTypeList"/>
    <dcterms:identifier>C56</dcterms:identifier>
    <skos:prefLabel>Rounding error</skos:prefLabel>
    <skos:definition xml:lang="en">A timeseries describing a rounding error.</skos:definition>
  </skos:Concept>
  <skos:Concept rdf:about="http://data.europa.eu/energy/StandardBusinessTypeList/C57">
    <skos:inScheme rdf:resource="http://data.europa.eu/energy/StandardBusinessTypeList"/>
    <skos:topConceptOf rdf:resource="http://data.europa.eu/energy/StandardBusinessTypeList"/>
    <dcterms:identifier>C57</dcterms:identifier>
    <skos:prefLabel>Metered frequency</skos:prefLabel>
    <skos:definition xml:lang="en">The timeseries provides information about metered frequency.</skos:definition>
  </skos:Concept>
  <skos:Concept rdf:about="http://data.europa.eu/energy/StandardBusinessTypeList/C58">
    <skos:inScheme rdf:resource="http://data.europa.eu/energy/StandardBusinessTypeList"/>
    <skos:topConceptOf rdf:resource="http://data.europa.eu/energy/StandardBusinessTypeList"/>
    <dcterms:identifier>C58</dcterms:identifier>
    <skos:prefLabel>Adjusted TTC to the nominal criteria</skos:prefLabel>
    <skos:definition xml:lang="en">The exchange program between two areas which guarantees that the Margin Available for Cross-Zonal Trade (MACZT) fulfils the nominal criteria at least on the most limiting Critical Network Element with Contingency (CNEC) which limits the transfer capacity.</skos:definition>
  </skos:Concept>
  <skos:Concept rdf:about="http://data.europa.eu/energy/StandardBusinessTypeList/C59">
    <skos:inScheme rdf:resource="http://data.europa.eu/energy/StandardBusinessTypeList"/>
    <skos:topConceptOf rdf:resource="http://data.europa.eu/energy/StandardBusinessTypeList"/>
    <dcterms:identifier>C59</dcterms:identifier>
    <skos:prefLabel>Adjusted TTC to the nominal criteria with TSOs limitation</skos:prefLabel>
    <skos:definition xml:lang="en">The exchange program between two areas which allows the Margin Available for Cross-Zonal Trade (MACZT) on, at least, the most limiting Critical Network Element with Contingency (CNEC) to get closer to the nominal criteria fulfilment with a limited impact on the rest of the network.</skos:definition>
  </skos:Concept>
  <skos:Concept rdf:about="http://data.europa.eu/energy/StandardBusinessTypeList/C60">
    <skos:inScheme rdf:resource="http://data.europa.eu/energy/StandardBusinessTypeList"/>
    <skos:topConceptOf rdf:resource="http://data.europa.eu/energy/StandardBusinessTypeList"/>
    <dcterms:identifier>C60</dcterms:identifier>
    <skos:prefLabel>Frequency deviation larger than standard deviation</skos:prefLabel>
    <skos:definition xml:lang="en">Total time in which the absolute value of the instantaneous frequency deviation was larger than the standard frequency deviation.</skos:definition>
  </skos:Concept>
  <skos:Concept rdf:about="http://data.europa.eu/energy/StandardBusinessTypeList/C61">
    <skos:inScheme rdf:resource="http://data.europa.eu/energy/StandardBusinessTypeList"/>
    <skos:topConceptOf rdf:resource="http://data.europa.eu/energy/StandardBusinessTypeList"/>
    <dcterms:identifier>C61</dcterms:identifier>
    <skos:prefLabel>Frequency deviation larger than maximum deviation</skos:prefLabel>
    <skos:definition xml:lang="en">Total time in which the absolute value of the instantaneous frequency deviation was larger than the maximum instantaneous frequency deviation.</skos:definition>
  </skos:Concept>
  <skos:Concept rdf:about="http://data.europa.eu/energy/StandardBusinessTypeList/C62">
    <skos:inScheme rdf:resource="http://data.europa.eu/energy/StandardBusinessTypeList"/>
    <skos:topConceptOf rdf:resource="http://data.europa.eu/energy/StandardBusinessTypeList"/>
    <dcterms:identifier>C62</dcterms:identifier>
    <skos:prefLabel>Frequency deviation not returned to 50%</skos:prefLabel>
    <skos:definition xml:lang="en">Number of events in which the absolute value of the instantaneous frequency deviation of the synchronous area exceeded 200 % of the standard frequency deviation as stated in SO GL (EU) regulation Art 131.1.a.vi.</skos:definition>
  </skos:Concept>
  <skos:Concept rdf:about="http://data.europa.eu/energy/StandardBusinessTypeList/C63">
    <skos:inScheme rdf:resource="http://data.europa.eu/energy/StandardBusinessTypeList"/>
    <skos:topConceptOf rdf:resource="http://data.europa.eu/energy/StandardBusinessTypeList"/>
    <dcterms:identifier>C63</dcterms:identifier>
    <skos:prefLabel>Frequency deviation not returned to restoration range</skos:prefLabel>
    <skos:definition xml:lang="en">Number of events in which the absolute value of the instantaneous frequency deviation of the synchronous area exceeded 200 % of the standard frequency deviation.</skos:definition>
  </skos:Concept>
  <skos:Concept rdf:about="http://data.europa.eu/energy/StandardBusinessTypeList/C64">
    <skos:inScheme rdf:resource="http://data.europa.eu/energy/StandardBusinessTypeList"/>
    <skos:topConceptOf rdf:resource="http://data.europa.eu/energy/StandardBusinessTypeList"/>
    <dcterms:identifier>C64</dcterms:identifier>
    <skos:prefLabel>Frequency deviation outside recovery range</skos:prefLabel>
    <skos:definition xml:lang="en">Number of events for which the absolute value of the instantaneous frequency deviation was outside of the frequency recovery range.</skos:definition>
  </skos:Concept>
  <skos:Concept rdf:about="http://data.europa.eu/energy/StandardBusinessTypeList/C65">
    <skos:inScheme rdf:resource="http://data.europa.eu/energy/StandardBusinessTypeList"/>
    <skos:topConceptOf rdf:resource="http://data.europa.eu/energy/StandardBusinessTypeList"/>
    <dcterms:identifier>C65</dcterms:identifier>
    <skos:prefLabel>Frequency</skos:prefLabel>
    <skos:definition xml:lang="en">A time series describing measurement frequency.</skos:definition>
  </skos:Concept>
  <skos:Concept rdf:about="http://data.europa.eu/energy/StandardBusinessTypeList/C66">
    <skos:inScheme rdf:resource="http://data.europa.eu/energy/StandardBusinessTypeList"/>
    <skos:topConceptOf rdf:resource="http://data.europa.eu/energy/StandardBusinessTypeList"/>
    <dcterms:identifier>C66</dcterms:identifier>
    <skos:prefLabel>Mean value</skos:prefLabel>
    <skos:definition xml:lang="en">A time series describing mean values.</skos:definition>
  </skos:Concept>
  <skos:Concept rdf:about="http://data.europa.eu/energy/StandardBusinessTypeList/C67">
    <skos:inScheme rdf:resource="http://data.europa.eu/energy/StandardBusinessTypeList"/>
    <skos:topConceptOf rdf:resource="http://data.europa.eu/energy/StandardBusinessTypeList"/>
    <dcterms:identifier>C67</dcterms:identifier>
    <skos:prefLabel>Standard deviation</skos:prefLabel>
    <skos:definition xml:lang="en">A time series describing standard deviation.</skos:definition>
  </skos:Concept>
  <skos:Concept rdf:about="http://data.europa.eu/energy/StandardBusinessTypeList/C68">
    <skos:inScheme rdf:resource="http://data.europa.eu/energy/StandardBusinessTypeList"/>
    <skos:topConceptOf rdf:resource="http://data.europa.eu/energy/StandardBusinessTypeList"/>
    <dcterms:identifier>C68</dcterms:identifier>
    <skos:prefLabel>Percentile</skos:prefLabel>
    <skos:definition xml:lang="en">A time series describing percentiles.</skos:definition>
  </skos:Concept>
  <skos:Concept rdf:about="http://data.europa.eu/energy/StandardBusinessTypeList/C69">
    <skos:inScheme rdf:resource="http://data.europa.eu/energy/StandardBusinessTypeList"/>
    <skos:topConceptOf rdf:resource="http://data.europa.eu/energy/StandardBusinessTypeList"/>
    <dcterms:identifier>C69</dcterms:identifier>
    <skos:prefLabel>Measured frequency resolution</skos:prefLabel>
    <skos:definition xml:lang="en">A time series describing the resolution of a measured frequency.</skos:definition>
  </skos:Concept>
  <skos:Concept rdf:about="http://data.europa.eu/energy/StandardBusinessTypeList/C70">
    <skos:inScheme rdf:resource="http://data.europa.eu/energy/StandardBusinessTypeList"/>
    <skos:topConceptOf rdf:resource="http://data.europa.eu/energy/StandardBusinessTypeList"/>
    <dcterms:identifier>C70</dcterms:identifier>
    <skos:prefLabel>Accuracy</skos:prefLabel>
    <skos:definition xml:lang="en">A time series describing measurement accuracy.</skos:definition>
  </skos:Concept>
  <skos:Concept rdf:about="http://data.europa.eu/energy/StandardBusinessTypeList/C71">
    <skos:inScheme rdf:resource="http://data.europa.eu/energy/StandardBusinessTypeList"/>
    <skos:topConceptOf rdf:resource="http://data.europa.eu/energy/StandardBusinessTypeList"/>
    <dcterms:identifier>C71</dcterms:identifier>
    <skos:prefLabel>FRCE outside level 1 range</skos:prefLabel>
    <skos:definition xml:lang="en">The number of time intervals in which the average value of the FRCE was outside the Level 1 FRCE range as stated in SO GL. (EU) regulation Art 131.1.b.i.</skos:definition>
  </skos:Concept>
  <skos:Concept rdf:about="http://data.europa.eu/energy/StandardBusinessTypeList/C72">
    <skos:inScheme rdf:resource="http://data.europa.eu/energy/StandardBusinessTypeList"/>
    <skos:topConceptOf rdf:resource="http://data.europa.eu/energy/StandardBusinessTypeList"/>
    <dcterms:identifier>C72</dcterms:identifier>
    <skos:prefLabel>FRCE outside level 2 range</skos:prefLabel>
    <skos:definition xml:lang="en">The number of time intervals in which the average value of the FRCE was outside the Level 2 FRCE range as stated in SO GL (EU) regulation. Art 131.1.b.i.</skos:definition>
  </skos:Concept>
  <skos:Concept rdf:about="http://data.europa.eu/energy/StandardBusinessTypeList/C73">
    <skos:inScheme rdf:resource="http://data.europa.eu/energy/StandardBusinessTypeList"/>
    <skos:topConceptOf rdf:resource="http://data.europa.eu/energy/StandardBusinessTypeList"/>
    <dcterms:identifier>C73</dcterms:identifier>
    <skos:prefLabel>FRCE exceeded 60% of FRR capacity</skos:prefLabel>
    <skos:definition xml:lang="en">The number of events for which the FRCE exceeded 60 % of the reserve capacity on FRR as stated in SO GL (EU) regulation Art 131.1.b.ii.</skos:definition>
  </skos:Concept>
  <skos:Concept rdf:about="http://data.europa.eu/energy/StandardBusinessTypeList/C74">
    <skos:inScheme rdf:resource="http://data.europa.eu/energy/StandardBusinessTypeList"/>
    <skos:topConceptOf rdf:resource="http://data.europa.eu/energy/StandardBusinessTypeList"/>
    <dcterms:identifier>C74</dcterms:identifier>
    <skos:prefLabel>FRCE exceeded steady state deviation</skos:prefLabel>
    <skos:definition xml:lang="en">The number of events for which the absolute value of the FRCE exceeded the maximum steady-state frequency deviation.</skos:definition>
  </skos:Concept>
  <skos:Concept rdf:about="http://data.europa.eu/energy/StandardBusinessTypeList/C75">
    <skos:inScheme rdf:resource="http://data.europa.eu/energy/StandardBusinessTypeList"/>
    <skos:topConceptOf rdf:resource="http://data.europa.eu/energy/StandardBusinessTypeList"/>
    <dcterms:identifier>C75</dcterms:identifier>
    <skos:prefLabel>FRCE calculation and accuracy descriptor</skos:prefLabel>
    <skos:definition xml:lang="en">A time series describing how FRCE is calculated and its accuracy.</skos:definition>
  </skos:Concept>
  <skos:Concept rdf:about="http://data.europa.eu/energy/StandardBusinessTypeList/C76">
    <skos:inScheme rdf:resource="http://data.europa.eu/energy/StandardBusinessTypeList"/>
    <skos:topConceptOf rdf:resource="http://data.europa.eu/energy/StandardBusinessTypeList"/>
    <dcterms:identifier>C76</dcterms:identifier>
    <skos:prefLabel>Forecasted capacity</skos:prefLabel>
    <skos:definition xml:lang="en">A time series describing forecasted capacity.</skos:definition>
  </skos:Concept>
  <skos:Concept rdf:about="http://data.europa.eu/energy/StandardBusinessTypeList/C77">
    <skos:inScheme rdf:resource="http://data.europa.eu/energy/StandardBusinessTypeList"/>
    <skos:topConceptOf rdf:resource="http://data.europa.eu/energy/StandardBusinessTypeList"/>
    <dcterms:identifier>C77</dcterms:identifier>
    <skos:prefLabel>Minimum available capacity</skos:prefLabel>
    <skos:definition xml:lang="en">A time series describing minimum available capacity.</skos:definition>
  </skos:Concept>
  <skos:Concept rdf:about="http://data.europa.eu/energy/StandardBusinessTypeList/C78">
    <skos:inScheme rdf:resource="http://data.europa.eu/energy/StandardBusinessTypeList"/>
    <skos:topConceptOf rdf:resource="http://data.europa.eu/energy/StandardBusinessTypeList"/>
    <dcterms:identifier>C78</dcterms:identifier>
    <skos:prefLabel>Average available capacity</skos:prefLabel>
    <skos:definition xml:lang="en">A time series describing average available capacity.</skos:definition>
  </skos:Concept>
  <skos:Concept rdf:about="http://data.europa.eu/energy/StandardBusinessTypeList/C79">
    <skos:inScheme rdf:resource="http://data.europa.eu/energy/StandardBusinessTypeList"/>
    <skos:topConceptOf rdf:resource="http://data.europa.eu/energy/StandardBusinessTypeList"/>
    <dcterms:identifier>C79</dcterms:identifier>
    <skos:prefLabel>Maximum available capacity</skos:prefLabel>
    <skos:definition xml:lang="en">A time series describing maximum available capacity.</skos:definition>
  </skos:Concept>
  <skos:Concept rdf:about="http://data.europa.eu/energy/StandardBusinessTypeList/C80">
    <skos:inScheme rdf:resource="http://data.europa.eu/energy/StandardBusinessTypeList"/>
    <skos:topConceptOf rdf:resource="http://data.europa.eu/energy/StandardBusinessTypeList"/>
    <dcterms:identifier>C80</dcterms:identifier>
    <skos:prefLabel>Frequency and accuracy descriptor</skos:prefLabel>
    <skos:definition xml:lang="en">A time series describing how system frequency and accuracy are determined.</skos:definition>
  </skos:Concept>
  <skos:Concept rdf:about="http://data.europa.eu/energy/StandardBusinessTypeList/C81">
    <skos:inScheme rdf:resource="http://data.europa.eu/energy/StandardBusinessTypeList"/>
    <skos:topConceptOf rdf:resource="http://data.europa.eu/energy/StandardBusinessTypeList"/>
    <dcterms:identifier>C81</dcterms:identifier>
    <skos:prefLabel>Long-Term internal redispatch</skos:prefLabel>
    <skos:definition xml:lang="en">A time series describing long-term redispatch to relieve Scheduling Area internal congestion.</skos:definition>
  </skos:Concept>
  <skos:Concept rdf:about="http://data.europa.eu/energy/StandardBusinessTypeList/C82">
    <skos:inScheme rdf:resource="http://data.europa.eu/energy/StandardBusinessTypeList"/>
    <skos:topConceptOf rdf:resource="http://data.europa.eu/energy/StandardBusinessTypeList"/>
    <dcterms:identifier>C82</dcterms:identifier>
    <skos:prefLabel>Other unavailability</skos:prefLabel>
    <skos:definition xml:lang="en">This is an unplanned unavailability. Not considered by market participants as a planned maintenance.</skos:definition>
  </skos:Concept>
  <skos:Concept rdf:about="http://data.europa.eu/energy/StandardBusinessTypeList/C83">
    <skos:inScheme rdf:resource="http://data.europa.eu/energy/StandardBusinessTypeList"/>
    <skos:topConceptOf rdf:resource="http://data.europa.eu/energy/StandardBusinessTypeList"/>
    <dcterms:identifier>C83</dcterms:identifier>
    <skos:prefLabel>Faster than standard FAT</skos:prefLabel>
    <skos:definition xml:lang="en">Bids that can support a “Full Activation Time” (FAT) that is faster than standard FAT. Fast activation can be done for bids with activation time shorter than the minimum requirement for the standard product. When circumstances call for it, the TSO can order activation of such bids on a shorter notice.</skos:definition>
  </skos:Concept>
  <skos:Concept rdf:about="http://data.europa.eu/energy/StandardBusinessTypeList/C84">
    <skos:inScheme rdf:resource="http://data.europa.eu/energy/StandardBusinessTypeList"/>
    <skos:topConceptOf rdf:resource="http://data.europa.eu/energy/StandardBusinessTypeList"/>
    <dcterms:identifier>C84</dcterms:identifier>
    <skos:prefLabel>Faster than standard deactivation time</skos:prefLabel>
    <skos:definition xml:lang="en">Fast deactivation can be done for bids with activation time shorter than the minimum requirement for the standard product. When circumstances call for it, the TSO can order activation of such bids on a shorter notice.</skos:definition>
  </skos:Concept>
  <skos:Concept rdf:about="http://data.europa.eu/energy/StandardBusinessTypeList/C85">
    <skos:inScheme rdf:resource="http://data.europa.eu/energy/StandardBusinessTypeList"/>
    <skos:topConceptOf rdf:resource="http://data.europa.eu/energy/StandardBusinessTypeList"/>
    <dcterms:identifier>C85</dcterms:identifier>
    <skos:prefLabel>Slower than standard FAT</skos:prefLabel>
    <skos:definition xml:lang="en">Bids that can support a Full Activation Time (FAT) that is slower than standard FAT.</skos:definition>
  </skos:Concept>
</rdf:RDF>
