<?xml version='1.0' encoding='UTF-8'?>
<rdf:RDF xmlns:cim="http://iec.ch/TC57/2013/CIM-schema-cim16#" xmlns:rdf="http://www.w3.org/1999/02/22-rdf-syntax-ns#" xmlns:rdfs="http://www.w3.org/2000/01/rdf-schema#" xmlns:dcat="http://www.w3.org/ns/dcat#" xmlns:dc="http://purl.org/dc/elements/1.1/" xmlns:dcterms="http://purl.org/dc/terms/" xmlns:skos="http://www.w3.org/2004/02/skos/core#" xmlns:ecl="urn:entsoe.eu:wgedi:codelists" xmlns:xs="http://www.w3.org/2001/XMLSchema">
  <skos:ConceptScheme rdf:about="http://energy.referencedata.eu/StandardFuelTypeList">
    <dcterms:modified>2022-03-31</dcterms:modified>
    <dcat:version>81</dcat:version>
    <skos:prefLabel>StandardFuelTypeList</skos:prefLabel>
    <dcterms:identifier>ET0051</dcterms:identifier>
    <skos:definition xml:lang="en">The identification of the type of fuel.</skos:definition>
  </skos:ConceptScheme>
  <skos:Concept rdf:about="http://energy.referencedata.eu/StandardFuelTypeList/A01">
    <skos:inScheme rdf:resource="http://energy.referencedata.eu/StandardFuelTypeList"/>
    <skos:topConceptOf rdf:resource="http://energy.referencedata.eu/StandardFuelTypeList"/>
    <dcterms:identifier>A01</dcterms:identifier>
    <skos:prefLabel>Unspecified</skos:prefLabel>
    <skos:definition xml:lang="en">Fuel that cannot be associated with any of available fuel codes.</skos:definition>
  </skos:Concept>
  <skos:Concept rdf:about="http://energy.referencedata.eu/StandardFuelTypeList/A02">
    <skos:inScheme rdf:resource="http://energy.referencedata.eu/StandardFuelTypeList"/>
    <skos:topConceptOf rdf:resource="http://energy.referencedata.eu/StandardFuelTypeList"/>
    <dcterms:identifier>A02</dcterms:identifier>
    <skos:prefLabel>Renewable solid unspecified</skos:prefLabel>
    <skos:definition xml:lang="en">Fuel produced in a solid form from renewable resources that cannot be associated with any of available renewable solid fuel codes.</skos:definition>
  </skos:Concept>
  <skos:Concept rdf:about="http://energy.referencedata.eu/StandardFuelTypeList/A03">
    <skos:inScheme rdf:resource="http://energy.referencedata.eu/StandardFuelTypeList"/>
    <skos:topConceptOf rdf:resource="http://energy.referencedata.eu/StandardFuelTypeList"/>
    <dcterms:identifier>A03</dcterms:identifier>
    <skos:prefLabel>Renewable solid municipal waste</skos:prefLabel>
    <skos:definition xml:lang="en">Solid waste of biological material produced by households, hospitals and the tertiary sector (in general all waste that resembles household waste).</skos:definition>
  </skos:Concept>
  <skos:Concept rdf:about="http://energy.referencedata.eu/StandardFuelTypeList/A04">
    <skos:inScheme rdf:resource="http://energy.referencedata.eu/StandardFuelTypeList"/>
    <skos:topConceptOf rdf:resource="http://energy.referencedata.eu/StandardFuelTypeList"/>
    <dcterms:identifier>A04</dcterms:identifier>
    <skos:prefLabel>Renewable solid industrial and commercial waste</skos:prefLabel>
    <skos:definition xml:lang="en">Solid waste generated by businesses, production units, bureaus and offices.</skos:definition>
  </skos:Concept>
  <skos:Concept rdf:about="http://energy.referencedata.eu/StandardFuelTypeList/A05">
    <skos:inScheme rdf:resource="http://energy.referencedata.eu/StandardFuelTypeList"/>
    <skos:topConceptOf rdf:resource="http://energy.referencedata.eu/StandardFuelTypeList"/>
    <dcterms:identifier>A05</dcterms:identifier>
    <skos:prefLabel>Renewable solid wood</skos:prefLabel>
    <skos:definition xml:lang="en">Solid wood energy resource.</skos:definition>
  </skos:Concept>
  <skos:Concept rdf:about="http://energy.referencedata.eu/StandardFuelTypeList/A06">
    <skos:inScheme rdf:resource="http://energy.referencedata.eu/StandardFuelTypeList"/>
    <skos:topConceptOf rdf:resource="http://energy.referencedata.eu/StandardFuelTypeList"/>
    <dcterms:identifier>A06</dcterms:identifier>
    <skos:prefLabel>Renewable solid animal fats</skos:prefLabel>
    <skos:definition xml:lang="en">Solid animal fats energy resource.</skos:definition>
  </skos:Concept>
  <skos:Concept rdf:about="http://energy.referencedata.eu/StandardFuelTypeList/A07">
    <skos:inScheme rdf:resource="http://energy.referencedata.eu/StandardFuelTypeList"/>
    <skos:topConceptOf rdf:resource="http://energy.referencedata.eu/StandardFuelTypeList"/>
    <dcterms:identifier>A07</dcterms:identifier>
    <skos:prefLabel>Renewable solid biomass from agriculture</skos:prefLabel>
    <skos:definition xml:lang="en">Solid by-products and residues from agriculture.</skos:definition>
  </skos:Concept>
  <skos:Concept rdf:about="http://energy.referencedata.eu/StandardFuelTypeList/A08">
    <skos:inScheme rdf:resource="http://energy.referencedata.eu/StandardFuelTypeList"/>
    <skos:topConceptOf rdf:resource="http://energy.referencedata.eu/StandardFuelTypeList"/>
    <dcterms:identifier>A08</dcterms:identifier>
    <skos:prefLabel>Renewable liquid unspecified</skos:prefLabel>
    <skos:definition xml:lang="en">Fuel produced in form of liquid from renewable resources that cannot be associated with any of available renewable liquid fuel codes.</skos:definition>
  </skos:Concept>
  <skos:Concept rdf:about="http://energy.referencedata.eu/StandardFuelTypeList/A09">
    <skos:inScheme rdf:resource="http://energy.referencedata.eu/StandardFuelTypeList"/>
    <skos:topConceptOf rdf:resource="http://energy.referencedata.eu/StandardFuelTypeList"/>
    <dcterms:identifier>A09</dcterms:identifier>
    <skos:prefLabel>Renewable liquid municipal biodegradable waste</skos:prefLabel>
    <skos:definition xml:lang="en">Liquid municipal waste capable of undergoing anaerobic or aerobic decomposition.</skos:definition>
  </skos:Concept>
  <skos:Concept rdf:about="http://energy.referencedata.eu/StandardFuelTypeList/A10">
    <skos:inScheme rdf:resource="http://energy.referencedata.eu/StandardFuelTypeList"/>
    <skos:topConceptOf rdf:resource="http://energy.referencedata.eu/StandardFuelTypeList"/>
    <dcterms:identifier>A10</dcterms:identifier>
    <skos:prefLabel>Renewable liquid black liquor</skos:prefLabel>
    <skos:definition xml:lang="en">Alkaline-spent liquor obtained from the digesters during the production of sulphate or soda pulp.</skos:definition>
  </skos:Concept>
  <skos:Concept rdf:about="http://energy.referencedata.eu/StandardFuelTypeList/A11">
    <skos:inScheme rdf:resource="http://energy.referencedata.eu/StandardFuelTypeList"/>
    <skos:topConceptOf rdf:resource="http://energy.referencedata.eu/StandardFuelTypeList"/>
    <dcterms:identifier>A11</dcterms:identifier>
    <skos:prefLabel>Renewable liquid pure plant oil</skos:prefLabel>
    <skos:definition xml:lang="en">Oil produced from plants, mainly from rapeseed and sunflower crops.</skos:definition>
  </skos:Concept>
  <skos:Concept rdf:about="http://energy.referencedata.eu/StandardFuelTypeList/A12">
    <skos:inScheme rdf:resource="http://energy.referencedata.eu/StandardFuelTypeList"/>
    <skos:topConceptOf rdf:resource="http://energy.referencedata.eu/StandardFuelTypeList"/>
    <dcterms:identifier>A12</dcterms:identifier>
    <skos:prefLabel>Renewable liquid waste plant oil</skos:prefLabel>
    <skos:definition xml:lang="en">Oil produced from plants that is no longer usable for its originally intended purpose.</skos:definition>
  </skos:Concept>
  <skos:Concept rdf:about="http://energy.referencedata.eu/StandardFuelTypeList/A13">
    <skos:inScheme rdf:resource="http://energy.referencedata.eu/StandardFuelTypeList"/>
    <skos:topConceptOf rdf:resource="http://energy.referencedata.eu/StandardFuelTypeList"/>
    <dcterms:identifier>A13</dcterms:identifier>
    <skos:prefLabel>Renewable liquid refined vegetable oil</skos:prefLabel>
    <skos:definition xml:lang="en">Oil produced from plants and transformed into fuel by refining process (hydrocracking or hydrogenation).</skos:definition>
  </skos:Concept>
  <skos:Concept rdf:about="http://energy.referencedata.eu/StandardFuelTypeList/A14">
    <skos:inScheme rdf:resource="http://energy.referencedata.eu/StandardFuelTypeList"/>
    <skos:topConceptOf rdf:resource="http://energy.referencedata.eu/StandardFuelTypeList"/>
    <dcterms:identifier>A14</dcterms:identifier>
    <skos:prefLabel>Renewable gaseous unspecified</skos:prefLabel>
    <skos:definition xml:lang="en">Fuel produced in form of gas from renewable resources that cannot be associated with any of available renewable gaseous fuel codes.</skos:definition>
  </skos:Concept>
  <skos:Concept rdf:about="http://energy.referencedata.eu/StandardFuelTypeList/A15">
    <skos:inScheme rdf:resource="http://energy.referencedata.eu/StandardFuelTypeList"/>
    <skos:topConceptOf rdf:resource="http://energy.referencedata.eu/StandardFuelTypeList"/>
    <dcterms:identifier>A15</dcterms:identifier>
    <skos:prefLabel>Renewable gaseous landfill gas</skos:prefLabel>
    <skos:definition xml:lang="en">Gas produced by digestion of land filled waste.</skos:definition>
  </skos:Concept>
  <skos:Concept rdf:about="http://energy.referencedata.eu/StandardFuelTypeList/A16">
    <skos:inScheme rdf:resource="http://energy.referencedata.eu/StandardFuelTypeList"/>
    <skos:topConceptOf rdf:resource="http://energy.referencedata.eu/StandardFuelTypeList"/>
    <dcterms:identifier>A16</dcterms:identifier>
    <skos:prefLabel>Renewable gaseous sewage gas</skos:prefLabel>
    <skos:definition xml:lang="en">Gas produced from the anaerobic fermentation of sewage sludge.</skos:definition>
  </skos:Concept>
  <skos:Concept rdf:about="http://energy.referencedata.eu/StandardFuelTypeList/A17">
    <skos:inScheme rdf:resource="http://energy.referencedata.eu/StandardFuelTypeList"/>
    <skos:topConceptOf rdf:resource="http://energy.referencedata.eu/StandardFuelTypeList"/>
    <dcterms:identifier>A17</dcterms:identifier>
    <skos:prefLabel>Renewable gaseous agricultural gas</skos:prefLabel>
    <skos:definition xml:lang="en">Gas produced from agricultural processes.</skos:definition>
  </skos:Concept>
  <skos:Concept rdf:about="http://energy.referencedata.eu/StandardFuelTypeList/A18">
    <skos:inScheme rdf:resource="http://energy.referencedata.eu/StandardFuelTypeList"/>
    <skos:topConceptOf rdf:resource="http://energy.referencedata.eu/StandardFuelTypeList"/>
    <dcterms:identifier>A18</dcterms:identifier>
    <skos:prefLabel>Renewable gaseous gas from organic waste digestion</skos:prefLabel>
    <skos:definition xml:lang="en">Gas produced by anaerobic digestion process from organic waste.</skos:definition>
  </skos:Concept>
  <skos:Concept rdf:about="http://energy.referencedata.eu/StandardFuelTypeList/A19">
    <skos:inScheme rdf:resource="http://energy.referencedata.eu/StandardFuelTypeList"/>
    <skos:topConceptOf rdf:resource="http://energy.referencedata.eu/StandardFuelTypeList"/>
    <dcterms:identifier>A19</dcterms:identifier>
    <skos:prefLabel>Renewable gaseous process gas</skos:prefLabel>
    <skos:definition xml:lang="en">Gas produced by an industrial process as a consequence.</skos:definition>
  </skos:Concept>
  <skos:Concept rdf:about="http://energy.referencedata.eu/StandardFuelTypeList/A20">
    <skos:inScheme rdf:resource="http://energy.referencedata.eu/StandardFuelTypeList"/>
    <skos:topConceptOf rdf:resource="http://energy.referencedata.eu/StandardFuelTypeList"/>
    <dcterms:identifier>A20</dcterms:identifier>
    <skos:prefLabel>Renewable gaseous other biogenic sources</skos:prefLabel>
    <skos:definition xml:lang="en">Gas produced by form of biogenic resource transformation that cannot be associated with any of available renewable gaseous fuel codes that use biogenic energy resource.</skos:definition>
  </skos:Concept>
  <skos:Concept rdf:about="http://energy.referencedata.eu/StandardFuelTypeList/A21">
    <skos:inScheme rdf:resource="http://energy.referencedata.eu/StandardFuelTypeList"/>
    <skos:topConceptOf rdf:resource="http://energy.referencedata.eu/StandardFuelTypeList"/>
    <dcterms:identifier>A21</dcterms:identifier>
    <skos:prefLabel>Renewable heating and cooling solar</skos:prefLabel>
    <skos:definition xml:lang="en">Sunlight energy source.</skos:definition>
  </skos:Concept>
  <skos:Concept rdf:about="http://energy.referencedata.eu/StandardFuelTypeList/A22">
    <skos:inScheme rdf:resource="http://energy.referencedata.eu/StandardFuelTypeList"/>
    <skos:topConceptOf rdf:resource="http://energy.referencedata.eu/StandardFuelTypeList"/>
    <dcterms:identifier>A22</dcterms:identifier>
    <skos:prefLabel>Renewable heating and cooling geothermal</skos:prefLabel>
    <skos:definition xml:lang="en">Geothermal energy source.</skos:definition>
  </skos:Concept>
  <skos:Concept rdf:about="http://energy.referencedata.eu/StandardFuelTypeList/A23">
    <skos:inScheme rdf:resource="http://energy.referencedata.eu/StandardFuelTypeList"/>
    <skos:topConceptOf rdf:resource="http://energy.referencedata.eu/StandardFuelTypeList"/>
    <dcterms:identifier>A23</dcterms:identifier>
    <skos:prefLabel>Renewable heating and cooling aerothermal</skos:prefLabel>
    <skos:definition xml:lang="en">Thermal energy obtained from air.</skos:definition>
  </skos:Concept>
  <skos:Concept rdf:about="http://energy.referencedata.eu/StandardFuelTypeList/A24">
    <skos:inScheme rdf:resource="http://energy.referencedata.eu/StandardFuelTypeList"/>
    <skos:topConceptOf rdf:resource="http://energy.referencedata.eu/StandardFuelTypeList"/>
    <dcterms:identifier>A24</dcterms:identifier>
    <skos:prefLabel>Renewable heating and cooling hydrothermal</skos:prefLabel>
    <skos:definition xml:lang="en">Thermal energy obtained from large body of water.</skos:definition>
  </skos:Concept>
  <skos:Concept rdf:about="http://energy.referencedata.eu/StandardFuelTypeList/A25">
    <skos:inScheme rdf:resource="http://energy.referencedata.eu/StandardFuelTypeList"/>
    <skos:topConceptOf rdf:resource="http://energy.referencedata.eu/StandardFuelTypeList"/>
    <dcterms:identifier>A25</dcterms:identifier>
    <skos:prefLabel>Renewable heating and cooling process heat</skos:prefLabel>
    <skos:definition xml:lang="en">Thermal energy obtained from process heat.</skos:definition>
  </skos:Concept>
  <skos:Concept rdf:about="http://energy.referencedata.eu/StandardFuelTypeList/A26">
    <skos:inScheme rdf:resource="http://energy.referencedata.eu/StandardFuelTypeList"/>
    <skos:topConceptOf rdf:resource="http://energy.referencedata.eu/StandardFuelTypeList"/>
    <dcterms:identifier>A26</dcterms:identifier>
    <skos:prefLabel>Renewable mechanical unspecified</skos:prefLabel>
    <skos:definition xml:lang="en">Energy from renewable resource transformed into mechanical energy that cannot be associated with any of available renewable mechanical fuel codes.</skos:definition>
  </skos:Concept>
  <skos:Concept rdf:about="http://energy.referencedata.eu/StandardFuelTypeList/A27">
    <skos:inScheme rdf:resource="http://energy.referencedata.eu/StandardFuelTypeList"/>
    <skos:topConceptOf rdf:resource="http://energy.referencedata.eu/StandardFuelTypeList"/>
    <dcterms:identifier>A27</dcterms:identifier>
    <skos:prefLabel>Renewable mechanical wind</skos:prefLabel>
    <skos:definition xml:lang="en">Kinetic energy of wind transformed into mechanical energy.</skos:definition>
  </skos:Concept>
  <skos:Concept rdf:about="http://energy.referencedata.eu/StandardFuelTypeList/A28">
    <skos:inScheme rdf:resource="http://energy.referencedata.eu/StandardFuelTypeList"/>
    <skos:topConceptOf rdf:resource="http://energy.referencedata.eu/StandardFuelTypeList"/>
    <dcterms:identifier>A28</dcterms:identifier>
    <skos:prefLabel>Renewable mechanical hydro and marine</skos:prefLabel>
    <skos:definition xml:lang="en">Falling or flowing water energy or energy derived from tidal movement, wave motion or ocean current.</skos:definition>
  </skos:Concept>
  <skos:Concept rdf:about="http://energy.referencedata.eu/StandardFuelTypeList/A29">
    <skos:inScheme rdf:resource="http://energy.referencedata.eu/StandardFuelTypeList"/>
    <skos:topConceptOf rdf:resource="http://energy.referencedata.eu/StandardFuelTypeList"/>
    <dcterms:identifier>A29</dcterms:identifier>
    <skos:prefLabel>Fossil unspecified</skos:prefLabel>
    <skos:definition xml:lang="en">Unspecified fossil energy source.</skos:definition>
  </skos:Concept>
  <skos:Concept rdf:about="http://energy.referencedata.eu/StandardFuelTypeList/A30">
    <skos:inScheme rdf:resource="http://energy.referencedata.eu/StandardFuelTypeList"/>
    <skos:topConceptOf rdf:resource="http://energy.referencedata.eu/StandardFuelTypeList"/>
    <dcterms:identifier>A30</dcterms:identifier>
    <skos:prefLabel>Fossil solid unspecified</skos:prefLabel>
    <skos:definition xml:lang="en">Unspecified fossil solid energy source.</skos:definition>
  </skos:Concept>
  <skos:Concept rdf:about="http://energy.referencedata.eu/StandardFuelTypeList/A31">
    <skos:inScheme rdf:resource="http://energy.referencedata.eu/StandardFuelTypeList"/>
    <skos:topConceptOf rdf:resource="http://energy.referencedata.eu/StandardFuelTypeList"/>
    <dcterms:identifier>A31</dcterms:identifier>
    <skos:prefLabel>Fossil solid hard coal</skos:prefLabel>
    <skos:definition xml:lang="en">Hard coal solid fossil energy source. This includes Anthracite, Bituminous coal, Coking coal, Coke-oven coke and Lignite coke.</skos:definition>
  </skos:Concept>
  <skos:Concept rdf:about="http://energy.referencedata.eu/StandardFuelTypeList/A32">
    <skos:inScheme rdf:resource="http://energy.referencedata.eu/StandardFuelTypeList"/>
    <skos:topConceptOf rdf:resource="http://energy.referencedata.eu/StandardFuelTypeList"/>
    <dcterms:identifier>A32</dcterms:identifier>
    <skos:prefLabel>Fossil solid brown coal</skos:prefLabel>
    <skos:definition xml:lang="en">Brown coal solid fossil energy source. This includes Sub-bituminous coal, Lignite, Brown coal briquette and Peat briquette.</skos:definition>
  </skos:Concept>
  <skos:Concept rdf:about="http://energy.referencedata.eu/StandardFuelTypeList/A33">
    <skos:inScheme rdf:resource="http://energy.referencedata.eu/StandardFuelTypeList"/>
    <skos:topConceptOf rdf:resource="http://energy.referencedata.eu/StandardFuelTypeList"/>
    <dcterms:identifier>A33</dcterms:identifier>
    <skos:prefLabel>Fossil solid peat</skos:prefLabel>
    <skos:definition xml:lang="en">Solid fossil peat energy source.</skos:definition>
  </skos:Concept>
  <skos:Concept rdf:about="http://energy.referencedata.eu/StandardFuelTypeList/A34">
    <skos:inScheme rdf:resource="http://energy.referencedata.eu/StandardFuelTypeList"/>
    <skos:topConceptOf rdf:resource="http://energy.referencedata.eu/StandardFuelTypeList"/>
    <dcterms:identifier>A34</dcterms:identifier>
    <skos:prefLabel>Fossil solid municipal waste</skos:prefLabel>
    <skos:definition xml:lang="en">Solid fossil municipal waste energy source.</skos:definition>
  </skos:Concept>
  <skos:Concept rdf:about="http://energy.referencedata.eu/StandardFuelTypeList/A35">
    <skos:inScheme rdf:resource="http://energy.referencedata.eu/StandardFuelTypeList"/>
    <skos:topConceptOf rdf:resource="http://energy.referencedata.eu/StandardFuelTypeList"/>
    <dcterms:identifier>A35</dcterms:identifier>
    <skos:prefLabel>Fossil solid industrial and commercial waste</skos:prefLabel>
    <skos:definition xml:lang="en">Solid fossil industrial and commercial waste energy source.</skos:definition>
  </skos:Concept>
  <skos:Concept rdf:about="http://energy.referencedata.eu/StandardFuelTypeList/A36">
    <skos:inScheme rdf:resource="http://energy.referencedata.eu/StandardFuelTypeList"/>
    <skos:topConceptOf rdf:resource="http://energy.referencedata.eu/StandardFuelTypeList"/>
    <dcterms:identifier>A36</dcterms:identifier>
    <skos:prefLabel>Fossil liquid unspecified</skos:prefLabel>
    <skos:definition xml:lang="en">Unspecified fossil liquid energy source.</skos:definition>
  </skos:Concept>
  <skos:Concept rdf:about="http://energy.referencedata.eu/StandardFuelTypeList/A37">
    <skos:inScheme rdf:resource="http://energy.referencedata.eu/StandardFuelTypeList"/>
    <skos:topConceptOf rdf:resource="http://energy.referencedata.eu/StandardFuelTypeList"/>
    <dcterms:identifier>A37</dcterms:identifier>
    <skos:prefLabel>Fossil liquid crude oil</skos:prefLabel>
    <skos:definition xml:lang="en">Liquid crude oil fossil energy source. This includes shale oil or other types.</skos:definition>
  </skos:Concept>
  <skos:Concept rdf:about="http://energy.referencedata.eu/StandardFuelTypeList/A38">
    <skos:inScheme rdf:resource="http://energy.referencedata.eu/StandardFuelTypeList"/>
    <skos:topConceptOf rdf:resource="http://energy.referencedata.eu/StandardFuelTypeList"/>
    <dcterms:identifier>A38</dcterms:identifier>
    <skos:prefLabel>Fossil liquid natural gas liquids (NGL)</skos:prefLabel>
    <skos:definition xml:lang="en">Liquid natural gas liquids (NGL) fossil energy source.</skos:definition>
  </skos:Concept>
  <skos:Concept rdf:about="http://energy.referencedata.eu/StandardFuelTypeList/A39">
    <skos:inScheme rdf:resource="http://energy.referencedata.eu/StandardFuelTypeList"/>
    <skos:topConceptOf rdf:resource="http://energy.referencedata.eu/StandardFuelTypeList"/>
    <dcterms:identifier>A39</dcterms:identifier>
    <skos:prefLabel>Fossil liquid petroleum products</skos:prefLabel>
    <skos:definition xml:lang="en">Liquid petroleum products energy source. This includes Ethane,Naphtha, Aviation gasoline , Motor gasoline, Aviation turbine fuel,Other kerosene,Gas/diesel oil , Fuel oil, low sulphur ,Fuel oil, high sulphur ,Liquid Petroleum Gas , Orimulsion , Bitumen ,Lubricants ,Petroleum coke , Refinery Feedstock.</skos:definition>
  </skos:Concept>
  <skos:Concept rdf:about="http://energy.referencedata.eu/StandardFuelTypeList/A40">
    <skos:inScheme rdf:resource="http://energy.referencedata.eu/StandardFuelTypeList"/>
    <skos:topConceptOf rdf:resource="http://energy.referencedata.eu/StandardFuelTypeList"/>
    <dcterms:identifier>A40</dcterms:identifier>
    <skos:prefLabel>Fossil gaseous unspecified</skos:prefLabel>
    <skos:definition xml:lang="en">Unspecified fossil gaseous  energy source.</skos:definition>
  </skos:Concept>
  <skos:Concept rdf:about="http://energy.referencedata.eu/StandardFuelTypeList/A41">
    <skos:inScheme rdf:resource="http://energy.referencedata.eu/StandardFuelTypeList"/>
    <skos:topConceptOf rdf:resource="http://energy.referencedata.eu/StandardFuelTypeList"/>
    <dcterms:identifier>A41</dcterms:identifier>
    <skos:prefLabel>Fossil gaseous natural gas</skos:prefLabel>
    <skos:definition xml:lang="en">Fossil gaseous natural gas energy source.</skos:definition>
  </skos:Concept>
  <skos:Concept rdf:about="http://energy.referencedata.eu/StandardFuelTypeList/A42">
    <skos:inScheme rdf:resource="http://energy.referencedata.eu/StandardFuelTypeList"/>
    <skos:topConceptOf rdf:resource="http://energy.referencedata.eu/StandardFuelTypeList"/>
    <dcterms:identifier>A42</dcterms:identifier>
    <skos:prefLabel>Fossil gaseous coal-derived gas</skos:prefLabel>
    <skos:definition xml:lang="en">Fossil gaseous coal-derived gas energy source. This includes Blast furnace gas,Coke-oven gas or other types.</skos:definition>
  </skos:Concept>
  <skos:Concept rdf:about="http://energy.referencedata.eu/StandardFuelTypeList/A43">
    <skos:inScheme rdf:resource="http://energy.referencedata.eu/StandardFuelTypeList"/>
    <skos:topConceptOf rdf:resource="http://energy.referencedata.eu/StandardFuelTypeList"/>
    <dcterms:identifier>A43</dcterms:identifier>
    <skos:prefLabel>Fossil gaseous petroleum products</skos:prefLabel>
    <skos:definition xml:lang="en">Fossil gaseous petroleum products energy  source. This includes Propane, Butane, Refinery gas, Chemical waste gas or other types.</skos:definition>
  </skos:Concept>
  <skos:Concept rdf:about="http://energy.referencedata.eu/StandardFuelTypeList/A44">
    <skos:inScheme rdf:resource="http://energy.referencedata.eu/StandardFuelTypeList"/>
    <skos:topConceptOf rdf:resource="http://energy.referencedata.eu/StandardFuelTypeList"/>
    <dcterms:identifier>A44</dcterms:identifier>
    <skos:prefLabel>Fossil gaseous municipal gas plant</skos:prefLabel>
    <skos:definition xml:lang="en">Fossil gaseous municipal gas plant energy source. </skos:definition>
  </skos:Concept>
  <skos:Concept rdf:about="http://energy.referencedata.eu/StandardFuelTypeList/A45">
    <skos:inScheme rdf:resource="http://energy.referencedata.eu/StandardFuelTypeList"/>
    <skos:topConceptOf rdf:resource="http://energy.referencedata.eu/StandardFuelTypeList"/>
    <dcterms:identifier>A45</dcterms:identifier>
    <skos:prefLabel>Fossil gaseous process gas</skos:prefLabel>
    <skos:definition xml:lang="en">Fossil gaseous process gas energy source. This includes Carbon monoxide,
Methane , Hydrogen (fossil sourced) ,Phosphor gas ,Oxy gas and other types.</skos:definition>
  </skos:Concept>
  <skos:Concept rdf:about="http://energy.referencedata.eu/StandardFuelTypeList/A46">
    <skos:inScheme rdf:resource="http://energy.referencedata.eu/StandardFuelTypeList"/>
    <skos:topConceptOf rdf:resource="http://energy.referencedata.eu/StandardFuelTypeList"/>
    <dcterms:identifier>A46</dcterms:identifier>
    <skos:prefLabel>Fossil heat unspecified</skos:prefLabel>
    <skos:definition xml:lang="en">Unspecified fossil heat energy source.</skos:definition>
  </skos:Concept>
  <skos:Concept rdf:about="http://energy.referencedata.eu/StandardFuelTypeList/A47">
    <skos:inScheme rdf:resource="http://energy.referencedata.eu/StandardFuelTypeList"/>
    <skos:topConceptOf rdf:resource="http://energy.referencedata.eu/StandardFuelTypeList"/>
    <dcterms:identifier>A47</dcterms:identifier>
    <skos:prefLabel>Fossil heat process heat</skos:prefLabel>
    <skos:definition xml:lang="en">Fossil process heat energy source.</skos:definition>
  </skos:Concept>
  <skos:Concept rdf:about="http://energy.referencedata.eu/StandardFuelTypeList/A48">
    <skos:inScheme rdf:resource="http://energy.referencedata.eu/StandardFuelTypeList"/>
    <skos:topConceptOf rdf:resource="http://energy.referencedata.eu/StandardFuelTypeList"/>
    <dcterms:identifier>A48</dcterms:identifier>
    <skos:prefLabel>Nuclear solid radioactive fuel</skos:prefLabel>
    <skos:definition xml:lang="en">Solid Nuclear  radioactive energy source. This includes UOX, AGR, MOX or other types.</skos:definition>
  </skos:Concept>
  <skos:Concept rdf:about="http://energy.referencedata.eu/StandardFuelTypeList/A49">
    <skos:inScheme rdf:resource="http://energy.referencedata.eu/StandardFuelTypeList"/>
    <skos:topConceptOf rdf:resource="http://energy.referencedata.eu/StandardFuelTypeList"/>
    <dcterms:identifier>A49</dcterms:identifier>
    <skos:prefLabel>Gas synthesis unspecified</skos:prefLabel>
    <skos:definition xml:lang="en">Unspecified gas synthesis energy source.</skos:definition>
  </skos:Concept>
  <skos:Concept rdf:about="http://energy.referencedata.eu/StandardFuelTypeList/A50">
    <skos:inScheme rdf:resource="http://energy.referencedata.eu/StandardFuelTypeList"/>
    <skos:topConceptOf rdf:resource="http://energy.referencedata.eu/StandardFuelTypeList"/>
    <dcterms:identifier>A50</dcterms:identifier>
    <skos:prefLabel>Gas synthesis furnace gas</skos:prefLabel>
    <skos:definition xml:lang="en">Gas synthesis from furnace gas energy source.</skos:definition>
  </skos:Concept>
  <skos:Concept rdf:about="http://energy.referencedata.eu/StandardFuelTypeList/A51">
    <skos:inScheme rdf:resource="http://energy.referencedata.eu/StandardFuelTypeList"/>
    <skos:topConceptOf rdf:resource="http://energy.referencedata.eu/StandardFuelTypeList"/>
    <dcterms:identifier>A51</dcterms:identifier>
    <skos:prefLabel>Waste heat and cold unspecified</skos:prefLabel>
    <skos:definition xml:lang="en">Unspecified Waste heat and cold energy source.</skos:definition>
  </skos:Concept>
  <skos:Concept rdf:about="http://energy.referencedata.eu/StandardFuelTypeList/A52">
    <skos:inScheme rdf:resource="http://energy.referencedata.eu/StandardFuelTypeList"/>
    <skos:topConceptOf rdf:resource="http://energy.referencedata.eu/StandardFuelTypeList"/>
    <dcterms:identifier>A52</dcterms:identifier>
    <skos:prefLabel>Waste heat and cold By-product in industrial installation</skos:prefLabel>
    <skos:definition xml:lang="en">Waste heat and cold from by-product in industrial installation energy source.</skos:definition>
  </skos:Concept>
  <skos:Concept rdf:about="http://energy.referencedata.eu/StandardFuelTypeList/A53">
    <skos:inScheme rdf:resource="http://energy.referencedata.eu/StandardFuelTypeList"/>
    <skos:topConceptOf rdf:resource="http://energy.referencedata.eu/StandardFuelTypeList"/>
    <dcterms:identifier>A53</dcterms:identifier>
    <skos:prefLabel>Waste heat and cold By-product in power generation</skos:prefLabel>
    <skos:definition xml:lang="en">Waste heat and cold from by-product in power generation energy source.</skos:definition>
  </skos:Concept>
  <skos:Concept rdf:about="http://energy.referencedata.eu/StandardFuelTypeList/A54">
    <skos:inScheme rdf:resource="http://energy.referencedata.eu/StandardFuelTypeList"/>
    <skos:topConceptOf rdf:resource="http://energy.referencedata.eu/StandardFuelTypeList"/>
    <dcterms:identifier>A54</dcterms:identifier>
    <skos:prefLabel>Waste heat and cold By-product in tertiary sector</skos:prefLabel>
    <skos:definition xml:lang="en">Waste heat and cold from by-product in tertiary sector energy  source.</skos:definition>
  </skos:Concept>
</rdf:RDF>
