<?xml version='1.0' encoding='UTF-8'?>
<rdf:RDF xmlns:cim="http://iec.ch/TC57/2013/CIM-schema-cim16#" xmlns:rdf="http://www.w3.org/1999/02/22-rdf-syntax-ns#" xmlns:rdfs="http://www.w3.org/2000/01/rdf-schema#" xmlns:dcat="http://www.w3.org/ns/dcat#" xmlns:dc="http://purl.org/dc/elements/1.1/" xmlns:dcterms="http://purl.org/dc/terms/" xmlns:skos="http://www.w3.org/2004/02/skos/core#" xmlns:ecl="urn:entsoe.eu:wgedi:codelists" xmlns:xs="http://www.w3.org/2001/XMLSchema">
  <skos:ConceptScheme rdf:about="http://energy.referencedata.eu/StandardRoleTypeList">
    <rdf:type rdf:resource="http://www.w3.org/ns/dcat#Dataset"/>
    <dcterms:modified>2022-08-26</dcterms:modified>
    <dcat:version>83</dcat:version>
    <skos:prefLabel>StandardRoleTypeList</skos:prefLabel>
    <dcterms:identifier>ET0005</dcterms:identifier>
    <skos:definition xml:lang="en">Identification of the role played by a party.</skos:definition>
  </skos:ConceptScheme>
  <skos:Concept rdf:about="http://energy.referencedata.eu/StandardRoleTypeList/A01">
    <skos:inScheme rdf:resource="http://energy.referencedata.eu/StandardRoleTypeList"/>
    <skos:topConceptOf rdf:resource="http://energy.referencedata.eu/StandardRoleTypeList"/>
    <dcterms:identifier>A01</dcterms:identifier>
    <skos:prefLabel>Trade responsible party</skos:prefLabel>
    <skos:definition xml:lang="en">Refer to role model definitions in the ENTSO-E Harmonised Role Model Document.</skos:definition>
  </skos:Concept>
  <skos:Concept rdf:about="http://energy.referencedata.eu/StandardRoleTypeList/A02">
    <skos:inScheme rdf:resource="http://energy.referencedata.eu/StandardRoleTypeList"/>
    <skos:topConceptOf rdf:resource="http://energy.referencedata.eu/StandardRoleTypeList"/>
    <dcterms:identifier>A02</dcterms:identifier>
    <skos:prefLabel>Consumption responsible party</skos:prefLabel>
    <skos:definition xml:lang="en">Refer to role model definitions in the ENTSO-E Harmonised Role Model Document.</skos:definition>
  </skos:Concept>
  <skos:Concept rdf:about="http://energy.referencedata.eu/StandardRoleTypeList/A03">
    <skos:inScheme rdf:resource="http://energy.referencedata.eu/StandardRoleTypeList"/>
    <skos:topConceptOf rdf:resource="http://energy.referencedata.eu/StandardRoleTypeList"/>
    <dcterms:identifier>A03</dcterms:identifier>
    <skos:prefLabel>Combined power exchange (not to be used)</skos:prefLabel>
    <skos:definition xml:lang="en">This role is no longer in the ENTSO-E Harmonised Role Model Document.</skos:definition>
  </skos:Concept>
  <skos:Concept rdf:about="http://energy.referencedata.eu/StandardRoleTypeList/A04">
    <skos:inScheme rdf:resource="http://energy.referencedata.eu/StandardRoleTypeList"/>
    <skos:topConceptOf rdf:resource="http://energy.referencedata.eu/StandardRoleTypeList"/>
    <dcterms:identifier>A04</dcterms:identifier>
    <skos:prefLabel>System operator</skos:prefLabel>
    <skos:definition xml:lang="en">Refer to role model definitions in the ENTSO-E Harmonised Role Model Document.</skos:definition>
  </skos:Concept>
  <skos:Concept rdf:about="http://energy.referencedata.eu/StandardRoleTypeList/A05">
    <skos:inScheme rdf:resource="http://energy.referencedata.eu/StandardRoleTypeList"/>
    <skos:topConceptOf rdf:resource="http://energy.referencedata.eu/StandardRoleTypeList"/>
    <dcterms:identifier>A05</dcterms:identifier>
    <skos:prefLabel>Imbalance settlement responsible</skos:prefLabel>
    <skos:definition xml:lang="en">Refer to role model definitions in the ENTSO-E Harmonised Role Model Document.</skos:definition>
  </skos:Concept>
  <skos:Concept rdf:about="http://energy.referencedata.eu/StandardRoleTypeList/A06">
    <skos:inScheme rdf:resource="http://energy.referencedata.eu/StandardRoleTypeList"/>
    <skos:topConceptOf rdf:resource="http://energy.referencedata.eu/StandardRoleTypeList"/>
    <dcterms:identifier>A06</dcterms:identifier>
    <skos:prefLabel>Production responsible party</skos:prefLabel>
    <skos:definition xml:lang="en">Refer to role model definitions in the ENTSO-E Harmonised Role Model Document.</skos:definition>
  </skos:Concept>
  <skos:Concept rdf:about="http://energy.referencedata.eu/StandardRoleTypeList/A07">
    <skos:inScheme rdf:resource="http://energy.referencedata.eu/StandardRoleTypeList"/>
    <skos:topConceptOf rdf:resource="http://energy.referencedata.eu/StandardRoleTypeList"/>
    <dcterms:identifier>A07</dcterms:identifier>
    <skos:prefLabel>Transmission capacity allocator</skos:prefLabel>
    <skos:definition xml:lang="en">Refer to role model definitions in the ENTSO-E Harmonised Role Model Document.</skos:definition>
  </skos:Concept>
  <skos:Concept rdf:about="http://energy.referencedata.eu/StandardRoleTypeList/A08">
    <skos:inScheme rdf:resource="http://energy.referencedata.eu/StandardRoleTypeList"/>
    <skos:topConceptOf rdf:resource="http://energy.referencedata.eu/StandardRoleTypeList"/>
    <dcterms:identifier>A08</dcterms:identifier>
    <skos:prefLabel>Balance responsible party</skos:prefLabel>
    <skos:definition xml:lang="en">Refer to role model definitions in the ENTSO-E Harmonised Role Model Document.</skos:definition>
  </skos:Concept>
  <skos:Concept rdf:about="http://energy.referencedata.eu/StandardRoleTypeList/A09">
    <skos:inScheme rdf:resource="http://energy.referencedata.eu/StandardRoleTypeList"/>
    <skos:topConceptOf rdf:resource="http://energy.referencedata.eu/StandardRoleTypeList"/>
    <dcterms:identifier>A09</dcterms:identifier>
    <skos:prefLabel>Metered data aggregator</skos:prefLabel>
    <skos:definition xml:lang="en">Refer to role model definitions in the ENTSO-E Harmonised Role Model Document.</skos:definition>
  </skos:Concept>
  <skos:Concept rdf:about="http://energy.referencedata.eu/StandardRoleTypeList/A10">
    <skos:inScheme rdf:resource="http://energy.referencedata.eu/StandardRoleTypeList"/>
    <skos:topConceptOf rdf:resource="http://energy.referencedata.eu/StandardRoleTypeList"/>
    <dcterms:identifier>A10</dcterms:identifier>
    <skos:prefLabel>Billing agent</skos:prefLabel>
    <skos:definition xml:lang="en">Refer to role model definitions in the ENTSO-E Harmonised Role Model Document.</skos:definition>
  </skos:Concept>
  <skos:Concept rdf:about="http://energy.referencedata.eu/StandardRoleTypeList/A11">
    <skos:inScheme rdf:resource="http://energy.referencedata.eu/StandardRoleTypeList"/>
    <skos:topConceptOf rdf:resource="http://energy.referencedata.eu/StandardRoleTypeList"/>
    <dcterms:identifier>A11</dcterms:identifier>
    <skos:prefLabel>Market operator</skos:prefLabel>
    <skos:definition xml:lang="en">Refer to role model definitions in the ENTSO-E Harmonised Role Model Document.</skos:definition>
  </skos:Concept>
  <skos:Concept rdf:about="http://energy.referencedata.eu/StandardRoleTypeList/A12">
    <skos:inScheme rdf:resource="http://energy.referencedata.eu/StandardRoleTypeList"/>
    <skos:topConceptOf rdf:resource="http://energy.referencedata.eu/StandardRoleTypeList"/>
    <dcterms:identifier>A12</dcterms:identifier>
    <skos:prefLabel>Energy supplier</skos:prefLabel>
    <skos:definition xml:lang="en">Refer to role model definitions in the ENTSO-E Harmonised Role Model Document.</skos:definition>
  </skos:Concept>
  <skos:Concept rdf:about="http://energy.referencedata.eu/StandardRoleTypeList/A13">
    <skos:inScheme rdf:resource="http://energy.referencedata.eu/StandardRoleTypeList"/>
    <skos:topConceptOf rdf:resource="http://energy.referencedata.eu/StandardRoleTypeList"/>
    <dcterms:identifier>A13</dcterms:identifier>
    <skos:prefLabel>Consumer</skos:prefLabel>
    <skos:definition xml:lang="en">Refer to role model definitions in the ENTSO-E Harmonised Role Model Document.</skos:definition>
  </skos:Concept>
  <skos:Concept rdf:about="http://energy.referencedata.eu/StandardRoleTypeList/A14">
    <skos:inScheme rdf:resource="http://energy.referencedata.eu/StandardRoleTypeList"/>
    <skos:topConceptOf rdf:resource="http://energy.referencedata.eu/StandardRoleTypeList"/>
    <dcterms:identifier>A14</dcterms:identifier>
    <skos:prefLabel>Control area operator</skos:prefLabel>
    <skos:definition xml:lang="en">Refer to role model definitions in the ENTSO-E Harmonised Role Model Document.</skos:definition>
  </skos:Concept>
  <skos:Concept rdf:about="http://energy.referencedata.eu/StandardRoleTypeList/A15">
    <skos:inScheme rdf:resource="http://energy.referencedata.eu/StandardRoleTypeList"/>
    <skos:topConceptOf rdf:resource="http://energy.referencedata.eu/StandardRoleTypeList"/>
    <dcterms:identifier>A15</dcterms:identifier>
    <skos:prefLabel>Control block operator</skos:prefLabel>
    <skos:definition xml:lang="en">Refer to role model definitions in the ENTSO-E Harmonised Role Model Document.</skos:definition>
  </skos:Concept>
  <skos:Concept rdf:about="http://energy.referencedata.eu/StandardRoleTypeList/A16">
    <skos:inScheme rdf:resource="http://energy.referencedata.eu/StandardRoleTypeList"/>
    <skos:topConceptOf rdf:resource="http://energy.referencedata.eu/StandardRoleTypeList"/>
    <dcterms:identifier>A16</dcterms:identifier>
    <skos:prefLabel>Coordination centre operator</skos:prefLabel>
    <skos:definition xml:lang="en">Refer to role model definitions in the ENTSO-E Harmonised Role Model Document.</skos:definition>
  </skos:Concept>
  <skos:Concept rdf:about="http://energy.referencedata.eu/StandardRoleTypeList/A17">
    <skos:inScheme rdf:resource="http://energy.referencedata.eu/StandardRoleTypeList"/>
    <skos:topConceptOf rdf:resource="http://energy.referencedata.eu/StandardRoleTypeList"/>
    <dcterms:identifier>A17</dcterms:identifier>
    <skos:prefLabel>Grid access provider</skos:prefLabel>
    <skos:definition xml:lang="en">Refer to role model definitions in the ENTSO-E Harmonised Role Model Document.</skos:definition>
  </skos:Concept>
  <skos:Concept rdf:about="http://energy.referencedata.eu/StandardRoleTypeList/A18">
    <skos:inScheme rdf:resource="http://energy.referencedata.eu/StandardRoleTypeList"/>
    <skos:topConceptOf rdf:resource="http://energy.referencedata.eu/StandardRoleTypeList"/>
    <dcterms:identifier>A18</dcterms:identifier>
    <skos:prefLabel>Grid operator</skos:prefLabel>
    <skos:definition xml:lang="en">Refer to role model definitions in the ENTSO-E Harmonised Role Model Document.</skos:definition>
  </skos:Concept>
  <skos:Concept rdf:about="http://energy.referencedata.eu/StandardRoleTypeList/A19">
    <skos:inScheme rdf:resource="http://energy.referencedata.eu/StandardRoleTypeList"/>
    <skos:topConceptOf rdf:resource="http://energy.referencedata.eu/StandardRoleTypeList"/>
    <dcterms:identifier>A19</dcterms:identifier>
    <skos:prefLabel>Meter administrator</skos:prefLabel>
    <skos:definition xml:lang="en">Refer to role model definitions in the ENTSO-E Harmonised Role Model Document.</skos:definition>
  </skos:Concept>
  <skos:Concept rdf:about="http://energy.referencedata.eu/StandardRoleTypeList/A20">
    <skos:inScheme rdf:resource="http://energy.referencedata.eu/StandardRoleTypeList"/>
    <skos:topConceptOf rdf:resource="http://energy.referencedata.eu/StandardRoleTypeList"/>
    <dcterms:identifier>A20</dcterms:identifier>
    <skos:prefLabel>Party connected to grid</skos:prefLabel>
    <skos:definition xml:lang="en">Refer to role model definitions in the ENTSO-E Harmonised Role Model Document.</skos:definition>
  </skos:Concept>
  <skos:Concept rdf:about="http://energy.referencedata.eu/StandardRoleTypeList/A21">
    <skos:inScheme rdf:resource="http://energy.referencedata.eu/StandardRoleTypeList"/>
    <skos:topConceptOf rdf:resource="http://energy.referencedata.eu/StandardRoleTypeList"/>
    <dcterms:identifier>A21</dcterms:identifier>
    <skos:prefLabel>Producer</skos:prefLabel>
    <skos:definition xml:lang="en">Refer to role model definitions in the ENTSO-E Harmonised Role Model Document.</skos:definition>
  </skos:Concept>
  <skos:Concept rdf:about="http://energy.referencedata.eu/StandardRoleTypeList/A22">
    <skos:inScheme rdf:resource="http://energy.referencedata.eu/StandardRoleTypeList"/>
    <skos:topConceptOf rdf:resource="http://energy.referencedata.eu/StandardRoleTypeList"/>
    <dcterms:identifier>A22</dcterms:identifier>
    <skos:prefLabel>Profile maintenance party</skos:prefLabel>
    <skos:definition xml:lang="en">Refer to role model definitions in the ENTSO-E Harmonised Role Model Document.</skos:definition>
  </skos:Concept>
  <skos:Concept rdf:about="http://energy.referencedata.eu/StandardRoleTypeList/A23">
    <skos:inScheme rdf:resource="http://energy.referencedata.eu/StandardRoleTypeList"/>
    <skos:topConceptOf rdf:resource="http://energy.referencedata.eu/StandardRoleTypeList"/>
    <dcterms:identifier>A23</dcterms:identifier>
    <skos:prefLabel>Meter operator</skos:prefLabel>
    <skos:definition xml:lang="en">Refer to role model definitions in the ENTSO-E Harmonised Role Model Document.</skos:definition>
  </skos:Concept>
  <skos:Concept rdf:about="http://energy.referencedata.eu/StandardRoleTypeList/A24">
    <skos:inScheme rdf:resource="http://energy.referencedata.eu/StandardRoleTypeList"/>
    <skos:topConceptOf rdf:resource="http://energy.referencedata.eu/StandardRoleTypeList"/>
    <dcterms:identifier>A24</dcterms:identifier>
    <skos:prefLabel>Metered data collector</skos:prefLabel>
    <skos:definition xml:lang="en">Refer to role model definitions in the ENTSO-E Harmonised Role Model Document.</skos:definition>
  </skos:Concept>
  <skos:Concept rdf:about="http://energy.referencedata.eu/StandardRoleTypeList/A25">
    <skos:inScheme rdf:resource="http://energy.referencedata.eu/StandardRoleTypeList"/>
    <skos:topConceptOf rdf:resource="http://energy.referencedata.eu/StandardRoleTypeList"/>
    <dcterms:identifier>A25</dcterms:identifier>
    <skos:prefLabel>Metered data responsible</skos:prefLabel>
    <skos:definition xml:lang="en">Refer to role model definitions in the ENTSO-E Harmonised Role Model Document.</skos:definition>
  </skos:Concept>
  <skos:Concept rdf:about="http://energy.referencedata.eu/StandardRoleTypeList/A26">
    <skos:inScheme rdf:resource="http://energy.referencedata.eu/StandardRoleTypeList"/>
    <skos:topConceptOf rdf:resource="http://energy.referencedata.eu/StandardRoleTypeList"/>
    <dcterms:identifier>A26</dcterms:identifier>
    <skos:prefLabel>Metering point administrator</skos:prefLabel>
    <skos:definition xml:lang="en">Refer to role model definitions in the ENTSO-E Harmonised Role Model Document.</skos:definition>
  </skos:Concept>
  <skos:Concept rdf:about="http://energy.referencedata.eu/StandardRoleTypeList/A27">
    <skos:inScheme rdf:resource="http://energy.referencedata.eu/StandardRoleTypeList"/>
    <skos:topConceptOf rdf:resource="http://energy.referencedata.eu/StandardRoleTypeList"/>
    <dcterms:identifier>A27</dcterms:identifier>
    <skos:prefLabel>Resource Provider</skos:prefLabel>
    <skos:definition xml:lang="en">Refer to role model definitions in the ENTSO-E Harmonised Role Model Document.</skos:definition>
  </skos:Concept>
  <skos:Concept rdf:about="http://energy.referencedata.eu/StandardRoleTypeList/A28">
    <skos:inScheme rdf:resource="http://energy.referencedata.eu/StandardRoleTypeList"/>
    <skos:topConceptOf rdf:resource="http://energy.referencedata.eu/StandardRoleTypeList"/>
    <dcterms:identifier>A28</dcterms:identifier>
    <skos:prefLabel>Scheduling coordinator</skos:prefLabel>
    <skos:definition xml:lang="en">Refer to role model definitions in the ENTSO-E Harmonised Role Model Document.</skos:definition>
  </skos:Concept>
  <skos:Concept rdf:about="http://energy.referencedata.eu/StandardRoleTypeList/A29">
    <skos:inScheme rdf:resource="http://energy.referencedata.eu/StandardRoleTypeList"/>
    <skos:topConceptOf rdf:resource="http://energy.referencedata.eu/StandardRoleTypeList"/>
    <dcterms:identifier>A29</dcterms:identifier>
    <skos:prefLabel>Capacity Trader</skos:prefLabel>
    <skos:definition xml:lang="en">Refer to role model definitions in the ENTSO-E Harmonised Role Model Document.</skos:definition>
  </skos:Concept>
  <skos:Concept rdf:about="http://energy.referencedata.eu/StandardRoleTypeList/A30">
    <skos:inScheme rdf:resource="http://energy.referencedata.eu/StandardRoleTypeList"/>
    <skos:topConceptOf rdf:resource="http://energy.referencedata.eu/StandardRoleTypeList"/>
    <dcterms:identifier>A30</dcterms:identifier>
    <skos:prefLabel>Interconnection Trade Responsible</skos:prefLabel>
    <skos:definition xml:lang="en">Refer to role model definitions in the ENTSO-E Harmonised Role Model Document.</skos:definition>
  </skos:Concept>
  <skos:Concept rdf:about="http://energy.referencedata.eu/StandardRoleTypeList/A31">
    <skos:inScheme rdf:resource="http://energy.referencedata.eu/StandardRoleTypeList"/>
    <skos:topConceptOf rdf:resource="http://energy.referencedata.eu/StandardRoleTypeList"/>
    <dcterms:identifier>A31</dcterms:identifier>
    <skos:prefLabel>Nomination Validator</skos:prefLabel>
    <skos:definition xml:lang="en">Refer to role model definitions in the ENTSO-E Harmonised Role Model Document.</skos:definition>
  </skos:Concept>
  <skos:Concept rdf:about="http://energy.referencedata.eu/StandardRoleTypeList/A32">
    <skos:inScheme rdf:resource="http://energy.referencedata.eu/StandardRoleTypeList"/>
    <skos:topConceptOf rdf:resource="http://energy.referencedata.eu/StandardRoleTypeList"/>
    <dcterms:identifier>A32</dcterms:identifier>
    <skos:prefLabel>Market information aggregator</skos:prefLabel>
    <skos:definition xml:lang="en">Refer to role model definitions in the ENTSO-E Harmonised Role Model Document.
A party that collects information from different sources and assembles  it to provide a summary of the market.</skos:definition>
  </skos:Concept>
  <skos:Concept rdf:about="http://energy.referencedata.eu/StandardRoleTypeList/A33">
    <skos:inScheme rdf:resource="http://energy.referencedata.eu/StandardRoleTypeList"/>
    <skos:topConceptOf rdf:resource="http://energy.referencedata.eu/StandardRoleTypeList"/>
    <dcterms:identifier>A33</dcterms:identifier>
    <skos:prefLabel>Information receiver</skos:prefLabel>
    <skos:definition xml:lang="en">Refer to role model definitions in the ENTSO-E Harmonised Role Model Document.
A party, not necessarily a market participant, which receives information about the market.</skos:definition>
  </skos:Concept>
  <skos:Concept rdf:about="http://energy.referencedata.eu/StandardRoleTypeList/A34">
    <skos:inScheme rdf:resource="http://energy.referencedata.eu/StandardRoleTypeList"/>
    <skos:topConceptOf rdf:resource="http://energy.referencedata.eu/StandardRoleTypeList"/>
    <dcterms:identifier>A34</dcterms:identifier>
    <skos:prefLabel>Reserve Allocator</skos:prefLabel>
    <skos:definition xml:lang="en">Refer to role model definitions in the ENTSO-E Harmonised Role Model Document.
A party that informs the market of reserve requirements, receives tenders against the requirements and in compliance with the prequalification criteria, determines what tenders meet requirements and assigns tenders.</skos:definition>
  </skos:Concept>
  <skos:Concept rdf:about="http://energy.referencedata.eu/StandardRoleTypeList/A35">
    <skos:inScheme rdf:resource="http://energy.referencedata.eu/StandardRoleTypeList"/>
    <skos:topConceptOf rdf:resource="http://energy.referencedata.eu/StandardRoleTypeList"/>
    <dcterms:identifier>A35</dcterms:identifier>
    <skos:prefLabel>MOL Responsible</skos:prefLabel>
    <skos:definition xml:lang="en">Refer to role model definitions in the ENTSO-E Harmonised Role Model Document.
A party that Informs the market of reserve requirements, receives tenders against the requirements and in compliance with the prequalification criteria, determines what tenders meet requirements and assigns tenders.</skos:definition>
  </skos:Concept>
  <skos:Concept rdf:about="http://energy.referencedata.eu/StandardRoleTypeList/A36">
    <skos:inScheme rdf:resource="http://energy.referencedata.eu/StandardRoleTypeList"/>
    <skos:topConceptOf rdf:resource="http://energy.referencedata.eu/StandardRoleTypeList"/>
    <dcterms:identifier>A36</dcterms:identifier>
    <skos:prefLabel>Capacity Coordinator</skos:prefLabel>
    <skos:definition xml:lang="en">A party, acting on behalf of the SOs involved, responsible for establishing a coordinated Offered Capacity and/or NTC and/or ATC between several Scheduling Areas.</skos:definition>
  </skos:Concept>
  <skos:Concept rdf:about="http://energy.referencedata.eu/StandardRoleTypeList/A37">
    <skos:inScheme rdf:resource="http://energy.referencedata.eu/StandardRoleTypeList"/>
    <skos:topConceptOf rdf:resource="http://energy.referencedata.eu/StandardRoleTypeList"/>
    <dcterms:identifier>A37</dcterms:identifier>
    <skos:prefLabel>Reconciliation Accountable</skos:prefLabel>
    <skos:definition xml:lang="en">Refer to role model definitions in the ENTSO-E Harmonised Role Model Document.
A party that is financially accountable for the reconciled volume of energy products for a profiled local metering point.</skos:definition>
  </skos:Concept>
  <skos:Concept rdf:about="http://energy.referencedata.eu/StandardRoleTypeList/A38">
    <skos:inScheme rdf:resource="http://energy.referencedata.eu/StandardRoleTypeList"/>
    <skos:topConceptOf rdf:resource="http://energy.referencedata.eu/StandardRoleTypeList"/>
    <dcterms:identifier>A38</dcterms:identifier>
    <skos:prefLabel>Reconciliation Responsible</skos:prefLabel>
    <skos:definition xml:lang="en">A party that is responsible for reconciling, within a metering grid area, the volumes used in the imbalance settlement process for profiled metering points and the actual metered quantities.</skos:definition>
  </skos:Concept>
  <skos:Concept rdf:about="http://energy.referencedata.eu/StandardRoleTypeList/A39">
    <skos:inScheme rdf:resource="http://energy.referencedata.eu/StandardRoleTypeList"/>
    <skos:topConceptOf rdf:resource="http://energy.referencedata.eu/StandardRoleTypeList"/>
    <dcterms:identifier>A39</dcterms:identifier>
    <skos:prefLabel>Data provider</skos:prefLabel>
    <skos:definition xml:lang="en">A party that is responsible for providing information to a central authority.</skos:definition>
  </skos:Concept>
  <skos:Concept rdf:about="http://energy.referencedata.eu/StandardRoleTypeList/A40">
    <skos:inScheme rdf:resource="http://energy.referencedata.eu/StandardRoleTypeList"/>
    <skos:topConceptOf rdf:resource="http://energy.referencedata.eu/StandardRoleTypeList"/>
    <dcterms:identifier>A40</dcterms:identifier>
    <skos:prefLabel>Local Issuing Office (LIO)</skos:prefLabel>
    <skos:definition xml:lang="en">A party that is responsible for operating a Local Issuing Office (LIO).</skos:definition>
  </skos:Concept>
  <skos:Concept rdf:about="http://energy.referencedata.eu/StandardRoleTypeList/A41">
    <skos:inScheme rdf:resource="http://energy.referencedata.eu/StandardRoleTypeList"/>
    <skos:topConceptOf rdf:resource="http://energy.referencedata.eu/StandardRoleTypeList"/>
    <dcterms:identifier>A41</dcterms:identifier>
    <skos:prefLabel>Central Issuing Office (CIO)</skos:prefLabel>
    <skos:definition xml:lang="en">A party that is responsible for operating a Central Issuing Office (CIO).</skos:definition>
  </skos:Concept>
  <skos:Concept rdf:about="http://energy.referencedata.eu/StandardRoleTypeList/A42">
    <skos:inScheme rdf:resource="http://energy.referencedata.eu/StandardRoleTypeList"/>
    <skos:topConceptOf rdf:resource="http://energy.referencedata.eu/StandardRoleTypeList"/>
    <dcterms:identifier>A42</dcterms:identifier>
    <skos:prefLabel>EIC Participant</skos:prefLabel>
    <skos:definition xml:lang="en">A party that participates in the EIC environment.</skos:definition>
  </skos:Concept>
  <skos:Concept rdf:about="http://energy.referencedata.eu/StandardRoleTypeList/A43">
    <skos:inScheme rdf:resource="http://energy.referencedata.eu/StandardRoleTypeList"/>
    <skos:topConceptOf rdf:resource="http://energy.referencedata.eu/StandardRoleTypeList"/>
    <dcterms:identifier>A43</dcterms:identifier>
    <skos:prefLabel>Weather analyser</skos:prefLabel>
    <skos:definition xml:lang="en">A party that analyses the current and forecast weather situation and establishes a prognosis of its impact on the renewable energy environment as well as the overall load.</skos:definition>
  </skos:Concept>
  <skos:Concept rdf:about="http://energy.referencedata.eu/StandardRoleTypeList/A44">
    <skos:inScheme rdf:resource="http://energy.referencedata.eu/StandardRoleTypeList"/>
    <skos:topConceptOf rdf:resource="http://energy.referencedata.eu/StandardRoleTypeList"/>
    <dcterms:identifier>A44</dcterms:identifier>
    <skos:prefLabel>Regional Security Coordinator (RSC)</skos:prefLabel>
    <skos:definition xml:lang="en">The RSC as defined in the System Operation guideline.</skos:definition>
  </skos:Concept>
  <skos:Concept rdf:about="http://energy.referencedata.eu/StandardRoleTypeList/A45">
    <skos:inScheme rdf:resource="http://energy.referencedata.eu/StandardRoleTypeList"/>
    <skos:topConceptOf rdf:resource="http://energy.referencedata.eu/StandardRoleTypeList"/>
    <dcterms:identifier>A45</dcterms:identifier>
    <skos:prefLabel>Energy Service Company (ESCO)</skos:prefLabel>
    <skos:definition xml:lang="en">A party offering energy-related services to the Party Connected to Grid, but not directly active in the energy value chain or the physical infrastructure itself. The ESCO may provide insight services as well as energy management services.</skos:definition>
  </skos:Concept>
  <skos:Concept rdf:about="http://energy.referencedata.eu/StandardRoleTypeList/A46">
    <skos:inScheme rdf:resource="http://energy.referencedata.eu/StandardRoleTypeList"/>
    <skos:topConceptOf rdf:resource="http://energy.referencedata.eu/StandardRoleTypeList"/>
    <dcterms:identifier>A46</dcterms:identifier>
    <skos:prefLabel>Balancing Service Provider</skos:prefLabel>
    <skos:definition xml:lang="en">A party with reserve-providing units or reserve-providing groups able to provide balancing services to LFC Operators.</skos:definition>
  </skos:Concept>
  <skos:Concept rdf:about="http://energy.referencedata.eu/StandardRoleTypeList/A47">
    <skos:inScheme rdf:resource="http://energy.referencedata.eu/StandardRoleTypeList"/>
    <skos:topConceptOf rdf:resource="http://energy.referencedata.eu/StandardRoleTypeList"/>
    <dcterms:identifier>A47</dcterms:identifier>
    <skos:prefLabel>Energy trader</skos:prefLabel>
    <skos:definition xml:lang="en">A party that is selling or buying energy.</skos:definition>
  </skos:Concept>
  <skos:Concept rdf:about="http://energy.referencedata.eu/StandardRoleTypeList/A48">
    <skos:inScheme rdf:resource="http://energy.referencedata.eu/StandardRoleTypeList"/>
    <skos:topConceptOf rdf:resource="http://energy.referencedata.eu/StandardRoleTypeList"/>
    <dcterms:identifier>A48</dcterms:identifier>
    <skos:prefLabel>LFC Operator</skos:prefLabel>
    <skos:definition xml:lang="en">A party that is responsible for the Load Frequency Control of its LFC Area or LFC Block.</skos:definition>
  </skos:Concept>
  <skos:Concept rdf:about="http://energy.referencedata.eu/StandardRoleTypeList/A49">
    <skos:inScheme rdf:resource="http://energy.referencedata.eu/StandardRoleTypeList"/>
    <skos:topConceptOf rdf:resource="http://energy.referencedata.eu/StandardRoleTypeList"/>
    <dcterms:identifier>A49</dcterms:identifier>
    <skos:prefLabel>Transmission System Operator (TSO)</skos:prefLabel>
    <skos:definition xml:lang="en">The Transmission System Operator (TSO) is responsible for the transport of electricity on the extra high-voltage and high-voltage interconnected system. This is a market participant and not a role in Harmonised Role Model.</skos:definition>
  </skos:Concept>
  <skos:Concept rdf:about="http://energy.referencedata.eu/StandardRoleTypeList/A50">
    <skos:inScheme rdf:resource="http://energy.referencedata.eu/StandardRoleTypeList"/>
    <skos:topConceptOf rdf:resource="http://energy.referencedata.eu/StandardRoleTypeList"/>
    <dcterms:identifier>A50</dcterms:identifier>
    <skos:prefLabel>Distribution System Operator (DSO)</skos:prefLabel>
    <skos:definition xml:lang="en">Distribution System Operator (DSO) is responsible for transport of electricity on high-voltage (optionally), medium-voltage and low-voltage distribution systems. This is a market participant and not a role in Harmonised Role Model.</skos:definition>
  </skos:Concept>
  <skos:Concept rdf:about="http://energy.referencedata.eu/StandardRoleTypeList/A51">
    <skos:inScheme rdf:resource="http://energy.referencedata.eu/StandardRoleTypeList"/>
    <skos:topConceptOf rdf:resource="http://energy.referencedata.eu/StandardRoleTypeList"/>
    <dcterms:identifier>A51</dcterms:identifier>
    <skos:prefLabel>Resource Capacity Mechanism Operator</skos:prefLabel>
    <skos:definition xml:lang="en">Resource capacity mechanism operator is the party responsible to operate the resource capacity mechanism in a member state. It can either be the TSO or an independent party.</skos:definition>
  </skos:Concept>
  <skos:Concept rdf:about="http://energy.referencedata.eu/StandardRoleTypeList/A52">
    <skos:inScheme rdf:resource="http://energy.referencedata.eu/StandardRoleTypeList"/>
    <skos:topConceptOf rdf:resource="http://energy.referencedata.eu/StandardRoleTypeList"/>
    <dcterms:identifier>A52</dcterms:identifier>
    <skos:prefLabel>Resource aggregator</skos:prefLabel>
    <skos:definition xml:lang="en">A party that aggregates resources for usage by a service provider for energy market services.</skos:definition>
  </skos:Concept>
  <skos:Concept rdf:about="http://energy.referencedata.eu/StandardRoleTypeList/A53">
    <skos:inScheme rdf:resource="http://energy.referencedata.eu/StandardRoleTypeList"/>
    <skos:topConceptOf rdf:resource="http://energy.referencedata.eu/StandardRoleTypeList"/>
    <dcterms:identifier>A53</dcterms:identifier>
    <skos:prefLabel>Cost sharing calculator</skos:prefLabel>
    <skos:definition xml:lang="en">A party responsible for the mapping of the costs between areas and parties.</skos:definition>
  </skos:Concept>
  <skos:Concept rdf:about="http://energy.referencedata.eu/StandardRoleTypeList/A54">
    <skos:inScheme rdf:resource="http://energy.referencedata.eu/StandardRoleTypeList"/>
    <skos:topConceptOf rdf:resource="http://energy.referencedata.eu/StandardRoleTypeList"/>
    <dcterms:identifier>A54</dcterms:identifier>
    <skos:prefLabel>Settlement responsible</skos:prefLabel>
    <skos:definition xml:lang="en">A party responsible for settling the costs.</skos:definition>
  </skos:Concept>
</rdf:RDF>
