<?xml version='1.0' encoding='UTF-8'?>
<rdf:RDF xmlns:cim="http://iec.ch/TC57/2013/CIM-schema-cim16#" xmlns:rdf="http://www.w3.org/1999/02/22-rdf-syntax-ns#" xmlns:rdfs="http://www.w3.org/2000/01/rdf-schema#" xmlns:dcat="http://www.w3.org/ns/dcat#" xmlns:dc="http://purl.org/dc/elements/1.1/" xmlns:dcterms="http://purl.org/dc/terms/" xmlns:skos="http://www.w3.org/2004/02/skos/core#" xmlns:ecl="urn:entsoe.eu:wgedi:codelists" xmlns:xs="http://www.w3.org/2001/XMLSchema">
  <skos:ConceptScheme rdf:about="http://energy.referencedata.eu/StandardReasonCodeTypeList">
    <rdf:type rdf:resource="http://www.w3.org/ns/dcat#Dataset"/>
    <dcterms:modified>2022-03-31</dcterms:modified>
    <dcat:version>81</dcat:version>
    <skos:prefLabel>StandardReasonCodeTypeList</skos:prefLabel>
    <dcterms:identifier>ET0015</dcterms:identifier>
    <skos:definition xml:lang="en">The coded motivation of an act.</skos:definition>
  </skos:ConceptScheme>
  <skos:Concept rdf:about="http://energy.referencedata.eu/StandardReasonCodeTypeList/999">
    <skos:inScheme rdf:resource="http://energy.referencedata.eu/StandardReasonCodeTypeList"/>
    <skos:topConceptOf rdf:resource="http://energy.referencedata.eu/StandardReasonCodeTypeList"/>
    <dcterms:identifier>999</dcterms:identifier>
    <skos:prefLabel>Errors not specifically identified </skos:prefLabel>
    <skos:definition xml:lang="en">This code is used to identify errors that have not been specifically addressed in the Reason code list. It can be used at any level and refers to the level for which it has been identified.</skos:definition>
  </skos:Concept>
  <skos:Concept rdf:about="http://energy.referencedata.eu/StandardReasonCodeTypeList/A01">
    <skos:inScheme rdf:resource="http://energy.referencedata.eu/StandardReasonCodeTypeList"/>
    <skos:topConceptOf rdf:resource="http://energy.referencedata.eu/StandardReasonCodeTypeList"/>
    <dcterms:identifier>A01</dcterms:identifier>
    <skos:prefLabel>Message fully accepted</skos:prefLabel>
    <skos:definition xml:lang="en">The message has been fully accepted for application processing.</skos:definition>
  </skos:Concept>
  <skos:Concept rdf:about="http://energy.referencedata.eu/StandardReasonCodeTypeList/A02">
    <skos:inScheme rdf:resource="http://energy.referencedata.eu/StandardReasonCodeTypeList"/>
    <skos:topConceptOf rdf:resource="http://energy.referencedata.eu/StandardReasonCodeTypeList"/>
    <dcterms:identifier>A02</dcterms:identifier>
    <skos:prefLabel>Message fully rejected </skos:prefLabel>
    <skos:definition xml:lang="en">No part of the message has been accepted for application processing, e.g. Global position incomplete.</skos:definition>
  </skos:Concept>
  <skos:Concept rdf:about="http://energy.referencedata.eu/StandardReasonCodeTypeList/A03">
    <skos:inScheme rdf:resource="http://energy.referencedata.eu/StandardReasonCodeTypeList"/>
    <skos:topConceptOf rdf:resource="http://energy.referencedata.eu/StandardReasonCodeTypeList"/>
    <dcterms:identifier>A03</dcterms:identifier>
    <skos:prefLabel>Message contains errors at the time series level </skos:prefLabel>
    <skos:definition xml:lang="en">Part of the message contents, i.e. certain time series, has been accepted for application processing. It is necessary to look at the time series level to determine the time series that have been rejected. The time series is excluded from the global position.</skos:definition>
  </skos:Concept>
  <skos:Concept rdf:about="http://energy.referencedata.eu/StandardReasonCodeTypeList/A04">
    <skos:inScheme rdf:resource="http://energy.referencedata.eu/StandardReasonCodeTypeList"/>
    <skos:topConceptOf rdf:resource="http://energy.referencedata.eu/StandardReasonCodeTypeList"/>
    <dcterms:identifier>A04</dcterms:identifier>
    <skos:prefLabel>Time interval incorrect </skos:prefLabel>
    <skos:definition xml:lang="en">The schedule time interval is not within the contractual agreement or the period does not agree with the schedule time interval.</skos:definition>
  </skos:Concept>
  <skos:Concept rdf:about="http://energy.referencedata.eu/StandardReasonCodeTypeList/A05">
    <skos:inScheme rdf:resource="http://energy.referencedata.eu/StandardReasonCodeTypeList"/>
    <skos:topConceptOf rdf:resource="http://energy.referencedata.eu/StandardReasonCodeTypeList"/>
    <dcterms:identifier>A05</dcterms:identifier>
    <skos:prefLabel>Sender without valid contract </skos:prefLabel>
    <skos:definition xml:lang="en">The sender has no current valid contract with the TSO. The message consequently will be fully rejected.</skos:definition>
  </skos:Concept>
  <skos:Concept rdf:about="http://energy.referencedata.eu/StandardReasonCodeTypeList/A06">
    <skos:inScheme rdf:resource="http://energy.referencedata.eu/StandardReasonCodeTypeList"/>
    <skos:topConceptOf rdf:resource="http://energy.referencedata.eu/StandardReasonCodeTypeList"/>
    <dcterms:identifier>A06</dcterms:identifier>
    <skos:prefLabel>Schedule accepted </skos:prefLabel>
    <skos:definition xml:lang="en">The schedule of the recipient as presented has been completely accepted.</skos:definition>
  </skos:Concept>
  <skos:Concept rdf:about="http://energy.referencedata.eu/StandardReasonCodeTypeList/A07">
    <skos:inScheme rdf:resource="http://energy.referencedata.eu/StandardReasonCodeTypeList"/>
    <skos:topConceptOf rdf:resource="http://energy.referencedata.eu/StandardReasonCodeTypeList"/>
    <dcterms:identifier>A07</dcterms:identifier>
    <skos:prefLabel>Schedule partially accepted </skos:prefLabel>
    <skos:definition xml:lang="en">The schedule of the recipient as presented has been partially accepted. It is necessary to look at the time series level to determine the changes (time series rejected, modified, etc.).</skos:definition>
  </skos:Concept>
  <skos:Concept rdf:about="http://energy.referencedata.eu/StandardReasonCodeTypeList/A08">
    <skos:inScheme rdf:resource="http://energy.referencedata.eu/StandardReasonCodeTypeList"/>
    <skos:topConceptOf rdf:resource="http://energy.referencedata.eu/StandardReasonCodeTypeList"/>
    <dcterms:identifier>A08</dcterms:identifier>
    <skos:prefLabel>Schedule rejected </skos:prefLabel>
    <skos:definition xml:lang="en">The schedule of the recipient as presented has been totally rejected. The cause could be the non presentation of a counter part for the involved trades.</skos:definition>
  </skos:Concept>
  <skos:Concept rdf:about="http://energy.referencedata.eu/StandardReasonCodeTypeList/A09">
    <skos:inScheme rdf:resource="http://energy.referencedata.eu/StandardReasonCodeTypeList"/>
    <skos:topConceptOf rdf:resource="http://energy.referencedata.eu/StandardReasonCodeTypeList"/>
    <dcterms:identifier>A09</dcterms:identifier>
    <skos:prefLabel>Time series not matching</skos:prefLabel>
    <skos:definition xml:lang="en">Time series mismatches. </skos:definition>
  </skos:Concept>
  <skos:Concept rdf:about="http://energy.referencedata.eu/StandardReasonCodeTypeList/A10">
    <skos:inScheme rdf:resource="http://energy.referencedata.eu/StandardReasonCodeTypeList"/>
    <skos:topConceptOf rdf:resource="http://energy.referencedata.eu/StandardReasonCodeTypeList"/>
    <dcterms:identifier>A10</dcterms:identifier>
    <skos:prefLabel>Credit limit exceeded </skos:prefLabel>
    <skos:definition xml:lang="en">The contractual credit limit has been exceeded and as such the message has been rejected.</skos:definition>
  </skos:Concept>
  <skos:Concept rdf:about="http://energy.referencedata.eu/StandardReasonCodeTypeList/A20">
    <skos:inScheme rdf:resource="http://energy.referencedata.eu/StandardReasonCodeTypeList"/>
    <skos:topConceptOf rdf:resource="http://energy.referencedata.eu/StandardReasonCodeTypeList"/>
    <dcterms:identifier>A20</dcterms:identifier>
    <skos:prefLabel>Time series fully rejected </skos:prefLabel>
    <skos:definition xml:lang="en">The time series has been fully rejected. In the case of a confirmation report, this reason code is used in conjunction with either A26 or A30.</skos:definition>
  </skos:Concept>
  <skos:Concept rdf:about="http://energy.referencedata.eu/StandardReasonCodeTypeList/A21">
    <skos:inScheme rdf:resource="http://energy.referencedata.eu/StandardReasonCodeTypeList"/>
    <skos:topConceptOf rdf:resource="http://energy.referencedata.eu/StandardReasonCodeTypeList"/>
    <dcterms:identifier>A21</dcterms:identifier>
    <skos:prefLabel>Time series accepted with specific time interval errors </skos:prefLabel>
    <skos:definition xml:lang="en">The time series has been accepted but some time interval quantities have been rectified or zeroed out.</skos:definition>
  </skos:Concept>
  <skos:Concept rdf:about="http://energy.referencedata.eu/StandardReasonCodeTypeList/A22">
    <skos:inScheme rdf:resource="http://energy.referencedata.eu/StandardReasonCodeTypeList"/>
    <skos:topConceptOf rdf:resource="http://energy.referencedata.eu/StandardReasonCodeTypeList"/>
    <dcterms:identifier>A22</dcterms:identifier>
    <skos:prefLabel>In party/Out party invalid</skos:prefLabel>
    <skos:definition xml:lang="en">There is no contract for the parties indicated or the rules for cross border nominations are not being respected. The time series has been rejected.</skos:definition>
  </skos:Concept>
  <skos:Concept rdf:about="http://energy.referencedata.eu/StandardReasonCodeTypeList/A23">
    <skos:inScheme rdf:resource="http://energy.referencedata.eu/StandardReasonCodeTypeList"/>
    <skos:topConceptOf rdf:resource="http://energy.referencedata.eu/StandardReasonCodeTypeList"/>
    <dcterms:identifier>A23</dcterms:identifier>
    <skos:prefLabel>Area invalid</skos:prefLabel>
    <skos:definition xml:lang="en">The area is unknown or not allowed. The time series has been rejected.</skos:definition>
  </skos:Concept>
  <skos:Concept rdf:about="http://energy.referencedata.eu/StandardReasonCodeTypeList/A24">
    <skos:inScheme rdf:resource="http://energy.referencedata.eu/StandardReasonCodeTypeList"/>
    <skos:topConceptOf rdf:resource="http://energy.referencedata.eu/StandardReasonCodeTypeList"/>
    <dcterms:identifier>A24</dcterms:identifier>
    <skos:prefLabel>A24 not applicable</skos:prefLabel>
    <skos:definition xml:lang="en">This code is no longer applicable.</skos:definition>
  </skos:Concept>
  <skos:Concept rdf:about="http://energy.referencedata.eu/StandardReasonCodeTypeList/A25">
    <skos:inScheme rdf:resource="http://energy.referencedata.eu/StandardReasonCodeTypeList"/>
    <skos:topConceptOf rdf:resource="http://energy.referencedata.eu/StandardReasonCodeTypeList"/>
    <dcterms:identifier>A25</dcterms:identifier>
    <skos:prefLabel>A25 not applicable</skos:prefLabel>
    <skos:definition xml:lang="en">This code is no longer applicable.</skos:definition>
  </skos:Concept>
  <skos:Concept rdf:about="http://energy.referencedata.eu/StandardReasonCodeTypeList/A26">
    <skos:inScheme rdf:resource="http://energy.referencedata.eu/StandardReasonCodeTypeList"/>
    <skos:topConceptOf rdf:resource="http://energy.referencedata.eu/StandardReasonCodeTypeList"/>
    <dcterms:identifier>A26</dcterms:identifier>
    <skos:prefLabel>Default time series applied </skos:prefLabel>
    <skos:definition xml:lang="en">The time series has been rejected and replaced with a default time series profile. This reason code may not be used in conjunction with A30.</skos:definition>
  </skos:Concept>
  <skos:Concept rdf:about="http://energy.referencedata.eu/StandardReasonCodeTypeList/A27">
    <skos:inScheme rdf:resource="http://energy.referencedata.eu/StandardReasonCodeTypeList"/>
    <skos:topConceptOf rdf:resource="http://energy.referencedata.eu/StandardReasonCodeTypeList"/>
    <dcterms:identifier>A27</dcterms:identifier>
    <skos:prefLabel>Cross border capacity exceeded </skos:prefLabel>
    <skos:definition xml:lang="en">The cross border capacity has been exceeded. The time series has been rejected or adjusted.</skos:definition>
  </skos:Concept>
  <skos:Concept rdf:about="http://energy.referencedata.eu/StandardReasonCodeTypeList/A28">
    <skos:inScheme rdf:resource="http://energy.referencedata.eu/StandardReasonCodeTypeList"/>
    <skos:topConceptOf rdf:resource="http://energy.referencedata.eu/StandardReasonCodeTypeList"/>
    <dcterms:identifier>A28</dcterms:identifier>
    <skos:prefLabel>Counterpart time series missing </skos:prefLabel>
    <skos:definition xml:lang="en">This provides an indication that the time series has not got a counterpart time series. 
In the case of an Intermediate Confirmation Report this is advising the recipient that the time series may be rejected at nomination closure if the counterpart time series is not received. 
In the case of a Final Confirmation Report this is informing the recipient that the time series has been rejected because the counterpart time series has not been forthcoming. </skos:definition>
  </skos:Concept>
  <skos:Concept rdf:about="http://energy.referencedata.eu/StandardReasonCodeTypeList/A29">
    <skos:inScheme rdf:resource="http://energy.referencedata.eu/StandardReasonCodeTypeList"/>
    <skos:topConceptOf rdf:resource="http://energy.referencedata.eu/StandardReasonCodeTypeList"/>
    <dcterms:identifier>A29</dcterms:identifier>
    <skos:prefLabel>Counterpart time series quantity differences </skos:prefLabel>
    <skos:definition xml:lang="en">The time series has been rejected as it does not match that of the counterpart who is considered by market rules to be correct.</skos:definition>
  </skos:Concept>
  <skos:Concept rdf:about="http://energy.referencedata.eu/StandardReasonCodeTypeList/A30">
    <skos:inScheme rdf:resource="http://energy.referencedata.eu/StandardReasonCodeTypeList"/>
    <skos:topConceptOf rdf:resource="http://energy.referencedata.eu/StandardReasonCodeTypeList"/>
    <dcterms:identifier>A30</dcterms:identifier>
    <skos:prefLabel>Imposed Time series from nominated party's time series (party identified in reason text)</skos:prefLabel>
    <skos:definition xml:lang="en">The nominated party's time series has replaced the current time series. This reason code may not be used in conjunction with A26.</skos:definition>
  </skos:Concept>
  <skos:Concept rdf:about="http://energy.referencedata.eu/StandardReasonCodeTypeList/A41">
    <skos:inScheme rdf:resource="http://energy.referencedata.eu/StandardReasonCodeTypeList"/>
    <skos:topConceptOf rdf:resource="http://energy.referencedata.eu/StandardReasonCodeTypeList"/>
    <dcterms:identifier>A41</dcterms:identifier>
    <skos:prefLabel>Resolution inconsistency </skos:prefLabel>
    <skos:definition xml:lang="en">The resolution is not coherent with the time interval, or resolution not valid.</skos:definition>
  </skos:Concept>
  <skos:Concept rdf:about="http://energy.referencedata.eu/StandardReasonCodeTypeList/A42">
    <skos:inScheme rdf:resource="http://energy.referencedata.eu/StandardReasonCodeTypeList"/>
    <skos:topConceptOf rdf:resource="http://energy.referencedata.eu/StandardReasonCodeTypeList"/>
    <dcterms:identifier>A42</dcterms:identifier>
    <skos:prefLabel>Quantity inconsistency </skos:prefLabel>
    <skos:definition xml:lang="en">The quantity is not coherent. For example a time period with the same version number but different quantities or an non permitted number of digits after the decimal point, etc.</skos:definition>
  </skos:Concept>
  <skos:Concept rdf:about="http://energy.referencedata.eu/StandardReasonCodeTypeList/A43">
    <skos:inScheme rdf:resource="http://energy.referencedata.eu/StandardReasonCodeTypeList"/>
    <skos:topConceptOf rdf:resource="http://energy.referencedata.eu/StandardReasonCodeTypeList"/>
    <dcterms:identifier>A43</dcterms:identifier>
    <skos:prefLabel>Quantity increased </skos:prefLabel>
    <skos:definition xml:lang="en">The quantity has been increased in order to satisfy minimum constraints.</skos:definition>
  </skos:Concept>
  <skos:Concept rdf:about="http://energy.referencedata.eu/StandardReasonCodeTypeList/A44">
    <skos:inScheme rdf:resource="http://energy.referencedata.eu/StandardReasonCodeTypeList"/>
    <skos:topConceptOf rdf:resource="http://energy.referencedata.eu/StandardReasonCodeTypeList"/>
    <dcterms:identifier>A44</dcterms:identifier>
    <skos:prefLabel>Quantity decreased </skos:prefLabel>
    <skos:definition xml:lang="en">The quantity has been decreased in order to satisfy congestion constraints.</skos:definition>
  </skos:Concept>
  <skos:Concept rdf:about="http://energy.referencedata.eu/StandardReasonCodeTypeList/A45">
    <skos:inScheme rdf:resource="http://energy.referencedata.eu/StandardReasonCodeTypeList"/>
    <skos:topConceptOf rdf:resource="http://energy.referencedata.eu/StandardReasonCodeTypeList"/>
    <dcterms:identifier>A45</dcterms:identifier>
    <skos:prefLabel>Default quantity applied </skos:prefLabel>
    <skos:definition xml:lang="en">The default quantity has been applied as the current quantity does not satisfy contractual obligations.</skos:definition>
  </skos:Concept>
  <skos:Concept rdf:about="http://energy.referencedata.eu/StandardReasonCodeTypeList/A46">
    <skos:inScheme rdf:resource="http://energy.referencedata.eu/StandardReasonCodeTypeList"/>
    <skos:topConceptOf rdf:resource="http://energy.referencedata.eu/StandardReasonCodeTypeList"/>
    <dcterms:identifier>A46</dcterms:identifier>
    <skos:prefLabel>Quantities must not be signed values</skos:prefLabel>
    <skos:definition xml:lang="en">The quantity proposed is illegal since signed values are only permitted in specific circumstances.</skos:definition>
  </skos:Concept>
  <skos:Concept rdf:about="http://energy.referencedata.eu/StandardReasonCodeTypeList/A47">
    <skos:inScheme rdf:resource="http://energy.referencedata.eu/StandardReasonCodeTypeList"/>
    <skos:topConceptOf rdf:resource="http://energy.referencedata.eu/StandardReasonCodeTypeList"/>
    <dcterms:identifier>A47</dcterms:identifier>
    <skos:prefLabel>A47 not applicable</skos:prefLabel>
    <skos:definition xml:lang="en">This code is no longer applicable.</skos:definition>
  </skos:Concept>
  <skos:Concept rdf:about="http://energy.referencedata.eu/StandardReasonCodeTypeList/A48">
    <skos:inScheme rdf:resource="http://energy.referencedata.eu/StandardReasonCodeTypeList"/>
    <skos:topConceptOf rdf:resource="http://energy.referencedata.eu/StandardReasonCodeTypeList"/>
    <dcterms:identifier>A48</dcterms:identifier>
    <skos:prefLabel>Modification reason</skos:prefLabel>
    <skos:definition xml:lang="en">In an intraday transmission, the reason for the modification is as follows (in the reason text).</skos:definition>
  </skos:Concept>
  <skos:Concept rdf:about="http://energy.referencedata.eu/StandardReasonCodeTypeList/A49">
    <skos:inScheme rdf:resource="http://energy.referencedata.eu/StandardReasonCodeTypeList"/>
    <skos:topConceptOf rdf:resource="http://energy.referencedata.eu/StandardReasonCodeTypeList"/>
    <dcterms:identifier>A49</dcterms:identifier>
    <skos:prefLabel>Position inconsistency</skos:prefLabel>
    <skos:definition xml:lang="en">A position is missing or too many.</skos:definition>
  </skos:Concept>
  <skos:Concept rdf:about="http://energy.referencedata.eu/StandardReasonCodeTypeList/A50">
    <skos:inScheme rdf:resource="http://energy.referencedata.eu/StandardReasonCodeTypeList"/>
    <skos:topConceptOf rdf:resource="http://energy.referencedata.eu/StandardReasonCodeTypeList"/>
    <dcterms:identifier>A50</dcterms:identifier>
    <skos:prefLabel>Senders time series version conflict</skos:prefLabel>
    <skos:definition xml:lang="en">There is an error in the sender time series version, i.e. it could be superior to the message version or is inconsistent with the existing data. The time series has been rejected.</skos:definition>
  </skos:Concept>
  <skos:Concept rdf:about="http://energy.referencedata.eu/StandardReasonCodeTypeList/A51">
    <skos:inScheme rdf:resource="http://energy.referencedata.eu/StandardReasonCodeTypeList"/>
    <skos:topConceptOf rdf:resource="http://energy.referencedata.eu/StandardReasonCodeTypeList"/>
    <dcterms:identifier>A51</dcterms:identifier>
    <skos:prefLabel>Message identification or version conflict</skos:prefLabel>
    <skos:definition xml:lang="en">The message identification is already in the receiving system. Or a higher version already exists. Message rejected.</skos:definition>
  </skos:Concept>
  <skos:Concept rdf:about="http://energy.referencedata.eu/StandardReasonCodeTypeList/A52">
    <skos:inScheme rdf:resource="http://energy.referencedata.eu/StandardReasonCodeTypeList"/>
    <skos:topConceptOf rdf:resource="http://energy.referencedata.eu/StandardReasonCodeTypeList"/>
    <dcterms:identifier>A52</dcterms:identifier>
    <skos:prefLabel>Time series missing from new version of message</skos:prefLabel>
    <skos:definition xml:lang="en">A time series is not contained in a new version of the message. Message rejected.</skos:definition>
  </skos:Concept>
  <skos:Concept rdf:about="http://energy.referencedata.eu/StandardReasonCodeTypeList/A53">
    <skos:inScheme rdf:resource="http://energy.referencedata.eu/StandardReasonCodeTypeList"/>
    <skos:topConceptOf rdf:resource="http://energy.referencedata.eu/StandardReasonCodeTypeList"/>
    <dcterms:identifier>A53</dcterms:identifier>
    <skos:prefLabel>Receiving party incorrect</skos:prefLabel>
    <skos:definition xml:lang="en">The receiving party is incorrect. Message rejected.</skos:definition>
  </skos:Concept>
  <skos:Concept rdf:about="http://energy.referencedata.eu/StandardReasonCodeTypeList/A54">
    <skos:inScheme rdf:resource="http://energy.referencedata.eu/StandardReasonCodeTypeList"/>
    <skos:topConceptOf rdf:resource="http://energy.referencedata.eu/StandardReasonCodeTypeList"/>
    <dcterms:identifier>A54</dcterms:identifier>
    <skos:prefLabel>Global position not in balance</skos:prefLabel>
    <skos:definition xml:lang="en">The message does not balance out to zero. Market rules might require that the message is rejected. </skos:definition>
  </skos:Concept>
  <skos:Concept rdf:about="http://energy.referencedata.eu/StandardReasonCodeTypeList/A55">
    <skos:inScheme rdf:resource="http://energy.referencedata.eu/StandardReasonCodeTypeList"/>
    <skos:topConceptOf rdf:resource="http://energy.referencedata.eu/StandardReasonCodeTypeList"/>
    <dcterms:identifier>A55</dcterms:identifier>
    <skos:prefLabel>Time series identification conflict</skos:prefLabel>
    <skos:definition xml:lang="en">The identification of the time series is duplicated or incorrect. Time series will be rejected.</skos:definition>
  </skos:Concept>
  <skos:Concept rdf:about="http://energy.referencedata.eu/StandardReasonCodeTypeList/A56">
    <skos:inScheme rdf:resource="http://energy.referencedata.eu/StandardReasonCodeTypeList"/>
    <skos:topConceptOf rdf:resource="http://energy.referencedata.eu/StandardReasonCodeTypeList"/>
    <dcterms:identifier>A56</dcterms:identifier>
    <skos:prefLabel>Corresponding Time series not netted</skos:prefLabel>
    <skos:definition xml:lang="en">All corresponding time series must be netted. Time series rejected.</skos:definition>
  </skos:Concept>
  <skos:Concept rdf:about="http://energy.referencedata.eu/StandardReasonCodeTypeList/A57">
    <skos:inScheme rdf:resource="http://energy.referencedata.eu/StandardReasonCodeTypeList"/>
    <skos:topConceptOf rdf:resource="http://energy.referencedata.eu/StandardReasonCodeTypeList"/>
    <dcterms:identifier>A57</dcterms:identifier>
    <skos:prefLabel>Deadline limit exceeded/Gate not open</skos:prefLabel>
    <skos:definition xml:lang="en">The deadline for receiving schedule messages has passed. Message or time series rejected.</skos:definition>
  </skos:Concept>
  <skos:Concept rdf:about="http://energy.referencedata.eu/StandardReasonCodeTypeList/A58">
    <skos:inScheme rdf:resource="http://energy.referencedata.eu/StandardReasonCodeTypeList"/>
    <skos:topConceptOf rdf:resource="http://energy.referencedata.eu/StandardReasonCodeTypeList"/>
    <dcterms:identifier>A58</dcterms:identifier>
    <skos:prefLabel>One to one nomination inconsistency</skos:prefLabel>
    <skos:definition xml:lang="en">There is a one to one nomination inconstancy with the in/out parties or areas. Time series rejected.</skos:definition>
  </skos:Concept>
  <skos:Concept rdf:about="http://energy.referencedata.eu/StandardReasonCodeTypeList/A59">
    <skos:inScheme rdf:resource="http://energy.referencedata.eu/StandardReasonCodeTypeList"/>
    <skos:topConceptOf rdf:resource="http://energy.referencedata.eu/StandardReasonCodeTypeList"/>
    <dcterms:identifier>A59</dcterms:identifier>
    <skos:prefLabel>Not compliant to local market rules</skos:prefLabel>
    <skos:definition xml:lang="en">The level in which this is identified is not in compliance with local market rules. The level in question has been rejected.</skos:definition>
  </skos:Concept>
  <skos:Concept rdf:about="http://energy.referencedata.eu/StandardReasonCodeTypeList/A60">
    <skos:inScheme rdf:resource="http://energy.referencedata.eu/StandardReasonCodeTypeList"/>
    <skos:topConceptOf rdf:resource="http://energy.referencedata.eu/StandardReasonCodeTypeList"/>
    <dcterms:identifier>A60</dcterms:identifier>
    <skos:prefLabel>Inter-area transit schedule exceeds nominated schedule</skos:prefLabel>
    <skos:definition xml:lang="en">The inter-area transit schedule exceeds the nominated schedule for the same time interval. The inter-area transit schedule is rejected.</skos:definition>
  </skos:Concept>
  <skos:Concept rdf:about="http://energy.referencedata.eu/StandardReasonCodeTypeList/A61">
    <skos:inScheme rdf:resource="http://energy.referencedata.eu/StandardReasonCodeTypeList"/>
    <skos:topConceptOf rdf:resource="http://energy.referencedata.eu/StandardReasonCodeTypeList"/>
    <dcterms:identifier>A61</dcterms:identifier>
    <skos:prefLabel>Currency invalid</skos:prefLabel>
    <skos:definition xml:lang="en">The currency is not in compliance with ISO 4217.</skos:definition>
  </skos:Concept>
  <skos:Concept rdf:about="http://energy.referencedata.eu/StandardReasonCodeTypeList/A62">
    <skos:inScheme rdf:resource="http://energy.referencedata.eu/StandardReasonCodeTypeList"/>
    <skos:topConceptOf rdf:resource="http://energy.referencedata.eu/StandardReasonCodeTypeList"/>
    <dcterms:identifier>A62</dcterms:identifier>
    <skos:prefLabel>Invalid business type</skos:prefLabel>
    <skos:definition xml:lang="en">The business type does not belong to the valid set of business types for the process in question.</skos:definition>
  </skos:Concept>
  <skos:Concept rdf:about="http://energy.referencedata.eu/StandardReasonCodeTypeList/A63">
    <skos:inScheme rdf:resource="http://energy.referencedata.eu/StandardReasonCodeTypeList"/>
    <skos:topConceptOf rdf:resource="http://energy.referencedata.eu/StandardReasonCodeTypeList"/>
    <dcterms:identifier>A63</dcterms:identifier>
    <skos:prefLabel>Time Series modified</skos:prefLabel>
    <skos:definition xml:lang="en">The time series has been modified.</skos:definition>
  </skos:Concept>
  <skos:Concept rdf:about="http://energy.referencedata.eu/StandardReasonCodeTypeList/A64">
    <skos:inScheme rdf:resource="http://energy.referencedata.eu/StandardReasonCodeTypeList"/>
    <skos:topConceptOf rdf:resource="http://energy.referencedata.eu/StandardReasonCodeTypeList"/>
    <dcterms:identifier>A64</dcterms:identifier>
    <skos:prefLabel>Resource Object Invalid</skos:prefLabel>
    <skos:definition xml:lang="en">The Resource Object defined in the document is not valid.</skos:definition>
  </skos:Concept>
  <skos:Concept rdf:about="http://energy.referencedata.eu/StandardReasonCodeTypeList/A65">
    <skos:inScheme rdf:resource="http://energy.referencedata.eu/StandardReasonCodeTypeList"/>
    <skos:topConceptOf rdf:resource="http://energy.referencedata.eu/StandardReasonCodeTypeList"/>
    <dcterms:identifier>A65</dcterms:identifier>
    <skos:prefLabel>Reserve object Technical  limits exceeded</skos:prefLabel>
    <skos:definition xml:lang="en">Reserve objects aggregated values are not within technical/prequalified limits</skos:definition>
  </skos:Concept>
  <skos:Concept rdf:about="http://energy.referencedata.eu/StandardReasonCodeTypeList/A66">
    <skos:inScheme rdf:resource="http://energy.referencedata.eu/StandardReasonCodeTypeList"/>
    <skos:topConceptOf rdf:resource="http://energy.referencedata.eu/StandardReasonCodeTypeList"/>
    <dcterms:identifier>A66</dcterms:identifier>
    <skos:prefLabel>Planned reserves do not correspond with contractual data</skos:prefLabel>
    <skos:definition xml:lang="en">Planned reserves do not correspond with contractual data.</skos:definition>
  </skos:Concept>
  <skos:Concept rdf:about="http://energy.referencedata.eu/StandardReasonCodeTypeList/A67">
    <skos:inScheme rdf:resource="http://energy.referencedata.eu/StandardReasonCodeTypeList"/>
    <skos:topConceptOf rdf:resource="http://energy.referencedata.eu/StandardReasonCodeTypeList"/>
    <dcterms:identifier>A67</dcterms:identifier>
    <skos:prefLabel>Limit Data is not available</skos:prefLabel>
    <skos:definition xml:lang="en">Limit Data is not available.</skos:definition>
  </skos:Concept>
  <skos:Concept rdf:about="http://energy.referencedata.eu/StandardReasonCodeTypeList/A68">
    <skos:inScheme rdf:resource="http://energy.referencedata.eu/StandardReasonCodeTypeList"/>
    <skos:topConceptOf rdf:resource="http://energy.referencedata.eu/StandardReasonCodeTypeList"/>
    <dcterms:identifier>A68</dcterms:identifier>
    <skos:prefLabel>Reserve Object not qualified for reserve type</skos:prefLabel>
    <skos:definition xml:lang="en">Reserve Object is not qualified for reserve type.</skos:definition>
  </skos:Concept>
  <skos:Concept rdf:about="http://energy.referencedata.eu/StandardReasonCodeTypeList/A69">
    <skos:inScheme rdf:resource="http://energy.referencedata.eu/StandardReasonCodeTypeList"/>
    <skos:topConceptOf rdf:resource="http://energy.referencedata.eu/StandardReasonCodeTypeList"/>
    <dcterms:identifier>A69</dcterms:identifier>
    <skos:prefLabel>Mandatory attributes missing</skos:prefLabel>
    <skos:definition xml:lang="en">Mandatory attributes missing.</skos:definition>
  </skos:Concept>
  <skos:Concept rdf:about="http://energy.referencedata.eu/StandardReasonCodeTypeList/A70">
    <skos:inScheme rdf:resource="http://energy.referencedata.eu/StandardReasonCodeTypeList"/>
    <skos:topConceptOf rdf:resource="http://energy.referencedata.eu/StandardReasonCodeTypeList"/>
    <dcterms:identifier>A70</dcterms:identifier>
    <skos:prefLabel>Curtailment</skos:prefLabel>
    <skos:definition xml:lang="en">The capacity in question has been curtailed.</skos:definition>
  </skos:Concept>
  <skos:Concept rdf:about="http://energy.referencedata.eu/StandardReasonCodeTypeList/A71">
    <skos:inScheme rdf:resource="http://energy.referencedata.eu/StandardReasonCodeTypeList"/>
    <skos:topConceptOf rdf:resource="http://energy.referencedata.eu/StandardReasonCodeTypeList"/>
    <dcterms:identifier>A71</dcterms:identifier>
    <skos:prefLabel>Linked bid rejected due to associated bid unsuccessful</skos:prefLabel>
    <skos:definition xml:lang="en">The bid in question has been rejected because an associated bid has been unsuccessful.</skos:definition>
  </skos:Concept>
  <skos:Concept rdf:about="http://energy.referencedata.eu/StandardReasonCodeTypeList/A72">
    <skos:inScheme rdf:resource="http://energy.referencedata.eu/StandardReasonCodeTypeList"/>
    <skos:topConceptOf rdf:resource="http://energy.referencedata.eu/StandardReasonCodeTypeList"/>
    <dcterms:identifier>A72</dcterms:identifier>
    <skos:prefLabel>Original bid divided to permit acceptance</skos:prefLabel>
    <skos:definition xml:lang="en">The original bid quantity has been divided to enable it to be accepted.</skos:definition>
  </skos:Concept>
  <skos:Concept rdf:about="http://energy.referencedata.eu/StandardReasonCodeTypeList/A73">
    <skos:inScheme rdf:resource="http://energy.referencedata.eu/StandardReasonCodeTypeList"/>
    <skos:topConceptOf rdf:resource="http://energy.referencedata.eu/StandardReasonCodeTypeList"/>
    <dcterms:identifier>A73</dcterms:identifier>
    <skos:prefLabel>Bid accepted</skos:prefLabel>
    <skos:definition xml:lang="en">The bid in question has been accepted.</skos:definition>
  </skos:Concept>
  <skos:Concept rdf:about="http://energy.referencedata.eu/StandardReasonCodeTypeList/A74">
    <skos:inScheme rdf:resource="http://energy.referencedata.eu/StandardReasonCodeTypeList"/>
    <skos:topConceptOf rdf:resource="http://energy.referencedata.eu/StandardReasonCodeTypeList"/>
    <dcterms:identifier>A74</dcterms:identifier>
    <skos:prefLabel>Auction Status</skos:prefLabel>
    <skos:definition xml:lang="en">The information in the Reason Text provides auction status information.</skos:definition>
  </skos:Concept>
  <skos:Concept rdf:about="http://energy.referencedata.eu/StandardReasonCodeTypeList/A75">
    <skos:inScheme rdf:resource="http://energy.referencedata.eu/StandardReasonCodeTypeList"/>
    <skos:topConceptOf rdf:resource="http://energy.referencedata.eu/StandardReasonCodeTypeList"/>
    <dcterms:identifier>A75</dcterms:identifier>
    <skos:prefLabel>Right status information</skos:prefLabel>
    <skos:definition xml:lang="en">The information in the Reason Text provides status information concerning the transmission rights in question.</skos:definition>
  </skos:Concept>
  <skos:Concept rdf:about="http://energy.referencedata.eu/StandardReasonCodeTypeList/A76">
    <skos:inScheme rdf:resource="http://energy.referencedata.eu/StandardReasonCodeTypeList"/>
    <skos:topConceptOf rdf:resource="http://energy.referencedata.eu/StandardReasonCodeTypeList"/>
    <dcterms:identifier>A76</dcterms:identifier>
    <skos:prefLabel>Agreement identification inconsistency</skos:prefLabel>
    <skos:definition xml:lang="en">There is an inconsistency between the contract type and the agreement identification.</skos:definition>
  </skos:Concept>
  <skos:Concept rdf:about="http://energy.referencedata.eu/StandardReasonCodeTypeList/A77">
    <skos:inScheme rdf:resource="http://energy.referencedata.eu/StandardReasonCodeTypeList"/>
    <skos:topConceptOf rdf:resource="http://energy.referencedata.eu/StandardReasonCodeTypeList"/>
    <dcterms:identifier>A77</dcterms:identifier>
    <skos:prefLabel>Dependency matrix not respected</skos:prefLabel>
    <skos:definition xml:lang="en">There is an inconsistency between the document contents and the dependency matrix.</skos:definition>
  </skos:Concept>
  <skos:Concept rdf:about="http://energy.referencedata.eu/StandardReasonCodeTypeList/A78">
    <skos:inScheme rdf:resource="http://energy.referencedata.eu/StandardReasonCodeTypeList"/>
    <skos:topConceptOf rdf:resource="http://energy.referencedata.eu/StandardReasonCodeTypeList"/>
    <dcterms:identifier>A78</dcterms:identifier>
    <skos:prefLabel>Sender identification and/or role invalid</skos:prefLabel>
    <skos:definition xml:lang="en">The identification of the sender or the sender/role combination is invalid.</skos:definition>
  </skos:Concept>
  <skos:Concept rdf:about="http://energy.referencedata.eu/StandardReasonCodeTypeList/A79">
    <skos:inScheme rdf:resource="http://energy.referencedata.eu/StandardReasonCodeTypeList"/>
    <skos:topConceptOf rdf:resource="http://energy.referencedata.eu/StandardReasonCodeTypeList"/>
    <dcterms:identifier>A79</dcterms:identifier>
    <skos:prefLabel>Process type invalid</skos:prefLabel>
    <skos:definition xml:lang="en">The process type does not figure in the list of valid process types for this document.</skos:definition>
  </skos:Concept>
  <skos:Concept rdf:about="http://energy.referencedata.eu/StandardReasonCodeTypeList/A80">
    <skos:inScheme rdf:resource="http://energy.referencedata.eu/StandardReasonCodeTypeList"/>
    <skos:topConceptOf rdf:resource="http://energy.referencedata.eu/StandardReasonCodeTypeList"/>
    <dcterms:identifier>A80</dcterms:identifier>
    <skos:prefLabel>Domain invalid</skos:prefLabel>
    <skos:definition xml:lang="en">The domain does not figure in the list of valid domains for this document and process.</skos:definition>
  </skos:Concept>
  <skos:Concept rdf:about="http://energy.referencedata.eu/StandardReasonCodeTypeList/A81">
    <skos:inScheme rdf:resource="http://energy.referencedata.eu/StandardReasonCodeTypeList"/>
    <skos:topConceptOf rdf:resource="http://energy.referencedata.eu/StandardReasonCodeTypeList"/>
    <dcterms:identifier>A81</dcterms:identifier>
    <skos:prefLabel>Matching period invalid</skos:prefLabel>
    <skos:definition xml:lang="en">The period is not within the expected limits.</skos:definition>
  </skos:Concept>
  <skos:Concept rdf:about="http://energy.referencedata.eu/StandardReasonCodeTypeList/A82">
    <skos:inScheme rdf:resource="http://energy.referencedata.eu/StandardReasonCodeTypeList"/>
    <skos:topConceptOf rdf:resource="http://energy.referencedata.eu/StandardReasonCodeTypeList"/>
    <dcterms:identifier>A82</dcterms:identifier>
    <skos:prefLabel>In/Out area inconsistent with domain</skos:prefLabel>
    <skos:definition xml:lang="en">The in and out area does not figure within the domain specified.</skos:definition>
  </skos:Concept>
  <skos:Concept rdf:about="http://energy.referencedata.eu/StandardReasonCodeTypeList/A83">
    <skos:inScheme rdf:resource="http://energy.referencedata.eu/StandardReasonCodeTypeList"/>
    <skos:topConceptOf rdf:resource="http://energy.referencedata.eu/StandardReasonCodeTypeList"/>
    <dcterms:identifier>A83</dcterms:identifier>
    <skos:prefLabel>Disagree with matching results</skos:prefLabel>
    <skos:definition xml:lang="en">The matching results provided are not consistent.</skos:definition>
  </skos:Concept>
  <skos:Concept rdf:about="http://energy.referencedata.eu/StandardReasonCodeTypeList/A84">
    <skos:inScheme rdf:resource="http://energy.referencedata.eu/StandardReasonCodeTypeList"/>
    <skos:topConceptOf rdf:resource="http://energy.referencedata.eu/StandardReasonCodeTypeList"/>
    <dcterms:identifier>A84</dcterms:identifier>
    <skos:prefLabel>Confirmation ignored due to higher version already received</skos:prefLabel>
    <skos:definition xml:lang="en">The report has been ignored since a higher version has been received.</skos:definition>
  </skos:Concept>
  <skos:Concept rdf:about="http://energy.referencedata.eu/StandardReasonCodeTypeList/A85">
    <skos:inScheme rdf:resource="http://energy.referencedata.eu/StandardReasonCodeTypeList"/>
    <skos:topConceptOf rdf:resource="http://energy.referencedata.eu/StandardReasonCodeTypeList"/>
    <dcterms:identifier>A85</dcterms:identifier>
    <skos:prefLabel>Confirmation without adjustment (time series have been matched without change)</skos:prefLabel>
    <skos:definition xml:lang="en">The report has been successfully matched without any changes.</skos:definition>
  </skos:Concept>
  <skos:Concept rdf:about="http://energy.referencedata.eu/StandardReasonCodeTypeList/A86">
    <skos:inScheme rdf:resource="http://energy.referencedata.eu/StandardReasonCodeTypeList"/>
    <skos:topConceptOf rdf:resource="http://energy.referencedata.eu/StandardReasonCodeTypeList"/>
    <dcterms:identifier>A86</dcterms:identifier>
    <skos:prefLabel>Confirmation with adjustment (time series have been modified)</skos:prefLabel>
    <skos:definition xml:lang="en">The report has been matched but required adjustment.</skos:definition>
  </skos:Concept>
  <skos:Concept rdf:about="http://energy.referencedata.eu/StandardReasonCodeTypeList/A87">
    <skos:inScheme rdf:resource="http://energy.referencedata.eu/StandardReasonCodeTypeList"/>
    <skos:topConceptOf rdf:resource="http://energy.referencedata.eu/StandardReasonCodeTypeList"/>
    <dcterms:identifier>A87</dcterms:identifier>
    <skos:prefLabel>For action (only in intermediate confirmation - time series need mutual agreement and action)</skos:prefLabel>
    <skos:definition xml:lang="en">The report in question is only for action in an intermediate stage.</skos:definition>
  </skos:Concept>
  <skos:Concept rdf:about="http://energy.referencedata.eu/StandardReasonCodeTypeList/A88">
    <skos:inScheme rdf:resource="http://energy.referencedata.eu/StandardReasonCodeTypeList"/>
    <skos:topConceptOf rdf:resource="http://energy.referencedata.eu/StandardReasonCodeTypeList"/>
    <dcterms:identifier>A88</dcterms:identifier>
    <skos:prefLabel>Time series matched</skos:prefLabel>
    <skos:definition xml:lang="en">The time series has been successfully matched.</skos:definition>
  </skos:Concept>
  <skos:Concept rdf:about="http://energy.referencedata.eu/StandardReasonCodeTypeList/A89">
    <skos:inScheme rdf:resource="http://energy.referencedata.eu/StandardReasonCodeTypeList"/>
    <skos:topConceptOf rdf:resource="http://energy.referencedata.eu/StandardReasonCodeTypeList"/>
    <dcterms:identifier>A89</dcterms:identifier>
    <skos:prefLabel>Time series ignored (note: this can only apply to time series that are set to zero - see matching principles)</skos:prefLabel>
    <skos:definition xml:lang="en">The time series has been ignored and not matched since it does not figure in a counterparty transmission. All are correctly equal to zero.</skos:definition>
  </skos:Concept>
  <skos:Concept rdf:about="http://energy.referencedata.eu/StandardReasonCodeTypeList/A90">
    <skos:inScheme rdf:resource="http://energy.referencedata.eu/StandardReasonCodeTypeList"/>
    <skos:topConceptOf rdf:resource="http://energy.referencedata.eu/StandardReasonCodeTypeList"/>
    <dcterms:identifier>A90</dcterms:identifier>
    <skos:prefLabel>Modification proposal (intermediate confirmation)</skos:prefLabel>
    <skos:definition xml:lang="en">The document is a proposal for change before finalization.</skos:definition>
  </skos:Concept>
  <skos:Concept rdf:about="http://energy.referencedata.eu/StandardReasonCodeTypeList/A91">
    <skos:inScheme rdf:resource="http://energy.referencedata.eu/StandardReasonCodeTypeList"/>
    <skos:topConceptOf rdf:resource="http://energy.referencedata.eu/StandardReasonCodeTypeList"/>
    <dcterms:identifier>A91</dcterms:identifier>
    <skos:prefLabel>Expected document not received</skos:prefLabel>
    <skos:definition xml:lang="en">The document that is expected has not been received within the expected timeframe.</skos:definition>
  </skos:Concept>
  <skos:Concept rdf:about="http://energy.referencedata.eu/StandardReasonCodeTypeList/A92">
    <skos:inScheme rdf:resource="http://energy.referencedata.eu/StandardReasonCodeTypeList"/>
    <skos:topConceptOf rdf:resource="http://energy.referencedata.eu/StandardReasonCodeTypeList"/>
    <dcterms:identifier>A92</dcterms:identifier>
    <skos:prefLabel>Not possible to send document on time, but estimated delivery time is provided</skos:prefLabel>
    <skos:definition xml:lang="en">The document that is due cannot be transmitted within the required timeframe. An estimated time of transmission is provided.</skos:definition>
  </skos:Concept>
  <skos:Concept rdf:about="http://energy.referencedata.eu/StandardReasonCodeTypeList/A93">
    <skos:inScheme rdf:resource="http://energy.referencedata.eu/StandardReasonCodeTypeList"/>
    <skos:topConceptOf rdf:resource="http://energy.referencedata.eu/StandardReasonCodeTypeList"/>
    <dcterms:identifier>A93</dcterms:identifier>
    <skos:prefLabel>Not possible to send document on time, and furthermore no expected time of return to normal situation</skos:prefLabel>
    <skos:definition xml:lang="en">The document that is due cannot be transmitted within the required timeframe. The time of transmission of the document is unknown.</skos:definition>
  </skos:Concept>
  <skos:Concept rdf:about="http://energy.referencedata.eu/StandardReasonCodeTypeList/A94">
    <skos:inScheme rdf:resource="http://energy.referencedata.eu/StandardReasonCodeTypeList"/>
    <skos:topConceptOf rdf:resource="http://energy.referencedata.eu/StandardReasonCodeTypeList"/>
    <dcterms:identifier>A94</dcterms:identifier>
    <skos:prefLabel>Document cannot be processed by receiving system</skos:prefLabel>
    <skos:definition xml:lang="en">The receiving system cannot process that document in question.</skos:definition>
  </skos:Concept>
  <skos:Concept rdf:about="http://energy.referencedata.eu/StandardReasonCodeTypeList/A95">
    <skos:inScheme rdf:resource="http://energy.referencedata.eu/StandardReasonCodeTypeList"/>
    <skos:topConceptOf rdf:resource="http://energy.referencedata.eu/StandardReasonCodeTypeList"/>
    <dcterms:identifier>A95</dcterms:identifier>
    <skos:prefLabel>Complementary information</skos:prefLabel>
    <skos:definition xml:lang="en">Additional text is provided in order to further explain a condition, for example to provide details of an outage.</skos:definition>
  </skos:Concept>
  <skos:Concept rdf:about="http://energy.referencedata.eu/StandardReasonCodeTypeList/A96">
    <skos:inScheme rdf:resource="http://energy.referencedata.eu/StandardReasonCodeTypeList"/>
    <skos:topConceptOf rdf:resource="http://energy.referencedata.eu/StandardReasonCodeTypeList"/>
    <dcterms:identifier>A96</dcterms:identifier>
    <skos:prefLabel>Technical constraint</skos:prefLabel>
    <skos:definition xml:lang="en">A technical constraint has been applied.</skos:definition>
  </skos:Concept>
  <skos:Concept rdf:about="http://energy.referencedata.eu/StandardReasonCodeTypeList/A97">
    <skos:inScheme rdf:resource="http://energy.referencedata.eu/StandardReasonCodeTypeList"/>
    <skos:topConceptOf rdf:resource="http://energy.referencedata.eu/StandardReasonCodeTypeList"/>
    <dcterms:identifier>A97</dcterms:identifier>
    <skos:prefLabel>Force majeure curtailment</skos:prefLabel>
    <skos:definition xml:lang="en">Curtailment due to Force Majeure. A code that enables the identification of the curtailment reason for settlement purposes.</skos:definition>
  </skos:Concept>
  <skos:Concept rdf:about="http://energy.referencedata.eu/StandardReasonCodeTypeList/A98">
    <skos:inScheme rdf:resource="http://energy.referencedata.eu/StandardReasonCodeTypeList"/>
    <skos:topConceptOf rdf:resource="http://energy.referencedata.eu/StandardReasonCodeTypeList"/>
    <dcterms:identifier>A98</dcterms:identifier>
    <skos:prefLabel>Network security curtailment</skos:prefLabel>
    <skos:definition xml:lang="en">Curtailment due to network security reasons A code that enables the identification of the curtailment reason for settlement purposes.</skos:definition>
  </skos:Concept>
  <skos:Concept rdf:about="http://energy.referencedata.eu/StandardReasonCodeTypeList/A99">
    <skos:inScheme rdf:resource="http://energy.referencedata.eu/StandardReasonCodeTypeList"/>
    <skos:topConceptOf rdf:resource="http://energy.referencedata.eu/StandardReasonCodeTypeList"/>
    <dcterms:identifier>A99</dcterms:identifier>
    <skos:prefLabel>Auction cancelled</skos:prefLabel>
    <skos:definition xml:lang="en">The auction has been cancelled.</skos:definition>
  </skos:Concept>
  <skos:Concept rdf:about="http://energy.referencedata.eu/StandardReasonCodeTypeList/B01">
    <skos:inScheme rdf:resource="http://energy.referencedata.eu/StandardReasonCodeTypeList"/>
    <skos:topConceptOf rdf:resource="http://energy.referencedata.eu/StandardReasonCodeTypeList"/>
    <dcterms:identifier>B01</dcterms:identifier>
    <skos:prefLabel>Incomplete document</skos:prefLabel>
    <skos:definition xml:lang="en">The document is incomplete and cannot be processed.</skos:definition>
  </skos:Concept>
  <skos:Concept rdf:about="http://energy.referencedata.eu/StandardReasonCodeTypeList/B02">
    <skos:inScheme rdf:resource="http://energy.referencedata.eu/StandardReasonCodeTypeList"/>
    <skos:topConceptOf rdf:resource="http://energy.referencedata.eu/StandardReasonCodeTypeList"/>
    <dcterms:identifier>B02</dcterms:identifier>
    <skos:prefLabel>Accounting Point (tie-line) Time Series missing</skos:prefLabel>
    <skos:definition xml:lang="en">The document is incomplete as a time series for an accounting point is missing.</skos:definition>
  </skos:Concept>
  <skos:Concept rdf:about="http://energy.referencedata.eu/StandardReasonCodeTypeList/B03">
    <skos:inScheme rdf:resource="http://energy.referencedata.eu/StandardReasonCodeTypeList"/>
    <skos:topConceptOf rdf:resource="http://energy.referencedata.eu/StandardReasonCodeTypeList"/>
    <dcterms:identifier>B03</dcterms:identifier>
    <skos:prefLabel>Meter data Time series missing</skos:prefLabel>
    <skos:definition xml:lang="en">The document is incomplete as a time series for meter data is missing.</skos:definition>
  </skos:Concept>
  <skos:Concept rdf:about="http://energy.referencedata.eu/StandardReasonCodeTypeList/B04">
    <skos:inScheme rdf:resource="http://energy.referencedata.eu/StandardReasonCodeTypeList"/>
    <skos:topConceptOf rdf:resource="http://energy.referencedata.eu/StandardReasonCodeTypeList"/>
    <dcterms:identifier>B04</dcterms:identifier>
    <skos:prefLabel>Estimated values not allowed in first transmission</skos:prefLabel>
    <skos:definition xml:lang="en">The document is in its initial form and estimated values are not allowed.</skos:definition>
  </skos:Concept>
  <skos:Concept rdf:about="http://energy.referencedata.eu/StandardReasonCodeTypeList/B05">
    <skos:inScheme rdf:resource="http://energy.referencedata.eu/StandardReasonCodeTypeList"/>
    <skos:topConceptOf rdf:resource="http://energy.referencedata.eu/StandardReasonCodeTypeList"/>
    <dcterms:identifier>B05</dcterms:identifier>
    <skos:prefLabel>No quantity values allowed for a quality that is not available</skos:prefLabel>
    <skos:definition xml:lang="en">No quantity values are allowed for a quality that is not available.</skos:definition>
  </skos:Concept>
  <skos:Concept rdf:about="http://energy.referencedata.eu/StandardReasonCodeTypeList/B06">
    <skos:inScheme rdf:resource="http://energy.referencedata.eu/StandardReasonCodeTypeList"/>
    <skos:topConceptOf rdf:resource="http://energy.referencedata.eu/StandardReasonCodeTypeList"/>
    <dcterms:identifier>B06</dcterms:identifier>
    <skos:prefLabel>Time series accepted</skos:prefLabel>
    <skos:definition xml:lang="en">Time series accepted.</skos:definition>
  </skos:Concept>
  <skos:Concept rdf:about="http://energy.referencedata.eu/StandardReasonCodeTypeList/B07">
    <skos:inScheme rdf:resource="http://energy.referencedata.eu/StandardReasonCodeTypeList"/>
    <skos:topConceptOf rdf:resource="http://energy.referencedata.eu/StandardReasonCodeTypeList"/>
    <dcterms:identifier>B07</dcterms:identifier>
    <skos:prefLabel>Auction without bids being entered</skos:prefLabel>
    <skos:definition xml:lang="en">The auction has terminated without any bids being submitted. The ReasonText may provide the identification of the auction in question.</skos:definition>
  </skos:Concept>
  <skos:Concept rdf:about="http://energy.referencedata.eu/StandardReasonCodeTypeList/B08">
    <skos:inScheme rdf:resource="http://energy.referencedata.eu/StandardReasonCodeTypeList"/>
    <skos:topConceptOf rdf:resource="http://energy.referencedata.eu/StandardReasonCodeTypeList"/>
    <dcterms:identifier>B08</dcterms:identifier>
    <skos:prefLabel>Data not yet available</skos:prefLabel>
    <skos:definition xml:lang="en">It is not possible to perform the necessary action since the required data for this action is not yet available.</skos:definition>
  </skos:Concept>
  <skos:Concept rdf:about="http://energy.referencedata.eu/StandardReasonCodeTypeList/B09">
    <skos:inScheme rdf:resource="http://energy.referencedata.eu/StandardReasonCodeTypeList"/>
    <skos:topConceptOf rdf:resource="http://energy.referencedata.eu/StandardReasonCodeTypeList"/>
    <dcterms:identifier>B09</dcterms:identifier>
    <skos:prefLabel>Bid not accepted</skos:prefLabel>
    <skos:definition xml:lang="en">The bid in question has not been accepted.</skos:definition>
  </skos:Concept>
  <skos:Concept rdf:about="http://energy.referencedata.eu/StandardReasonCodeTypeList/B10">
    <skos:inScheme rdf:resource="http://energy.referencedata.eu/StandardReasonCodeTypeList"/>
    <skos:topConceptOf rdf:resource="http://energy.referencedata.eu/StandardReasonCodeTypeList"/>
    <dcterms:identifier>B10</dcterms:identifier>
    <skos:prefLabel>Initiator area problem</skos:prefLabel>
    <skos:definition xml:lang="en">The problem concerns the initiator area.</skos:definition>
  </skos:Concept>
  <skos:Concept rdf:about="http://energy.referencedata.eu/StandardReasonCodeTypeList/B11">
    <skos:inScheme rdf:resource="http://energy.referencedata.eu/StandardReasonCodeTypeList"/>
    <skos:topConceptOf rdf:resource="http://energy.referencedata.eu/StandardReasonCodeTypeList"/>
    <dcterms:identifier>B11</dcterms:identifier>
    <skos:prefLabel>Cooperating area problem</skos:prefLabel>
    <skos:definition xml:lang="en">The problem concerns the cooperating area.</skos:definition>
  </skos:Concept>
  <skos:Concept rdf:about="http://energy.referencedata.eu/StandardReasonCodeTypeList/B12">
    <skos:inScheme rdf:resource="http://energy.referencedata.eu/StandardReasonCodeTypeList"/>
    <skos:topConceptOf rdf:resource="http://energy.referencedata.eu/StandardReasonCodeTypeList"/>
    <dcterms:identifier>B12</dcterms:identifier>
    <skos:prefLabel>Communication status currently active</skos:prefLabel>
    <skos:definition xml:lang="en">The status within the system indicates that the communication capability is currently active.</skos:definition>
  </skos:Concept>
  <skos:Concept rdf:about="http://energy.referencedata.eu/StandardReasonCodeTypeList/B13">
    <skos:inScheme rdf:resource="http://energy.referencedata.eu/StandardReasonCodeTypeList"/>
    <skos:topConceptOf rdf:resource="http://energy.referencedata.eu/StandardReasonCodeTypeList"/>
    <dcterms:identifier>B13</dcterms:identifier>
    <skos:prefLabel>Communication status currently inactive</skos:prefLabel>
    <skos:definition xml:lang="en">The status within the system indicates that the communication capability is currently inactive.</skos:definition>
  </skos:Concept>
  <skos:Concept rdf:about="http://energy.referencedata.eu/StandardReasonCodeTypeList/B14">
    <skos:inScheme rdf:resource="http://energy.referencedata.eu/StandardReasonCodeTypeList"/>
    <skos:topConceptOf rdf:resource="http://energy.referencedata.eu/StandardReasonCodeTypeList"/>
    <dcterms:identifier>B14</dcterms:identifier>
    <skos:prefLabel>Communication status currently restricted</skos:prefLabel>
    <skos:definition xml:lang="en">The status within the system indicates that the communication capability is currently restricted.</skos:definition>
  </skos:Concept>
  <skos:Concept rdf:about="http://energy.referencedata.eu/StandardReasonCodeTypeList/B15">
    <skos:inScheme rdf:resource="http://energy.referencedata.eu/StandardReasonCodeTypeList"/>
    <skos:topConceptOf rdf:resource="http://energy.referencedata.eu/StandardReasonCodeTypeList"/>
    <dcterms:identifier>B15</dcterms:identifier>
    <skos:prefLabel>Problem associated with both areas</skos:prefLabel>
    <skos:definition xml:lang="en">The problem concerns both areas.</skos:definition>
  </skos:Concept>
  <skos:Concept rdf:about="http://energy.referencedata.eu/StandardReasonCodeTypeList/B16">
    <skos:inScheme rdf:resource="http://energy.referencedata.eu/StandardReasonCodeTypeList"/>
    <skos:topConceptOf rdf:resource="http://energy.referencedata.eu/StandardReasonCodeTypeList"/>
    <dcterms:identifier>B16</dcterms:identifier>
    <skos:prefLabel>Tender unavailable in MOL list</skos:prefLabel>
    <skos:definition xml:lang="en">A tender that has been requested is no longer available in the MOL.</skos:definition>
  </skos:Concept>
  <skos:Concept rdf:about="http://energy.referencedata.eu/StandardReasonCodeTypeList/B17">
    <skos:inScheme rdf:resource="http://energy.referencedata.eu/StandardReasonCodeTypeList"/>
    <skos:topConceptOf rdf:resource="http://energy.referencedata.eu/StandardReasonCodeTypeList"/>
    <dcterms:identifier>B17</dcterms:identifier>
    <skos:prefLabel>Price based on preliminary exchange rate</skos:prefLabel>
    <skos:definition xml:lang="en">The price is based on a preliminary exchange rate.</skos:definition>
  </skos:Concept>
  <skos:Concept rdf:about="http://energy.referencedata.eu/StandardReasonCodeTypeList/B18">
    <skos:inScheme rdf:resource="http://energy.referencedata.eu/StandardReasonCodeTypeList"/>
    <skos:topConceptOf rdf:resource="http://energy.referencedata.eu/StandardReasonCodeTypeList"/>
    <dcterms:identifier>B18</dcterms:identifier>
    <skos:prefLabel>Failure</skos:prefLabel>
    <skos:definition xml:lang="en">A failure has occurred.</skos:definition>
  </skos:Concept>
  <skos:Concept rdf:about="http://energy.referencedata.eu/StandardReasonCodeTypeList/B19">
    <skos:inScheme rdf:resource="http://energy.referencedata.eu/StandardReasonCodeTypeList"/>
    <skos:topConceptOf rdf:resource="http://energy.referencedata.eu/StandardReasonCodeTypeList"/>
    <dcterms:identifier>B19</dcterms:identifier>
    <skos:prefLabel>Foreseen maintenance</skos:prefLabel>
    <skos:definition xml:lang="en">Maintenance is foreseen.</skos:definition>
  </skos:Concept>
  <skos:Concept rdf:about="http://energy.referencedata.eu/StandardReasonCodeTypeList/B20">
    <skos:inScheme rdf:resource="http://energy.referencedata.eu/StandardReasonCodeTypeList"/>
    <skos:topConceptOf rdf:resource="http://energy.referencedata.eu/StandardReasonCodeTypeList"/>
    <dcterms:identifier>B20</dcterms:identifier>
    <skos:prefLabel>Shutdown</skos:prefLabel>
    <skos:definition xml:lang="en">A shutdown has occurred.</skos:definition>
  </skos:Concept>
  <skos:Concept rdf:about="http://energy.referencedata.eu/StandardReasonCodeTypeList/B21">
    <skos:inScheme rdf:resource="http://energy.referencedata.eu/StandardReasonCodeTypeList"/>
    <skos:topConceptOf rdf:resource="http://energy.referencedata.eu/StandardReasonCodeTypeList"/>
    <dcterms:identifier>B21</dcterms:identifier>
    <skos:prefLabel>Official exchange rate approved</skos:prefLabel>
    <skos:definition xml:lang="en">The official exchange rate has been approved.</skos:definition>
  </skos:Concept>
  <skos:Concept rdf:about="http://energy.referencedata.eu/StandardReasonCodeTypeList/B22">
    <skos:inScheme rdf:resource="http://energy.referencedata.eu/StandardReasonCodeTypeList"/>
    <skos:topConceptOf rdf:resource="http://energy.referencedata.eu/StandardReasonCodeTypeList"/>
    <dcterms:identifier>B22</dcterms:identifier>
    <skos:prefLabel>System regulation</skos:prefLabel>
    <skos:definition xml:lang="en">The information provided regards a regulation for system purposes.</skos:definition>
  </skos:Concept>
  <skos:Concept rdf:about="http://energy.referencedata.eu/StandardReasonCodeTypeList/B23">
    <skos:inScheme rdf:resource="http://energy.referencedata.eu/StandardReasonCodeTypeList"/>
    <skos:topConceptOf rdf:resource="http://energy.referencedata.eu/StandardReasonCodeTypeList"/>
    <dcterms:identifier>B23</dcterms:identifier>
    <skos:prefLabel>Frequency regulation</skos:prefLabel>
    <skos:definition xml:lang="en">The information provided regards a regulation for frequency purposes.</skos:definition>
  </skos:Concept>
  <skos:Concept rdf:about="http://energy.referencedata.eu/StandardReasonCodeTypeList/B24">
    <skos:inScheme rdf:resource="http://energy.referencedata.eu/StandardReasonCodeTypeList"/>
    <skos:topConceptOf rdf:resource="http://energy.referencedata.eu/StandardReasonCodeTypeList"/>
    <dcterms:identifier>B24</dcterms:identifier>
    <skos:prefLabel>Load flow overload</skos:prefLabel>
    <skos:definition xml:lang="en">Situation in the grid, where loading of a certain grid element, e.g. overhead line, is above defined technical limits.</skos:definition>
  </skos:Concept>
  <skos:Concept rdf:about="http://energy.referencedata.eu/StandardReasonCodeTypeList/B25">
    <skos:inScheme rdf:resource="http://energy.referencedata.eu/StandardReasonCodeTypeList"/>
    <skos:topConceptOf rdf:resource="http://energy.referencedata.eu/StandardReasonCodeTypeList"/>
    <dcterms:identifier>B25</dcterms:identifier>
    <skos:prefLabel>Voltage level adjustment</skos:prefLabel>
    <skos:definition xml:lang="en">A TSO activity to maintain an acceptable voltage profile throughout the network. This is achieved by balancing of the respective reactive power requirements of the network and the customers.</skos:definition>
  </skos:Concept>
  <skos:Concept rdf:about="http://energy.referencedata.eu/StandardReasonCodeTypeList/B26">
    <skos:inScheme rdf:resource="http://energy.referencedata.eu/StandardReasonCodeTypeList"/>
    <skos:topConceptOf rdf:resource="http://energy.referencedata.eu/StandardReasonCodeTypeList"/>
    <dcterms:identifier>B26</dcterms:identifier>
    <skos:prefLabel>Emergency situation curtailment</skos:prefLabel>
    <skos:definition xml:lang="en">Curtailment due to emergency situation. A code that enables the identification of the curtailment reason for settlement purposes.</skos:definition>
  </skos:Concept>
  <skos:Concept rdf:about="http://energy.referencedata.eu/StandardReasonCodeTypeList/B27">
    <skos:inScheme rdf:resource="http://energy.referencedata.eu/StandardReasonCodeTypeList"/>
    <skos:topConceptOf rdf:resource="http://energy.referencedata.eu/StandardReasonCodeTypeList"/>
    <dcterms:identifier>B27</dcterms:identifier>
    <skos:prefLabel>Calculation process failed</skos:prefLabel>
    <skos:definition xml:lang="en">The calculation has not been performed.</skos:definition>
  </skos:Concept>
  <skos:Concept rdf:about="http://energy.referencedata.eu/StandardReasonCodeTypeList/B28">
    <skos:inScheme rdf:resource="http://energy.referencedata.eu/StandardReasonCodeTypeList"/>
    <skos:topConceptOf rdf:resource="http://energy.referencedata.eu/StandardReasonCodeTypeList"/>
    <dcterms:identifier>B28</dcterms:identifier>
    <skos:prefLabel>No capacity constraint impact on the market</skos:prefLabel>
    <skos:definition xml:lang="en">The market position is such as no capacity constraint is applied to limit the cross border exchanges.</skos:definition>
  </skos:Concept>
  <skos:Concept rdf:about="http://energy.referencedata.eu/StandardReasonCodeTypeList/B29">
    <skos:inScheme rdf:resource="http://energy.referencedata.eu/StandardReasonCodeTypeList"/>
    <skos:topConceptOf rdf:resource="http://energy.referencedata.eu/StandardReasonCodeTypeList"/>
    <dcterms:identifier>B29</dcterms:identifier>
    <skos:prefLabel>Special Condition</skos:prefLabel>
    <skos:definition xml:lang="en">Special condition need to be fulfilled.</skos:definition>
  </skos:Concept>
  <skos:Concept rdf:about="http://energy.referencedata.eu/StandardReasonCodeTypeList/B30">
    <skos:inScheme rdf:resource="http://energy.referencedata.eu/StandardReasonCodeTypeList"/>
    <skos:topConceptOf rdf:resource="http://energy.referencedata.eu/StandardReasonCodeTypeList"/>
    <dcterms:identifier>B30</dcterms:identifier>
    <skos:prefLabel>Unverified</skos:prefLabel>
    <skos:definition xml:lang="en">Missing or not validated data.</skos:definition>
  </skos:Concept>
  <skos:Concept rdf:about="http://energy.referencedata.eu/StandardReasonCodeTypeList/B31">
    <skos:inScheme rdf:resource="http://energy.referencedata.eu/StandardReasonCodeTypeList"/>
    <skos:topConceptOf rdf:resource="http://energy.referencedata.eu/StandardReasonCodeTypeList"/>
    <dcterms:identifier>B31</dcterms:identifier>
    <skos:prefLabel>Verified</skos:prefLabel>
    <skos:definition xml:lang="en">Data has successfully passed the verification process.</skos:definition>
  </skos:Concept>
  <skos:Concept rdf:about="http://energy.referencedata.eu/StandardReasonCodeTypeList/B32">
    <skos:inScheme rdf:resource="http://energy.referencedata.eu/StandardReasonCodeTypeList"/>
    <skos:topConceptOf rdf:resource="http://energy.referencedata.eu/StandardReasonCodeTypeList"/>
    <dcterms:identifier>B32</dcterms:identifier>
    <skos:prefLabel>CGM inconsistency</skos:prefLabel>
    <skos:definition xml:lang="en">Describes an element which was not found in the CGM.</skos:definition>
  </skos:Concept>
  <skos:Concept rdf:about="http://energy.referencedata.eu/StandardReasonCodeTypeList/B33">
    <skos:inScheme rdf:resource="http://energy.referencedata.eu/StandardReasonCodeTypeList"/>
    <skos:topConceptOf rdf:resource="http://energy.referencedata.eu/StandardReasonCodeTypeList"/>
    <dcterms:identifier>B33</dcterms:identifier>
    <skos:prefLabel>Network dictionary inconsistency</skos:prefLabel>
    <skos:definition xml:lang="en">Describes an element which was not found in the network dictionary.</skos:definition>
  </skos:Concept>
  <skos:Concept rdf:about="http://energy.referencedata.eu/StandardReasonCodeTypeList/B34">
    <skos:inScheme rdf:resource="http://energy.referencedata.eu/StandardReasonCodeTypeList"/>
    <skos:topConceptOf rdf:resource="http://energy.referencedata.eu/StandardReasonCodeTypeList"/>
    <dcterms:identifier>B34</dcterms:identifier>
    <skos:prefLabel>Capacity reduced by TSO</skos:prefLabel>
    <skos:definition xml:lang="en">Describes a capacity that was reduced by a TSO.</skos:definition>
  </skos:Concept>
  <skos:Concept rdf:about="http://energy.referencedata.eu/StandardReasonCodeTypeList/B35">
    <skos:inScheme rdf:resource="http://energy.referencedata.eu/StandardReasonCodeTypeList"/>
    <skos:topConceptOf rdf:resource="http://energy.referencedata.eu/StandardReasonCodeTypeList"/>
    <dcterms:identifier>B35</dcterms:identifier>
    <skos:prefLabel>Overload</skos:prefLabel>
    <skos:definition xml:lang="en">Describes an N-k or N state overload.</skos:definition>
  </skos:Concept>
  <skos:Concept rdf:about="http://energy.referencedata.eu/StandardReasonCodeTypeList/B36">
    <skos:inScheme rdf:resource="http://energy.referencedata.eu/StandardReasonCodeTypeList"/>
    <skos:topConceptOf rdf:resource="http://energy.referencedata.eu/StandardReasonCodeTypeList"/>
    <dcterms:identifier>B36</dcterms:identifier>
    <skos:prefLabel>GLSK limitation</skos:prefLabel>
    <skos:definition xml:lang="en">Describes a situation in which there is not enough power adjustment in the GLSK file to cover the capacity.</skos:definition>
  </skos:Concept>
  <skos:Concept rdf:about="http://energy.referencedata.eu/StandardReasonCodeTypeList/B37">
    <skos:inScheme rdf:resource="http://energy.referencedata.eu/StandardReasonCodeTypeList"/>
    <skos:topConceptOf rdf:resource="http://energy.referencedata.eu/StandardReasonCodeTypeList"/>
    <dcterms:identifier>B37</dcterms:identifier>
    <skos:prefLabel>Voltage constraint</skos:prefLabel>
    <skos:definition xml:lang="en">Describes an N-k or N state voltage violation.</skos:definition>
  </skos:Concept>
  <skos:Concept rdf:about="http://energy.referencedata.eu/StandardReasonCodeTypeList/B38">
    <skos:inScheme rdf:resource="http://energy.referencedata.eu/StandardReasonCodeTypeList"/>
    <skos:topConceptOf rdf:resource="http://energy.referencedata.eu/StandardReasonCodeTypeList"/>
    <dcterms:identifier>B38</dcterms:identifier>
    <skos:prefLabel>Angle constraint</skos:prefLabel>
    <skos:definition xml:lang="en">Describes an N-k or N state angle violation.</skos:definition>
  </skos:Concept>
  <skos:Concept rdf:about="http://energy.referencedata.eu/StandardReasonCodeTypeList/B39">
    <skos:inScheme rdf:resource="http://energy.referencedata.eu/StandardReasonCodeTypeList"/>
    <skos:topConceptOf rdf:resource="http://energy.referencedata.eu/StandardReasonCodeTypeList"/>
    <dcterms:identifier>B39</dcterms:identifier>
    <skos:prefLabel>Stability</skos:prefLabel>
    <skos:definition xml:lang="en">Describes a situation in which the dynamic behaviour of the network violated.</skos:definition>
  </skos:Concept>
  <skos:Concept rdf:about="http://energy.referencedata.eu/StandardReasonCodeTypeList/B40">
    <skos:inScheme rdf:resource="http://energy.referencedata.eu/StandardReasonCodeTypeList"/>
    <skos:topConceptOf rdf:resource="http://energy.referencedata.eu/StandardReasonCodeTypeList"/>
    <dcterms:identifier>B40</dcterms:identifier>
    <skos:prefLabel>Loadflow divergence</skos:prefLabel>
    <skos:definition xml:lang="en">Describes a network situation in which the provided capacity values are part of a load flow divergence situation.</skos:definition>
  </skos:Concept>
  <skos:Concept rdf:about="http://energy.referencedata.eu/StandardReasonCodeTypeList/B41">
    <skos:inScheme rdf:resource="http://energy.referencedata.eu/StandardReasonCodeTypeList"/>
    <skos:topConceptOf rdf:resource="http://energy.referencedata.eu/StandardReasonCodeTypeList"/>
    <dcterms:identifier>B41</dcterms:identifier>
    <skos:prefLabel>Exclusion for SoS reasons</skos:prefLabel>
    <skos:definition xml:lang="en">This is the adjustment applied to the capacity of a branch to have a minimum RAM (Remaining Available Margin) available for commercial exchanges.</skos:definition>
  </skos:Concept>
  <skos:Concept rdf:about="http://energy.referencedata.eu/StandardReasonCodeTypeList/B42">
    <skos:inScheme rdf:resource="http://energy.referencedata.eu/StandardReasonCodeTypeList"/>
    <skos:topConceptOf rdf:resource="http://energy.referencedata.eu/StandardReasonCodeTypeList"/>
    <dcterms:identifier>B42</dcterms:identifier>
    <skos:prefLabel>Constraint by the market</skos:prefLabel>
    <skos:definition xml:lang="en">A constraint due to market restrictions.</skos:definition>
  </skos:Concept>
  <skos:Concept rdf:about="http://energy.referencedata.eu/StandardReasonCodeTypeList/B43">
    <skos:inScheme rdf:resource="http://energy.referencedata.eu/StandardReasonCodeTypeList"/>
    <skos:topConceptOf rdf:resource="http://energy.referencedata.eu/StandardReasonCodeTypeList"/>
    <dcterms:identifier>B43</dcterms:identifier>
    <skos:prefLabel>Ordinary</skos:prefLabel>
    <skos:definition xml:lang="en">The contingency is ordinary (methodology for coordinating operational security analysis, article 6).</skos:definition>
  </skos:Concept>
  <skos:Concept rdf:about="http://energy.referencedata.eu/StandardReasonCodeTypeList/B44">
    <skos:inScheme rdf:resource="http://energy.referencedata.eu/StandardReasonCodeTypeList"/>
    <skos:topConceptOf rdf:resource="http://energy.referencedata.eu/StandardReasonCodeTypeList"/>
    <dcterms:identifier>B44</dcterms:identifier>
    <skos:prefLabel>Exceptional</skos:prefLabel>
    <skos:definition xml:lang="en">The contingency is exceptional (methodology for coordinating operational security analysis, article 6).</skos:definition>
  </skos:Concept>
  <skos:Concept rdf:about="http://energy.referencedata.eu/StandardReasonCodeTypeList/B45">
    <skos:inScheme rdf:resource="http://energy.referencedata.eu/StandardReasonCodeTypeList"/>
    <skos:topConceptOf rdf:resource="http://energy.referencedata.eu/StandardReasonCodeTypeList"/>
    <dcterms:identifier>B45</dcterms:identifier>
    <skos:prefLabel>Out of range</skos:prefLabel>
    <skos:definition xml:lang="en">The contingency is out of range (methodology for coordinating operational security analysis, article 6).</skos:definition>
  </skos:Concept>
  <skos:Concept rdf:about="http://energy.referencedata.eu/StandardReasonCodeTypeList/B46">
    <skos:inScheme rdf:resource="http://energy.referencedata.eu/StandardReasonCodeTypeList"/>
    <skos:topConceptOf rdf:resource="http://energy.referencedata.eu/StandardReasonCodeTypeList"/>
    <dcterms:identifier>B46</dcterms:identifier>
    <skos:prefLabel>Internal congestion</skos:prefLabel>
    <skos:definition xml:lang="en">A temporary congestion within a bidding zone or scheduling area.</skos:definition>
  </skos:Concept>
  <skos:Concept rdf:about="http://energy.referencedata.eu/StandardReasonCodeTypeList/B47">
    <skos:inScheme rdf:resource="http://energy.referencedata.eu/StandardReasonCodeTypeList"/>
    <skos:topConceptOf rdf:resource="http://energy.referencedata.eu/StandardReasonCodeTypeList"/>
    <dcterms:identifier>B47</dcterms:identifier>
    <skos:prefLabel>Operational security constraints</skos:prefLabel>
    <skos:definition xml:lang="en">Operational security constraints identified by TSOs.</skos:definition>
  </skos:Concept>
  <skos:Concept rdf:about="http://energy.referencedata.eu/StandardReasonCodeTypeList/B48">
    <skos:inScheme rdf:resource="http://energy.referencedata.eu/StandardReasonCodeTypeList"/>
    <skos:topConceptOf rdf:resource="http://energy.referencedata.eu/StandardReasonCodeTypeList"/>
    <dcterms:identifier>B48</dcterms:identifier>
    <skos:prefLabel>Estimated value</skos:prefLabel>
    <skos:definition xml:lang="en">Describes a situation where a calculation process has failed and extrapolated or interpolated values will be applied.</skos:definition>
  </skos:Concept>
  <skos:Concept rdf:about="http://energy.referencedata.eu/StandardReasonCodeTypeList/B49">
    <skos:inScheme rdf:resource="http://energy.referencedata.eu/StandardReasonCodeTypeList"/>
    <skos:topConceptOf rdf:resource="http://energy.referencedata.eu/StandardReasonCodeTypeList"/>
    <dcterms:identifier>B49</dcterms:identifier>
    <skos:prefLabel>Balancing</skos:prefLabel>
    <skos:definition xml:lang="en">Activated for balancing purposes.</skos:definition>
  </skos:Concept>
  <skos:Concept rdf:about="http://energy.referencedata.eu/StandardReasonCodeTypeList/B50">
    <skos:inScheme rdf:resource="http://energy.referencedata.eu/StandardReasonCodeTypeList"/>
    <skos:topConceptOf rdf:resource="http://energy.referencedata.eu/StandardReasonCodeTypeList"/>
    <dcterms:identifier>B50</dcterms:identifier>
    <skos:prefLabel>Values shared</skos:prefLabel>
    <skos:definition xml:lang="en">Values of this time series are also valid for counter-party.</skos:definition>
  </skos:Concept>
  <skos:Concept rdf:about="http://energy.referencedata.eu/StandardReasonCodeTypeList/B51">
    <skos:inScheme rdf:resource="http://energy.referencedata.eu/StandardReasonCodeTypeList"/>
    <skos:topConceptOf rdf:resource="http://energy.referencedata.eu/StandardReasonCodeTypeList"/>
    <dcterms:identifier>B51</dcterms:identifier>
    <skos:prefLabel>Outside price limits</skos:prefLabel>
    <skos:definition xml:lang="en">The offered price is not within the valid limits.</skos:definition>
  </skos:Concept>
  <skos:Concept rdf:about="http://energy.referencedata.eu/StandardReasonCodeTypeList/B52">
    <skos:inScheme rdf:resource="http://energy.referencedata.eu/StandardReasonCodeTypeList"/>
    <skos:topConceptOf rdf:resource="http://energy.referencedata.eu/StandardReasonCodeTypeList"/>
    <dcterms:identifier>B52</dcterms:identifier>
    <skos:prefLabel>Previous timeframe data</skos:prefLabel>
    <skos:definition xml:lang="en">In case of processing issue, sent data are based on the previous timeframe.</skos:definition>
  </skos:Concept>
  <skos:Concept rdf:about="http://energy.referencedata.eu/StandardReasonCodeTypeList/B53">
    <skos:inScheme rdf:resource="http://energy.referencedata.eu/StandardReasonCodeTypeList"/>
    <skos:topConceptOf rdf:resource="http://energy.referencedata.eu/StandardReasonCodeTypeList"/>
    <dcterms:identifier>B53</dcterms:identifier>
    <skos:prefLabel>MOL merging succesful</skos:prefLabel>
    <skos:definition xml:lang="en">The merging of the Merit Order List has been successfully processed.</skos:definition>
  </skos:Concept>
  <skos:Concept rdf:about="http://energy.referencedata.eu/StandardReasonCodeTypeList/B54">
    <skos:inScheme rdf:resource="http://energy.referencedata.eu/StandardReasonCodeTypeList"/>
    <skos:topConceptOf rdf:resource="http://energy.referencedata.eu/StandardReasonCodeTypeList"/>
    <dcterms:identifier>B54</dcterms:identifier>
    <skos:prefLabel>MOL merging failed</skos:prefLabel>
    <skos:definition xml:lang="en">The merging of the Merit Order List has failed.</skos:definition>
  </skos:Concept>
  <skos:Concept rdf:about="http://energy.referencedata.eu/StandardReasonCodeTypeList/B55">
    <skos:inScheme rdf:resource="http://energy.referencedata.eu/StandardReasonCodeTypeList"/>
    <skos:topConceptOf rdf:resource="http://energy.referencedata.eu/StandardReasonCodeTypeList"/>
    <dcterms:identifier>B55</dcterms:identifier>
    <skos:prefLabel>Because of redispatching</skos:prefLabel>
    <skos:definition xml:lang="en">Because of redispatching according to Article 2(26) of Commission Regulation (EU) 543/2013</skos:definition>
  </skos:Concept>
  <skos:Concept rdf:about="http://energy.referencedata.eu/StandardReasonCodeTypeList/B56">
    <skos:inScheme rdf:resource="http://energy.referencedata.eu/StandardReasonCodeTypeList"/>
    <skos:topConceptOf rdf:resource="http://energy.referencedata.eu/StandardReasonCodeTypeList"/>
    <dcterms:identifier>B56</dcterms:identifier>
    <skos:prefLabel>Because of countertrading</skos:prefLabel>
    <skos:definition xml:lang="en">Because of countertrading according to Article 2(13) of Commission Regulation (EU) 543/2013</skos:definition>
  </skos:Concept>
  <skos:Concept rdf:about="http://energy.referencedata.eu/StandardReasonCodeTypeList/B57">
    <skos:inScheme rdf:resource="http://energy.referencedata.eu/StandardReasonCodeTypeList"/>
    <skos:topConceptOf rdf:resource="http://energy.referencedata.eu/StandardReasonCodeTypeList"/>
    <dcterms:identifier>B57</dcterms:identifier>
    <skos:prefLabel>Because of other remedial action</skos:prefLabel>
    <skos:definition xml:lang="en">Not available because of any remedial action.</skos:definition>
  </skos:Concept>
  <skos:Concept rdf:about="http://energy.referencedata.eu/StandardReasonCodeTypeList/B58">
    <skos:inScheme rdf:resource="http://energy.referencedata.eu/StandardReasonCodeTypeList"/>
    <skos:topConceptOf rdf:resource="http://energy.referencedata.eu/StandardReasonCodeTypeList"/>
    <dcterms:identifier>B58</dcterms:identifier>
    <skos:prefLabel>Insufficiency of reserves</skos:prefLabel>
    <skos:definition xml:lang="en">The reserve capacity is not sufficient.</skos:definition>
  </skos:Concept>
  <skos:Concept rdf:about="http://energy.referencedata.eu/StandardReasonCodeTypeList/B59">
    <skos:inScheme rdf:resource="http://energy.referencedata.eu/StandardReasonCodeTypeList"/>
    <skos:topConceptOf rdf:resource="http://energy.referencedata.eu/StandardReasonCodeTypeList"/>
    <dcterms:identifier>B59</dcterms:identifier>
    <skos:prefLabel>Unavailability of reserve providing unit</skos:prefLabel>
    <skos:definition xml:lang="en">The unit providing the reserve is subject to technical unavailability.</skos:definition>
  </skos:Concept>
  <skos:Concept rdf:about="http://energy.referencedata.eu/StandardReasonCodeTypeList/B60">
    <skos:inScheme rdf:resource="http://energy.referencedata.eu/StandardReasonCodeTypeList"/>
    <skos:topConceptOf rdf:resource="http://energy.referencedata.eu/StandardReasonCodeTypeList"/>
    <dcterms:identifier>B60</dcterms:identifier>
    <skos:prefLabel>Unavailability of automatic protection systems</skos:prefLabel>
    <skos:definition xml:lang="en">Unavailability of tools to detect predetermined system conditions that have a high probability of causing unusual stress on the power system, for which pre-planned remedial action is considered necessary or for which automatic protective actions may be triggered such as special protection schemes or automatic load shedding.</skos:definition>
  </skos:Concept>
  <skos:Concept rdf:about="http://energy.referencedata.eu/StandardReasonCodeTypeList/B61">
    <skos:inScheme rdf:resource="http://energy.referencedata.eu/StandardReasonCodeTypeList"/>
    <skos:topConceptOf rdf:resource="http://energy.referencedata.eu/StandardReasonCodeTypeList"/>
    <dcterms:identifier>B61</dcterms:identifier>
    <skos:prefLabel>Physical cable or converter restrictions</skos:prefLabel>
    <skos:definition xml:lang="en">Limitation due to physical cable or converter restrictions.</skos:definition>
  </skos:Concept>
  <skos:Concept rdf:about="http://energy.referencedata.eu/StandardReasonCodeTypeList/B62">
    <skos:inScheme rdf:resource="http://energy.referencedata.eu/StandardReasonCodeTypeList"/>
    <skos:topConceptOf rdf:resource="http://energy.referencedata.eu/StandardReasonCodeTypeList"/>
    <dcterms:identifier>B62</dcterms:identifier>
    <skos:prefLabel>Constraints in controller systems</skos:prefLabel>
    <skos:definition xml:lang="en">Limitation due to constraints in controller systems.</skos:definition>
  </skos:Concept>
  <skos:Concept rdf:about="http://energy.referencedata.eu/StandardReasonCodeTypeList/B63">
    <skos:inScheme rdf:resource="http://energy.referencedata.eu/StandardReasonCodeTypeList"/>
    <skos:topConceptOf rdf:resource="http://energy.referencedata.eu/StandardReasonCodeTypeList"/>
    <dcterms:identifier>B63</dcterms:identifier>
    <skos:prefLabel>Adjusted because of expected violation of operational security</skos:prefLabel>
    <skos:definition xml:lang="en">The capacity is adjusted because of an expected violation of operational security limits of physical transmission assets.</skos:definition>
  </skos:Concept>
  <skos:Concept rdf:about="http://energy.referencedata.eu/StandardReasonCodeTypeList/B64">
    <skos:inScheme rdf:resource="http://energy.referencedata.eu/StandardReasonCodeTypeList"/>
    <skos:topConceptOf rdf:resource="http://energy.referencedata.eu/StandardReasonCodeTypeList"/>
    <dcterms:identifier>B64</dcterms:identifier>
    <skos:prefLabel>Adjusted because already considered remedial actions are assessed as not sufficient</skos:prefLabel>
    <skos:definition xml:lang="en">The capacity is adjusted because the remedial actions were assessed as not sufficient or ineffective to avoid the expected violation of operational security limit(s).</skos:definition>
  </skos:Concept>
  <skos:Concept rdf:about="http://energy.referencedata.eu/StandardReasonCodeTypeList/B65">
    <skos:inScheme rdf:resource="http://energy.referencedata.eu/StandardReasonCodeTypeList"/>
    <skos:topConceptOf rdf:resource="http://energy.referencedata.eu/StandardReasonCodeTypeList"/>
    <dcterms:identifier>B65</dcterms:identifier>
    <skos:prefLabel>Time series partially accepted</skos:prefLabel>
    <skos:definition xml:lang="en">The time series is partially accepted.</skos:definition>
  </skos:Concept>
  <skos:Concept rdf:about="http://energy.referencedata.eu/StandardReasonCodeTypeList/B66">
    <skos:inScheme rdf:resource="http://energy.referencedata.eu/StandardReasonCodeTypeList"/>
    <skos:topConceptOf rdf:resource="http://energy.referencedata.eu/StandardReasonCodeTypeList"/>
    <dcterms:identifier>B66</dcterms:identifier>
    <skos:prefLabel>Demand fully netted</skos:prefLabel>
    <skos:definition xml:lang="en">Demand was fully netted against other demand(s).</skos:definition>
  </skos:Concept>
  <skos:Concept rdf:about="http://energy.referencedata.eu/StandardReasonCodeTypeList/B67">
    <skos:inScheme rdf:resource="http://energy.referencedata.eu/StandardReasonCodeTypeList"/>
    <skos:topConceptOf rdf:resource="http://energy.referencedata.eu/StandardReasonCodeTypeList"/>
    <dcterms:identifier>B67</dcterms:identifier>
    <skos:prefLabel>Bid activated in same direction</skos:prefLabel>
    <skos:definition xml:lang="en">One or several bids were activated in the same direction within the same uncongested area as the demand.</skos:definition>
  </skos:Concept>
</rdf:RDF>
