<?xml version='1.0' encoding='UTF-8'?>
<rdf:RDF xmlns:cim="http://iec.ch/TC57/2013/CIM-schema-cim16#" xmlns:rdf="http://www.w3.org/1999/02/22-rdf-syntax-ns#" xmlns:rdfs="http://www.w3.org/2000/01/rdf-schema#" xmlns:dcat="http://www.w3.org/ns/dcat#" xmlns:dc="http://purl.org/dc/elements/1.1/" xmlns:dcterms="http://purl.org/dc/terms/" xmlns:skos="http://www.w3.org/2004/02/skos/core#" xmlns:ecl="urn:entsoe.eu:wgedi:codelists" xmlns:xs="http://www.w3.org/2001/XMLSchema">
  <skos:ConceptScheme rdf:about="http://energy.referencedata.eu/StandardPriceComponentTypeList">
    <rdf:type rdf:resource="http://www.w3.org/ns/dcat#Dataset"/>
    <dcterms:modified>2023-12-14</dcterms:modified>
    <dcat:version>91</dcat:version>
    <skos:prefLabel>StandardPriceComponentTypeList</skos:prefLabel>
    <dcterms:identifier>ET0052</dcterms:identifier>
    <skos:definition xml:lang="en">Indicates the component type for  a price.</skos:definition>
  </skos:ConceptScheme>
  <skos:Concept rdf:about="http://energy.referencedata.eu/StandardPriceComponentTypeList/A01">
    <skos:inScheme rdf:resource="http://energy.referencedata.eu/StandardPriceComponentTypeList"/>
    <skos:topConceptOf rdf:resource="http://energy.referencedata.eu/StandardPriceComponentTypeList"/>
    <dcterms:identifier>A01</dcterms:identifier>
    <skos:prefLabel>Scarcity</skos:prefLabel>
    <skos:definition xml:lang="en">A scarcity component to be used in nationally defined scarcity situations.</skos:definition>
  </skos:Concept>
  <skos:Concept rdf:about="http://energy.referencedata.eu/StandardPriceComponentTypeList/A02">
    <skos:inScheme rdf:resource="http://energy.referencedata.eu/StandardPriceComponentTypeList"/>
    <skos:topConceptOf rdf:resource="http://energy.referencedata.eu/StandardPriceComponentTypeList"/>
    <dcterms:identifier>A02</dcterms:identifier>
    <skos:prefLabel>Incentive</skos:prefLabel>
    <skos:definition xml:lang="en">An incentive component to be used to fulfil nationally defined boundary conditions.</skos:definition>
  </skos:Concept>
  <skos:Concept rdf:about="http://energy.referencedata.eu/StandardPriceComponentTypeList/A03">
    <skos:inScheme rdf:resource="http://energy.referencedata.eu/StandardPriceComponentTypeList"/>
    <skos:topConceptOf rdf:resource="http://energy.referencedata.eu/StandardPriceComponentTypeList"/>
    <dcterms:identifier>A03</dcterms:identifier>
    <skos:prefLabel>Financial neutrality</skos:prefLabel>
    <skos:definition xml:lang="en">A component related to the financial neutrality of the connecting TSO.</skos:definition>
  </skos:Concept>
</rdf:RDF>
