<?xml version='1.0' encoding='UTF-8'?>
<rdf:RDF xmlns:cim="http://iec.ch/TC57/2013/CIM-schema-cim16#" xmlns:rdf="http://www.w3.org/1999/02/22-rdf-syntax-ns#" xmlns:rdfs="http://www.w3.org/2000/01/rdf-schema#" xmlns:dcat="http://www.w3.org/ns/dcat#" xmlns:dc="http://purl.org/dc/elements/1.1/" xmlns:dcterms="http://purl.org/dc/terms/" xmlns:skos="http://www.w3.org/2004/02/skos/core#" xmlns:ecl="urn:entsoe.eu:wgedi:codelists" xmlns:xs="http://www.w3.org/2001/XMLSchema">
  <skos:ConceptScheme rdf:about="http://energy.referencedata.eu/StandardEnergyProductTypeList">
    <rdf:type rdf:resource="http://www.w3.org/ns/dcat#Dataset"/>
    <dcterms:modified>2022-03-31</dcterms:modified>
    <dcat:version>81</dcat:version>
    <skos:prefLabel>StandardEnergyProductTypeList</skos:prefLabel>
    <dcterms:identifier>ET0008</dcterms:identifier>
    <skos:definition xml:lang="en">The identification of the nature of an energy product such as power, energy, reactive power, etc.</skos:definition>
  </skos:ConceptScheme>
  <skos:Concept rdf:about="http://energy.referencedata.eu/StandardEnergyProductTypeList/8716867000016">
    <skos:inScheme rdf:resource="http://energy.referencedata.eu/StandardEnergyProductTypeList"/>
    <skos:topConceptOf rdf:resource="http://energy.referencedata.eu/StandardEnergyProductTypeList"/>
    <dcterms:identifier>8716867000016</dcterms:identifier>
    <skos:prefLabel>Active power</skos:prefLabel>
    <skos:definition xml:lang="en">The product of voltage and the in-phase component of alternating current measured in units of watts and standard multiples thereof.</skos:definition>
  </skos:Concept>
  <skos:Concept rdf:about="http://energy.referencedata.eu/StandardEnergyProductTypeList/8716867000023">
    <skos:inScheme rdf:resource="http://energy.referencedata.eu/StandardEnergyProductTypeList"/>
    <skos:topConceptOf rdf:resource="http://energy.referencedata.eu/StandardEnergyProductTypeList"/>
    <dcterms:identifier>8716867000023</dcterms:identifier>
    <skos:prefLabel>Reactive power</skos:prefLabel>
    <skos:definition xml:lang="en">The product of voltage and current and the sine of the phase angle between them, measured in units of voltamperes reactive and standard multiples thereof. (not used for planned schedules).</skos:definition>
  </skos:Concept>
  <skos:Concept rdf:about="http://energy.referencedata.eu/StandardEnergyProductTypeList/8716867000030">
    <skos:inScheme rdf:resource="http://energy.referencedata.eu/StandardEnergyProductTypeList"/>
    <skos:topConceptOf rdf:resource="http://energy.referencedata.eu/StandardEnergyProductTypeList"/>
    <dcterms:identifier>8716867000030</dcterms:identifier>
    <skos:prefLabel>Active energy</skos:prefLabel>
    <skos:definition xml:lang="en">The electrical energy produced, flowing or supplied by an electrical circuit during a time interval, being the integral with respect to time of instantaneous active power, measured in units of watt-hours, or standard multiples thereof.</skos:definition>
  </skos:Concept>
  <skos:Concept rdf:about="http://energy.referencedata.eu/StandardEnergyProductTypeList/8716867000047">
    <skos:inScheme rdf:resource="http://energy.referencedata.eu/StandardEnergyProductTypeList"/>
    <skos:topConceptOf rdf:resource="http://energy.referencedata.eu/StandardEnergyProductTypeList"/>
    <dcterms:identifier>8716867000047</dcterms:identifier>
    <skos:prefLabel>Reactive energy</skos:prefLabel>
    <skos:definition xml:lang="en">The integral with respect to time of reactive power (not used for planned schedules).</skos:definition>
  </skos:Concept>
  <skos:Concept rdf:about="http://energy.referencedata.eu/StandardEnergyProductTypeList/8716867000115">
    <skos:inScheme rdf:resource="http://energy.referencedata.eu/StandardEnergyProductTypeList"/>
    <skos:topConceptOf rdf:resource="http://energy.referencedata.eu/StandardEnergyProductTypeList"/>
    <dcterms:identifier>8716867000115</dcterms:identifier>
    <skos:prefLabel>Capacitive reactive power</skos:prefLabel>
    <skos:definition xml:lang="en">Capacitive reactive power.</skos:definition>
  </skos:Concept>
  <skos:Concept rdf:about="http://energy.referencedata.eu/StandardEnergyProductTypeList/8716867000122">
    <skos:inScheme rdf:resource="http://energy.referencedata.eu/StandardEnergyProductTypeList"/>
    <skos:topConceptOf rdf:resource="http://energy.referencedata.eu/StandardEnergyProductTypeList"/>
    <dcterms:identifier>8716867000122</dcterms:identifier>
    <skos:prefLabel>Inductive reactive power</skos:prefLabel>
    <skos:definition xml:lang="en">Inductive reactive power.</skos:definition>
  </skos:Concept>
  <skos:Concept rdf:about="http://energy.referencedata.eu/StandardEnergyProductTypeList/8716867000139">
    <skos:inScheme rdf:resource="http://energy.referencedata.eu/StandardEnergyProductTypeList"/>
    <skos:topConceptOf rdf:resource="http://energy.referencedata.eu/StandardEnergyProductTypeList"/>
    <dcterms:identifier>8716867000139</dcterms:identifier>
    <skos:prefLabel>Capacitive Reactive energy</skos:prefLabel>
    <skos:definition xml:lang="en">Capacitive reactive energy.</skos:definition>
  </skos:Concept>
  <skos:Concept rdf:about="http://energy.referencedata.eu/StandardEnergyProductTypeList/8716867000146">
    <skos:inScheme rdf:resource="http://energy.referencedata.eu/StandardEnergyProductTypeList"/>
    <skos:topConceptOf rdf:resource="http://energy.referencedata.eu/StandardEnergyProductTypeList"/>
    <dcterms:identifier>8716867000146</dcterms:identifier>
    <skos:prefLabel>Inductive Reactive energy</skos:prefLabel>
    <skos:definition xml:lang="en">Inductive reactive energy.</skos:definition>
  </skos:Concept>
  <skos:Concept rdf:about="http://energy.referencedata.eu/StandardEnergyProductTypeList/8716867009911">
    <skos:inScheme rdf:resource="http://energy.referencedata.eu/StandardEnergyProductTypeList"/>
    <skos:topConceptOf rdf:resource="http://energy.referencedata.eu/StandardEnergyProductTypeList"/>
    <dcterms:identifier>8716867009911</dcterms:identifier>
    <skos:prefLabel>Water</skos:prefLabel>
    <skos:definition xml:lang="en">For hydro power stations, this enables the identification of the quantity of water stored behind a dam (volume, head level, etc.), or the constraints in the flow of water.</skos:definition>
  </skos:Concept>
</rdf:RDF>
