<?xml version='1.0' encoding='UTF-8'?>
<rdf:RDF xmlns:cim="http://iec.ch/TC57/2013/CIM-schema-cim16#" xmlns:rdf="http://www.w3.org/1999/02/22-rdf-syntax-ns#" xmlns:rdfs="http://www.w3.org/2000/01/rdf-schema#" xmlns:dcat="http://www.w3.org/ns/dcat#" xmlns:dc="http://purl.org/dc/elements/1.1/" xmlns:dcterms="http://purl.org/dc/terms/" xmlns:skos="http://www.w3.org/2004/02/skos/core#" xmlns:ecl="urn:entsoe.eu:wgedi:codelists" xmlns:xs="http://www.w3.org/2001/XMLSchema">
  <skos:ConceptScheme rdf:about="http://energy.referencedata.eu/StandardQualityTypeList">
    <dcterms:modified>2022-03-31</dcterms:modified>
    <dcat:version>81</dcat:version>
    <skos:prefLabel>StandardQualityTypeList</skos:prefLabel>
    <dcterms:identifier>ET0036</dcterms:identifier>
    <skos:definition xml:lang="en">The quality of an object.</skos:definition>
  </skos:ConceptScheme>
  <skos:Concept rdf:about="http://energy.referencedata.eu/StandardQualityTypeList/A01">
    <skos:inScheme rdf:resource="http://energy.referencedata.eu/StandardQualityTypeList"/>
    <skos:topConceptOf rdf:resource="http://energy.referencedata.eu/StandardQualityTypeList"/>
    <dcterms:identifier>A01</dcterms:identifier>
    <skos:prefLabel>Adjusted</skos:prefLabel>
    <skos:definition xml:lang="en">The contents of the object have been adjusted.</skos:definition>
  </skos:Concept>
  <skos:Concept rdf:about="http://energy.referencedata.eu/StandardQualityTypeList/A02">
    <skos:inScheme rdf:resource="http://energy.referencedata.eu/StandardQualityTypeList"/>
    <skos:topConceptOf rdf:resource="http://energy.referencedata.eu/StandardQualityTypeList"/>
    <dcterms:identifier>A02</dcterms:identifier>
    <skos:prefLabel>Not available</skos:prefLabel>
    <skos:definition xml:lang="en">The contents of the object are not available.</skos:definition>
  </skos:Concept>
  <skos:Concept rdf:about="http://energy.referencedata.eu/StandardQualityTypeList/A03">
    <skos:inScheme rdf:resource="http://energy.referencedata.eu/StandardQualityTypeList"/>
    <skos:topConceptOf rdf:resource="http://energy.referencedata.eu/StandardQualityTypeList"/>
    <dcterms:identifier>A03</dcterms:identifier>
    <skos:prefLabel>Estimated</skos:prefLabel>
    <skos:definition xml:lang="en">The contents of the object are estimated. The code is typically used when measured values are missing and an estimate is made based on historical data. </skos:definition>
  </skos:Concept>
  <skos:Concept rdf:about="http://energy.referencedata.eu/StandardQualityTypeList/A04">
    <skos:inScheme rdf:resource="http://energy.referencedata.eu/StandardQualityTypeList"/>
    <skos:topConceptOf rdf:resource="http://energy.referencedata.eu/StandardQualityTypeList"/>
    <dcterms:identifier>A04</dcterms:identifier>
    <skos:prefLabel>As provided</skos:prefLabel>
    <skos:definition xml:lang="en">The contents of the object are as provided.</skos:definition>
  </skos:Concept>
  <skos:Concept rdf:about="http://energy.referencedata.eu/StandardQualityTypeList/A05">
    <skos:inScheme rdf:resource="http://energy.referencedata.eu/StandardQualityTypeList"/>
    <skos:topConceptOf rdf:resource="http://energy.referencedata.eu/StandardQualityTypeList"/>
    <dcterms:identifier>A05</dcterms:identifier>
    <skos:prefLabel>Incomplete</skos:prefLabel>
    <skos:definition xml:lang="en">The contents of the object are calculated based on incomplete data.</skos:definition>
  </skos:Concept>
  <skos:Concept rdf:about="http://energy.referencedata.eu/StandardQualityTypeList/A06">
    <skos:inScheme rdf:resource="http://energy.referencedata.eu/StandardQualityTypeList"/>
    <skos:topConceptOf rdf:resource="http://energy.referencedata.eu/StandardQualityTypeList"/>
    <dcterms:identifier>A06</dcterms:identifier>
    <skos:prefLabel>Calculated</skos:prefLabel>
    <skos:definition xml:lang="en">The contents of the object are calculated. The code is typically used when a value is calculated based on several other known values.</skos:definition>
  </skos:Concept>
</rdf:RDF>
