<?xml version='1.0' encoding='UTF-8'?>
<rdf:RDF xmlns:cim="http://iec.ch/TC57/2013/CIM-schema-cim16#" xmlns:rdf="http://www.w3.org/1999/02/22-rdf-syntax-ns#" xmlns:rdfs="http://www.w3.org/2000/01/rdf-schema#" xmlns:dcat="http://www.w3.org/ns/dcat#" xmlns:dc="http://purl.org/dc/elements/1.1/" xmlns:dcterms="http://purl.org/dc/terms/" xmlns:skos="http://www.w3.org/2004/02/skos/core#" xmlns:ecl="urn:entsoe.eu:wgedi:codelists" xmlns:xs="http://www.w3.org/2001/XMLSchema">
  <skos:ConceptScheme rdf:about="http://energy.referencedata.eu/StandardContractTypeList">
    <rdf:type rdf:resource="http://www.w3.org/ns/dcat#Dataset"/>
    <dcterms:modified>2022-08-26</dcterms:modified>
    <dcat:version>83</dcat:version>
    <skos:prefLabel>StandardContractTypeList</skos:prefLabel>
    <dcterms:identifier>ET0010</dcterms:identifier>
    <skos:definition xml:lang="en">The contract type defines the conditions under which the capacity is allocated and handled, e.g. daily auction, weekly auction, monthly auction, yearly auction, etc.
The significance of this type is dependent on area specific coded working methods.</skos:definition>
  </skos:ConceptScheme>
  <skos:Concept rdf:about="http://energy.referencedata.eu/StandardContractTypeList/A01">
    <skos:inScheme rdf:resource="http://energy.referencedata.eu/StandardContractTypeList"/>
    <skos:topConceptOf rdf:resource="http://energy.referencedata.eu/StandardContractTypeList"/>
    <dcterms:identifier>A01</dcterms:identifier>
    <skos:prefLabel>Daily</skos:prefLabel>
    <skos:definition xml:lang="en">The condition under which capacity is allocated and handled is by daily auction or a daily transmission allocation procedure.</skos:definition>
  </skos:Concept>
  <skos:Concept rdf:about="http://energy.referencedata.eu/StandardContractTypeList/A02">
    <skos:inScheme rdf:resource="http://energy.referencedata.eu/StandardContractTypeList"/>
    <skos:topConceptOf rdf:resource="http://energy.referencedata.eu/StandardContractTypeList"/>
    <dcterms:identifier>A02</dcterms:identifier>
    <skos:prefLabel>Weekly</skos:prefLabel>
    <skos:definition xml:lang="en">The condition under which capacity is allocated and handled is by weekly auction or a weekly transmission allocation procedure.</skos:definition>
  </skos:Concept>
  <skos:Concept rdf:about="http://energy.referencedata.eu/StandardContractTypeList/A03">
    <skos:inScheme rdf:resource="http://energy.referencedata.eu/StandardContractTypeList"/>
    <skos:topConceptOf rdf:resource="http://energy.referencedata.eu/StandardContractTypeList"/>
    <dcterms:identifier>A03</dcterms:identifier>
    <skos:prefLabel>Monthly</skos:prefLabel>
    <skos:definition xml:lang="en">The condition under which capacity is allocated and handled is by monthly auction or a monthly transmission allocation procedure.</skos:definition>
  </skos:Concept>
  <skos:Concept rdf:about="http://energy.referencedata.eu/StandardContractTypeList/A04">
    <skos:inScheme rdf:resource="http://energy.referencedata.eu/StandardContractTypeList"/>
    <skos:topConceptOf rdf:resource="http://energy.referencedata.eu/StandardContractTypeList"/>
    <dcterms:identifier>A04</dcterms:identifier>
    <skos:prefLabel>Yearly</skos:prefLabel>
    <skos:definition xml:lang="en">The condition under which capacity is allocated and handled is by yearly auction or a yearly transmission allocation procedure.</skos:definition>
  </skos:Concept>
  <skos:Concept rdf:about="http://energy.referencedata.eu/StandardContractTypeList/A05">
    <skos:inScheme rdf:resource="http://energy.referencedata.eu/StandardContractTypeList"/>
    <skos:topConceptOf rdf:resource="http://energy.referencedata.eu/StandardContractTypeList"/>
    <dcterms:identifier>A05</dcterms:identifier>
    <skos:prefLabel>Total</skos:prefLabel>
    <skos:definition xml:lang="en">This is the sum of all capacity contract types for the period covered.</skos:definition>
  </skos:Concept>
  <skos:Concept rdf:about="http://energy.referencedata.eu/StandardContractTypeList/A06">
    <skos:inScheme rdf:resource="http://energy.referencedata.eu/StandardContractTypeList"/>
    <skos:topConceptOf rdf:resource="http://energy.referencedata.eu/StandardContractTypeList"/>
    <dcterms:identifier>A06</dcterms:identifier>
    <skos:prefLabel>Long term contract</skos:prefLabel>
    <skos:definition xml:lang="en">The condition under which capacity is allocated and handled is by long term trade agreements according to European regulations (EU Directive 1228/2003).</skos:definition>
  </skos:Concept>
  <skos:Concept rdf:about="http://energy.referencedata.eu/StandardContractTypeList/A07">
    <skos:inScheme rdf:resource="http://energy.referencedata.eu/StandardContractTypeList"/>
    <skos:topConceptOf rdf:resource="http://energy.referencedata.eu/StandardContractTypeList"/>
    <dcterms:identifier>A07</dcterms:identifier>
    <skos:prefLabel>Intraday contract</skos:prefLabel>
    <skos:definition xml:lang="en">The condition under which the capacity is allocated and handled is through an intraday auction and allocation process.</skos:definition>
  </skos:Concept>
  <skos:Concept rdf:about="http://energy.referencedata.eu/StandardContractTypeList/A08">
    <skos:inScheme rdf:resource="http://energy.referencedata.eu/StandardContractTypeList"/>
    <skos:topConceptOf rdf:resource="http://energy.referencedata.eu/StandardContractTypeList"/>
    <dcterms:identifier>A08</dcterms:identifier>
    <skos:prefLabel>Quarter yearly</skos:prefLabel>
    <skos:definition xml:lang="en">The condition under which capacity is allocated and handled is by quarter yearly auction or a quarter yearly transmission allocation procedure.</skos:definition>
  </skos:Concept>
  <skos:Concept rdf:about="http://energy.referencedata.eu/StandardContractTypeList/A09">
    <skos:inScheme rdf:resource="http://energy.referencedata.eu/StandardContractTypeList"/>
    <skos:topConceptOf rdf:resource="http://energy.referencedata.eu/StandardContractTypeList"/>
    <dcterms:identifier>A09</dcterms:identifier>
    <skos:prefLabel>Semestrial</skos:prefLabel>
    <skos:definition xml:lang="en">The condition under which capacity is allocated and handled is by half yearly auction or a half yearly transmission allocation procedure.</skos:definition>
  </skos:Concept>
  <skos:Concept rdf:about="http://energy.referencedata.eu/StandardContractTypeList/A10">
    <skos:inScheme rdf:resource="http://energy.referencedata.eu/StandardContractTypeList"/>
    <skos:topConceptOf rdf:resource="http://energy.referencedata.eu/StandardContractTypeList"/>
    <dcterms:identifier>A10</dcterms:identifier>
    <skos:prefLabel>Multiple year</skos:prefLabel>
    <skos:definition xml:lang="en">The condition under which capacity is allocated and handled is by multiple year auctions.</skos:definition>
  </skos:Concept>
  <skos:Concept rdf:about="http://energy.referencedata.eu/StandardContractTypeList/A11">
    <skos:inScheme rdf:resource="http://energy.referencedata.eu/StandardContractTypeList"/>
    <skos:topConceptOf rdf:resource="http://energy.referencedata.eu/StandardContractTypeList"/>
    <dcterms:identifier>A11</dcterms:identifier>
    <skos:prefLabel>Intraday balancing mechanism</skos:prefLabel>
    <skos:definition xml:lang="en">The condition under which the capacity is allocated and handled is through intraday energy balancing services.</skos:definition>
  </skos:Concept>
  <skos:Concept rdf:about="http://energy.referencedata.eu/StandardContractTypeList/A12">
    <skos:inScheme rdf:resource="http://energy.referencedata.eu/StandardContractTypeList"/>
    <skos:topConceptOf rdf:resource="http://energy.referencedata.eu/StandardContractTypeList"/>
    <dcterms:identifier>A12</dcterms:identifier>
    <skos:prefLabel>Historical contract</skos:prefLabel>
    <skos:definition xml:lang="en">A Contract established before the EU directive that are valid until the term of the contract.</skos:definition>
  </skos:Concept>
  <skos:Concept rdf:about="http://energy.referencedata.eu/StandardContractTypeList/A13">
    <skos:inScheme rdf:resource="http://energy.referencedata.eu/StandardContractTypeList"/>
    <skos:topConceptOf rdf:resource="http://energy.referencedata.eu/StandardContractTypeList"/>
    <dcterms:identifier>A13</dcterms:identifier>
    <skos:prefLabel>Hourly</skos:prefLabel>
    <skos:definition xml:lang="en">The condition under which capacity is allocated and handled is by hourly auctions.</skos:definition>
  </skos:Concept>
</rdf:RDF>
