<?xml version='1.0' encoding='UTF-8'?>
<rdf:RDF xmlns:cim="http://iec.ch/TC57/2013/CIM-schema-cim16#" xmlns:rdf="http://www.w3.org/1999/02/22-rdf-syntax-ns#" xmlns:rdfs="http://www.w3.org/2000/01/rdf-schema#" xmlns:dcat="http://www.w3.org/ns/dcat#" xmlns:dc="http://purl.org/dc/elements/1.1/" xmlns:dcterms="http://purl.org/dc/terms/" xmlns:skos="http://www.w3.org/2004/02/skos/core#" xmlns:ecl="urn:entsoe.eu:wgedi:codelists" xmlns:xs="http://www.w3.org/2001/XMLSchema">
  <dcat:Distribution rdf:about="urn:uuid:2b574087-9b0c-4919-acd3-c67f5520b3b2">
    <rdfs:label>entsoe-codelist-StandardContractTypeList.rdf</rdfs:label>
    <dcterms:issued>2021-12-03</dcterms:issued>
    <dcat:version>80</dcat:version>
    <ecl:Version>80</ecl:Version>
    <ecl:Title>Complete compilation of ENTSO-E Code Lists used by ENTSO-E XML electronic documents and CIM XML electronic documents.</ecl:Title>
    <ecl:Release>0</ecl:Release>
    <ecl:ReleaseDate>2021-12-03</ecl:ReleaseDate>
  </dcat:Distribution>
  <skos:ConceptScheme rdf:about="http://data.europa.eu/energy/StandardContractTypeList">
    <rdfs:label>StandardContractTypeList</rdfs:label>
    <skos:prefLabel>StandardContractTypeList</skos:prefLabel>
    <dc:identifier>ET0010</dc:identifier>
    <skos:definition>The contract type defines the conditions under which the capacity is allocated and handled, e.g. daily auction, weekly auction, monthly auction, yearly auction, etc. 
The significance of this type is dependent on area specific coded working methods.</skos:definition>
    <ecl:Uid>ET0010</ecl:Uid>
    <ecl:Definition>The contract type defines the conditions under which the capacity is allocated and handled, e.g. daily auction, weekly auction, monthly auction, yearly auction, etc. 
The significance of this type is dependent on area specific coded working methods.</ecl:Definition>
  </skos:ConceptScheme>
  <skos:Concept rdf:about="http://data.europa.eu/energy/StandardContractTypeList/A01">
    <skos:inScheme rdf:resource="http://data.europa.eu/energy/StandardContractTypeList"/>
    <skos:topConceptOf rdf:resource="http://data.europa.eu/energy/StandardContractTypeList"/>
    <xs:enumeration>A01</xs:enumeration>
    <dc:identifier>A01</dc:identifier>
    <rdfs:label>Daily</rdfs:label>
    <skos:prefLabel>Daily</skos:prefLabel>
    <skos:definition>The condition under which capacity is allocated and handled is by daily auction or a daily transmission allocation procedure.</skos:definition>
  </skos:Concept>
  <skos:Concept rdf:about="http://data.europa.eu/energy/StandardContractTypeList/A02">
    <skos:inScheme rdf:resource="http://data.europa.eu/energy/StandardContractTypeList"/>
    <skos:topConceptOf rdf:resource="http://data.europa.eu/energy/StandardContractTypeList"/>
    <xs:enumeration>A02</xs:enumeration>
    <dc:identifier>A02</dc:identifier>
    <rdfs:label>Weekly</rdfs:label>
    <skos:prefLabel>Weekly</skos:prefLabel>
    <skos:definition>The condition under which capacity is allocated and handled is by weekly auction or a weekly transmission allocation procedure.</skos:definition>
  </skos:Concept>
  <skos:Concept rdf:about="http://data.europa.eu/energy/StandardContractTypeList/A03">
    <skos:inScheme rdf:resource="http://data.europa.eu/energy/StandardContractTypeList"/>
    <skos:topConceptOf rdf:resource="http://data.europa.eu/energy/StandardContractTypeList"/>
    <xs:enumeration>A03</xs:enumeration>
    <dc:identifier>A03</dc:identifier>
    <rdfs:label>Monthly</rdfs:label>
    <skos:prefLabel>Monthly</skos:prefLabel>
    <skos:definition>The condition under which capacity is allocated and handled is by monthly auction or a monthly transmission allocation procedure.</skos:definition>
  </skos:Concept>
  <skos:Concept rdf:about="http://data.europa.eu/energy/StandardContractTypeList/A04">
    <skos:inScheme rdf:resource="http://data.europa.eu/energy/StandardContractTypeList"/>
    <skos:topConceptOf rdf:resource="http://data.europa.eu/energy/StandardContractTypeList"/>
    <xs:enumeration>A04</xs:enumeration>
    <dc:identifier>A04</dc:identifier>
    <rdfs:label>Yearly</rdfs:label>
    <skos:prefLabel>Yearly</skos:prefLabel>
    <skos:definition>The condition under which capacity is allocated and handled is by yearly auction or a yearly transmission allocation procedure.</skos:definition>
  </skos:Concept>
  <skos:Concept rdf:about="http://data.europa.eu/energy/StandardContractTypeList/A05">
    <skos:inScheme rdf:resource="http://data.europa.eu/energy/StandardContractTypeList"/>
    <skos:topConceptOf rdf:resource="http://data.europa.eu/energy/StandardContractTypeList"/>
    <xs:enumeration>A05</xs:enumeration>
    <dc:identifier>A05</dc:identifier>
    <rdfs:label>Total</rdfs:label>
    <skos:prefLabel>Total</skos:prefLabel>
    <skos:definition>This is the sum of all capacity contract types for the period covered.</skos:definition>
  </skos:Concept>
  <skos:Concept rdf:about="http://data.europa.eu/energy/StandardContractTypeList/A06">
    <skos:inScheme rdf:resource="http://data.europa.eu/energy/StandardContractTypeList"/>
    <skos:topConceptOf rdf:resource="http://data.europa.eu/energy/StandardContractTypeList"/>
    <xs:enumeration>A06</xs:enumeration>
    <dc:identifier>A06</dc:identifier>
    <rdfs:label>Long term contract</rdfs:label>
    <skos:prefLabel>Long term contract</skos:prefLabel>
    <skos:definition>The condition under which capacity is allocated and handled is by long term trade agreements according to European regulations (EU Directive 1228/2003).</skos:definition>
  </skos:Concept>
  <skos:Concept rdf:about="http://data.europa.eu/energy/StandardContractTypeList/A07">
    <skos:inScheme rdf:resource="http://data.europa.eu/energy/StandardContractTypeList"/>
    <skos:topConceptOf rdf:resource="http://data.europa.eu/energy/StandardContractTypeList"/>
    <xs:enumeration>A07</xs:enumeration>
    <dc:identifier>A07</dc:identifier>
    <rdfs:label>Intraday contract</rdfs:label>
    <skos:prefLabel>Intraday contract</skos:prefLabel>
    <skos:definition>The condition under which the capacity is allocated and handled is through an intraday auction and allocation process.</skos:definition>
  </skos:Concept>
  <skos:Concept rdf:about="http://data.europa.eu/energy/StandardContractTypeList/A08">
    <skos:inScheme rdf:resource="http://data.europa.eu/energy/StandardContractTypeList"/>
    <skos:topConceptOf rdf:resource="http://data.europa.eu/energy/StandardContractTypeList"/>
    <xs:enumeration>A08</xs:enumeration>
    <dc:identifier>A08</dc:identifier>
    <rdfs:label>Quarter yearly</rdfs:label>
    <skos:prefLabel>Quarter yearly</skos:prefLabel>
    <skos:definition>The condition under which capacity is allocated and handled is by quarter yearly auction or a quarter yearly transmission allocation procedure.</skos:definition>
  </skos:Concept>
  <skos:Concept rdf:about="http://data.europa.eu/energy/StandardContractTypeList/A09">
    <skos:inScheme rdf:resource="http://data.europa.eu/energy/StandardContractTypeList"/>
    <skos:topConceptOf rdf:resource="http://data.europa.eu/energy/StandardContractTypeList"/>
    <xs:enumeration>A09</xs:enumeration>
    <dc:identifier>A09</dc:identifier>
    <rdfs:label>Semestrial</rdfs:label>
    <skos:prefLabel>Semestrial</skos:prefLabel>
    <skos:definition>The condition under which capacity is allocated and handled is by half yearly auction or a half yearly transmission allocation procedure.</skos:definition>
  </skos:Concept>
  <skos:Concept rdf:about="http://data.europa.eu/energy/StandardContractTypeList/A10">
    <skos:inScheme rdf:resource="http://data.europa.eu/energy/StandardContractTypeList"/>
    <skos:topConceptOf rdf:resource="http://data.europa.eu/energy/StandardContractTypeList"/>
    <xs:enumeration>A10</xs:enumeration>
    <dc:identifier>A10</dc:identifier>
    <rdfs:label>Multiple year</rdfs:label>
    <skos:prefLabel>Multiple year</skos:prefLabel>
    <skos:definition>The condition under which capacity is allocated and handled is by multiple year auctions.</skos:definition>
  </skos:Concept>
  <skos:Concept rdf:about="http://data.europa.eu/energy/StandardContractTypeList/A11">
    <skos:inScheme rdf:resource="http://data.europa.eu/energy/StandardContractTypeList"/>
    <skos:topConceptOf rdf:resource="http://data.europa.eu/energy/StandardContractTypeList"/>
    <xs:enumeration>A11</xs:enumeration>
    <dc:identifier>A11</dc:identifier>
    <rdfs:label>Intraday balancing mechanism</rdfs:label>
    <skos:prefLabel>Intraday balancing mechanism</skos:prefLabel>
    <skos:definition>The condition under which the capacity is allocated and handled is through intraday energy balancing services.</skos:definition>
  </skos:Concept>
  <skos:Concept rdf:about="http://data.europa.eu/energy/StandardContractTypeList/A12">
    <skos:inScheme rdf:resource="http://data.europa.eu/energy/StandardContractTypeList"/>
    <skos:topConceptOf rdf:resource="http://data.europa.eu/energy/StandardContractTypeList"/>
    <xs:enumeration>A12</xs:enumeration>
    <dc:identifier>A12</dc:identifier>
    <rdfs:label>Historical contract</rdfs:label>
    <skos:prefLabel>Historical contract</skos:prefLabel>
    <skos:definition>A Contract established before the EU directive that are valid until the term of the contract.</skos:definition>
  </skos:Concept>
  <skos:Concept rdf:about="http://data.europa.eu/energy/StandardContractTypeList/A13">
    <skos:inScheme rdf:resource="http://data.europa.eu/energy/StandardContractTypeList"/>
    <skos:topConceptOf rdf:resource="http://data.europa.eu/energy/StandardContractTypeList"/>
    <xs:enumeration>A13</xs:enumeration>
    <dc:identifier>A13</dc:identifier>
    <rdfs:label>Hourly</rdfs:label>
    <skos:prefLabel>Hourly</skos:prefLabel>
    <skos:definition>The condition under which capacity is allocated and handled is by hourly auctions.</skos:definition>
  </skos:Concept>
</rdf:RDF>
