<?xml version='1.0' encoding='UTF-8'?>
<rdf:RDF xmlns:cim="http://iec.ch/TC57/2013/CIM-schema-cim16#" xmlns:rdf="http://www.w3.org/1999/02/22-rdf-syntax-ns#" xmlns:rdfs="http://www.w3.org/2000/01/rdf-schema#" xmlns:dcat="http://www.w3.org/ns/dcat#" xmlns:dc="http://purl.org/dc/elements/1.1/" xmlns:dcterms="http://purl.org/dc/terms/" xmlns:skos="http://www.w3.org/2004/02/skos/core#" xmlns:ecl="urn:entsoe.eu:wgedi:codelists" xmlns:xs="http://www.w3.org/2001/XMLSchema">
  <dcat:Distribution rdf:about="urn:uuid:a4f388bf-504e-40d7-bed5-5fe4e2cd9473">
    <rdfs:label>entsoe-codelist-StandardCurveTypeList.rdf</rdfs:label>
    <dcterms:issued>2021-12-03</dcterms:issued>
    <dcat:version>80</dcat:version>
    <ecl:Version>80</ecl:Version>
    <ecl:Title>Complete compilation of ENTSO-E Code Lists used by ENTSO-E XML electronic documents and CIM XML electronic documents.</ecl:Title>
    <ecl:Release>0</ecl:Release>
    <ecl:ReleaseDate>2021-12-03</ecl:ReleaseDate>
  </dcat:Distribution>
  <skos:ConceptScheme rdf:about="http://data.europa.eu/energy/StandardCurveTypeList">
    <dcterms:issued>2021-12-03</dcterms:issued>
    <dcat:version>80</dcat:version>
    <skos:prefLabel>StandardCurveTypeList</skos:prefLabel>
    <dc:identifier>ET0042</dc:identifier>
    <skos:definition xml:lang="en">The type of curve being defined in the time series.</skos:definition>
  </skos:ConceptScheme>
  <skos:Concept rdf:about="http://data.europa.eu/energy/StandardCurveTypeList/A01">
    <skos:inScheme rdf:resource="http://data.europa.eu/energy/StandardCurveTypeList"/>
    <skos:topConceptOf rdf:resource="http://data.europa.eu/energy/StandardCurveTypeList"/>
    <dc:identifier>A01</dc:identifier>
    <skos:prefLabel>Sequential fixed size block</skos:prefLabel>
    <skos:definition xml:lang="en">The curve is made of successive Intervals of time (Blocks) of constant duration (size), where the size of the Blocks is equal to the Resolution of the Period.</skos:definition>
  </skos:Concept>
  <skos:Concept rdf:about="http://data.europa.eu/energy/StandardCurveTypeList/A02">
    <skos:inScheme rdf:resource="http://data.europa.eu/energy/StandardCurveTypeList"/>
    <skos:topConceptOf rdf:resource="http://data.europa.eu/energy/StandardCurveTypeList"/>
    <dc:identifier>A02</dc:identifier>
    <skos:prefLabel>Point</skos:prefLabel>
    <skos:definition xml:lang="en">The curve is made of successive instants of time (Points).</skos:definition>
  </skos:Concept>
  <skos:Concept rdf:about="http://data.europa.eu/energy/StandardCurveTypeList/A03">
    <skos:inScheme rdf:resource="http://data.europa.eu/energy/StandardCurveTypeList"/>
    <skos:topConceptOf rdf:resource="http://data.europa.eu/energy/StandardCurveTypeList"/>
    <dc:identifier>A03</dc:identifier>
    <skos:prefLabel>Variable sized Block</skos:prefLabel>
    <skos:definition xml:lang="en">The curve is made of successive Intervals of time (Blocks) of variable duration (size), where the end date and end time of each Block are equal to the start date and start time of the next Interval. For the last Block the end date and end time of the last Interval would be equal to EndDateTime of TimeInterval.</skos:definition>
  </skos:Concept>
  <skos:Concept rdf:about="http://data.europa.eu/energy/StandardCurveTypeList/A04">
    <skos:inScheme rdf:resource="http://data.europa.eu/energy/StandardCurveTypeList"/>
    <skos:topConceptOf rdf:resource="http://data.europa.eu/energy/StandardCurveTypeList"/>
    <dc:identifier>A04</dc:identifier>
    <skos:prefLabel>Overlapping breakpoint</skos:prefLabel>
    <skos:definition xml:lang="en">The curve is made of successive Intervals of time of variable duration (size), where the end date and end time of each interval are equal to the start date and start time of the next Interval.</skos:definition>
  </skos:Concept>
  <skos:Concept rdf:about="http://data.europa.eu/energy/StandardCurveTypeList/A05">
    <skos:inScheme rdf:resource="http://data.europa.eu/energy/StandardCurveTypeList"/>
    <skos:topConceptOf rdf:resource="http://data.europa.eu/energy/StandardCurveTypeList"/>
    <dc:identifier>A05</dc:identifier>
    <skos:prefLabel>Non-overlapping breakpoint</skos:prefLabel>
    <skos:definition xml:lang="en">This curve is a restriction of the curve type A04, i.e. overlapping breakpoints. The restriction is that a single Period is allowed.</skos:definition>
  </skos:Concept>
</rdf:RDF>
