<?xml version='1.0' encoding='UTF-8'?>
<rdf:RDF xmlns:cim="http://iec.ch/TC57/2013/CIM-schema-cim16#" xmlns:rdf="http://www.w3.org/1999/02/22-rdf-syntax-ns#" xmlns:rdfs="http://www.w3.org/2000/01/rdf-schema#" xmlns:dcat="http://www.w3.org/ns/dcat#" xmlns:dc="http://purl.org/dc/elements/1.1/" xmlns:dcterms="http://purl.org/dc/terms/" xmlns:skos="http://www.w3.org/2004/02/skos/core#" xmlns:ecl="urn:entsoe.eu:wgedi:codelists" xmlns:xs="http://www.w3.org/2001/XMLSchema">
  <skos:ConceptScheme rdf:about="http://data.europa.eu/energy/StandardMessageTypeList">
    <dcterms:modified>2021-12-03</dcterms:modified>
    <dcat:version>80</dcat:version>
    <skos:prefLabel>StandardMessageTypeList</skos:prefLabel>
    <dc:identifier>ET0003</dc:identifier>
    <skos:definition xml:lang="en">The coded type of a document. The message type describes the principal characteristic of a document.
This enumeration is used in the XML instances based on IEC 62325.</skos:definition>
  </skos:ConceptScheme>
  <skos:Concept rdf:about="http://data.europa.eu/energy/StandardMessageTypeList/A01">
    <skos:inScheme rdf:resource="http://data.europa.eu/energy/StandardMessageTypeList"/>
    <skos:topConceptOf rdf:resource="http://data.europa.eu/energy/StandardMessageTypeList"/>
    <dc:identifier>A01</dc:identifier>
    <skos:prefLabel>Balance responsible schedule</skos:prefLabel>
    <skos:definition xml:lang="en">A schedule which has been prepared by a balance responsible party providing planned schedule information.</skos:definition>
  </skos:Concept>
  <skos:Concept rdf:about="http://data.europa.eu/energy/StandardMessageTypeList/A02">
    <skos:inScheme rdf:resource="http://data.europa.eu/energy/StandardMessageTypeList"/>
    <skos:topConceptOf rdf:resource="http://data.europa.eu/energy/StandardMessageTypeList"/>
    <dc:identifier>A02</dc:identifier>
    <skos:prefLabel>Allocated capacity schedule</skos:prefLabel>
    <skos:definition xml:lang="en">A schedule which has been prepared by a capacity allocator providing allocated capacity.</skos:definition>
  </skos:Concept>
  <skos:Concept rdf:about="http://data.europa.eu/energy/StandardMessageTypeList/A03">
    <skos:inScheme rdf:resource="http://data.europa.eu/energy/StandardMessageTypeList"/>
    <skos:topConceptOf rdf:resource="http://data.europa.eu/energy/StandardMessageTypeList"/>
    <dc:identifier>A03</dc:identifier>
    <skos:prefLabel>Balance area schedule</skos:prefLabel>
    <skos:definition xml:lang="en">A schedule that provides the planned schedule information for a balance area.</skos:definition>
  </skos:Concept>
  <skos:Concept rdf:about="http://data.europa.eu/energy/StandardMessageTypeList/A04">
    <skos:inScheme rdf:resource="http://data.europa.eu/energy/StandardMessageTypeList"/>
    <skos:topConceptOf rdf:resource="http://data.europa.eu/energy/StandardMessageTypeList"/>
    <dc:identifier>A04</dc:identifier>
    <skos:prefLabel>System Operator area schedule</skos:prefLabel>
    <skos:definition xml:lang="en">A compilation of all external schedules concerning two System Operator areas or a connector concerning two System Operator of all balance responsible parties.</skos:definition>
  </skos:Concept>
  <skos:Concept rdf:about="http://data.europa.eu/energy/StandardMessageTypeList/A05">
    <skos:inScheme rdf:resource="http://data.europa.eu/energy/StandardMessageTypeList"/>
    <skos:topConceptOf rdf:resource="http://data.europa.eu/energy/StandardMessageTypeList"/>
    <dc:identifier>A05</dc:identifier>
    <skos:prefLabel>Control block area schedule</skos:prefLabel>
    <skos:definition xml:lang="en">A compilation of all the exchange programs of all control areas for one control block with all neighbouring control areas of a neighbouring control block.</skos:definition>
  </skos:Concept>
  <skos:Concept rdf:about="http://data.europa.eu/energy/StandardMessageTypeList/A06">
    <skos:inScheme rdf:resource="http://data.europa.eu/energy/StandardMessageTypeList"/>
    <skos:topConceptOf rdf:resource="http://data.europa.eu/energy/StandardMessageTypeList"/>
    <dc:identifier>A06</dc:identifier>
    <skos:prefLabel>Coordination center area schedule</skos:prefLabel>
    <skos:definition xml:lang="en">A compilation of the exchange programs of all exchange blocks divided into UCTE south and north.</skos:definition>
  </skos:Concept>
  <skos:Concept rdf:about="http://data.europa.eu/energy/StandardMessageTypeList/A07">
    <skos:inScheme rdf:resource="http://data.europa.eu/energy/StandardMessageTypeList"/>
    <skos:topConceptOf rdf:resource="http://data.europa.eu/energy/StandardMessageTypeList"/>
    <dc:identifier>A07</dc:identifier>
    <skos:prefLabel>Intermediate confirmation report</skos:prefLabel>
    <skos:definition xml:lang="en">An intermediate confirmation report that may be produced between final cutoffs.</skos:definition>
  </skos:Concept>
  <skos:Concept rdf:about="http://data.europa.eu/energy/StandardMessageTypeList/A08">
    <skos:inScheme rdf:resource="http://data.europa.eu/energy/StandardMessageTypeList"/>
    <skos:topConceptOf rdf:resource="http://data.europa.eu/energy/StandardMessageTypeList"/>
    <dc:identifier>A08</dc:identifier>
    <skos:prefLabel>Final confirmation report</skos:prefLabel>
    <skos:definition xml:lang="en">A final confirmation report that is produced after a final cutoff.</skos:definition>
  </skos:Concept>
  <skos:Concept rdf:about="http://data.europa.eu/energy/StandardMessageTypeList/A09">
    <skos:inScheme rdf:resource="http://data.europa.eu/energy/StandardMessageTypeList"/>
    <skos:topConceptOf rdf:resource="http://data.europa.eu/energy/StandardMessageTypeList"/>
    <dc:identifier>A09</dc:identifier>
    <skos:prefLabel>Finalised schedule</skos:prefLabel>
    <skos:definition xml:lang="en">A compilation of a set of schedules that have been finalized after a given cutoff.</skos:definition>
  </skos:Concept>
  <skos:Concept rdf:about="http://data.europa.eu/energy/StandardMessageTypeList/A10">
    <skos:inScheme rdf:resource="http://data.europa.eu/energy/StandardMessageTypeList"/>
    <skos:topConceptOf rdf:resource="http://data.europa.eu/energy/StandardMessageTypeList"/>
    <dc:identifier>A10</dc:identifier>
    <skos:prefLabel>Regulation data report</skos:prefLabel>
    <skos:definition xml:lang="en">A compilation of the time series employed on a given day to ensure the balance of the system.</skos:definition>
  </skos:Concept>
  <skos:Concept rdf:about="http://data.europa.eu/energy/StandardMessageTypeList/A11">
    <skos:inScheme rdf:resource="http://data.europa.eu/energy/StandardMessageTypeList"/>
    <skos:topConceptOf rdf:resource="http://data.europa.eu/energy/StandardMessageTypeList"/>
    <dc:identifier>A11</dc:identifier>
    <skos:prefLabel>Aggregated energy data report</skos:prefLabel>
    <skos:definition xml:lang="en">A compilation of the time series of all the meter readings or their equivalent for a given period.</skos:definition>
  </skos:Concept>
  <skos:Concept rdf:about="http://data.europa.eu/energy/StandardMessageTypeList/A12">
    <skos:inScheme rdf:resource="http://data.europa.eu/energy/StandardMessageTypeList"/>
    <skos:topConceptOf rdf:resource="http://data.europa.eu/energy/StandardMessageTypeList"/>
    <dc:identifier>A12</dc:identifier>
    <skos:prefLabel>Imbalance report</skos:prefLabel>
    <skos:definition xml:lang="en">The report containing the complete situation of a given period for a party and including the schedules, regulation data and actual or calculated readings.</skos:definition>
  </skos:Concept>
  <skos:Concept rdf:about="http://data.europa.eu/energy/StandardMessageTypeList/A13">
    <skos:inScheme rdf:resource="http://data.europa.eu/energy/StandardMessageTypeList"/>
    <skos:topConceptOf rdf:resource="http://data.europa.eu/energy/StandardMessageTypeList"/>
    <dc:identifier>A13</dc:identifier>
    <skos:prefLabel>Interconnection Capacity</skos:prefLabel>
    <skos:definition xml:lang="en">Document for cross-border capacity exchanges.</skos:definition>
  </skos:Concept>
  <skos:Concept rdf:about="http://data.europa.eu/energy/StandardMessageTypeList/A14">
    <skos:inScheme rdf:resource="http://data.europa.eu/energy/StandardMessageTypeList"/>
    <skos:topConceptOf rdf:resource="http://data.europa.eu/energy/StandardMessageTypeList"/>
    <dc:identifier>A14</dc:identifier>
    <skos:prefLabel>Resource Provider Resource Schedule</skos:prefLabel>
    <skos:definition xml:lang="en">A document providing the schedules for resource objects submitted by a resource provider.</skos:definition>
  </skos:Concept>
  <skos:Concept rdf:about="http://data.europa.eu/energy/StandardMessageTypeList/A15">
    <skos:inScheme rdf:resource="http://data.europa.eu/energy/StandardMessageTypeList"/>
    <skos:topConceptOf rdf:resource="http://data.europa.eu/energy/StandardMessageTypeList"/>
    <dc:identifier>A15</dc:identifier>
    <skos:prefLabel>Acquiring System Operator Reserve Schedule</skos:prefLabel>
    <skos:definition xml:lang="en">A document providing reserve purchases submitted by an Acquiring System Operator.</skos:definition>
  </skos:Concept>
  <skos:Concept rdf:about="http://data.europa.eu/energy/StandardMessageTypeList/A16">
    <skos:inScheme rdf:resource="http://data.europa.eu/energy/StandardMessageTypeList"/>
    <skos:topConceptOf rdf:resource="http://data.europa.eu/energy/StandardMessageTypeList"/>
    <dc:identifier>A16</dc:identifier>
    <skos:prefLabel>Anomaly Report</skos:prefLabel>
    <skos:definition xml:lang="en">A document providing anomaly information for the receiving party to correct.</skos:definition>
  </skos:Concept>
  <skos:Concept rdf:about="http://data.europa.eu/energy/StandardMessageTypeList/A17">
    <skos:inScheme rdf:resource="http://data.europa.eu/energy/StandardMessageTypeList"/>
    <skos:topConceptOf rdf:resource="http://data.europa.eu/energy/StandardMessageTypeList"/>
    <dc:identifier>A17</dc:identifier>
    <skos:prefLabel>Acknowledgement Document</skos:prefLabel>
    <skos:definition xml:lang="en">A document providing acknowledgement information.</skos:definition>
  </skos:Concept>
  <skos:Concept rdf:about="http://data.europa.eu/energy/StandardMessageTypeList/A18">
    <skos:inScheme rdf:resource="http://data.europa.eu/energy/StandardMessageTypeList"/>
    <skos:topConceptOf rdf:resource="http://data.europa.eu/energy/StandardMessageTypeList"/>
    <dc:identifier>A18</dc:identifier>
    <skos:prefLabel>Confirmation report</skos:prefLabel>
    <skos:definition xml:lang="en">A document providing confirmation information.</skos:definition>
  </skos:Concept>
  <skos:Concept rdf:about="http://data.europa.eu/energy/StandardMessageTypeList/A19">
    <skos:inScheme rdf:resource="http://data.europa.eu/energy/StandardMessageTypeList"/>
    <skos:topConceptOf rdf:resource="http://data.europa.eu/energy/StandardMessageTypeList"/>
    <dc:identifier>A19</dc:identifier>
    <skos:prefLabel>Capacity for Resale</skos:prefLabel>
    <skos:definition xml:lang="en">A document providing information about capacity for resale.</skos:definition>
  </skos:Concept>
  <skos:Concept rdf:about="http://data.europa.eu/energy/StandardMessageTypeList/A20">
    <skos:inScheme rdf:resource="http://data.europa.eu/energy/StandardMessageTypeList"/>
    <skos:topConceptOf rdf:resource="http://data.europa.eu/energy/StandardMessageTypeList"/>
    <dc:identifier>A20</dc:identifier>
    <skos:prefLabel>Approved Capacity Transfer</skos:prefLabel>
    <skos:definition xml:lang="en">A document to approve a capacity transfer.</skos:definition>
  </skos:Concept>
  <skos:Concept rdf:about="http://data.europa.eu/energy/StandardMessageTypeList/A21">
    <skos:inScheme rdf:resource="http://data.europa.eu/energy/StandardMessageTypeList"/>
    <skos:topConceptOf rdf:resource="http://data.europa.eu/energy/StandardMessageTypeList"/>
    <dc:identifier>A21</dc:identifier>
    <skos:prefLabel>Capacity transfer notification</skos:prefLabel>
    <skos:definition xml:lang="en">A document notifying a capacity transfer.</skos:definition>
  </skos:Concept>
  <skos:Concept rdf:about="http://data.europa.eu/energy/StandardMessageTypeList/A22">
    <skos:inScheme rdf:resource="http://data.europa.eu/energy/StandardMessageTypeList"/>
    <skos:topConceptOf rdf:resource="http://data.europa.eu/energy/StandardMessageTypeList"/>
    <dc:identifier>A22</dc:identifier>
    <skos:prefLabel>Transmission rights portfolio</skos:prefLabel>
    <skos:definition xml:lang="en">A document providing the portfolio of the transmission capacity rights of a market participant.</skos:definition>
  </skos:Concept>
  <skos:Concept rdf:about="http://data.europa.eu/energy/StandardMessageTypeList/A23">
    <skos:inScheme rdf:resource="http://data.europa.eu/energy/StandardMessageTypeList"/>
    <skos:topConceptOf rdf:resource="http://data.europa.eu/energy/StandardMessageTypeList"/>
    <dc:identifier>A23</dc:identifier>
    <skos:prefLabel>Allocations</skos:prefLabel>
    <skos:definition xml:lang="en">A document providing the capacity allocations for a border.</skos:definition>
  </skos:Concept>
  <skos:Concept rdf:about="http://data.europa.eu/energy/StandardMessageTypeList/A24">
    <skos:inScheme rdf:resource="http://data.europa.eu/energy/StandardMessageTypeList"/>
    <skos:topConceptOf rdf:resource="http://data.europa.eu/energy/StandardMessageTypeList"/>
    <dc:identifier>A24</dc:identifier>
    <skos:prefLabel>Bid document</skos:prefLabel>
    <skos:definition xml:lang="en">A document providing bid information.</skos:definition>
  </skos:Concept>
  <skos:Concept rdf:about="http://data.europa.eu/energy/StandardMessageTypeList/A25">
    <skos:inScheme rdf:resource="http://data.europa.eu/energy/StandardMessageTypeList"/>
    <skos:topConceptOf rdf:resource="http://data.europa.eu/energy/StandardMessageTypeList"/>
    <dc:identifier>A25</dc:identifier>
    <skos:prefLabel>Allocation result document</skos:prefLabel>
    <skos:definition xml:lang="en">A document providing the allocation results of an auction.</skos:definition>
  </skos:Concept>
  <skos:Concept rdf:about="http://data.europa.eu/energy/StandardMessageTypeList/A26">
    <skos:inScheme rdf:resource="http://data.europa.eu/energy/StandardMessageTypeList"/>
    <skos:topConceptOf rdf:resource="http://data.europa.eu/energy/StandardMessageTypeList"/>
    <dc:identifier>A26</dc:identifier>
    <skos:prefLabel>Capacity document</skos:prefLabel>
    <skos:definition xml:lang="en">A document providing capacity information.</skos:definition>
  </skos:Concept>
  <skos:Concept rdf:about="http://data.europa.eu/energy/StandardMessageTypeList/A27">
    <skos:inScheme rdf:resource="http://data.europa.eu/energy/StandardMessageTypeList"/>
    <skos:topConceptOf rdf:resource="http://data.europa.eu/energy/StandardMessageTypeList"/>
    <dc:identifier>A27</dc:identifier>
    <skos:prefLabel>Rights document</skos:prefLabel>
    <skos:definition xml:lang="en">A document providing transmission capacity rights information.</skos:definition>
  </skos:Concept>
  <skos:Concept rdf:about="http://data.europa.eu/energy/StandardMessageTypeList/A28">
    <skos:inScheme rdf:resource="http://data.europa.eu/energy/StandardMessageTypeList"/>
    <skos:topConceptOf rdf:resource="http://data.europa.eu/energy/StandardMessageTypeList"/>
    <dc:identifier>A28</dc:identifier>
    <skos:prefLabel>Generation availability schedule</skos:prefLabel>
    <skos:definition xml:lang="en">This document contains information related to energy availability.</skos:definition>
  </skos:Concept>
  <skos:Concept rdf:about="http://data.europa.eu/energy/StandardMessageTypeList/A30">
    <skos:inScheme rdf:resource="http://data.europa.eu/energy/StandardMessageTypeList"/>
    <skos:topConceptOf rdf:resource="http://data.europa.eu/energy/StandardMessageTypeList"/>
    <dc:identifier>A30</dc:identifier>
    <skos:prefLabel>Cross border schedule</skos:prefLabel>
    <skos:definition xml:lang="en">This document contains the cross border schedules for all the borders of a given country where energy is exchanged.</skos:definition>
  </skos:Concept>
  <skos:Concept rdf:about="http://data.europa.eu/energy/StandardMessageTypeList/A31">
    <skos:inScheme rdf:resource="http://data.europa.eu/energy/StandardMessageTypeList"/>
    <skos:topConceptOf rdf:resource="http://data.europa.eu/energy/StandardMessageTypeList"/>
    <dc:identifier>A31</dc:identifier>
    <skos:prefLabel>Agreed capacity</skos:prefLabel>
    <skos:definition xml:lang="en">The capacity agreed between parties.</skos:definition>
  </skos:Concept>
  <skos:Concept rdf:about="http://data.europa.eu/energy/StandardMessageTypeList/A32">
    <skos:inScheme rdf:resource="http://data.europa.eu/energy/StandardMessageTypeList"/>
    <skos:topConceptOf rdf:resource="http://data.europa.eu/energy/StandardMessageTypeList"/>
    <dc:identifier>A32</dc:identifier>
    <skos:prefLabel>Proposed capacity</skos:prefLabel>
    <skos:definition xml:lang="en">The capacity proposed for agreement between parties.</skos:definition>
  </skos:Concept>
  <skos:Concept rdf:about="http://data.europa.eu/energy/StandardMessageTypeList/A33">
    <skos:inScheme rdf:resource="http://data.europa.eu/energy/StandardMessageTypeList"/>
    <skos:topConceptOf rdf:resource="http://data.europa.eu/energy/StandardMessageTypeList"/>
    <dc:identifier>A33</dc:identifier>
    <skos:prefLabel>System vertical load</skos:prefLabel>
    <skos:definition xml:lang="en">The sum of all flows out of the transmission grid via directly connected transformers and lines to distribution grids and end consumers as known by the System Operator.</skos:definition>
  </skos:Concept>
  <skos:Concept rdf:about="http://data.europa.eu/energy/StandardMessageTypeList/A34">
    <skos:inScheme rdf:resource="http://data.europa.eu/energy/StandardMessageTypeList"/>
    <skos:topConceptOf rdf:resource="http://data.europa.eu/energy/StandardMessageTypeList"/>
    <dc:identifier>A34</dc:identifier>
    <skos:prefLabel>Escalation document</skos:prefLabel>
    <skos:definition xml:lang="en">A document which requesting the escalation of a situation.</skos:definition>
  </skos:Concept>
  <skos:Concept rdf:about="http://data.europa.eu/energy/StandardMessageTypeList/A35">
    <skos:inScheme rdf:resource="http://data.europa.eu/energy/StandardMessageTypeList"/>
    <skos:topConceptOf rdf:resource="http://data.europa.eu/energy/StandardMessageTypeList"/>
    <dc:identifier>A35</dc:identifier>
    <skos:prefLabel>Trouble shooting document</skos:prefLabel>
    <skos:definition xml:lang="en">A document providing trouble shooting information for the resolution of a problem.</skos:definition>
  </skos:Concept>
  <skos:Concept rdf:about="http://data.europa.eu/energy/StandardMessageTypeList/A36">
    <skos:inScheme rdf:resource="http://data.europa.eu/energy/StandardMessageTypeList"/>
    <skos:topConceptOf rdf:resource="http://data.europa.eu/energy/StandardMessageTypeList"/>
    <dc:identifier>A36</dc:identifier>
    <skos:prefLabel>Deactivation document</skos:prefLabel>
    <skos:definition xml:lang="en">A document providing deactivation information.</skos:definition>
  </skos:Concept>
  <skos:Concept rdf:about="http://data.europa.eu/energy/StandardMessageTypeList/A37">
    <skos:inScheme rdf:resource="http://data.europa.eu/energy/StandardMessageTypeList"/>
    <skos:topConceptOf rdf:resource="http://data.europa.eu/energy/StandardMessageTypeList"/>
    <dc:identifier>A37</dc:identifier>
    <skos:prefLabel>Reserve tender document</skos:prefLabel>
    <skos:definition xml:lang="en">The document that is used for the tendering for reserves within the ERRP process.</skos:definition>
  </skos:Concept>
  <skos:Concept rdf:about="http://data.europa.eu/energy/StandardMessageTypeList/A38">
    <skos:inScheme rdf:resource="http://data.europa.eu/energy/StandardMessageTypeList"/>
    <skos:topConceptOf rdf:resource="http://data.europa.eu/energy/StandardMessageTypeList"/>
    <dc:identifier>A38</dc:identifier>
    <skos:prefLabel>Reserve Allocation Result Document</skos:prefLabel>
    <skos:definition xml:lang="en">The document used to provide the results of a Reserve auction.</skos:definition>
  </skos:Concept>
  <skos:Concept rdf:about="http://data.europa.eu/energy/StandardMessageTypeList/A39">
    <skos:inScheme rdf:resource="http://data.europa.eu/energy/StandardMessageTypeList"/>
    <skos:topConceptOf rdf:resource="http://data.europa.eu/energy/StandardMessageTypeList"/>
    <dc:identifier>A39</dc:identifier>
    <skos:prefLabel>SATCR activation</skos:prefLabel>
    <skos:definition xml:lang="en">The document is used to provide the activation of reserves through the SATCR process.</skos:definition>
  </skos:Concept>
  <skos:Concept rdf:about="http://data.europa.eu/energy/StandardMessageTypeList/A40">
    <skos:inScheme rdf:resource="http://data.europa.eu/energy/StandardMessageTypeList"/>
    <skos:topConceptOf rdf:resource="http://data.europa.eu/energy/StandardMessageTypeList"/>
    <dc:identifier>A40</dc:identifier>
    <skos:prefLabel>DATCR activation</skos:prefLabel>
    <skos:definition xml:lang="en">The document is used to provide the activation of reserves through the DATCR process.</skos:definition>
  </skos:Concept>
  <skos:Concept rdf:about="http://data.europa.eu/energy/StandardMessageTypeList/A41">
    <skos:inScheme rdf:resource="http://data.europa.eu/energy/StandardMessageTypeList"/>
    <skos:topConceptOf rdf:resource="http://data.europa.eu/energy/StandardMessageTypeList"/>
    <dc:identifier>A41</dc:identifier>
    <skos:prefLabel>Activation response</skos:prefLabel>
    <skos:definition xml:lang="en">The document is used to provide a response to a request to activate reserves.</skos:definition>
  </skos:Concept>
  <skos:Concept rdf:about="http://data.europa.eu/energy/StandardMessageTypeList/A42">
    <skos:inScheme rdf:resource="http://data.europa.eu/energy/StandardMessageTypeList"/>
    <skos:topConceptOf rdf:resource="http://data.europa.eu/energy/StandardMessageTypeList"/>
    <dc:identifier>A42</dc:identifier>
    <skos:prefLabel>Tender reduction</skos:prefLabel>
    <skos:definition xml:lang="en">The document is used to provide information concerning the reduction of a previously submitted tender.</skos:definition>
  </skos:Concept>
  <skos:Concept rdf:about="http://data.europa.eu/energy/StandardMessageTypeList/A43">
    <skos:inScheme rdf:resource="http://data.europa.eu/energy/StandardMessageTypeList"/>
    <skos:topConceptOf rdf:resource="http://data.europa.eu/energy/StandardMessageTypeList"/>
    <dc:identifier>A43</dc:identifier>
    <skos:prefLabel>MOL Document</skos:prefLabel>
    <skos:definition xml:lang="en">The document is used to provide Merit Order List information.</skos:definition>
  </skos:Concept>
  <skos:Concept rdf:about="http://data.europa.eu/energy/StandardMessageTypeList/A44">
    <skos:inScheme rdf:resource="http://data.europa.eu/energy/StandardMessageTypeList"/>
    <skos:topConceptOf rdf:resource="http://data.europa.eu/energy/StandardMessageTypeList"/>
    <dc:identifier>A44</dc:identifier>
    <skos:prefLabel>Price Document</skos:prefLabel>
    <skos:definition xml:lang="en">The document is used to provide market price information.</skos:definition>
  </skos:Concept>
  <skos:Concept rdf:about="http://data.europa.eu/energy/StandardMessageTypeList/A45">
    <skos:inScheme rdf:resource="http://data.europa.eu/energy/StandardMessageTypeList"/>
    <skos:topConceptOf rdf:resource="http://data.europa.eu/energy/StandardMessageTypeList"/>
    <dc:identifier>A45</dc:identifier>
    <skos:prefLabel>Measurement Value Document</skos:prefLabel>
    <skos:definition xml:lang="en">The document is used to provide measurement information from measurement devices.</skos:definition>
  </skos:Concept>
  <skos:Concept rdf:about="http://data.europa.eu/energy/StandardMessageTypeList/A46">
    <skos:inScheme rdf:resource="http://data.europa.eu/energy/StandardMessageTypeList"/>
    <skos:topConceptOf rdf:resource="http://data.europa.eu/energy/StandardMessageTypeList"/>
    <dc:identifier>A46</dc:identifier>
    <skos:prefLabel>SOAM Document</skos:prefLabel>
    <skos:definition xml:lang="en">The document is used to provide system operator accounting data for matching.</skos:definition>
  </skos:Concept>
  <skos:Concept rdf:about="http://data.europa.eu/energy/StandardMessageTypeList/A47">
    <skos:inScheme rdf:resource="http://data.europa.eu/energy/StandardMessageTypeList"/>
    <skos:topConceptOf rdf:resource="http://data.europa.eu/energy/StandardMessageTypeList"/>
    <dc:identifier>A47</dc:identifier>
    <skos:prefLabel>SOVA Document</skos:prefLabel>
    <skos:definition xml:lang="en">The document is used to provide system operator validated accounting data.</skos:definition>
  </skos:Concept>
  <skos:Concept rdf:about="http://data.europa.eu/energy/StandardMessageTypeList/A48">
    <skos:inScheme rdf:resource="http://data.europa.eu/energy/StandardMessageTypeList"/>
    <skos:topConceptOf rdf:resource="http://data.europa.eu/energy/StandardMessageTypeList"/>
    <dc:identifier>A48</dc:identifier>
    <skos:prefLabel>CCVA Document</skos:prefLabel>
    <skos:definition xml:lang="en">The document is used to provide coordination center validated accounting data.</skos:definition>
  </skos:Concept>
  <skos:Concept rdf:about="http://data.europa.eu/energy/StandardMessageTypeList/A49">
    <skos:inScheme rdf:resource="http://data.europa.eu/energy/StandardMessageTypeList"/>
    <skos:topConceptOf rdf:resource="http://data.europa.eu/energy/StandardMessageTypeList"/>
    <dc:identifier>A49</dc:identifier>
    <skos:prefLabel>Daily settlement document</skos:prefLabel>
    <skos:definition xml:lang="en">The document is used to provide daily settlement information.</skos:definition>
  </skos:Concept>
  <skos:Concept rdf:about="http://data.europa.eu/energy/StandardMessageTypeList/A50">
    <skos:inScheme rdf:resource="http://data.europa.eu/energy/StandardMessageTypeList"/>
    <skos:topConceptOf rdf:resource="http://data.europa.eu/energy/StandardMessageTypeList"/>
    <dc:identifier>A50</dc:identifier>
    <skos:prefLabel>Weekly settlement document</skos:prefLabel>
    <skos:definition xml:lang="en">The document is used to provide weekly settlement information.</skos:definition>
  </skos:Concept>
  <skos:Concept rdf:about="http://data.europa.eu/energy/StandardMessageTypeList/A51">
    <skos:inScheme rdf:resource="http://data.europa.eu/energy/StandardMessageTypeList"/>
    <skos:topConceptOf rdf:resource="http://data.europa.eu/energy/StandardMessageTypeList"/>
    <dc:identifier>A51</dc:identifier>
    <skos:prefLabel>Capacity Auction Specification Document</skos:prefLabel>
    <skos:definition xml:lang="en">The document is used to provide capacity auction specification information.</skos:definition>
  </skos:Concept>
  <skos:Concept rdf:about="http://data.europa.eu/energy/StandardMessageTypeList/A52">
    <skos:inScheme rdf:resource="http://data.europa.eu/energy/StandardMessageTypeList"/>
    <skos:topConceptOf rdf:resource="http://data.europa.eu/energy/StandardMessageTypeList"/>
    <dc:identifier>A52</dc:identifier>
    <skos:prefLabel>Market Coupling Results Document</skos:prefLabel>
    <skos:definition xml:lang="en">The document is used to provide the results of a market coupling auction.</skos:definition>
  </skos:Concept>
  <skos:Concept rdf:about="http://data.europa.eu/energy/StandardMessageTypeList/A53">
    <skos:inScheme rdf:resource="http://data.europa.eu/energy/StandardMessageTypeList"/>
    <skos:topConceptOf rdf:resource="http://data.europa.eu/energy/StandardMessageTypeList"/>
    <dc:identifier>A53</dc:identifier>
    <skos:prefLabel>Outage publication Document</skos:prefLabel>
    <skos:definition xml:lang="en">The document is used to provide the outage information for publication.</skos:definition>
  </skos:Concept>
  <skos:Concept rdf:about="http://data.europa.eu/energy/StandardMessageTypeList/A54">
    <skos:inScheme rdf:resource="http://data.europa.eu/energy/StandardMessageTypeList"/>
    <skos:topConceptOf rdf:resource="http://data.europa.eu/energy/StandardMessageTypeList"/>
    <dc:identifier>A54</dc:identifier>
    <skos:prefLabel>Forced generation outage Document</skos:prefLabel>
    <skos:definition xml:lang="en">A document providing information on forced generation outages.</skos:definition>
  </skos:Concept>
  <skos:Concept rdf:about="http://data.europa.eu/energy/StandardMessageTypeList/A55">
    <skos:inScheme rdf:resource="http://data.europa.eu/energy/StandardMessageTypeList"/>
    <skos:topConceptOf rdf:resource="http://data.europa.eu/energy/StandardMessageTypeList"/>
    <dc:identifier>A55</dc:identifier>
    <skos:prefLabel>Summarised Market Schedule</skos:prefLabel>
    <skos:definition xml:lang="en">A compilation of all external schedules concerning two Market Balance Areas of all balance responsible parties.</skos:definition>
  </skos:Concept>
  <skos:Concept rdf:about="http://data.europa.eu/energy/StandardMessageTypeList/A56">
    <skos:inScheme rdf:resource="http://data.europa.eu/energy/StandardMessageTypeList"/>
    <skos:topConceptOf rdf:resource="http://data.europa.eu/energy/StandardMessageTypeList"/>
    <dc:identifier>A56</dc:identifier>
    <skos:prefLabel>Compensation Program Schedule</skos:prefLabel>
    <skos:definition xml:lang="en">A schedule that provides the schedule information for the compensation of unintended deviation.</skos:definition>
  </skos:Concept>
  <skos:Concept rdf:about="http://data.europa.eu/energy/StandardMessageTypeList/A57">
    <skos:inScheme rdf:resource="http://data.europa.eu/energy/StandardMessageTypeList"/>
    <skos:topConceptOf rdf:resource="http://data.europa.eu/energy/StandardMessageTypeList"/>
    <dc:identifier>A57</dc:identifier>
    <skos:prefLabel>Load Frequency Control Program Schedule</skos:prefLabel>
    <skos:definition xml:lang="en">A schedule that provides the schedule information for the Load Frequency Control Program of a Control Area or a Control Block.</skos:definition>
  </skos:Concept>
  <skos:Concept rdf:about="http://data.europa.eu/energy/StandardMessageTypeList/A58">
    <skos:inScheme rdf:resource="http://data.europa.eu/energy/StandardMessageTypeList"/>
    <skos:topConceptOf rdf:resource="http://data.europa.eu/energy/StandardMessageTypeList"/>
    <dc:identifier>A58</dc:identifier>
    <skos:prefLabel>Timeframe Independent Schedule</skos:prefLabel>
    <skos:definition xml:lang="en">A compilation of all external Timeframe Independent Schedules concerning two System Operators.</skos:definition>
  </skos:Concept>
  <skos:Concept rdf:about="http://data.europa.eu/energy/StandardMessageTypeList/A59">
    <skos:inScheme rdf:resource="http://data.europa.eu/energy/StandardMessageTypeList"/>
    <skos:topConceptOf rdf:resource="http://data.europa.eu/energy/StandardMessageTypeList"/>
    <dc:identifier>A59</dc:identifier>
    <skos:prefLabel>Information request</skos:prefLabel>
    <skos:definition xml:lang="en">An information request being made concerning some specific information.</skos:definition>
  </skos:Concept>
  <skos:Concept rdf:about="http://data.europa.eu/energy/StandardMessageTypeList/A60">
    <skos:inScheme rdf:resource="http://data.europa.eu/energy/StandardMessageTypeList"/>
    <skos:topConceptOf rdf:resource="http://data.europa.eu/energy/StandardMessageTypeList"/>
    <dc:identifier>A60</dc:identifier>
    <skos:prefLabel>status request for a position independently from a specific process</skos:prefLabel>
    <skos:definition xml:lang="en">A status request concerning the position of an object independently of any ongoing processes.</skos:definition>
  </skos:Concept>
  <skos:Concept rdf:about="http://data.europa.eu/energy/StandardMessageTypeList/A61">
    <skos:inScheme rdf:resource="http://data.europa.eu/energy/StandardMessageTypeList"/>
    <skos:topConceptOf rdf:resource="http://data.europa.eu/energy/StandardMessageTypeList"/>
    <dc:identifier>A61</dc:identifier>
    <skos:prefLabel>Estimated Net Transfer Capacity</skos:prefLabel>
    <skos:definition xml:lang="en">The estimated net transfer capacity for a given border.</skos:definition>
  </skos:Concept>
  <skos:Concept rdf:about="http://data.europa.eu/energy/StandardMessageTypeList/A62">
    <skos:inScheme rdf:resource="http://data.europa.eu/energy/StandardMessageTypeList"/>
    <skos:topConceptOf rdf:resource="http://data.europa.eu/energy/StandardMessageTypeList"/>
    <dc:identifier>A62</dc:identifier>
    <skos:prefLabel>Compensation rights</skos:prefLabel>
    <skos:definition xml:lang="en">The capacity rights that have been allocated as compensation.</skos:definition>
  </skos:Concept>
  <skos:Concept rdf:about="http://data.europa.eu/energy/StandardMessageTypeList/A63">
    <skos:inScheme rdf:resource="http://data.europa.eu/energy/StandardMessageTypeList"/>
    <skos:topConceptOf rdf:resource="http://data.europa.eu/energy/StandardMessageTypeList"/>
    <dc:identifier>A63</dc:identifier>
    <skos:prefLabel>Redispatch notice</skos:prefLabel>
    <skos:definition xml:lang="en">A notice to confirm the actions agreed between System Operators to resolve a congestion situation through redispatch.</skos:definition>
  </skos:Concept>
  <skos:Concept rdf:about="http://data.europa.eu/energy/StandardMessageTypeList/A64">
    <skos:inScheme rdf:resource="http://data.europa.eu/energy/StandardMessageTypeList"/>
    <skos:topConceptOf rdf:resource="http://data.europa.eu/energy/StandardMessageTypeList"/>
    <dc:identifier>A64</dc:identifier>
    <skos:prefLabel>Tender reduction response</skos:prefLabel>
    <skos:definition xml:lang="en">A response to a tender reduction request that provides  corrections to the initial document.</skos:definition>
  </skos:Concept>
  <skos:Concept rdf:about="http://data.europa.eu/energy/StandardMessageTypeList/A65">
    <skos:inScheme rdf:resource="http://data.europa.eu/energy/StandardMessageTypeList"/>
    <skos:topConceptOf rdf:resource="http://data.europa.eu/energy/StandardMessageTypeList"/>
    <dc:identifier>A65</dc:identifier>
    <skos:prefLabel>System total load</skos:prefLabel>
    <skos:definition xml:lang="en">Total load', including losses without power used for energy storage, is equal to generation deducted with exports, added with imports and deducted with power used for energy storage.</skos:definition>
  </skos:Concept>
  <skos:Concept rdf:about="http://data.europa.eu/energy/StandardMessageTypeList/A66">
    <skos:inScheme rdf:resource="http://data.europa.eu/energy/StandardMessageTypeList"/>
    <skos:topConceptOf rdf:resource="http://data.europa.eu/energy/StandardMessageTypeList"/>
    <dc:identifier>A66</dc:identifier>
    <skos:prefLabel>Final MOL</skos:prefLabel>
    <skos:definition xml:lang="en">A document providing the information concerning the situation of the MOL at the end of an activation period.</skos:definition>
  </skos:Concept>
  <skos:Concept rdf:about="http://data.europa.eu/energy/StandardMessageTypeList/A67">
    <skos:inScheme rdf:resource="http://data.europa.eu/energy/StandardMessageTypeList"/>
    <skos:topConceptOf rdf:resource="http://data.europa.eu/energy/StandardMessageTypeList"/>
    <dc:identifier>A67</dc:identifier>
    <skos:prefLabel>Resource Provider Schedule for production/consumption</skos:prefLabel>
    <skos:definition xml:lang="en">A document providing the schedules for production/consumption for resource objects submitted by a resource provider.</skos:definition>
  </skos:Concept>
  <skos:Concept rdf:about="http://data.europa.eu/energy/StandardMessageTypeList/A68">
    <skos:inScheme rdf:resource="http://data.europa.eu/energy/StandardMessageTypeList"/>
    <skos:topConceptOf rdf:resource="http://data.europa.eu/energy/StandardMessageTypeList"/>
    <dc:identifier>A68</dc:identifier>
    <skos:prefLabel>Installed generation per type</skos:prefLabel>
    <skos:definition xml:lang="en">A document providing the installed generation per generation type.</skos:definition>
  </skos:Concept>
  <skos:Concept rdf:about="http://data.europa.eu/energy/StandardMessageTypeList/A69">
    <skos:inScheme rdf:resource="http://data.europa.eu/energy/StandardMessageTypeList"/>
    <skos:topConceptOf rdf:resource="http://data.europa.eu/energy/StandardMessageTypeList"/>
    <dc:identifier>A69</dc:identifier>
    <skos:prefLabel>Wind and solar forecast</skos:prefLabel>
    <skos:definition xml:lang="en">A document providing the forecast of wind and solar generation.</skos:definition>
  </skos:Concept>
  <skos:Concept rdf:about="http://data.europa.eu/energy/StandardMessageTypeList/A70">
    <skos:inScheme rdf:resource="http://data.europa.eu/energy/StandardMessageTypeList"/>
    <skos:topConceptOf rdf:resource="http://data.europa.eu/energy/StandardMessageTypeList"/>
    <dc:identifier>A70</dc:identifier>
    <skos:prefLabel>Load forecast margin</skos:prefLabel>
    <skos:definition xml:lang="en">A document providing the load forecast margin for a period.</skos:definition>
  </skos:Concept>
  <skos:Concept rdf:about="http://data.europa.eu/energy/StandardMessageTypeList/A71">
    <skos:inScheme rdf:resource="http://data.europa.eu/energy/StandardMessageTypeList"/>
    <skos:topConceptOf rdf:resource="http://data.europa.eu/energy/StandardMessageTypeList"/>
    <dc:identifier>A71</dc:identifier>
    <skos:prefLabel>Generation forecast</skos:prefLabel>
    <skos:definition xml:lang="en">A document providing the generation forecast for a period.</skos:definition>
  </skos:Concept>
  <skos:Concept rdf:about="http://data.europa.eu/energy/StandardMessageTypeList/A72">
    <skos:inScheme rdf:resource="http://data.europa.eu/energy/StandardMessageTypeList"/>
    <skos:topConceptOf rdf:resource="http://data.europa.eu/energy/StandardMessageTypeList"/>
    <dc:identifier>A72</dc:identifier>
    <skos:prefLabel>Reservoir filling information</skos:prefLabel>
    <skos:definition xml:lang="en">A document providing information concerning the filling of reservoirs.</skos:definition>
  </skos:Concept>
  <skos:Concept rdf:about="http://data.europa.eu/energy/StandardMessageTypeList/A73">
    <skos:inScheme rdf:resource="http://data.europa.eu/energy/StandardMessageTypeList"/>
    <skos:topConceptOf rdf:resource="http://data.europa.eu/energy/StandardMessageTypeList"/>
    <dc:identifier>A73</dc:identifier>
    <skos:prefLabel>Actual generation</skos:prefLabel>
    <skos:definition xml:lang="en">A document providing the actual generation for a period.</skos:definition>
  </skos:Concept>
  <skos:Concept rdf:about="http://data.europa.eu/energy/StandardMessageTypeList/A74">
    <skos:inScheme rdf:resource="http://data.europa.eu/energy/StandardMessageTypeList"/>
    <skos:topConceptOf rdf:resource="http://data.europa.eu/energy/StandardMessageTypeList"/>
    <dc:identifier>A74</dc:identifier>
    <skos:prefLabel>Wind and solar generation</skos:prefLabel>
    <skos:definition xml:lang="en">A document providing the generation of wind and solar energy for a period.</skos:definition>
  </skos:Concept>
  <skos:Concept rdf:about="http://data.europa.eu/energy/StandardMessageTypeList/A75">
    <skos:inScheme rdf:resource="http://data.europa.eu/energy/StandardMessageTypeList"/>
    <skos:topConceptOf rdf:resource="http://data.europa.eu/energy/StandardMessageTypeList"/>
    <dc:identifier>A75</dc:identifier>
    <skos:prefLabel>Actual generation per type</skos:prefLabel>
    <skos:definition xml:lang="en">A document providing the actual generation per generation type for a period.</skos:definition>
  </skos:Concept>
  <skos:Concept rdf:about="http://data.europa.eu/energy/StandardMessageTypeList/A76">
    <skos:inScheme rdf:resource="http://data.europa.eu/energy/StandardMessageTypeList"/>
    <skos:topConceptOf rdf:resource="http://data.europa.eu/energy/StandardMessageTypeList"/>
    <dc:identifier>A76</dc:identifier>
    <skos:prefLabel>Load unavailability</skos:prefLabel>
    <skos:definition xml:lang="en">A document providing the unavailability of units providing load on the network.</skos:definition>
  </skos:Concept>
  <skos:Concept rdf:about="http://data.europa.eu/energy/StandardMessageTypeList/A77">
    <skos:inScheme rdf:resource="http://data.europa.eu/energy/StandardMessageTypeList"/>
    <skos:topConceptOf rdf:resource="http://data.europa.eu/energy/StandardMessageTypeList"/>
    <dc:identifier>A77</dc:identifier>
    <skos:prefLabel>Production unavailability</skos:prefLabel>
    <skos:definition xml:lang="en">A document providing the unavailability of production units providing energy to the network.</skos:definition>
  </skos:Concept>
  <skos:Concept rdf:about="http://data.europa.eu/energy/StandardMessageTypeList/A78">
    <skos:inScheme rdf:resource="http://data.europa.eu/energy/StandardMessageTypeList"/>
    <skos:topConceptOf rdf:resource="http://data.europa.eu/energy/StandardMessageTypeList"/>
    <dc:identifier>A78</dc:identifier>
    <skos:prefLabel>Transmission unavailability</skos:prefLabel>
    <skos:definition xml:lang="en">A document providing the unavailability of transmission capacity on the network.</skos:definition>
  </skos:Concept>
  <skos:Concept rdf:about="http://data.europa.eu/energy/StandardMessageTypeList/A79">
    <skos:inScheme rdf:resource="http://data.europa.eu/energy/StandardMessageTypeList"/>
    <skos:topConceptOf rdf:resource="http://data.europa.eu/energy/StandardMessageTypeList"/>
    <dc:identifier>A79</dc:identifier>
    <skos:prefLabel>Offshore grid infrastructure unavailability</skos:prefLabel>
    <skos:definition xml:lang="en">A document providing the unavailability of an offshore grid infrastructure to the network.</skos:definition>
  </skos:Concept>
  <skos:Concept rdf:about="http://data.europa.eu/energy/StandardMessageTypeList/A80">
    <skos:inScheme rdf:resource="http://data.europa.eu/energy/StandardMessageTypeList"/>
    <skos:topConceptOf rdf:resource="http://data.europa.eu/energy/StandardMessageTypeList"/>
    <dc:identifier>A80</dc:identifier>
    <skos:prefLabel>Generation unavailability</skos:prefLabel>
    <skos:definition xml:lang="en">A document providing the unavailability of generation units providing energy to the network.</skos:definition>
  </skos:Concept>
  <skos:Concept rdf:about="http://data.europa.eu/energy/StandardMessageTypeList/A81">
    <skos:inScheme rdf:resource="http://data.europa.eu/energy/StandardMessageTypeList"/>
    <skos:topConceptOf rdf:resource="http://data.europa.eu/energy/StandardMessageTypeList"/>
    <dc:identifier>A81</dc:identifier>
    <skos:prefLabel>Contracted reserves</skos:prefLabel>
    <skos:definition xml:lang="en">A document providing the reserves contracted for a period.</skos:definition>
  </skos:Concept>
  <skos:Concept rdf:about="http://data.europa.eu/energy/StandardMessageTypeList/A82">
    <skos:inScheme rdf:resource="http://data.europa.eu/energy/StandardMessageTypeList"/>
    <skos:topConceptOf rdf:resource="http://data.europa.eu/energy/StandardMessageTypeList"/>
    <dc:identifier>A82</dc:identifier>
    <skos:prefLabel>Accepted offers</skos:prefLabel>
    <skos:definition xml:lang="en">A document providing the offers of reserves that have been accepted for a period.</skos:definition>
  </skos:Concept>
  <skos:Concept rdf:about="http://data.europa.eu/energy/StandardMessageTypeList/A83">
    <skos:inScheme rdf:resource="http://data.europa.eu/energy/StandardMessageTypeList"/>
    <skos:topConceptOf rdf:resource="http://data.europa.eu/energy/StandardMessageTypeList"/>
    <dc:identifier>A83</dc:identifier>
    <skos:prefLabel>Activated balancing quantities</skos:prefLabel>
    <skos:definition xml:lang="en">A document providing the quantities of reserves that have been activated for balancing.</skos:definition>
  </skos:Concept>
  <skos:Concept rdf:about="http://data.europa.eu/energy/StandardMessageTypeList/A84">
    <skos:inScheme rdf:resource="http://data.europa.eu/energy/StandardMessageTypeList"/>
    <skos:topConceptOf rdf:resource="http://data.europa.eu/energy/StandardMessageTypeList"/>
    <dc:identifier>A84</dc:identifier>
    <skos:prefLabel>Activated balancing prices</skos:prefLabel>
    <skos:definition xml:lang="en">A document providing the prices of the reserves that have been activated for balancing.</skos:definition>
  </skos:Concept>
  <skos:Concept rdf:about="http://data.europa.eu/energy/StandardMessageTypeList/A85">
    <skos:inScheme rdf:resource="http://data.europa.eu/energy/StandardMessageTypeList"/>
    <skos:topConceptOf rdf:resource="http://data.europa.eu/energy/StandardMessageTypeList"/>
    <dc:identifier>A85</dc:identifier>
    <skos:prefLabel>Imbalance prices</skos:prefLabel>
    <skos:definition xml:lang="en">A document providing the prices of reserves due to imbalance for a period.</skos:definition>
  </skos:Concept>
  <skos:Concept rdf:about="http://data.europa.eu/energy/StandardMessageTypeList/A86">
    <skos:inScheme rdf:resource="http://data.europa.eu/energy/StandardMessageTypeList"/>
    <skos:topConceptOf rdf:resource="http://data.europa.eu/energy/StandardMessageTypeList"/>
    <dc:identifier>A86</dc:identifier>
    <skos:prefLabel>Imbalance volume</skos:prefLabel>
    <skos:definition xml:lang="en">A document providing the volume of the imbalance for a period.</skos:definition>
  </skos:Concept>
  <skos:Concept rdf:about="http://data.europa.eu/energy/StandardMessageTypeList/A87">
    <skos:inScheme rdf:resource="http://data.europa.eu/energy/StandardMessageTypeList"/>
    <skos:topConceptOf rdf:resource="http://data.europa.eu/energy/StandardMessageTypeList"/>
    <dc:identifier>A87</dc:identifier>
    <skos:prefLabel>Financial situation</skos:prefLabel>
    <skos:definition xml:lang="en">A document providing the financial situation for reserves.</skos:definition>
  </skos:Concept>
  <skos:Concept rdf:about="http://data.europa.eu/energy/StandardMessageTypeList/A88">
    <skos:inScheme rdf:resource="http://data.europa.eu/energy/StandardMessageTypeList"/>
    <skos:topConceptOf rdf:resource="http://data.europa.eu/energy/StandardMessageTypeList"/>
    <dc:identifier>A88</dc:identifier>
    <skos:prefLabel>Cross border balancing</skos:prefLabel>
    <skos:definition xml:lang="en">A document providing the cross border balancing requirements for a period.</skos:definition>
  </skos:Concept>
  <skos:Concept rdf:about="http://data.europa.eu/energy/StandardMessageTypeList/A89">
    <skos:inScheme rdf:resource="http://data.europa.eu/energy/StandardMessageTypeList"/>
    <skos:topConceptOf rdf:resource="http://data.europa.eu/energy/StandardMessageTypeList"/>
    <dc:identifier>A89</dc:identifier>
    <skos:prefLabel>Contracted reserve prices</skos:prefLabel>
    <skos:definition xml:lang="en">A document providing the price of reserves contracted for a period.</skos:definition>
  </skos:Concept>
  <skos:Concept rdf:about="http://data.europa.eu/energy/StandardMessageTypeList/A90">
    <skos:inScheme rdf:resource="http://data.europa.eu/energy/StandardMessageTypeList"/>
    <skos:topConceptOf rdf:resource="http://data.europa.eu/energy/StandardMessageTypeList"/>
    <dc:identifier>A90</dc:identifier>
    <skos:prefLabel>Interconnection network expansion</skos:prefLabel>
    <skos:definition xml:lang="en">A document providing information on the expansion of the interconnection network.</skos:definition>
  </skos:Concept>
  <skos:Concept rdf:about="http://data.europa.eu/energy/StandardMessageTypeList/A91">
    <skos:inScheme rdf:resource="http://data.europa.eu/energy/StandardMessageTypeList"/>
    <skos:topConceptOf rdf:resource="http://data.europa.eu/energy/StandardMessageTypeList"/>
    <dc:identifier>A91</dc:identifier>
    <skos:prefLabel>Counter trade notice</skos:prefLabel>
    <skos:definition xml:lang="en">A document providing information on counter trades for a period.</skos:definition>
  </skos:Concept>
  <skos:Concept rdf:about="http://data.europa.eu/energy/StandardMessageTypeList/A92">
    <skos:inScheme rdf:resource="http://data.europa.eu/energy/StandardMessageTypeList"/>
    <skos:topConceptOf rdf:resource="http://data.europa.eu/energy/StandardMessageTypeList"/>
    <dc:identifier>A92</dc:identifier>
    <skos:prefLabel>Congestion costs</skos:prefLabel>
    <skos:definition xml:lang="en">A document providing the cost of congestion for a period.</skos:definition>
  </skos:Concept>
  <skos:Concept rdf:about="http://data.europa.eu/energy/StandardMessageTypeList/A93">
    <skos:inScheme rdf:resource="http://data.europa.eu/energy/StandardMessageTypeList"/>
    <skos:topConceptOf rdf:resource="http://data.europa.eu/energy/StandardMessageTypeList"/>
    <dc:identifier>A93</dc:identifier>
    <skos:prefLabel>DC link capacity</skos:prefLabel>
    <skos:definition xml:lang="en">A document providing the DC links for a period.</skos:definition>
  </skos:Concept>
  <skos:Concept rdf:about="http://data.europa.eu/energy/StandardMessageTypeList/A94">
    <skos:inScheme rdf:resource="http://data.europa.eu/energy/StandardMessageTypeList"/>
    <skos:topConceptOf rdf:resource="http://data.europa.eu/energy/StandardMessageTypeList"/>
    <dc:identifier>A94</dc:identifier>
    <skos:prefLabel>Non EU allocations</skos:prefLabel>
    <skos:definition xml:lang="en">A document providing allocations made to non EU member states.</skos:definition>
  </skos:Concept>
  <skos:Concept rdf:about="http://data.europa.eu/energy/StandardMessageTypeList/A95">
    <skos:inScheme rdf:resource="http://data.europa.eu/energy/StandardMessageTypeList"/>
    <skos:topConceptOf rdf:resource="http://data.europa.eu/energy/StandardMessageTypeList"/>
    <dc:identifier>A95</dc:identifier>
    <skos:prefLabel>Configuration document</skos:prefLabel>
    <skos:definition xml:lang="en">A document providing configuration information.</skos:definition>
  </skos:Concept>
  <skos:Concept rdf:about="http://data.europa.eu/energy/StandardMessageTypeList/A96">
    <skos:inScheme rdf:resource="http://data.europa.eu/energy/StandardMessageTypeList"/>
    <skos:topConceptOf rdf:resource="http://data.europa.eu/energy/StandardMessageTypeList"/>
    <dc:identifier>A96</dc:identifier>
    <skos:prefLabel>Redispatch activation document</skos:prefLabel>
    <skos:definition xml:lang="en">A document enabling the activation of a redispatch notice.</skos:definition>
  </skos:Concept>
  <skos:Concept rdf:about="http://data.europa.eu/energy/StandardMessageTypeList/A97">
    <skos:inScheme rdf:resource="http://data.europa.eu/energy/StandardMessageTypeList"/>
    <skos:topConceptOf rdf:resource="http://data.europa.eu/energy/StandardMessageTypeList"/>
    <dc:identifier>A97</dc:identifier>
    <skos:prefLabel>Detailed activation history document</skos:prefLabel>
    <skos:definition xml:lang="en">A document enabling a detailed history of activations.</skos:definition>
  </skos:Concept>
  <skos:Concept rdf:about="http://data.europa.eu/energy/StandardMessageTypeList/A98">
    <skos:inScheme rdf:resource="http://data.europa.eu/energy/StandardMessageTypeList"/>
    <skos:topConceptOf rdf:resource="http://data.europa.eu/energy/StandardMessageTypeList"/>
    <dc:identifier>A98</dc:identifier>
    <skos:prefLabel>Aggregated activation history document</skos:prefLabel>
    <skos:definition xml:lang="en">A document enabling an aggregated history of activations.</skos:definition>
  </skos:Concept>
  <skos:Concept rdf:about="http://data.europa.eu/energy/StandardMessageTypeList/A99">
    <skos:inScheme rdf:resource="http://data.europa.eu/energy/StandardMessageTypeList"/>
    <skos:topConceptOf rdf:resource="http://data.europa.eu/energy/StandardMessageTypeList"/>
    <dc:identifier>A99</dc:identifier>
    <skos:prefLabel>HVDC Link constraints</skos:prefLabel>
    <skos:definition xml:lang="en">A document providing the information concerning the maximum and minimum active power flow through each link can limited.</skos:definition>
  </skos:Concept>
  <skos:Concept rdf:about="http://data.europa.eu/energy/StandardMessageTypeList/B01">
    <skos:inScheme rdf:resource="http://data.europa.eu/energy/StandardMessageTypeList"/>
    <skos:topConceptOf rdf:resource="http://data.europa.eu/energy/StandardMessageTypeList"/>
    <dc:identifier>B01</dc:identifier>
    <skos:prefLabel>HVDC Configuration</skos:prefLabel>
    <skos:definition xml:lang="en">A document providing the information concerning the power set point. The mode in which the  HVDC is managed.</skos:definition>
  </skos:Concept>
  <skos:Concept rdf:about="http://data.europa.eu/energy/StandardMessageTypeList/B02">
    <skos:inScheme rdf:resource="http://data.europa.eu/energy/StandardMessageTypeList"/>
    <skos:topConceptOf rdf:resource="http://data.europa.eu/energy/StandardMessageTypeList"/>
    <dc:identifier>B02</dc:identifier>
    <skos:prefLabel>HVDC Schedule</skos:prefLabel>
    <skos:definition xml:lang="en">A document providing the information for operating DC links.</skos:definition>
  </skos:Concept>
  <skos:Concept rdf:about="http://data.europa.eu/energy/StandardMessageTypeList/B03">
    <skos:inScheme rdf:resource="http://data.europa.eu/energy/StandardMessageTypeList"/>
    <skos:topConceptOf rdf:resource="http://data.europa.eu/energy/StandardMessageTypeList"/>
    <dc:identifier>B03</dc:identifier>
    <skos:prefLabel>EIC code request</skos:prefLabel>
    <skos:definition xml:lang="en">A document providing the information requesting a new EIC code.</skos:definition>
  </skos:Concept>
  <skos:Concept rdf:about="http://data.europa.eu/energy/StandardMessageTypeList/B04">
    <skos:inScheme rdf:resource="http://data.europa.eu/energy/StandardMessageTypeList"/>
    <skos:topConceptOf rdf:resource="http://data.europa.eu/energy/StandardMessageTypeList"/>
    <dc:identifier>B04</dc:identifier>
    <skos:prefLabel>EIC code information</skos:prefLabel>
    <skos:definition xml:lang="en">A document providing EIC information  in a central registry exchange or information to an EIC participant.</skos:definition>
  </skos:Concept>
  <skos:Concept rdf:about="http://data.europa.eu/energy/StandardMessageTypeList/B05">
    <skos:inScheme rdf:resource="http://data.europa.eu/energy/StandardMessageTypeList"/>
    <skos:topConceptOf rdf:resource="http://data.europa.eu/energy/StandardMessageTypeList"/>
    <dc:identifier>B05</dc:identifier>
    <skos:prefLabel>EIC code publication</skos:prefLabel>
    <skos:definition xml:lang="en">A document providing EIC publication information in a web site publication of a limited set of information.</skos:definition>
  </skos:Concept>
  <skos:Concept rdf:about="http://data.europa.eu/energy/StandardMessageTypeList/B06">
    <skos:inScheme rdf:resource="http://data.europa.eu/energy/StandardMessageTypeList"/>
    <skos:topConceptOf rdf:resource="http://data.europa.eu/energy/StandardMessageTypeList"/>
    <dc:identifier>B06</dc:identifier>
    <skos:prefLabel>Critical network element determination</skos:prefLabel>
    <skos:definition xml:lang="en">A document providing all the elements necessary for the capacity coordinator to determine the transfer capacity and the associated critical network elements.</skos:definition>
  </skos:Concept>
  <skos:Concept rdf:about="http://data.europa.eu/energy/StandardMessageTypeList/B07">
    <skos:inScheme rdf:resource="http://data.europa.eu/energy/StandardMessageTypeList"/>
    <skos:topConceptOf rdf:resource="http://data.europa.eu/energy/StandardMessageTypeList"/>
    <dc:identifier>B07</dc:identifier>
    <skos:prefLabel>Critical network element publication</skos:prefLabel>
    <skos:definition xml:lang="en">A document providing all the elements necessary for the market information aggregator and TSOs to know the critical network elements which limit the transfer capacity.</skos:definition>
  </skos:Concept>
  <skos:Concept rdf:about="http://data.europa.eu/energy/StandardMessageTypeList/B08">
    <skos:inScheme rdf:resource="http://data.europa.eu/energy/StandardMessageTypeList"/>
    <skos:topConceptOf rdf:resource="http://data.europa.eu/energy/StandardMessageTypeList"/>
    <dc:identifier>B08</dc:identifier>
    <skos:prefLabel>Flow based domain</skos:prefLabel>
    <skos:definition xml:lang="en">A document providing the capacity domain and its limits available for the TSO.</skos:definition>
  </skos:Concept>
  <skos:Concept rdf:about="http://data.europa.eu/energy/StandardMessageTypeList/B09">
    <skos:inScheme rdf:resource="http://data.europa.eu/energy/StandardMessageTypeList"/>
    <skos:topConceptOf rdf:resource="http://data.europa.eu/energy/StandardMessageTypeList"/>
    <dc:identifier>B09</dc:identifier>
    <skos:prefLabel>Flow based domain publication</skos:prefLabel>
    <skos:definition xml:lang="en">A document providing the capacity domain and its limits available for the market.</skos:definition>
  </skos:Concept>
  <skos:Concept rdf:about="http://data.europa.eu/energy/StandardMessageTypeList/B10">
    <skos:inScheme rdf:resource="http://data.europa.eu/energy/StandardMessageTypeList"/>
    <skos:topConceptOf rdf:resource="http://data.europa.eu/energy/StandardMessageTypeList"/>
    <dc:identifier>B10</dc:identifier>
    <skos:prefLabel>Flow based domain market impact publication</skos:prefLabel>
    <skos:definition xml:lang="en">A document providing the capacity domain and its impacts on the market to be published.</skos:definition>
  </skos:Concept>
  <skos:Concept rdf:about="http://data.europa.eu/energy/StandardMessageTypeList/B11">
    <skos:inScheme rdf:resource="http://data.europa.eu/energy/StandardMessageTypeList"/>
    <skos:topConceptOf rdf:resource="http://data.europa.eu/energy/StandardMessageTypeList"/>
    <dc:identifier>B11</dc:identifier>
    <skos:prefLabel>Anonymized flow based parameters publication</skos:prefLabel>
    <skos:definition xml:lang="en">A document providing all the relevant flow based parameters in case of flow based capacity allocation.</skos:definition>
  </skos:Concept>
  <skos:Concept rdf:about="http://data.europa.eu/energy/StandardMessageTypeList/B12">
    <skos:inScheme rdf:resource="http://data.europa.eu/energy/StandardMessageTypeList"/>
    <skos:topConceptOf rdf:resource="http://data.europa.eu/energy/StandardMessageTypeList"/>
    <dc:identifier>B12</dc:identifier>
    <skos:prefLabel>Critical network element market impact publication</skos:prefLabel>
    <skos:definition xml:lang="en">A document providing the critical network elements and its impacts on the market to be published.</skos:definition>
  </skos:Concept>
  <skos:Concept rdf:about="http://data.europa.eu/energy/StandardMessageTypeList/B13">
    <skos:inScheme rdf:resource="http://data.europa.eu/energy/StandardMessageTypeList"/>
    <skos:topConceptOf rdf:resource="http://data.europa.eu/energy/StandardMessageTypeList"/>
    <dc:identifier>B13</dc:identifier>
    <skos:prefLabel>Weather document</skos:prefLabel>
    <skos:definition xml:lang="en">An estimation or prediction in advance of the weather by analysis of meteorological data and the results of what actually happened with the weather.</skos:definition>
  </skos:Concept>
  <skos:Concept rdf:about="http://data.europa.eu/energy/StandardMessageTypeList/B14">
    <skos:inScheme rdf:resource="http://data.europa.eu/energy/StandardMessageTypeList"/>
    <skos:topConceptOf rdf:resource="http://data.europa.eu/energy/StandardMessageTypeList"/>
    <dc:identifier>B14</dc:identifier>
    <skos:prefLabel>Energy prognosis document</skos:prefLabel>
    <skos:definition xml:lang="en">A document to provide the prognosis of energy production/load for a given period.</skos:definition>
  </skos:Concept>
  <skos:Concept rdf:about="http://data.europa.eu/energy/StandardMessageTypeList/B15">
    <skos:inScheme rdf:resource="http://data.europa.eu/energy/StandardMessageTypeList"/>
    <skos:topConceptOf rdf:resource="http://data.europa.eu/energy/StandardMessageTypeList"/>
    <dc:identifier>B15</dc:identifier>
    <skos:prefLabel>Network constraint document</skos:prefLabel>
    <skos:definition xml:lang="en">A document providing the network constraint situations used for the load flow studies. A network constraint situation includes contingencies, monitored elements and remedial actions.</skos:definition>
  </skos:Concept>
  <skos:Concept rdf:about="http://data.europa.eu/energy/StandardMessageTypeList/B16">
    <skos:inScheme rdf:resource="http://data.europa.eu/energy/StandardMessageTypeList"/>
    <skos:topConceptOf rdf:resource="http://data.europa.eu/energy/StandardMessageTypeList"/>
    <dc:identifier>B16</dc:identifier>
    <skos:prefLabel>Aggregated netted external market schedule document</skos:prefLabel>
    <skos:definition xml:lang="en">A document used to report aggregated netted external market schedules for a given border.</skos:definition>
  </skos:Concept>
  <skos:Concept rdf:about="http://data.europa.eu/energy/StandardMessageTypeList/B17">
    <skos:inScheme rdf:resource="http://data.europa.eu/energy/StandardMessageTypeList"/>
    <skos:topConceptOf rdf:resource="http://data.europa.eu/energy/StandardMessageTypeList"/>
    <dc:identifier>B17</dc:identifier>
    <skos:prefLabel>Aggregated netted external TSO schedule document</skos:prefLabel>
    <skos:definition xml:lang="en">A document used to report aggregated netted external TSO schedules for a given border.</skos:definition>
  </skos:Concept>
  <skos:Concept rdf:about="http://data.europa.eu/energy/StandardMessageTypeList/B18">
    <skos:inScheme rdf:resource="http://data.europa.eu/energy/StandardMessageTypeList"/>
    <skos:topConceptOf rdf:resource="http://data.europa.eu/energy/StandardMessageTypeList"/>
    <dc:identifier>B18</dc:identifier>
    <skos:prefLabel>Reporting status market document</skos:prefLabel>
    <skos:definition xml:lang="en">A document used to report the status of aggregated netted external market schedules, aggregated netted external TSO schedules and compensation program schedules on a given border.</skos:definition>
  </skos:Concept>
  <skos:Concept rdf:about="http://data.europa.eu/energy/StandardMessageTypeList/B19">
    <skos:inScheme rdf:resource="http://data.europa.eu/energy/StandardMessageTypeList"/>
    <skos:topConceptOf rdf:resource="http://data.europa.eu/energy/StandardMessageTypeList"/>
    <dc:identifier>B19</dc:identifier>
    <skos:prefLabel>Reporting information market document</skos:prefLabel>
    <skos:definition xml:lang="en">A document used to report  the information concerning aggregated netted external schedules, aggregated netted external market schedules, aggregated netted external TSO schedules, compensation program schedules, netted area position schedules and netted area AC position schedules to an interested party.</skos:definition>
  </skos:Concept>
  <skos:Concept rdf:about="http://data.europa.eu/energy/StandardMessageTypeList/B20">
    <skos:inScheme rdf:resource="http://data.europa.eu/energy/StandardMessageTypeList"/>
    <skos:topConceptOf rdf:resource="http://data.europa.eu/energy/StandardMessageTypeList"/>
    <dc:identifier>B20</dc:identifier>
    <skos:prefLabel>Status request for a reporting information market document</skos:prefLabel>
    <skos:definition xml:lang="en">A document requesting the provision of a reporting information document.</skos:definition>
  </skos:Concept>
  <skos:Concept rdf:about="http://data.europa.eu/energy/StandardMessageTypeList/B21">
    <skos:inScheme rdf:resource="http://data.europa.eu/energy/StandardMessageTypeList"/>
    <skos:topConceptOf rdf:resource="http://data.europa.eu/energy/StandardMessageTypeList"/>
    <dc:identifier>B21</dc:identifier>
    <skos:prefLabel>Reserve need document</skos:prefLabel>
    <skos:definition xml:lang="en">Used by a TSO to send its reserve needs.</skos:definition>
  </skos:Concept>
  <skos:Concept rdf:about="http://data.europa.eu/energy/StandardMessageTypeList/B22">
    <skos:inScheme rdf:resource="http://data.europa.eu/energy/StandardMessageTypeList"/>
    <skos:topConceptOf rdf:resource="http://data.europa.eu/energy/StandardMessageTypeList"/>
    <dc:identifier>B22</dc:identifier>
    <skos:prefLabel>Generation and load shift keys document</skos:prefLabel>
    <skos:definition xml:lang="en">A document providing the values of the generation and load shift keys to be used on network model.</skos:definition>
  </skos:Concept>
  <skos:Concept rdf:about="http://data.europa.eu/energy/StandardMessageTypeList/B23">
    <skos:inScheme rdf:resource="http://data.europa.eu/energy/StandardMessageTypeList"/>
    <skos:topConceptOf rdf:resource="http://data.europa.eu/energy/StandardMessageTypeList"/>
    <dc:identifier>B23</dc:identifier>
    <skos:prefLabel>Offers to be activated</skos:prefLabel>
    <skos:definition xml:lang="en">A document containing the outcome of the process, with the list of offers that are to be activated by the TSO concerned and the results for its reserve needs.</skos:definition>
  </skos:Concept>
  <skos:Concept rdf:about="http://data.europa.eu/energy/StandardMessageTypeList/B24">
    <skos:inScheme rdf:resource="http://data.europa.eu/energy/StandardMessageTypeList"/>
    <skos:topConceptOf rdf:resource="http://data.europa.eu/energy/StandardMessageTypeList"/>
    <dc:identifier>B24</dc:identifier>
    <skos:prefLabel>Clearing price</skos:prefLabel>
    <skos:definition xml:lang="en">A document containing the outcome of the process, with the clearing prices for a period.</skos:definition>
  </skos:Concept>
  <skos:Concept rdf:about="http://data.europa.eu/energy/StandardMessageTypeList/B25">
    <skos:inScheme rdf:resource="http://data.europa.eu/energy/StandardMessageTypeList"/>
    <skos:topConceptOf rdf:resource="http://data.europa.eu/energy/StandardMessageTypeList"/>
    <dc:identifier>B25</dc:identifier>
    <skos:prefLabel>Security analysis report</skos:prefLabel>
    <skos:definition xml:lang="en">A document providing a report on a performed security analysis.</skos:definition>
  </skos:Concept>
  <skos:Concept rdf:about="http://data.europa.eu/energy/StandardMessageTypeList/B26">
    <skos:inScheme rdf:resource="http://data.europa.eu/energy/StandardMessageTypeList"/>
    <skos:topConceptOf rdf:resource="http://data.europa.eu/energy/StandardMessageTypeList"/>
    <dc:identifier>B26</dc:identifier>
    <skos:prefLabel>Aggregated netted external schedule document</skos:prefLabel>
    <skos:definition xml:lang="en">A document used to report aggregated netted external schedules for a given border. </skos:definition>
  </skos:Concept>
  <skos:Concept rdf:about="http://data.europa.eu/energy/StandardMessageTypeList/B27">
    <skos:inScheme rdf:resource="http://data.europa.eu/energy/StandardMessageTypeList"/>
    <skos:topConceptOf rdf:resource="http://data.europa.eu/energy/StandardMessageTypeList"/>
    <dc:identifier>B27</dc:identifier>
    <skos:prefLabel>External TSO schedule</skos:prefLabel>
    <skos:definition xml:lang="en">A document used to report external TSO schedules for a given border or interconnector.</skos:definition>
  </skos:Concept>
  <skos:Concept rdf:about="http://data.europa.eu/energy/StandardMessageTypeList/B28">
    <skos:inScheme rdf:resource="http://data.europa.eu/energy/StandardMessageTypeList"/>
    <skos:topConceptOf rdf:resource="http://data.europa.eu/energy/StandardMessageTypeList"/>
    <dc:identifier>B28</dc:identifier>
    <skos:prefLabel>Move of scheduled production</skos:prefLabel>
    <skos:definition xml:lang="en">A document indication a move of scheduled production.</skos:definition>
  </skos:Concept>
  <skos:Concept rdf:about="http://data.europa.eu/energy/StandardMessageTypeList/B29">
    <skos:inScheme rdf:resource="http://data.europa.eu/energy/StandardMessageTypeList"/>
    <skos:topConceptOf rdf:resource="http://data.europa.eu/energy/StandardMessageTypeList"/>
    <dc:identifier>B29</dc:identifier>
    <skos:prefLabel>PS&amp;LC results document</skos:prefLabel>
    <skos:definition xml:lang="en">A document providing Pole Splitting &amp;amp; Loss Calculation results.</skos:definition>
  </skos:Concept>
  <skos:Concept rdf:about="http://data.europa.eu/energy/StandardMessageTypeList/B30">
    <skos:inScheme rdf:resource="http://data.europa.eu/energy/StandardMessageTypeList"/>
    <skos:topConceptOf rdf:resource="http://data.europa.eu/energy/StandardMessageTypeList"/>
    <dc:identifier>B30</dc:identifier>
    <skos:prefLabel>Notification data market document</skos:prefLabel>
    <skos:definition xml:lang="en">A document used to notify data to any information receiver.</skos:definition>
  </skos:Concept>
  <skos:Concept rdf:about="http://data.europa.eu/energy/StandardMessageTypeList/B31">
    <skos:inScheme rdf:resource="http://data.europa.eu/energy/StandardMessageTypeList"/>
    <skos:topConceptOf rdf:resource="http://data.europa.eu/energy/StandardMessageTypeList"/>
    <dc:identifier>B31</dc:identifier>
    <skos:prefLabel>Additional Constraint document</skos:prefLabel>
    <skos:definition xml:lang="en">A document describing additional constraints for a capacity calculation process.</skos:definition>
  </skos:Concept>
  <skos:Concept rdf:about="http://data.europa.eu/energy/StandardMessageTypeList/B32">
    <skos:inScheme rdf:resource="http://data.europa.eu/energy/StandardMessageTypeList"/>
    <skos:topConceptOf rdf:resource="http://data.europa.eu/energy/StandardMessageTypeList"/>
    <dc:identifier>B32</dc:identifier>
    <skos:prefLabel>Operational state document</skos:prefLabel>
    <skos:definition xml:lang="en">A document used for exchanging operational states for grid assets.</skos:definition>
  </skos:Concept>
  <skos:Concept rdf:about="http://data.europa.eu/energy/StandardMessageTypeList/B33">
    <skos:inScheme rdf:resource="http://data.europa.eu/energy/StandardMessageTypeList"/>
    <skos:topConceptOf rdf:resource="http://data.europa.eu/energy/StandardMessageTypeList"/>
    <dc:identifier>B33</dc:identifier>
    <skos:prefLabel>Published offered capacity</skos:prefLabel>
    <skos:definition xml:lang="en">A document providing the most recent values of offered capacity.</skos:definition>
  </skos:Concept>
  <skos:Concept rdf:about="http://data.europa.eu/energy/StandardMessageTypeList/B34">
    <skos:inScheme rdf:resource="http://data.europa.eu/energy/StandardMessageTypeList"/>
    <skos:topConceptOf rdf:resource="http://data.europa.eu/energy/StandardMessageTypeList"/>
    <dc:identifier>B34</dc:identifier>
    <skos:prefLabel>Market result document</skos:prefLabel>
    <skos:definition xml:lang="en">Published prices and volumes</skos:definition>
  </skos:Concept>
  <skos:Concept rdf:about="http://data.europa.eu/energy/StandardMessageTypeList/B35">
    <skos:inScheme rdf:resource="http://data.europa.eu/energy/StandardMessageTypeList"/>
    <skos:topConceptOf rdf:resource="http://data.europa.eu/energy/StandardMessageTypeList"/>
    <dc:identifier>B35</dc:identifier>
    <skos:prefLabel>Area Configuration document</skos:prefLabel>
    <skos:definition xml:lang="en">A document containing the definition of areas.</skos:definition>
  </skos:Concept>
  <skos:Concept rdf:about="http://data.europa.eu/energy/StandardMessageTypeList/B36">
    <skos:inScheme rdf:resource="http://data.europa.eu/energy/StandardMessageTypeList"/>
    <skos:topConceptOf rdf:resource="http://data.europa.eu/energy/StandardMessageTypeList"/>
    <dc:identifier>B36</dc:identifier>
    <skos:prefLabel>Area Composition document</skos:prefLabel>
    <skos:definition xml:lang="en">A document containing the relations between areas, i.e which Metering Grid Areas a Bidding Zone composed of.</skos:definition>
  </skos:Concept>
  <skos:Concept rdf:about="http://data.europa.eu/energy/StandardMessageTypeList/B37">
    <skos:inScheme rdf:resource="http://data.europa.eu/energy/StandardMessageTypeList"/>
    <skos:topConceptOf rdf:resource="http://data.europa.eu/energy/StandardMessageTypeList"/>
    <dc:identifier>B37</dc:identifier>
    <skos:prefLabel>Connected Areas document</skos:prefLabel>
    <skos:definition xml:lang="en">A document containing which other areas an area is connected to i.e. which Metering Grid Areas a Metering Grid Area is connected to.</skos:definition>
  </skos:Concept>
  <skos:Concept rdf:about="http://data.europa.eu/energy/StandardMessageTypeList/B38">
    <skos:inScheme rdf:resource="http://data.europa.eu/energy/StandardMessageTypeList"/>
    <skos:topConceptOf rdf:resource="http://data.europa.eu/energy/StandardMessageTypeList"/>
    <dc:identifier>B38</dc:identifier>
    <skos:prefLabel>Settlement document</skos:prefLabel>
    <skos:definition xml:lang="en">A document providing settlement information.</skos:definition>
  </skos:Concept>
  <skos:Concept rdf:about="http://data.europa.eu/energy/StandardMessageTypeList/B39">
    <skos:inScheme rdf:resource="http://data.europa.eu/energy/StandardMessageTypeList"/>
    <skos:topConceptOf rdf:resource="http://data.europa.eu/energy/StandardMessageTypeList"/>
    <dc:identifier>B39</dc:identifier>
    <skos:prefLabel>Imbalance prognosis document</skos:prefLabel>
    <skos:definition xml:lang="en">A document to provide the prognosis of energy imbalances for a given period.</skos:definition>
  </skos:Concept>
  <skos:Concept rdf:about="http://data.europa.eu/energy/StandardMessageTypeList/B40">
    <skos:inScheme rdf:resource="http://data.europa.eu/energy/StandardMessageTypeList"/>
    <skos:topConceptOf rdf:resource="http://data.europa.eu/energy/StandardMessageTypeList"/>
    <dc:identifier>B40</dc:identifier>
    <skos:prefLabel>Complete set of bids</skos:prefLabel>
    <skos:definition xml:lang="en">Submission of complete set of bids. If there are existing bids, they should be replaced.</skos:definition>
  </skos:Concept>
  <skos:Concept rdf:about="http://data.europa.eu/energy/StandardMessageTypeList/B41">
    <skos:inScheme rdf:resource="http://data.europa.eu/energy/StandardMessageTypeList"/>
    <skos:topConceptOf rdf:resource="http://data.europa.eu/energy/StandardMessageTypeList"/>
    <dc:identifier>B41</dc:identifier>
    <skos:prefLabel>Merged MOL notice</skos:prefLabel>
    <skos:definition xml:lang="en">A notice providing information on the MOL merging process.</skos:definition>
  </skos:Concept>
  <skos:Concept rdf:about="http://data.europa.eu/energy/StandardMessageTypeList/B42">
    <skos:inScheme rdf:resource="http://data.europa.eu/energy/StandardMessageTypeList"/>
    <skos:topConceptOf rdf:resource="http://data.europa.eu/energy/StandardMessageTypeList"/>
    <dc:identifier>B42</dc:identifier>
    <skos:prefLabel>K-factor document</skos:prefLabel>
    <skos:definition xml:lang="en">A document providing K-factor values.</skos:definition>
  </skos:Concept>
  <skos:Concept rdf:about="http://data.europa.eu/energy/StandardMessageTypeList/B43">
    <skos:inScheme rdf:resource="http://data.europa.eu/energy/StandardMessageTypeList"/>
    <skos:topConceptOf rdf:resource="http://data.europa.eu/energy/StandardMessageTypeList"/>
    <dc:identifier>B43</dc:identifier>
    <skos:prefLabel>Settlement coordination document</skos:prefLabel>
    <skos:definition xml:lang="en">A document providing settlement information for coordination between different parties.</skos:definition>
  </skos:Concept>
  <skos:Concept rdf:about="http://data.europa.eu/energy/StandardMessageTypeList/B44">
    <skos:inScheme rdf:resource="http://data.europa.eu/energy/StandardMessageTypeList"/>
    <skos:topConceptOf rdf:resource="http://data.europa.eu/energy/StandardMessageTypeList"/>
    <dc:identifier>B44</dc:identifier>
    <skos:prefLabel>Financial settlement document</skos:prefLabel>
    <skos:definition xml:lang="en">A document providing financial settlement information.</skos:definition>
  </skos:Concept>
  <skos:Concept rdf:about="http://data.europa.eu/energy/StandardMessageTypeList/B45">
    <skos:inScheme rdf:resource="http://data.europa.eu/energy/StandardMessageTypeList"/>
    <skos:topConceptOf rdf:resource="http://data.europa.eu/energy/StandardMessageTypeList"/>
    <dc:identifier>B45</dc:identifier>
    <skos:prefLabel>Bid availability document</skos:prefLabel>
    <skos:definition xml:lang="en">A document providing the detailed reasons for changing the availability or volume of a bid.</skos:definition>
  </skos:Concept>
  <skos:Concept rdf:about="http://data.europa.eu/energy/StandardMessageTypeList/B46">
    <skos:inScheme rdf:resource="http://data.europa.eu/energy/StandardMessageTypeList"/>
    <skos:topConceptOf rdf:resource="http://data.europa.eu/energy/StandardMessageTypeList"/>
    <dc:identifier>B46</dc:identifier>
    <skos:prefLabel>Resource capacity unit document</skos:prefLabel>
    <skos:definition xml:lang="en">A document providing information about resource capacity units.</skos:definition>
  </skos:Concept>
</rdf:RDF>
