@prefix dcat: <http://www.w3.org/ns/dcat#> .
@prefix dcterms: <http://purl.org/dc/terms/> .
@prefix skos: <http://www.w3.org/2004/02/skos/core#> .

<http://energy.referencedata.eu/StandardMarketProductTypeList/A01> a skos:Concept ;
    dcterms:identifier "A01" ;
    skos:definition "A harmonised balancing product defined by all TSOs for the exchange of balancing services."@en ;
    skos:inScheme <http://energy.referencedata.eu/StandardMarketProductTypeList> ;
    skos:prefLabel "Standard balancing product" ;
    skos:topConceptOf <http://energy.referencedata.eu/StandardMarketProductTypeList> .

<http://energy.referencedata.eu/StandardMarketProductTypeList/A02> a skos:Concept ;
    dcterms:identifier "A02" ;
    skos:definition "A product different from a standard product."@en ;
    skos:inScheme <http://energy.referencedata.eu/StandardMarketProductTypeList> ;
    skos:prefLabel "Specific balancing product" ;
    skos:topConceptOf <http://energy.referencedata.eu/StandardMarketProductTypeList> .

<http://energy.referencedata.eu/StandardMarketProductTypeList/A03> a skos:Concept ;
    dcterms:identifier "A03" ;
    skos:definition "From the EBGL Article 2 (19), means an iterative process that uses at least integrated scheduling process bids that contain commercial data, complex technical data of individual power generating facilities or demand facilities and explicitly includes the start-up characteristics, the latest control area adequacy analysis and the operational security limits as an input to the process."@en ;
    skos:inScheme <http://energy.referencedata.eu/StandardMarketProductTypeList> ;
    skos:prefLabel "Product from integrated scheduling process" ;
    skos:topConceptOf <http://energy.referencedata.eu/StandardMarketProductTypeList> .

<http://energy.referencedata.eu/StandardMarketProductTypeList/A04> a skos:Concept ;
    dcterms:identifier "A04" ;
    skos:definition "A balancing product that is neither standard nor specific. This type may be applicable only in the interim period until standard and specific products have been defined within the given scheduling area."@en ;
    skos:inScheme <http://energy.referencedata.eu/StandardMarketProductTypeList> ;
    skos:prefLabel "Local balancing product" ;
    skos:topConceptOf <http://energy.referencedata.eu/StandardMarketProductTypeList> .

<http://energy.referencedata.eu/StandardMarketProductTypeList/A05> a skos:Concept ;
    dcterms:identifier "A05" ;
    skos:definition "Standard mFRR product eligible for scheduled activation."@en ;
    skos:inScheme <http://energy.referencedata.eu/StandardMarketProductTypeList> ;
    skos:prefLabel "Standard mFRR product eligible for scheduled activation" ;
    skos:topConceptOf <http://energy.referencedata.eu/StandardMarketProductTypeList> .

<http://energy.referencedata.eu/StandardMarketProductTypeList/A06> a skos:Concept ;
    dcterms:identifier "A06" ;
    skos:definition "Standard mFRR product eligible for direct activation."@en ;
    skos:inScheme <http://energy.referencedata.eu/StandardMarketProductTypeList> ;
    skos:prefLabel "Standard mFRR product eligible for direct activation" ;
    skos:topConceptOf <http://energy.referencedata.eu/StandardMarketProductTypeList> .

<http://energy.referencedata.eu/StandardMarketProductTypeList/A07> a skos:Concept ;
    dcterms:identifier "A07" ;
    skos:definition "Standard mFRR product eligible for direct as well as scheduled activation."@en ;
    skos:inScheme <http://energy.referencedata.eu/StandardMarketProductTypeList> ;
    skos:prefLabel "Standard mFRR product eligible for direct and scheduled activation" ;
    skos:topConceptOf <http://energy.referencedata.eu/StandardMarketProductTypeList> .

<http://energy.referencedata.eu/StandardMarketProductTypeList/A08> a skos:Concept ;
    dcterms:identifier "A08" ;
    skos:definition "This is a market-wide resource capacity mechanism where all resource capacity required to ensure security of supply receives payment. These mechanisms are open for participation to all capacity resources contributing to adequacy."@en ;
    skos:inScheme <http://energy.referencedata.eu/StandardMarketProductTypeList> ;
    skos:prefLabel "Market wide resource capacity mechanism" ;
    skos:topConceptOf <http://energy.referencedata.eu/StandardMarketProductTypeList> .

<http://energy.referencedata.eu/StandardMarketProductTypeList/A09> a skos:Concept ;
    dcterms:identifier "A09" ;
    skos:definition "This is a market resource capacity mechanism that is kept outside of the electricity market and only used if the market participants do not offer enough generation to meet short-term demand."@en ;
    skos:inScheme <http://energy.referencedata.eu/StandardMarketProductTypeList> ;
    skos:prefLabel "Strategic reserve resource capacity mechanism" ;
    skos:topConceptOf <http://energy.referencedata.eu/StandardMarketProductTypeList> .

<http://energy.referencedata.eu/StandardMarketProductTypeList/A10> a skos:Concept ;
    dcterms:identifier "A10" ;
    skos:definition "This is any other kind of market resource capacity mechanism."@en ;
    skos:inScheme <http://energy.referencedata.eu/StandardMarketProductTypeList> ;
    skos:prefLabel "Other resource capacity mechanism" ;
    skos:topConceptOf <http://energy.referencedata.eu/StandardMarketProductTypeList> .

<http://energy.referencedata.eu/StandardMarketProductTypeList/A11> a skos:Concept ;
    dcterms:identifier "A11" ;
    skos:definition "The fast activation product shall be considered as a fall-back solution for situations where coordination with all parties is no longer possible due to insufficient time and the regular product could not be properly applied."@en ;
    skos:inScheme <http://energy.referencedata.eu/StandardMarketProductTypeList> ;
    skos:prefLabel "Fast activation product" ;
    skos:topConceptOf <http://energy.referencedata.eu/StandardMarketProductTypeList> .

<http://energy.referencedata.eu/StandardMarketProductTypeList> a skos:ConceptScheme,
        dcat:Dataset ;
    dcterms:identifier "ET0008" ;
    dcterms:modified "2023-12-14" ;
    skos:definition "The identification of the type of a product on a market view"@en ;
    skos:prefLabel "StandardMarketProductTypeList" ;
    dcat:version "91" .

